<?xml version="1.0" encoding="utf-8"?>
<rdf:RDF
   xmlns:bibo="http://purl.org/ontology/bibo/"
   xmlns:dct="http://purl.org/dc/terms/"
   xmlns:foaf="http://xmlns.com/foaf/0.1/"
   xmlns:org="http://www.w3.org/ns/org#"
   xmlns:owl="http://www.w3.org/2002/07/owl#"
   xmlns:profile="http://www.w3.org/ns/dx/prof/"
   xmlns:rdf="http://www.w3.org/1999/02/22-rdf-syntax-ns#"
   xmlns:rdfs="http://www.w3.org/2000/01/rdf-schema#"
   xmlns:schema="https://schema.org/"
   xmlns:scoro="http://purl.org/spar/scoro/"
   xmlns:skos="http://www.w3.org/2004/02/skos/core#"
   xmlns:sw="http://www.w3.org/2003/06/sw-vocab-status/ns#"
   xmlns:vann="http://purl.org/vocab/vann/"
>
  <rdf:Description rdf:about="https://w3id.org/dpv/justifications/owl#UnlawfulActivityObjection">
    <sw:term_status xml:lang="en">accepted</sw:term_status>
    <dct:contributor rdf:nodeID="person-harshvardhan-j-pandit"/>
    <dct:contributor rdf:nodeID="person-beatriz-esteves"/>
    <rdf:type rdf:resource="https://w3id.org/dpv/owl#Justification"/>
    <rdf:type rdf:resource="http://www.w3.org/2000/01/rdf-schema#Class"/>
    <rdf:type rdf:resource="http://www.w3.org/2002/07/owl#Class"/>
    <rdfs:isDefinedBy rdf:resource="https://w3id.org/dpv/justifications/owl#"/>
    <skos:prefLabel xml:lang="en">Unlawful Activity Objection</skos:prefLabel>
    <skos:definition xml:lang="en">Justification that the process should be carried out due to it being an objection of unlawful activity</skos:definition>
    <dct:created rdf:datatype="http://www.w3.org/2001/XMLSchema#date">2024-04-21</dct:created>
    <rdfs:subClassOf rdf:resource="https://w3id.org/dpv/justifications/owl#Objection"/>
  </rdf:Description>
  <rdf:Description rdf:about="https://w3id.org/dpv/justifications/owl#EntityAlreadyInformed">
    <rdf:type rdf:resource="http://www.w3.org/2000/01/rdf-schema#Class"/>
    <rdf:type rdf:resource="https://w3id.org/dpv/owl#Justification"/>
    <rdf:type rdf:resource="http://www.w3.org/2002/07/owl#Class"/>
    <rdfs:isDefinedBy rdf:resource="https://w3id.org/dpv/justifications/owl#"/>
    <skos:definition xml:lang="en">Justification that the process could not be fulfilled or was not successful because the entity already has the information</skos:definition>
    <dct:contributor rdf:nodeID="person-harshvardhan-j-pandit"/>
    <dct:contributor rdf:nodeID="person-beatriz-esteves"/>
    <skos:prefLabel xml:lang="en">Entity Already Informed</skos:prefLabel>
    <dct:created rdf:datatype="http://www.w3.org/2001/XMLSchema#date">2024-04-21</dct:created>
    <sw:term_status xml:lang="en">accepted</sw:term_status>
    <rdfs:subClassOf rdf:resource="https://w3id.org/dpv/justifications/owl#DisproportionateEffortRequired"/>
  </rdf:Description>
  <rdf:Description rdf:about="https://w3id.org/dpv/justifications/owl#CivilLawEnforcementImpaired">
    <rdf:type rdf:resource="http://www.w3.org/2000/01/rdf-schema#Class"/>
    <rdf:type rdf:resource="https://w3id.org/dpv/owl#Justification"/>
    <rdf:type rdf:resource="http://www.w3.org/2002/07/owl#Class"/>
    <rdfs:isDefinedBy rdf:resource="https://w3id.org/dpv/justifications/owl#"/>
    <skos:prefLabel xml:lang="en">Civil Law Enforcement Impaired</skos:prefLabel>
    <dct:contributor rdf:nodeID="person-harshvardhan-j-pandit"/>
    <dct:contributor rdf:nodeID="person-beatriz-esteves"/>
    <dct:created rdf:datatype="http://www.w3.org/2001/XMLSchema#date">2024-04-21</dct:created>
    <sw:term_status xml:lang="en">accepted</sw:term_status>
    <skos:definition xml:lang="en">Justification that the process could not be fulfilled or was not successful because it would interfere with the enforcement of civil laws, including civil claims</skos:definition>
    <rdfs:subClassOf rdf:resource="https://w3id.org/dpv/justifications/owl#LegalProcessImpaired"/>
  </rdf:Description>
  <rdf:Description rdf:about="https://w3id.org/dpv/justifications/owl#DefenceImpaired">
    <dct:contributor rdf:nodeID="person-beatriz-esteves"/>
    <dct:contributor rdf:nodeID="person-harshvardhan-j-pandit"/>
    <skos:prefLabel xml:lang="en">Defence Impaired</skos:prefLabel>
    <dct:created rdf:datatype="http://www.w3.org/2001/XMLSchema#date">2024-04-21</dct:created>
    <rdfs:isDefinedBy rdf:resource="https://w3id.org/dpv/justifications/owl#"/>
    <rdf:type rdf:resource="http://www.w3.org/2000/01/rdf-schema#Class"/>
    <rdf:type rdf:resource="https://w3id.org/dpv/owl#Justification"/>
    <rdf:type rdf:resource="http://www.w3.org/2002/07/owl#Class"/>
    <sw:term_status xml:lang="en">accepted</sw:term_status>
    <skos:definition xml:lang="en">Justification that the process could not be fulfilled or was not successful because it would interfere with necessary tasks to safeguard defence</skos:definition>
    <rdfs:subClassOf rdf:resource="https://w3id.org/dpv/justifications/owl#SecurityImpaired"/>
    <rdfs:subClassOf rdf:resource="https://w3id.org/dpv/justifications/owl#LegalProcessImpaired"/>
  </rdf:Description>
  <rdf:Description rdf:about="https://w3id.org/dpv/justifications/owl#LegalClaimExerciseImpaired">
    <rdfs:isDefinedBy rdf:resource="https://w3id.org/dpv/justifications/owl#"/>
    <skos:prefLabel xml:lang="en">Legal Claim Exercise Impaired</skos:prefLabel>
    <rdf:type rdf:resource="http://www.w3.org/2000/01/rdf-schema#Class"/>
    <rdf:type rdf:resource="https://w3id.org/dpv/owl#Justification"/>
    <rdf:type rdf:resource="http://www.w3.org/2002/07/owl#Class"/>
    <dct:contributor rdf:nodeID="person-harshvardhan-j-pandit"/>
    <dct:contributor rdf:nodeID="person-beatriz-esteves"/>
    <dct:created rdf:datatype="http://www.w3.org/2001/XMLSchema#date">2024-04-21</dct:created>
    <skos:definition xml:lang="en">Justification that the process could not be fulfilled or was not successful because it would interfere with the exercise of legal claims</skos:definition>
    <dct:modified rdf:datatype="http://www.w3.org/2001/XMLSchema#date">2024-12-17</dct:modified>
    <sw:term_status xml:lang="en">modified</sw:term_status>
    <rdfs:subClassOf rdf:resource="https://w3id.org/dpv/justifications/owl#LegalClaimImpaired"/>
  </rdf:Description>
  <rdf:Description rdf:about="https://w3id.org/dpv/justifications/owl#">
    <owl:versionIRI rdf:resource="https://w3id.org/dpv/2.2/justifications/owl#"/>
    <dct:description xml:lang="en">Extension to the Data Privacy Vocabulary (DPV) providing concepts for representing information about justifications</dct:description>
    <profile:hasResource rdf:resource="https://w3id.org/dpv/guides"/>
    <profile:hasResource rdf:resource="https://w3id.org/dpv/justifications/owl#serialisation-jsonld"/>
    <profile:hasResource rdf:resource="https://w3id.org/dpv/justifications/owl#serialisation-html"/>
    <profile:hasResource rdf:resource="https://w3id.org/dpv/justifications/owl#serialisation-n3"/>
    <profile:hasResource rdf:resource="https://w3id.org/dpv/justifications/owl#serialisation-ttl"/>
    <profile:hasResource rdf:resource="https://w3id.org/dpv/primer"/>
    <profile:hasResource rdf:resource="https://w3id.org/dpv/justifications/owl#serialisation-rdf"/>
    <profile:hasResource rdf:resource="https://w3id.org/dpv/examples"/>
    <dct:conformsTo>http://www.w3.org/2000/01/rdf-schema</dct:conformsTo>
    <dct:conformsTo>http://www.w3.org/2004/02/skos/core</dct:conformsTo>
    <dct:conformsTo rdf:resource="http://www.w3.org/2002/07/owl"/>
    <dct:creator rdf:nodeID="person-paul-ryan"/>
    <dct:creator rdf:nodeID="person-harshvardhan-j-pandit"/>
    <dct:creator rdf:nodeID="person-beatriz-esteves"/>
    <dct:creator rdf:nodeID="person-georg-p-krog"/>
    <dct:bibliographicCitation>Harshvardhan J. Pandit, Beatriz Esteves, Georg P. Krog, Paul Ryan, Delaram Golpayegani, Julian Flake (2025) Data Privacy Vocabulary (DPV) – Version 2.0. In: Demartini, G., et al. The Semantic Web – ISWC 2024. ISWC 2024. Lecture Notes in Computer Science, vol 15233. Springer, Cham. https://doi.org/10.1007/978-3-031-77847-6_10</dct:bibliographicCitation>
    <dct:created xml:lang="en">2024-04-21</dct:created>
    <dct:license rdf:resource="https://www.w3.org/copyright/document-license-2023/"/>
    <dct:contributor rdf:nodeID="person-beatriz-esteves"/>
    <dct:contributor rdf:nodeID="person-harshvardhan-j-pandit"/>
    <dct:issued xml:lang="en">2024-04-21</dct:issued>
    <bibo:status>http://purl.org/ontology/bibo/status/published</bibo:status>
    <foaf:logo rdf:resource="https://w3id.org/dpv/media/logo.png"/>
    <dct:hasVersion rdf:resource="https://w3id.org/dpv/justifications/owl#"/>
    <rdf:type rdf:resource="http://www.w3.org/2002/07/owl#Ontology"/>
    <rdf:type rdf:resource="http://www.w3.org/ns/dx/prof/Profile"/>
    <dct:source rdf:resource="https://www.w3.org/groups/cg/dpvcg/"/>
    <dct:identifier>https://w3id.org/dpv/justifications</dct:identifier>
    <rdfs:Label xml:lang="en">JUSTIFICATIONS</rdfs:Label>
    <vann:preferredNamespaceUri>https://w3id.org/dpv/justifications#</vann:preferredNamespaceUri>
    <schema:version>2.2</schema:version>
    <vann:preferredNamespacePrefix>justifications</vann:preferredNamespacePrefix>
    <bibo:doi>10.5281/zenodo.12505841</bibo:doi>
    <profile:isProfileOf rdf:resource="https://w3id.org/dpv/owl"/>
    <profile:isProfileOf rdf:resource="http://www.w3.org/2002/07/owl"/>
    <profile:isProfileOf rdf:resource="https://w3id.org/dpv/justifications/owl#"/>
    <dct:publisher rdf:resource="https://www.w3.org/"/>
    <owl:versionInfo>2.2</owl:versionInfo>
    <dct:modified xml:lang="en">2025-08-01</dct:modified>
    <dct:title xml:lang="en">Justification Concepts</dct:title>
  </rdf:Description>
  <rdf:Description rdf:about="https://w3id.org/dpv/justifications/owl#ProcessSafeguarded">
    <rdfs:isDefinedBy rdf:resource="https://w3id.org/dpv/justifications/owl#"/>
    <rdf:type rdf:resource="https://w3id.org/dpv/owl#Justification"/>
    <rdf:type rdf:resource="http://www.w3.org/2000/01/rdf-schema#Class"/>
    <rdf:type rdf:resource="http://www.w3.org/2002/07/owl#Class"/>
    <sw:term_status xml:lang="en">accepted</sw:term_status>
    <dct:contributor rdf:nodeID="person-harshvardhan-j-pandit"/>
    <dct:contributor rdf:nodeID="person-beatriz-esteves"/>
    <skos:definition xml:lang="en">Justification that the process is not required as it is safeguarded by appropriate technical and organisational measures</skos:definition>
    <dct:created rdf:datatype="http://www.w3.org/2001/XMLSchema#date">2024-04-21</dct:created>
    <skos:prefLabel xml:lang="en">Process Safeguarded</skos:prefLabel>
    <rdfs:subClassOf rdf:resource="https://w3id.org/dpv/justifications/owl#NotRequiredJustification"/>
  </rdf:Description>
  <rdf:Description rdf:about="https://w3id.org/dpv/justifications/owl#ObjectivesImpaired">
    <rdfs:isDefinedBy rdf:resource="https://w3id.org/dpv/justifications/owl#"/>
    <rdf:type rdf:resource="http://www.w3.org/2000/01/rdf-schema#Class"/>
    <rdf:type rdf:resource="https://w3id.org/dpv/owl#Justification"/>
    <rdf:type rdf:resource="http://www.w3.org/2002/07/owl#Class"/>
    <sw:term_status xml:lang="en">accepted</sw:term_status>
    <dct:contributor rdf:nodeID="person-harshvardhan-j-pandit"/>
    <dct:contributor rdf:nodeID="person-beatriz-esteves"/>
    <skos:definition xml:lang="en">Justification that the process could not be fulfilled or was not successful because it impairs the objectives of associated context</skos:definition>
    <dct:created rdf:datatype="http://www.w3.org/2001/XMLSchema#date">2024-04-21</dct:created>
    <skos:prefLabel xml:lang="en">Objectives Impaired</skos:prefLabel>
    <rdfs:subClassOf rdf:resource="https://w3id.org/dpv/justifications/owl#NonFulfilmentJustification"/>
  </rdf:Description>
  <rdf:Description rdf:about="https://w3id.org/dpv/justifications/owl#LackOfIntent">
    <rdf:type rdf:resource="http://www.w3.org/2000/01/rdf-schema#Class"/>
    <rdf:type rdf:resource="https://w3id.org/dpv/owl#Justification"/>
    <rdf:type rdf:resource="http://www.w3.org/2002/07/owl#Class"/>
    <dct:contributor rdf:nodeID="person-harshvardhan-j-pandit"/>
    <skos:scopeNote xml:lang="en">An example of such intent is where the individual makes a request but then offers to withdraw it in return for some form of benefit from the organisation - see https://ico.org.uk/for-organisations/uk-gdpr-guidance-and-resources/individual-rights/right-of-access/when-can-we-refuse-to-comply-with-a-request/#refuse2</skos:scopeNote>
    <skos:prefLabel xml:lang="en">Lack of Intent</skos:prefLabel>
    <dct:created rdf:datatype="http://www.w3.org/2001/XMLSchema#date">2024-12-17</dct:created>
    <skos:definition xml:lang="en">Justification that the process could not be fulfilled as the requestor or initiator did not have a sufficient intent to complete it</skos:definition>
    <sw:term_status xml:lang="en">accepted</sw:term_status>
    <rdfs:isDefinedBy rdf:resource="https://w3id.org/dpv/justifications/owl#"/>
    <rdfs:subClassOf rdf:resource="https://w3id.org/dpv/justifications/owl#NonFulfilmentJustification"/>
  </rdf:Description>
  <rdf:Description rdf:about="https://w3id.org/dpv/justifications/owl#SecurityImpaired">
    <rdf:type rdf:resource="https://w3id.org/dpv/owl#Justification"/>
    <rdf:type rdf:resource="http://www.w3.org/2000/01/rdf-schema#Class"/>
    <rdf:type rdf:resource="http://www.w3.org/2002/07/owl#Class"/>
    <dct:created rdf:datatype="http://www.w3.org/2001/XMLSchema#date">2024-04-21</dct:created>
    <skos:prefLabel xml:lang="en">Security Impaired</skos:prefLabel>
    <dct:contributor rdf:nodeID="person-beatriz-esteves"/>
    <dct:contributor rdf:nodeID="person-harshvardhan-j-pandit"/>
    <sw:term_status xml:lang="en">accepted</sw:term_status>
    <rdfs:isDefinedBy rdf:resource="https://w3id.org/dpv/justifications/owl#"/>
    <skos:definition xml:lang="en">Justification that the process could not be fulfilled or was not successful because it would interfere with tasks required for maintaining security</skos:definition>
    <rdfs:subClassOf rdf:resource="https://w3id.org/dpv/justifications/owl#NonFulfilmentJustification"/>
  </rdf:Description>
  <rdf:Description rdf:about="https://w3id.org/dpv/justifications/owl#IdentityVerificationRequired">
    <skos:prefLabel xml:lang="en">Identity Verification Required</skos:prefLabel>
    <rdf:type rdf:resource="http://www.w3.org/2000/01/rdf-schema#Class"/>
    <rdf:type rdf:resource="https://w3id.org/dpv/owl#Justification"/>
    <rdf:type rdf:resource="http://www.w3.org/2002/07/owl#Class"/>
    <sw:term_status xml:lang="en">accepted</sw:term_status>
    <dct:contributor rdf:nodeID="person-harshvardhan-j-pandit"/>
    <dct:contributor rdf:nodeID="person-beatriz-esteves"/>
    <skos:definition xml:lang="en">Justification that the process could not be fulfilled or was not successful because identity verification is required</skos:definition>
    <dct:created rdf:datatype="http://www.w3.org/2001/XMLSchema#date">2024-04-21</dct:created>
    <rdfs:isDefinedBy rdf:resource="https://w3id.org/dpv/justifications/owl#"/>
    <rdfs:subClassOf rdf:resource="https://w3id.org/dpv/justifications/owl#DelayJustification"/>
  </rdf:Description>
  <rdf:Description rdf:about="https://w3id.org/dpv/justifications/owl#NotRequiredJustification">
    <dct:contributor rdf:nodeID="person-beatriz-esteves"/>
    <dct:contributor rdf:nodeID="person-harshvardhan-j-pandit"/>
    <rdfs:subClassOf rdf:resource="https://w3id.org/dpv/owl#Justification"/>
    <dct:created rdf:datatype="http://www.w3.org/2001/XMLSchema#date">2024-04-21</dct:created>
    <rdf:type rdf:resource="http://www.w3.org/2000/01/rdf-schema#Class"/>
    <rdf:type rdf:resource="http://www.w3.org/2002/07/owl#Class"/>
    <skos:prefLabel xml:lang="en">Not Required Justification</skos:prefLabel>
    <rdfs:isDefinedBy rdf:resource="https://w3id.org/dpv/justifications/owl#"/>
    <skos:definition xml:lang="en">Justification to reject or not complete a process as it is not required or isn't applicable</skos:definition>
    <sw:term_status xml:lang="en">accepted</sw:term_status>
  </rdf:Description>
  <rdf:Description rdf:about="https://w3id.org/dpv/justifications/owl#LegalityLackingObjection">
    <skos:definition xml:lang="en">Justification that the process should be carried out due to it being an objection to the lack of further legality or legal basis of specified context</skos:definition>
    <rdfs:isDefinedBy rdf:resource="https://w3id.org/dpv/justifications/owl#"/>
    <rdf:type rdf:resource="http://www.w3.org/2000/01/rdf-schema#Class"/>
    <rdf:type rdf:resource="https://w3id.org/dpv/owl#Justification"/>
    <rdf:type rdf:resource="http://www.w3.org/2002/07/owl#Class"/>
    <skos:prefLabel xml:lang="en">Legality Lacking Objection</skos:prefLabel>
    <sw:term_status xml:lang="en">accepted</sw:term_status>
    <dct:contributor rdf:nodeID="person-harshvardhan-j-pandit"/>
    <dct:contributor rdf:nodeID="person-beatriz-esteves"/>
    <dct:created rdf:datatype="http://www.w3.org/2001/XMLSchema#date">2024-04-21</dct:created>
    <rdfs:subClassOf rdf:resource="https://w3id.org/dpv/justifications/owl#Objection"/>
  </rdf:Description>
  <rdf:Description rdf:about="https://w3id.org/dpv/justifications/owl#NonNecessityObjection">
    <rdf:type rdf:resource="http://www.w3.org/2000/01/rdf-schema#Class"/>
    <rdf:type rdf:resource="https://w3id.org/dpv/owl#Justification"/>
    <rdf:type rdf:resource="http://www.w3.org/2002/07/owl#Class"/>
    <rdfs:isDefinedBy rdf:resource="https://w3id.org/dpv/justifications/owl#"/>
    <dct:contributor rdf:nodeID="person-harshvardhan-j-pandit"/>
    <dct:contributor rdf:nodeID="person-beatriz-esteves"/>
    <skos:prefLabel xml:lang="en">Non Necessity Objection</skos:prefLabel>
    <dct:created rdf:datatype="http://www.w3.org/2001/XMLSchema#date">2024-04-21</dct:created>
    <sw:term_status xml:lang="en">accepted</sw:term_status>
    <skos:definition xml:lang="en">Justification that the process should be carried out due to it being an objection to the non-necessity of specified context</skos:definition>
    <rdfs:subClassOf rdf:resource="https://w3id.org/dpv/justifications/owl#Objection"/>
  </rdf:Description>
  <rdf:Description rdf:about="https://w3id.org/dpv/justifications/owl#CrimePreventionImpaired">
    <rdf:type rdf:resource="http://www.w3.org/2000/01/rdf-schema#Class"/>
    <rdf:type rdf:resource="https://w3id.org/dpv/owl#Justification"/>
    <rdf:type rdf:resource="http://www.w3.org/2002/07/owl#Class"/>
    <sw:term_status xml:lang="en">accepted</sw:term_status>
    <rdfs:isDefinedBy rdf:resource="https://w3id.org/dpv/justifications/owl#"/>
    <dct:contributor rdf:nodeID="person-harshvardhan-j-pandit"/>
    <dct:contributor rdf:nodeID="person-beatriz-esteves"/>
    <skos:prefLabel xml:lang="en">Crime Prevention Impaired</skos:prefLabel>
    <dct:created rdf:datatype="http://www.w3.org/2001/XMLSchema#date">2024-04-21</dct:created>
    <skos:definition xml:lang="en">Justification that the process could not be fulfilled or was not successful because it would interfere with the prevention of criminal offences</skos:definition>
    <rdfs:subClassOf rdf:resource="https://w3id.org/dpv/justifications/owl#SecurityImpaired"/>
    <rdfs:subClassOf rdf:resource="https://w3id.org/dpv/justifications/owl#LegalProcessImpaired"/>
  </rdf:Description>
  <rdf:Description rdf:about="https://w3id.org/dpv/justifications/owl#LegallyExempted">
    <skos:definition xml:lang="en">Justification that the process could not be fulfilled or was not successful because it falls under legal exemption i.e. a law allows the non-fulfilment</skos:definition>
    <rdf:type rdf:resource="http://www.w3.org/2000/01/rdf-schema#Class"/>
    <rdf:type rdf:resource="https://w3id.org/dpv/owl#Justification"/>
    <rdf:type rdf:resource="http://www.w3.org/2002/07/owl#Class"/>
    <rdfs:isDefinedBy rdf:resource="https://w3id.org/dpv/justifications/owl#"/>
    <skos:prefLabel xml:lang="en">Legally Exempted</skos:prefLabel>
    <sw:term_status xml:lang="en">accepted</sw:term_status>
    <dct:contributor rdf:nodeID="person-harshvardhan-j-pandit"/>
    <dct:contributor rdf:nodeID="person-beatriz-esteves"/>
    <dct:created rdf:datatype="http://www.w3.org/2001/XMLSchema#date">2024-04-21</dct:created>
    <rdfs:subClassOf rdf:resource="https://w3id.org/dpv/justifications/owl#LegalProcessImpaired"/>
  </rdf:Description>
  <rdf:Description rdf:about="https://w3id.org/dpv/justifications/owl#HighVolumeOfProcesses">
    <rdf:type rdf:resource="http://www.w3.org/2000/01/rdf-schema#Class"/>
    <rdf:type rdf:resource="https://w3id.org/dpv/owl#Justification"/>
    <rdf:type rdf:resource="http://www.w3.org/2002/07/owl#Class"/>
    <rdfs:isDefinedBy rdf:resource="https://w3id.org/dpv/justifications/owl#"/>
    <sw:term_status xml:lang="en">accepted</sw:term_status>
    <dct:contributor rdf:nodeID="person-harshvardhan-j-pandit"/>
    <dct:contributor rdf:nodeID="person-beatriz-esteves"/>
    <dct:created rdf:datatype="http://www.w3.org/2001/XMLSchema#date">2024-04-21</dct:created>
    <skos:definition xml:lang="en">Justification that the process is delayed due to high volume of similar processes required to be fulfilled</skos:definition>
    <skos:prefLabel xml:lang="en">High Volume Of Processes</skos:prefLabel>
    <rdfs:subClassOf rdf:resource="https://w3id.org/dpv/justifications/owl#DelayJustification"/>
  </rdf:Description>
  <rdf:Description rdf:about="https://w3id.org/dpv/justifications/owl#Objection">
    <rdf:type rdf:resource="https://w3id.org/dpv/owl#Justification"/>
    <rdf:type rdf:resource="http://www.w3.org/2000/01/rdf-schema#Class"/>
    <rdf:type rdf:resource="http://www.w3.org/2002/07/owl#Class"/>
    <rdfs:isDefinedBy rdf:resource="https://w3id.org/dpv/justifications/owl#"/>
    <skos:prefLabel xml:lang="en">Objection</skos:prefLabel>
    <dct:contributor rdf:nodeID="person-harshvardhan-j-pandit"/>
    <dct:contributor rdf:nodeID="person-beatriz-esteves"/>
    <dct:created rdf:datatype="http://www.w3.org/2001/XMLSchema#date">2024-04-21</dct:created>
    <sw:term_status xml:lang="en">accepted</sw:term_status>
    <skos:definition xml:lang="en">Justification that the process should be carried out due to specified objection(s)</skos:definition>
    <rdfs:subClassOf rdf:resource="https://w3id.org/dpv/justifications/owl#ExerciseJustification"/>
  </rdf:Description>
  <rdf:Description rdf:about="https://w3id.org/dpv/justifications/owl#OfficialStatisticsImpaired">
    <dct:contributor rdf:nodeID="person-harshvardhan-j-pandit"/>
    <dct:contributor rdf:nodeID="person-beatriz-esteves"/>
    <skos:definition xml:lang="en">Justification that the process could not be fulfilled or was not successful because it would interfere with official statistics</skos:definition>
    <sw:term_status xml:lang="en">accepted</sw:term_status>
    <rdf:type rdf:resource="https://w3id.org/dpv/owl#Justification"/>
    <rdf:type rdf:resource="http://www.w3.org/2000/01/rdf-schema#Class"/>
    <rdf:type rdf:resource="http://www.w3.org/2002/07/owl#Class"/>
    <dct:created rdf:datatype="http://www.w3.org/2001/XMLSchema#date">2024-04-21</dct:created>
    <skos:prefLabel xml:lang="en">Official Statistics Impaired</skos:prefLabel>
    <rdfs:isDefinedBy rdf:resource="https://w3id.org/dpv/justifications/owl#"/>
    <rdfs:subClassOf rdf:resource="https://w3id.org/dpv/justifications/owl#LegalProcessImpaired"/>
  </rdf:Description>
  <rdf:Description rdf:about="https://w3id.org/dpv/justifications/owl#serialisation-html">
    <dct:format rdf:resource="https://www.iana.org/assignments/media-types/text/html"/>
    <profile:hasArtifact rdf:resource="https://w3id.org/dpv/justifications/justifications-owl.html"/>
    <dct:title>Justification Concepts - HTML serialisation</dct:title>
    <profile:hasRole rdf:resource="http://www.w3.org/ns/dx/prof/role/specification"/>
    <rdf:type rdf:resource="http://www.w3.org/ns/dx/prof/ResourceDescriptor"/>
    <dct:conformsTo rdf:resource="https://www.w3.org/TR/html/"/>
  </rdf:Description>
  <rdf:Description rdf:about="https://w3id.org/dpv/justifications/owl#LegalClaimEstablishmentImpaired">
    <dct:modified rdf:datatype="http://www.w3.org/2001/XMLSchema#date">2024-12-17</dct:modified>
    <rdf:type rdf:resource="https://w3id.org/dpv/owl#Justification"/>
    <rdf:type rdf:resource="http://www.w3.org/2000/01/rdf-schema#Class"/>
    <rdf:type rdf:resource="http://www.w3.org/2002/07/owl#Class"/>
    <dct:contributor rdf:nodeID="person-beatriz-esteves"/>
    <dct:contributor rdf:nodeID="person-harshvardhan-j-pandit"/>
    <sw:term_status xml:lang="en">modified</sw:term_status>
    <skos:definition xml:lang="en">Justification that the process could not be fulfilled or was not successful because it would interfere with the establishment of legal claims</skos:definition>
    <skos:prefLabel xml:lang="en">Legal Claim Establishment Impaired</skos:prefLabel>
    <rdfs:isDefinedBy rdf:resource="https://w3id.org/dpv/justifications/owl#"/>
    <dct:created rdf:datatype="http://www.w3.org/2001/XMLSchema#date">2024-04-21</dct:created>
    <rdfs:subClassOf rdf:resource="https://w3id.org/dpv/justifications/owl#LegalClaimImpaired"/>
  </rdf:Description>
  <rdf:Description rdf:about="https://w3id.org/dpv/justifications/owl#ExerciseJustification">
    <dct:contributor rdf:nodeID="person-beatriz-esteves"/>
    <dct:contributor rdf:nodeID="person-harshvardhan-j-pandit"/>
    <skos:definition xml:lang="en">Justification for why the process should be carried out</skos:definition>
    <rdfs:subClassOf rdf:resource="https://w3id.org/dpv/owl#Justification"/>
    <skos:prefLabel xml:lang="en">Exercise Justification</skos:prefLabel>
    <rdf:type rdf:resource="http://www.w3.org/2000/01/rdf-schema#Class"/>
    <rdf:type rdf:resource="http://www.w3.org/2002/07/owl#Class"/>
    <rdfs:isDefinedBy rdf:resource="https://w3id.org/dpv/justifications/owl#"/>
    <sw:term_status xml:lang="en">accepted</sw:term_status>
    <dct:created rdf:datatype="http://www.w3.org/2001/XMLSchema#date">2024-04-21</dct:created>
  </rdf:Description>
  <rdf:Description rdf:about="https://w3id.org/dpv/justifications/owl#EthicsBreachDetectionImpaired">
    <dct:created rdf:datatype="http://www.w3.org/2001/XMLSchema#date">2024-04-21</dct:created>
    <rdfs:isDefinedBy rdf:resource="https://w3id.org/dpv/justifications/owl#"/>
    <skos:prefLabel xml:lang="en">Ethics Breach Detection Impaired</skos:prefLabel>
    <skos:definition xml:lang="en">Justification that the process could not be fulfilled or was not successful because it would interfere with the detection of breaches of ethics for regulated professions</skos:definition>
    <rdf:type rdf:resource="http://www.w3.org/2000/01/rdf-schema#Class"/>
    <rdf:type rdf:resource="https://w3id.org/dpv/owl#Justification"/>
    <rdf:type rdf:resource="http://www.w3.org/2002/07/owl#Class"/>
    <sw:term_status xml:lang="en">accepted</sw:term_status>
    <dct:contributor rdf:nodeID="person-harshvardhan-j-pandit"/>
    <dct:contributor rdf:nodeID="person-beatriz-esteves"/>
    <rdfs:subClassOf rdf:resource="https://w3id.org/dpv/justifications/owl#EthicsProcedureImpaired"/>
  </rdf:Description>
  <rdf:Description rdf:about="https://w3id.org/dpv/justifications/owl#CrimeProsecutionImpaired">
    <dct:contributor rdf:nodeID="person-harshvardhan-j-pandit"/>
    <dct:contributor rdf:nodeID="person-beatriz-esteves"/>
    <rdf:type rdf:resource="https://w3id.org/dpv/owl#Justification"/>
    <rdf:type rdf:resource="http://www.w3.org/2000/01/rdf-schema#Class"/>
    <rdf:type rdf:resource="http://www.w3.org/2002/07/owl#Class"/>
    <dct:created rdf:datatype="http://www.w3.org/2001/XMLSchema#date">2024-04-21</dct:created>
    <skos:definition xml:lang="en">Justification that the process could not be fulfilled or was not successful because it would interfere with the prosecution of criminal offences</skos:definition>
    <rdfs:isDefinedBy rdf:resource="https://w3id.org/dpv/justifications/owl#"/>
    <skos:prefLabel xml:lang="en">Crime Prosecution Impaired</skos:prefLabel>
    <sw:term_status xml:lang="en">accepted</sw:term_status>
    <rdfs:subClassOf rdf:resource="https://w3id.org/dpv/justifications/owl#LegalProcessImpaired"/>
    <rdfs:subClassOf rdf:resource="https://w3id.org/dpv/justifications/owl#SecurityImpaired"/>
  </rdf:Description>
  <rdf:Description rdf:about="https://w3id.org/dpv/justifications/owl#LegalObligation">
    <skos:definition xml:lang="en">Justification that the process should be carried out due to it being a legal obligation</skos:definition>
    <rdf:type rdf:resource="http://www.w3.org/2000/01/rdf-schema#Class"/>
    <rdf:type rdf:resource="https://w3id.org/dpv/owl#Justification"/>
    <rdf:type rdf:resource="http://www.w3.org/2002/07/owl#Class"/>
    <rdfs:isDefinedBy rdf:resource="https://w3id.org/dpv/justifications/owl#"/>
    <dct:contributor rdf:nodeID="person-harshvardhan-j-pandit"/>
    <dct:contributor rdf:nodeID="person-beatriz-esteves"/>
    <skos:prefLabel xml:lang="en">Legal Obligation</skos:prefLabel>
    <sw:term_status xml:lang="en">accepted</sw:term_status>
    <dct:created rdf:datatype="http://www.w3.org/2001/XMLSchema#date">2024-04-21</dct:created>
    <rdfs:subClassOf rdf:resource="https://w3id.org/dpv/justifications/owl#ExerciseJustification"/>
  </rdf:Description>
  <rdf:Description rdf:about="https://w3id.org/dpv/justifications/owl#LegalClaimDefenceImpaired">
    <dct:contributor rdf:nodeID="person-beatriz-esteves"/>
    <dct:contributor rdf:nodeID="person-harshvardhan-j-pandit"/>
    <skos:prefLabel xml:lang="en">Legal Claim Defence Impaired</skos:prefLabel>
    <sw:term_status xml:lang="en">modified</sw:term_status>
    <dct:created rdf:datatype="http://www.w3.org/2001/XMLSchema#date">2024-04-21</dct:created>
    <skos:definition xml:lang="en">Justification that the process could not be fulfilled or was not successful because it would interfere with the defence of legal claims</skos:definition>
    <dct:modified rdf:datatype="http://www.w3.org/2001/XMLSchema#date">2024-12-17</dct:modified>
    <rdf:type rdf:resource="http://www.w3.org/2000/01/rdf-schema#Class"/>
    <rdf:type rdf:resource="https://w3id.org/dpv/owl#Justification"/>
    <rdf:type rdf:resource="http://www.w3.org/2002/07/owl#Class"/>
    <rdfs:isDefinedBy rdf:resource="https://w3id.org/dpv/justifications/owl#"/>
    <rdfs:subClassOf rdf:resource="https://w3id.org/dpv/justifications/owl#LegalClaimImpaired"/>
  </rdf:Description>
  <rdf:Description rdf:about="https://w3id.org/dpv/justifications/owl#EthicsProcedureImpaired">
    <rdfs:isDefinedBy rdf:resource="https://w3id.org/dpv/justifications/owl#"/>
    <dct:contributor rdf:nodeID="person-harshvardhan-j-pandit"/>
    <dct:contributor rdf:nodeID="person-beatriz-esteves"/>
    <skos:prefLabel xml:lang="en">Ethics Procedure Impaired</skos:prefLabel>
    <sw:term_status xml:lang="en">accepted</sw:term_status>
    <rdf:type rdf:resource="https://w3id.org/dpv/owl#Justification"/>
    <rdf:type rdf:resource="http://www.w3.org/2000/01/rdf-schema#Class"/>
    <rdf:type rdf:resource="http://www.w3.org/2002/07/owl#Class"/>
    <dct:created rdf:datatype="http://www.w3.org/2001/XMLSchema#date">2024-04-21</dct:created>
    <skos:definition xml:lang="en">Justification that the process could not be fulfilled or was not successful because it would compromise ethics or ethics procedures</skos:definition>
    <rdfs:subClassOf rdf:resource="https://w3id.org/dpv/justifications/owl#NonFulfilmentJustification"/>
  </rdf:Description>
  <rdf:Description rdf:about="https://w3id.org/dpv/justifications/owl#CrimePenaltyExecutionImpaired">
    <rdf:type rdf:resource="https://w3id.org/dpv/owl#Justification"/>
    <rdf:type rdf:resource="http://www.w3.org/2000/01/rdf-schema#Class"/>
    <rdf:type rdf:resource="http://www.w3.org/2002/07/owl#Class"/>
    <skos:prefLabel xml:lang="en">Crime Penalty Execution Impaired</skos:prefLabel>
    <sw:term_status xml:lang="en">accepted</sw:term_status>
    <dct:contributor rdf:nodeID="person-harshvardhan-j-pandit"/>
    <dct:contributor rdf:nodeID="person-beatriz-esteves"/>
    <dct:created rdf:datatype="http://www.w3.org/2001/XMLSchema#date">2024-04-21</dct:created>
    <rdfs:isDefinedBy rdf:resource="https://w3id.org/dpv/justifications/owl#"/>
    <skos:definition xml:lang="en">Justification that the process could not be fulfilled or was not successful because it would interfere with the execution of criminal penalties</skos:definition>
    <rdfs:subClassOf rdf:resource="https://w3id.org/dpv/justifications/owl#SecurityImpaired"/>
    <rdfs:subClassOf rdf:resource="https://w3id.org/dpv/justifications/owl#LegalProcessImpaired"/>
  </rdf:Description>
  <rdf:Description rdf:about="https://w3id.org/dpv/justifications/owl#ProcessFrivolous">
    <sw:term_status xml:lang="en">accepted</sw:term_status>
    <rdf:type rdf:resource="https://w3id.org/dpv/owl#Justification"/>
    <rdf:type rdf:resource="http://www.w3.org/2000/01/rdf-schema#Class"/>
    <rdf:type rdf:resource="http://www.w3.org/2002/07/owl#Class"/>
    <dct:contributor rdf:nodeID="person-harshvardhan-j-pandit"/>
    <dct:contributor rdf:nodeID="person-beatriz-esteves"/>
    <dct:created rdf:datatype="http://www.w3.org/2001/XMLSchema#date">2024-04-21</dct:created>
    <skos:prefLabel xml:lang="en">Process Frivolous</skos:prefLabel>
    <skos:definition xml:lang="en">Justification that the process could not be fulfilled or was not successful because it was found to be based on frivolous reasons</skos:definition>
    <rdfs:isDefinedBy rdf:resource="https://w3id.org/dpv/justifications/owl#"/>
    <rdfs:subClassOf rdf:resource="https://w3id.org/dpv/justifications/owl#ProcessRejected"/>
  </rdf:Description>
  <rdf:Description rdf:about="https://w3id.org/dpv/guides">
    <dct:format rdf:resource="https://www.iana.org/assignments/media-types/text/html"/>
    <profile:hasRole rdf:resource="http://www.w3.org/ns/dx/prof/role/guidance"/>
    <dct:title>Guides for Data Privacy Vocabulary</dct:title>
    <rdf:type rdf:resource="http://www.w3.org/ns/dx/prof/ResourceDescriptor"/>
    <dct:conformsTo rdf:resource="https://www.w3.org/TR/html/"/>
    <profile:hasArtifact rdf:resource="https://w3id.org/dpv/guides"/>
  </rdf:Description>
  <rdf:Description rdf:about="https://w3id.org/dpv/justifications/owl#LegalObligationImpaired">
    <rdf:type rdf:resource="https://w3id.org/dpv/owl#Justification"/>
    <rdf:type rdf:resource="http://www.w3.org/2000/01/rdf-schema#Class"/>
    <rdf:type rdf:resource="http://www.w3.org/2002/07/owl#Class"/>
    <dct:created rdf:datatype="http://www.w3.org/2001/XMLSchema#date">2024-12-17</dct:created>
    <rdfs:isDefinedBy rdf:resource="https://w3id.org/dpv/justifications/owl#"/>
    <skos:definition xml:lang="en">Justification that the process could not be fulfilled as it would impair or conflict with a legal obligation</skos:definition>
    <skos:prefLabel xml:lang="en">Required for Legal Obligation</skos:prefLabel>
    <sw:term_status xml:lang="en">accepted</sw:term_status>
    <dct:contributor rdf:nodeID="person-harshvardhan-j-pandit"/>
    <rdfs:subClassOf rdf:resource="https://w3id.org/dpv/justifications/owl#LegalProcessImpaired"/>
  </rdf:Description>
  <rdf:Description rdf:about="https://w3id.org/dpv/justifications/owl#OfficialAuthorityExerciseImpaired">
    <rdfs:isDefinedBy rdf:resource="https://w3id.org/dpv/justifications/owl#"/>
    <rdf:type rdf:resource="http://www.w3.org/2000/01/rdf-schema#Class"/>
    <rdf:type rdf:resource="https://w3id.org/dpv/owl#Justification"/>
    <rdf:type rdf:resource="http://www.w3.org/2002/07/owl#Class"/>
    <sw:term_status xml:lang="en">accepted</sw:term_status>
    <skos:prefLabel xml:lang="en">Official Authority Exercise Impaired</skos:prefLabel>
    <dct:contributor rdf:nodeID="person-harshvardhan-j-pandit"/>
    <dct:contributor rdf:nodeID="person-beatriz-esteves"/>
    <dct:created rdf:datatype="http://www.w3.org/2001/XMLSchema#date">2024-04-21</dct:created>
    <skos:definition xml:lang="en">Justification that the process could not be fulfilled or was not successful because it would interfere with the exercise of official authorities</skos:definition>
    <rdfs:subClassOf rdf:resource="https://w3id.org/dpv/justifications/owl#LegalProcessImpaired"/>
  </rdf:Description>
  <rdf:Description rdf:nodeID="person-paul-ryan">
    <rdf:type rdf:resource="http://xmlns.com/foaf/0.1/Person"/>
    <rdf:type rdf:resource="http://purl.org/dc/terms/Agent"/>
    <scoro:hasORCID>0000-0003-0770-2737</scoro:hasORCID>
    <org:memberOf rdf:nodeID="org-uniphar-plc"/>
    <foaf:name>Paul Ryan</foaf:name>
  </rdf:Description>
  <rdf:Description rdf:about="https://w3id.org/dpv/justifications/owl#CrimeDetectionImpaired">
    <rdf:type rdf:resource="http://www.w3.org/2000/01/rdf-schema#Class"/>
    <rdf:type rdf:resource="https://w3id.org/dpv/owl#Justification"/>
    <rdf:type rdf:resource="http://www.w3.org/2002/07/owl#Class"/>
    <skos:prefLabel xml:lang="en">Crime Detection Impaired</skos:prefLabel>
    <rdfs:isDefinedBy rdf:resource="https://w3id.org/dpv/justifications/owl#"/>
    <dct:contributor rdf:nodeID="person-harshvardhan-j-pandit"/>
    <dct:contributor rdf:nodeID="person-beatriz-esteves"/>
    <dct:created rdf:datatype="http://www.w3.org/2001/XMLSchema#date">2024-04-21</dct:created>
    <sw:term_status xml:lang="en">accepted</sw:term_status>
    <skos:definition xml:lang="en">Justification that the process could not be fulfilled or was not successful because it would interfere with the detection of criminal offences</skos:definition>
    <rdfs:subClassOf rdf:resource="https://w3id.org/dpv/justifications/owl#LegalProcessImpaired"/>
    <rdfs:subClassOf rdf:resource="https://w3id.org/dpv/justifications/owl#SecurityImpaired"/>
  </rdf:Description>
  <rdf:Description rdf:about="https://w3id.org/dpv/examples">
    <rdf:type rdf:resource="http://www.w3.org/ns/dx/prof/ResourceDescriptor"/>
    <dct:title>Examples</dct:title>
    <dct:conformsTo rdf:resource="https://www.w3.org/TR/html/"/>
    <dct:format rdf:resource="https://www.iana.org/assignments/media-types/text/html"/>
    <profile:hasRole rdf:resource="http://www.w3.org/ns/dx/prof/role/guidance"/>
    <profile:hasArtifact rdf:resource="https://w3id.org/dpv/examples"/>
  </rdf:Description>
  <rdf:Description rdf:about="https://w3id.org/dpv/justifications/owl#PublicInterestArchivingImpaired">
    <dct:contributor rdf:nodeID="person-harshvardhan-j-pandit"/>
    <dct:contributor rdf:nodeID="person-beatriz-esteves"/>
    <rdf:type rdf:resource="https://w3id.org/dpv/owl#Justification"/>
    <rdf:type rdf:resource="http://www.w3.org/2000/01/rdf-schema#Class"/>
    <rdf:type rdf:resource="http://www.w3.org/2002/07/owl#Class"/>
    <skos:definition xml:lang="en">Justification that the process could not be fulfilled or was not successful because it impairs archiving for public interest</skos:definition>
    <dct:created rdf:datatype="http://www.w3.org/2001/XMLSchema#date">2024-04-21</dct:created>
    <sw:term_status xml:lang="en">accepted</sw:term_status>
    <skos:prefLabel xml:lang="en">Public Interest Archiving Impaired</skos:prefLabel>
    <rdfs:isDefinedBy rdf:resource="https://w3id.org/dpv/justifications/owl#"/>
    <rdfs:subClassOf rdf:resource="https://w3id.org/dpv/justifications/owl#LegalProcessImpaired"/>
  </rdf:Description>
  <rdf:Description rdf:about="https://w3id.org/dpv/justifications/owl#EthicsBreachInvestigationImpaired">
    <rdfs:isDefinedBy rdf:resource="https://w3id.org/dpv/justifications/owl#"/>
    <skos:definition xml:lang="en">Justification that the process could not be fulfilled or was not successful because it would interfere with the investigation of breaches of ethics for regulated professions</skos:definition>
    <skos:prefLabel xml:lang="en">Ethics Breach Investigation Impaired</skos:prefLabel>
    <rdf:type rdf:resource="http://www.w3.org/2000/01/rdf-schema#Class"/>
    <rdf:type rdf:resource="https://w3id.org/dpv/owl#Justification"/>
    <rdf:type rdf:resource="http://www.w3.org/2002/07/owl#Class"/>
    <sw:term_status xml:lang="en">accepted</sw:term_status>
    <dct:contributor rdf:nodeID="person-harshvardhan-j-pandit"/>
    <dct:contributor rdf:nodeID="person-beatriz-esteves"/>
    <dct:created rdf:datatype="http://www.w3.org/2001/XMLSchema#date">2024-04-21</dct:created>
    <rdfs:subClassOf rdf:resource="https://w3id.org/dpv/justifications/owl#EthicsProcedureImpaired"/>
  </rdf:Description>
  <rdf:Description rdf:about="https://w3id.org/dpv/justifications/owl#InformationRequired">
    <sw:term_status xml:lang="en">accepted</sw:term_status>
    <rdf:type rdf:resource="https://w3id.org/dpv/owl#Justification"/>
    <rdf:type rdf:resource="http://www.w3.org/2000/01/rdf-schema#Class"/>
    <rdf:type rdf:resource="http://www.w3.org/2002/07/owl#Class"/>
    <dct:contributor rdf:nodeID="person-beatriz-esteves"/>
    <dct:contributor rdf:nodeID="person-harshvardhan-j-pandit"/>
    <dct:created rdf:datatype="http://www.w3.org/2001/XMLSchema#date">2024-04-21</dct:created>
    <skos:definition xml:lang="en">Justification that the process is delayed due to additional information being required</skos:definition>
    <rdfs:isDefinedBy rdf:resource="https://w3id.org/dpv/justifications/owl#"/>
    <skos:prefLabel xml:lang="en">Information Required</skos:prefLabel>
    <rdfs:subClassOf rdf:resource="https://w3id.org/dpv/justifications/owl#DelayJustification"/>
  </rdf:Description>
  <rdf:Description rdf:about="https://w3id.org/dpv/justifications/owl#ComplexityOfProcess">
    <rdfs:isDefinedBy rdf:resource="https://w3id.org/dpv/justifications/owl#"/>
    <dct:contributor rdf:nodeID="person-harshvardhan-j-pandit"/>
    <dct:contributor rdf:nodeID="person-beatriz-esteves"/>
    <skos:prefLabel xml:lang="en">Complexity Of Process</skos:prefLabel>
    <dct:created rdf:datatype="http://www.w3.org/2001/XMLSchema#date">2024-04-21</dct:created>
    <rdf:type rdf:resource="https://w3id.org/dpv/owl#Justification"/>
    <rdf:type rdf:resource="http://www.w3.org/2000/01/rdf-schema#Class"/>
    <rdf:type rdf:resource="http://www.w3.org/2002/07/owl#Class"/>
    <sw:term_status xml:lang="en">accepted</sw:term_status>
    <skos:definition xml:lang="en">Justification that the process is delayed due to complexity in fulfilling it</skos:definition>
    <rdfs:subClassOf rdf:resource="https://w3id.org/dpv/justifications/owl#DelayJustification"/>
  </rdf:Description>
  <rdf:Description rdf:about="https://w3id.org/dpv/justifications/owl#DelayJustification">
    <rdf:type rdf:resource="http://www.w3.org/2000/01/rdf-schema#Class"/>
    <rdf:type rdf:resource="http://www.w3.org/2002/07/owl#Class"/>
    <sw:term_status xml:lang="en">accepted</sw:term_status>
    <rdfs:isDefinedBy rdf:resource="https://w3id.org/dpv/justifications/owl#"/>
    <dct:contributor rdf:nodeID="person-harshvardhan-j-pandit"/>
    <dct:contributor rdf:nodeID="person-beatriz-esteves"/>
    <skos:definition xml:lang="en">Justification to delay a process</skos:definition>
    <dct:created rdf:datatype="http://www.w3.org/2001/XMLSchema#date">2024-04-21</dct:created>
    <skos:prefLabel xml:lang="en">Delay Justification</skos:prefLabel>
    <rdfs:subClassOf rdf:resource="https://w3id.org/dpv/owl#Justification"/>
  </rdf:Description>
  <rdf:Description rdf:about="https://w3id.org/dpv/primer">
    <dct:title>Primer for Data Privacy Vocabulary</dct:title>
    <rdf:type rdf:resource="http://www.w3.org/ns/dx/prof/ResourceDescriptor"/>
    <dct:conformsTo rdf:resource="https://www.w3.org/TR/html/"/>
    <dct:format rdf:resource="https://www.iana.org/assignments/media-types/text/html"/>
    <profile:hasRole rdf:resource="http://www.w3.org/ns/dx/prof/role/guidance"/>
    <profile:hasArtifact rdf:resource="https://w3id.org/dpv/primer"/>
  </rdf:Description>
  <rdf:Description rdf:about="https://w3id.org/dpv/justifications/owl#EthicsBreachProsecutionImpaired">
    <skos:prefLabel xml:lang="en">Ethics Breach Prosecution Impaired</skos:prefLabel>
    <rdf:type rdf:resource="http://www.w3.org/2000/01/rdf-schema#Class"/>
    <rdf:type rdf:resource="https://w3id.org/dpv/owl#Justification"/>
    <rdf:type rdf:resource="http://www.w3.org/2002/07/owl#Class"/>
    <sw:term_status xml:lang="en">accepted</sw:term_status>
    <rdfs:isDefinedBy rdf:resource="https://w3id.org/dpv/justifications/owl#"/>
    <skos:definition xml:lang="en">Justification that the process could not be fulfilled or was not successful because it would interfere with the prosecution of breaches of ethics for regulated professions</skos:definition>
    <dct:contributor rdf:nodeID="person-harshvardhan-j-pandit"/>
    <dct:contributor rdf:nodeID="person-beatriz-esteves"/>
    <dct:created rdf:datatype="http://www.w3.org/2001/XMLSchema#date">2024-04-21</dct:created>
    <rdfs:subClassOf rdf:resource="https://w3id.org/dpv/justifications/owl#EthicsProcedureImpaired"/>
  </rdf:Description>
  <rdf:Description rdf:about="https://w3id.org/dpv/justifications/owl#ProcessMalicious">
    <rdf:type rdf:resource="http://www.w3.org/2000/01/rdf-schema#Class"/>
    <rdf:type rdf:resource="https://w3id.org/dpv/owl#Justification"/>
    <rdf:type rdf:resource="http://www.w3.org/2002/07/owl#Class"/>
    <rdfs:isDefinedBy rdf:resource="https://w3id.org/dpv/justifications/owl#"/>
    <dct:contributor rdf:nodeID="person-harshvardhan-j-pandit"/>
    <dct:contributor rdf:nodeID="person-beatriz-esteves"/>
    <sw:term_status xml:lang="en">accepted</sw:term_status>
    <dct:created rdf:datatype="http://www.w3.org/2001/XMLSchema#date">2024-04-21</dct:created>
    <skos:definition xml:lang="en">Justification that the process could not be fulfilled or was not successful because it was found to be malicious e.g. with intent to cause disruption or harassment</skos:definition>
    <skos:prefLabel xml:lang="en">Process Malicious</skos:prefLabel>
    <rdfs:subClassOf rdf:resource="https://w3id.org/dpv/justifications/owl#ProcessRejected"/>
  </rdf:Description>
  <rdf:Description rdf:about="https://w3id.org/dpv/justifications/owl#serialisation-jsonld">
    <profile:hasRole rdf:resource="http://www.w3.org/ns/dx/prof/role/vocabulary"/>
    <rdf:type rdf:resource="http://www.w3.org/ns/dx/prof/ResourceDescriptor"/>
    <dct:format rdf:resource="https://www.iana.org/assignments/media-types/application/ld+json"/>
    <dct:conformsTo rdf:resource="https://www.w3.org/TR/json-ld11/"/>
    <profile:hasArtifact rdf:resource="https://w3id.org/dpv/justifications/justifications-owl.jsonld"/>
    <dct:title>Justification Concepts - JSON-LD serialisation</dct:title>
  </rdf:Description>
  <rdf:Description rdf:about="https://w3id.org/dpv/justifications/owl#DataSubjectProtectionImpaired">
    <dct:created rdf:datatype="http://www.w3.org/2001/XMLSchema#date">2024-04-21</dct:created>
    <sw:term_status xml:lang="en">accepted</sw:term_status>
    <rdf:type rdf:resource="https://w3id.org/dpv/owl#Justification"/>
    <rdf:type rdf:resource="http://www.w3.org/2000/01/rdf-schema#Class"/>
    <rdf:type rdf:resource="http://www.w3.org/2002/07/owl#Class"/>
    <rdfs:isDefinedBy rdf:resource="https://w3id.org/dpv/justifications/owl#"/>
    <skos:definition xml:lang="en">Justification that the process could not be fulfilled or was not successful because it would interfere with the protection of the data subject</skos:definition>
    <skos:prefLabel xml:lang="en">Data Subject Protection Impaired</skos:prefLabel>
    <dct:contributor rdf:nodeID="person-harshvardhan-j-pandit"/>
    <dct:contributor rdf:nodeID="person-beatriz-esteves"/>
    <rdfs:subClassOf rdf:resource="https://w3id.org/dpv/justifications/owl#SecurityImpaired"/>
    <rdfs:subClassOf rdf:resource="https://w3id.org/dpv/justifications/owl#LegalProcessImpaired"/>
  </rdf:Description>
  <rdf:Description rdf:about="https://w3id.org/dpv/justifications/owl#ConsentProvided">
    <rdf:type rdf:resource="http://www.w3.org/2000/01/rdf-schema#Class"/>
    <rdf:type rdf:resource="https://w3id.org/dpv/owl#Justification"/>
    <rdf:type rdf:resource="http://www.w3.org/2002/07/owl#Class"/>
    <rdfs:isDefinedBy rdf:resource="https://w3id.org/dpv/justifications/owl#"/>
    <skos:definition xml:lang="en">Justification that the process could not be fulfilled or was not successful because it is based on (a previously given) consent</skos:definition>
    <skos:prefLabel xml:lang="en">Consent Provided</skos:prefLabel>
    <sw:term_status xml:lang="en">accepted</sw:term_status>
    <dct:contributor rdf:nodeID="person-harshvardhan-j-pandit"/>
    <dct:contributor rdf:nodeID="person-beatriz-esteves"/>
    <dct:created rdf:datatype="http://www.w3.org/2001/XMLSchema#date">2024-04-21</dct:created>
    <rdfs:subClassOf rdf:resource="https://w3id.org/dpv/justifications/owl#NonFulfilmentJustification"/>
  </rdf:Description>
  <rdf:Description rdf:about="https://w3id.org/dpv/justifications/owl#RiskMitigated">
    <rdf:type rdf:resource="https://w3id.org/dpv/owl#Justification"/>
    <rdf:type rdf:resource="http://www.w3.org/2000/01/rdf-schema#Class"/>
    <rdf:type rdf:resource="http://www.w3.org/2002/07/owl#Class"/>
    <dct:contributor rdf:nodeID="person-harshvardhan-j-pandit"/>
    <skos:definition xml:lang="en">Justification that the process is not required as the risks have been effectively mitigated by technical and organisational measures</skos:definition>
    <skos:prefLabel xml:lang="en">Risk Mitigated</skos:prefLabel>
    <dct:created rdf:datatype="http://www.w3.org/2001/XMLSchema#date">2024-12-17</dct:created>
    <rdfs:isDefinedBy rdf:resource="https://w3id.org/dpv/justifications/owl#"/>
    <sw:term_status xml:lang="en">accepted</sw:term_status>
    <rdfs:subClassOf rdf:resource="https://w3id.org/dpv/justifications/owl#NotRequiredJustification"/>
  </rdf:Description>
  <rdf:Description rdf:about="https://w3id.org/dpv/justifications/owl#PublicSecurityImpaired">
    <rdf:type rdf:resource="http://www.w3.org/2000/01/rdf-schema#Class"/>
    <rdf:type rdf:resource="https://w3id.org/dpv/owl#Justification"/>
    <rdf:type rdf:resource="http://www.w3.org/2002/07/owl#Class"/>
    <rdfs:isDefinedBy rdf:resource="https://w3id.org/dpv/justifications/owl#"/>
    <skos:prefLabel xml:lang="en">Public Security Impaired</skos:prefLabel>
    <sw:term_status xml:lang="en">accepted</sw:term_status>
    <skos:definition xml:lang="en">Justification that the process could not be fulfilled or was not successful because it would interfere with necessary tasks to safeguard public security</skos:definition>
    <dct:contributor rdf:nodeID="person-harshvardhan-j-pandit"/>
    <dct:contributor rdf:nodeID="person-beatriz-esteves"/>
    <dct:created rdf:datatype="http://www.w3.org/2001/XMLSchema#date">2024-04-21</dct:created>
    <rdfs:subClassOf rdf:resource="https://w3id.org/dpv/justifications/owl#LegalProcessImpaired"/>
    <rdfs:subClassOf rdf:resource="https://w3id.org/dpv/justifications/owl#SecurityImpaired"/>
  </rdf:Description>
  <rdf:Description rdf:about="https://w3id.org/dpv/justifications/owl#NationalSecurityImpaired">
    <dct:contributor rdf:nodeID="person-harshvardhan-j-pandit"/>
    <dct:contributor rdf:nodeID="person-beatriz-esteves"/>
    <rdf:type rdf:resource="https://w3id.org/dpv/owl#Justification"/>
    <rdf:type rdf:resource="http://www.w3.org/2000/01/rdf-schema#Class"/>
    <rdf:type rdf:resource="http://www.w3.org/2002/07/owl#Class"/>
    <dct:created rdf:datatype="http://www.w3.org/2001/XMLSchema#date">2024-04-21</dct:created>
    <rdfs:isDefinedBy rdf:resource="https://w3id.org/dpv/justifications/owl#"/>
    <skos:prefLabel xml:lang="en">National Security Impaired</skos:prefLabel>
    <sw:term_status xml:lang="en">accepted</sw:term_status>
    <skos:definition xml:lang="en">Justification that the process could not be fulfilled or was not successful because it would interfere with necessary tasks to safeguard national security</skos:definition>
    <rdfs:subClassOf rdf:resource="https://w3id.org/dpv/justifications/owl#SecurityImpaired"/>
    <rdfs:subClassOf rdf:resource="https://w3id.org/dpv/justifications/owl#LegalProcessImpaired"/>
  </rdf:Description>
  <rdf:Description rdf:about="https://w3id.org/dpv/justifications/owl#JudicialProceedingsImpaired">
    <rdf:type rdf:resource="https://w3id.org/dpv/owl#Justification"/>
    <rdf:type rdf:resource="http://www.w3.org/2000/01/rdf-schema#Class"/>
    <rdf:type rdf:resource="http://www.w3.org/2002/07/owl#Class"/>
    <dct:contributor rdf:nodeID="person-beatriz-esteves"/>
    <dct:contributor rdf:nodeID="person-harshvardhan-j-pandit"/>
    <skos:definition xml:lang="en">Justification that the process could not be fulfilled or was not successful because it would interfere with the protection of judicial independence and proceedings</skos:definition>
    <skos:prefLabel xml:lang="en">Judicial Proceedings Impaired</skos:prefLabel>
    <rdfs:isDefinedBy rdf:resource="https://w3id.org/dpv/justifications/owl#"/>
    <dct:created rdf:datatype="http://www.w3.org/2001/XMLSchema#date">2024-04-21</dct:created>
    <sw:term_status xml:lang="en">accepted</sw:term_status>
    <rdfs:subClassOf rdf:resource="https://w3id.org/dpv/justifications/owl#LegalProcessImpaired"/>
  </rdf:Description>
  <rdf:Description rdf:about="https://w3id.org/dpv/justifications/owl#ContestAccuracy">
    <rdf:type rdf:resource="http://www.w3.org/2000/01/rdf-schema#Class"/>
    <rdf:type rdf:resource="https://w3id.org/dpv/owl#Justification"/>
    <rdf:type rdf:resource="http://www.w3.org/2002/07/owl#Class"/>
    <sw:term_status xml:lang="en">accepted</sw:term_status>
    <skos:prefLabel xml:lang="en">Contest Accuracy</skos:prefLabel>
    <rdfs:isDefinedBy rdf:resource="https://w3id.org/dpv/justifications/owl#"/>
    <dct:contributor rdf:nodeID="person-harshvardhan-j-pandit"/>
    <dct:contributor rdf:nodeID="person-beatriz-esteves"/>
    <dct:created rdf:datatype="http://www.w3.org/2001/XMLSchema#date">2024-04-21</dct:created>
    <skos:definition xml:lang="en">Justification that the process should be carried out due it being an objection to the accuracy e.g. of system, outputs, data</skos:definition>
    <rdfs:subClassOf rdf:resource="https://w3id.org/dpv/justifications/owl#Objection"/>
  </rdf:Description>
  <rdf:Description rdf:about="https://w3id.org/dpv/justifications/owl#LegalProcessImpaired">
    <skos:definition xml:lang="en">Justification that the process could not be fulfilled as it impairs or interferes with a legal or official process or procedure</skos:definition>
    <dct:contributor rdf:nodeID="person-harshvardhan-j-pandit"/>
    <dct:contributor rdf:nodeID="person-beatriz-esteves"/>
    <dct:created rdf:datatype="http://www.w3.org/2001/XMLSchema#date">2024-04-21</dct:created>
    <sw:term_status xml:lang="en">accepted</sw:term_status>
    <rdf:type rdf:resource="https://w3id.org/dpv/owl#Justification"/>
    <rdf:type rdf:resource="http://www.w3.org/2000/01/rdf-schema#Class"/>
    <rdf:type rdf:resource="http://www.w3.org/2002/07/owl#Class"/>
    <skos:prefLabel xml:lang="en">Legal Process Impaired</skos:prefLabel>
    <rdfs:isDefinedBy rdf:resource="https://w3id.org/dpv/justifications/owl#"/>
    <rdfs:subClassOf rdf:resource="https://w3id.org/dpv/justifications/owl#NonFulfilmentJustification"/>
  </rdf:Description>
  <rdf:Description rdf:about="https://w3id.org/dpv/justifications/owl#RightsFreedomsImpactUnlikely">
    <skos:prefLabel xml:lang="en">Rights Freedoms Impact Unlikely</skos:prefLabel>
    <rdf:type rdf:resource="http://www.w3.org/2000/01/rdf-schema#Class"/>
    <rdf:type rdf:resource="https://w3id.org/dpv/owl#Justification"/>
    <rdf:type rdf:resource="http://www.w3.org/2002/07/owl#Class"/>
    <rdfs:isDefinedBy rdf:resource="https://w3id.org/dpv/justifications/owl#"/>
    <skos:definition xml:lang="en">Justification that the process is not required as it is considered to be an unlikely impact on rights and freedoms</skos:definition>
    <sw:term_status xml:lang="en">accepted</sw:term_status>
    <dct:contributor rdf:nodeID="person-harshvardhan-j-pandit"/>
    <dct:contributor rdf:nodeID="person-beatriz-esteves"/>
    <dct:created rdf:datatype="http://www.w3.org/2001/XMLSchema#date">2024-04-21</dct:created>
    <rdfs:subClassOf rdf:resource="https://w3id.org/dpv/justifications/owl#NotRequiredJustification"/>
  </rdf:Description>
  <rdf:Description rdf:about="https://w3id.org/dpv/justifications/owl#ContractPerformanceNecessity">
    <skos:definition xml:lang="en">Justification that the process could not be fulfilled or was not successful because it is necessary for the performance of a contract</skos:definition>
    <rdf:type rdf:resource="http://www.w3.org/2000/01/rdf-schema#Class"/>
    <rdf:type rdf:resource="https://w3id.org/dpv/owl#Justification"/>
    <rdf:type rdf:resource="http://www.w3.org/2002/07/owl#Class"/>
    <rdfs:isDefinedBy rdf:resource="https://w3id.org/dpv/justifications/owl#"/>
    <dct:contributor rdf:nodeID="person-harshvardhan-j-pandit"/>
    <dct:contributor rdf:nodeID="person-beatriz-esteves"/>
    <sw:term_status xml:lang="en">accepted</sw:term_status>
    <dct:created rdf:datatype="http://www.w3.org/2001/XMLSchema#date">2024-04-21</dct:created>
    <skos:prefLabel xml:lang="en">Contract Performance Necessity</skos:prefLabel>
    <rdfs:subClassOf rdf:resource="https://w3id.org/dpv/justifications/owl#LegalProcessImpaired"/>
  </rdf:Description>
  <rdf:Description rdf:about="https://w3id.org/dpv/justifications/owl#IdentityVerificationFailure">
    <dct:contributor rdf:nodeID="person-harshvardhan-j-pandit"/>
    <dct:contributor rdf:nodeID="person-beatriz-esteves"/>
    <sw:term_status xml:lang="en">accepted</sw:term_status>
    <rdf:type rdf:resource="https://w3id.org/dpv/owl#Justification"/>
    <rdf:type rdf:resource="http://www.w3.org/2000/01/rdf-schema#Class"/>
    <rdf:type rdf:resource="http://www.w3.org/2002/07/owl#Class"/>
    <dct:created rdf:datatype="http://www.w3.org/2001/XMLSchema#date">2024-04-21</dct:created>
    <skos:prefLabel xml:lang="en">Identity Verification Failure</skos:prefLabel>
    <skos:definition xml:lang="en">Justification that the process could not be fulfilled or was not successful because identity verification failed</skos:definition>
    <rdfs:isDefinedBy rdf:resource="https://w3id.org/dpv/justifications/owl#"/>
    <rdfs:subClassOf rdf:resource="https://w3id.org/dpv/justifications/owl#LegalProcessImpaired"/>
    <rdfs:subClassOf rdf:resource="https://w3id.org/dpv/justifications/owl#SecurityImpaired"/>
  </rdf:Description>
  <rdf:Description rdf:about="https://w3id.org/dpv/justifications/owl#CrimeInvestigationImpaired">
    <rdf:type rdf:resource="http://www.w3.org/2000/01/rdf-schema#Class"/>
    <rdf:type rdf:resource="https://w3id.org/dpv/owl#Justification"/>
    <rdf:type rdf:resource="http://www.w3.org/2002/07/owl#Class"/>
    <rdfs:isDefinedBy rdf:resource="https://w3id.org/dpv/justifications/owl#"/>
    <dct:contributor rdf:nodeID="person-harshvardhan-j-pandit"/>
    <dct:contributor rdf:nodeID="person-beatriz-esteves"/>
    <skos:prefLabel xml:lang="en">Crime Investigation Impaired</skos:prefLabel>
    <sw:term_status xml:lang="en">accepted</sw:term_status>
    <dct:created rdf:datatype="http://www.w3.org/2001/XMLSchema#date">2024-04-21</dct:created>
    <skos:definition xml:lang="en">Justification that the process could not be fulfilled or was not successful because it would interfere with the investigation of criminal offences</skos:definition>
    <rdfs:subClassOf rdf:resource="https://w3id.org/dpv/justifications/owl#LegalProcessImpaired"/>
    <rdfs:subClassOf rdf:resource="https://w3id.org/dpv/justifications/owl#SecurityImpaired"/>
  </rdf:Description>
  <rdf:Description rdf:about="https://w3id.org/dpv/justifications/owl#EthicsBreachPreventionImpaired">
    <rdfs:isDefinedBy rdf:resource="https://w3id.org/dpv/justifications/owl#"/>
    <rdf:type rdf:resource="http://www.w3.org/2000/01/rdf-schema#Class"/>
    <rdf:type rdf:resource="https://w3id.org/dpv/owl#Justification"/>
    <rdf:type rdf:resource="http://www.w3.org/2002/07/owl#Class"/>
    <sw:term_status xml:lang="en">accepted</sw:term_status>
    <dct:contributor rdf:nodeID="person-harshvardhan-j-pandit"/>
    <dct:contributor rdf:nodeID="person-beatriz-esteves"/>
    <skos:prefLabel xml:lang="en">Ethics Breach Prevention Impaired</skos:prefLabel>
    <dct:created rdf:datatype="http://www.w3.org/2001/XMLSchema#date">2024-04-21</dct:created>
    <skos:definition xml:lang="en">Justification that the process could not be fulfilled or was not successful because it would interfere with the prevention of breaches of ethics for regulated professions</skos:definition>
    <rdfs:subClassOf rdf:resource="https://w3id.org/dpv/justifications/owl#EthicsProcedureImpaired"/>
  </rdf:Description>
  <rdf:Description rdf:about="https://w3id.org/dpv/justifications/owl#PublicInterestCompromised">
    <rdfs:isDefinedBy rdf:resource="https://w3id.org/dpv/justifications/owl#"/>
    <rdf:type rdf:resource="http://www.w3.org/2000/01/rdf-schema#Class"/>
    <rdf:type rdf:resource="https://w3id.org/dpv/owl#Justification"/>
    <rdf:type rdf:resource="http://www.w3.org/2002/07/owl#Class"/>
    <sw:term_status xml:lang="en">accepted</sw:term_status>
    <dct:contributor rdf:nodeID="person-harshvardhan-j-pandit"/>
    <dct:contributor rdf:nodeID="person-beatriz-esteves"/>
    <skos:prefLabel xml:lang="en">Public Interest Compromised</skos:prefLabel>
    <skos:definition xml:lang="en">Justification that the process could not be fulfilled or was not successful because it would interfere with necessary tasks carried out for public interest</skos:definition>
    <dct:created rdf:datatype="http://www.w3.org/2001/XMLSchema#date">2024-04-21</dct:created>
    <rdfs:subClassOf rdf:resource="https://w3id.org/dpv/justifications/owl#LegalProcessImpaired"/>
  </rdf:Description>
  <rdf:Description rdf:about="https://w3id.org/dpv/justifications/owl#ConfidentialityObligationCompromised">
    <rdfs:isDefinedBy rdf:resource="https://w3id.org/dpv/justifications/owl#"/>
    <rdf:type rdf:resource="http://www.w3.org/2000/01/rdf-schema#Class"/>
    <rdf:type rdf:resource="https://w3id.org/dpv/owl#Justification"/>
    <rdf:type rdf:resource="http://www.w3.org/2002/07/owl#Class"/>
    <skos:prefLabel xml:lang="en">Confidentiality Obligation Compromised</skos:prefLabel>
    <sw:term_status xml:lang="en">accepted</sw:term_status>
    <dct:contributor rdf:nodeID="person-harshvardhan-j-pandit"/>
    <dct:contributor rdf:nodeID="person-beatriz-esteves"/>
    <skos:definition xml:lang="en">Justification that the process could not be fulfilled or was not successful because it would compromise a confidentiality obligation</skos:definition>
    <dct:created rdf:datatype="http://www.w3.org/2001/XMLSchema#date">2024-04-21</dct:created>
    <rdfs:subClassOf rdf:resource="https://w3id.org/dpv/justifications/owl#LegalProcessImpaired"/>
  </rdf:Description>
  <rdf:Description rdf:about="https://w3id.org/dpv/justifications/owl#NonFulfilmentJustification">
    <rdf:type rdf:resource="http://www.w3.org/2000/01/rdf-schema#Class"/>
    <rdf:type rdf:resource="http://www.w3.org/2002/07/owl#Class"/>
    <skos:prefLabel xml:lang="en">Non-Fulfilment Justification</skos:prefLabel>
    <dct:contributor rdf:nodeID="person-harshvardhan-j-pandit"/>
    <dct:contributor rdf:nodeID="person-beatriz-esteves"/>
    <dct:created rdf:datatype="http://www.w3.org/2001/XMLSchema#date">2024-04-21</dct:created>
    <sw:term_status xml:lang="en">accepted</sw:term_status>
    <skos:definition xml:lang="en">Justification for not fulfilling a process or requirement or obligation</skos:definition>
    <rdfs:subClassOf rdf:resource="https://w3id.org/dpv/owl#Justification"/>
    <rdfs:isDefinedBy rdf:resource="https://w3id.org/dpv/justifications/owl#"/>
  </rdf:Description>
  <rdf:Description rdf:about="https://w3id.org/dpv/justifications/owl#ProcessRejected">
    <rdf:type rdf:resource="http://www.w3.org/2000/01/rdf-schema#Class"/>
    <rdf:type rdf:resource="https://w3id.org/dpv/owl#Justification"/>
    <rdf:type rdf:resource="http://www.w3.org/2002/07/owl#Class"/>
    <rdfs:isDefinedBy rdf:resource="https://w3id.org/dpv/justifications/owl#"/>
    <dct:contributor rdf:nodeID="person-harshvardhan-j-pandit"/>
    <dct:contributor rdf:nodeID="person-beatriz-esteves"/>
    <skos:definition xml:lang="en">Justification that the process could not be fulfilled because of one of more reasons associated with the process itself e.g. it was excessive, malicious, etc.</skos:definition>
    <dct:created rdf:datatype="http://www.w3.org/2001/XMLSchema#date">2024-04-21</dct:created>
    <sw:term_status xml:lang="en">accepted</sw:term_status>
    <skos:prefLabel xml:lang="en">Process Rejected</skos:prefLabel>
    <rdfs:subClassOf rdf:resource="https://w3id.org/dpv/justifications/owl#NonFulfilmentJustification"/>
  </rdf:Description>
  <rdf:Description rdf:about="https://w3id.org/dpv/justifications/owl#DisproportionateEffortRequired">
    <skos:definition xml:lang="en">Justification that the process could not be fulfilled or was not successful because it requires a disproportionate effort</skos:definition>
    <rdf:type rdf:resource="http://www.w3.org/2000/01/rdf-schema#Class"/>
    <rdf:type rdf:resource="https://w3id.org/dpv/owl#Justification"/>
    <rdf:type rdf:resource="http://www.w3.org/2002/07/owl#Class"/>
    <rdfs:isDefinedBy rdf:resource="https://w3id.org/dpv/justifications/owl#"/>
    <dct:contributor rdf:nodeID="person-harshvardhan-j-pandit"/>
    <dct:contributor rdf:nodeID="person-beatriz-esteves"/>
    <skos:prefLabel xml:lang="en">Disproportionate Effort Required</skos:prefLabel>
    <sw:term_status xml:lang="en">accepted</sw:term_status>
    <dct:created rdf:datatype="http://www.w3.org/2001/XMLSchema#date">2024-04-21</dct:created>
    <rdfs:subClassOf rdf:resource="https://w3id.org/dpv/justifications/owl#NonFulfilmentJustification"/>
  </rdf:Description>
  <rdf:Description rdf:about="https://w3id.org/dpv/justifications/owl#PublicHealthCompromised">
    <dct:contributor rdf:nodeID="person-harshvardhan-j-pandit"/>
    <dct:contributor rdf:nodeID="person-beatriz-esteves"/>
    <rdf:type rdf:resource="https://w3id.org/dpv/owl#Justification"/>
    <rdf:type rdf:resource="http://www.w3.org/2000/01/rdf-schema#Class"/>
    <rdf:type rdf:resource="http://www.w3.org/2002/07/owl#Class"/>
    <dct:created rdf:datatype="http://www.w3.org/2001/XMLSchema#date">2024-04-21</dct:created>
    <sw:term_status xml:lang="en">accepted</sw:term_status>
    <skos:definition xml:lang="en">Justification that the process could not be fulfilled or was not successful because it would interfere with necessary tasks carried out for public health reasons</skos:definition>
    <skos:prefLabel xml:lang="en">Public Health Compromised</skos:prefLabel>
    <rdfs:isDefinedBy rdf:resource="https://w3id.org/dpv/justifications/owl#"/>
    <rdfs:subClassOf rdf:resource="https://w3id.org/dpv/justifications/owl#LegalProcessImpaired"/>
  </rdf:Description>
  <rdf:Description rdf:about="https://w3id.org/dpv/justifications/owl#ScientificHistoricalResearchImpaired">
    <dct:contributor rdf:nodeID="person-harshvardhan-j-pandit"/>
    <dct:contributor rdf:nodeID="person-beatriz-esteves"/>
    <rdf:type rdf:resource="https://w3id.org/dpv/owl#Justification"/>
    <rdf:type rdf:resource="http://www.w3.org/2000/01/rdf-schema#Class"/>
    <rdf:type rdf:resource="http://www.w3.org/2002/07/owl#Class"/>
    <skos:definition xml:lang="en">Justification that the process could not be fulfilled or was not successful because it impairs scientific or historical research</skos:definition>
    <dct:created rdf:datatype="http://www.w3.org/2001/XMLSchema#date">2024-04-21</dct:created>
    <rdfs:isDefinedBy rdf:resource="https://w3id.org/dpv/justifications/owl#"/>
    <skos:prefLabel xml:lang="en">Scientific Historical Research Impaired</skos:prefLabel>
    <sw:term_status xml:lang="en">accepted</sw:term_status>
    <rdfs:subClassOf rdf:resource="https://w3id.org/dpv/justifications/owl#NonFulfilmentJustification"/>
  </rdf:Description>
  <rdf:Description rdf:about="https://w3id.org/dpv/justifications/owl#ProcessUnfounded">
    <rdf:type rdf:resource="http://www.w3.org/2000/01/rdf-schema#Class"/>
    <rdf:type rdf:resource="https://w3id.org/dpv/owl#Justification"/>
    <rdf:type rdf:resource="http://www.w3.org/2002/07/owl#Class"/>
    <dct:contributor rdf:nodeID="person-harshvardhan-j-pandit"/>
    <dct:contributor rdf:nodeID="person-beatriz-esteves"/>
    <dct:created rdf:datatype="http://www.w3.org/2001/XMLSchema#date">2024-04-21</dct:created>
    <skos:prefLabel xml:lang="en">Process Unfounded</skos:prefLabel>
    <sw:term_status xml:lang="en">accepted</sw:term_status>
    <skos:definition xml:lang="en">Justification that the process could not be fulfilled or was not successful because it was found to be based on manifestly unfounded reasons</skos:definition>
    <rdfs:isDefinedBy rdf:resource="https://w3id.org/dpv/justifications/owl#"/>
    <rdfs:subClassOf rdf:resource="https://w3id.org/dpv/justifications/owl#ProcessRejected"/>
  </rdf:Description>
  <rdf:Description rdf:about="https://w3id.org/dpv/justifications/owl#ContractEstablishmentNecessity">
    <skos:definition xml:lang="en">Justification that the process could not be fulfilled or was not successful because it is necessary for entering into a contract</skos:definition>
    <rdf:type rdf:resource="http://www.w3.org/2000/01/rdf-schema#Class"/>
    <rdf:type rdf:resource="https://w3id.org/dpv/owl#Justification"/>
    <rdf:type rdf:resource="http://www.w3.org/2002/07/owl#Class"/>
    <rdfs:isDefinedBy rdf:resource="https://w3id.org/dpv/justifications/owl#"/>
    <dct:contributor rdf:nodeID="person-harshvardhan-j-pandit"/>
    <dct:contributor rdf:nodeID="person-beatriz-esteves"/>
    <skos:prefLabel xml:lang="en">Contract Establishment Necessity</skos:prefLabel>
    <dct:created rdf:datatype="http://www.w3.org/2001/XMLSchema#date">2024-04-21</dct:created>
    <sw:term_status xml:lang="en">accepted</sw:term_status>
    <rdfs:subClassOf rdf:resource="https://w3id.org/dpv/justifications/owl#LegalProcessImpaired"/>
  </rdf:Description>
  <rdf:Description rdf:about="https://w3id.org/dpv/justifications/owl#InformationSocietyServicesOffer">
    <skos:definition xml:lang="en">Justification that the process should be carried out due to it being related to the offer of information society services</skos:definition>
    <skos:prefLabel xml:lang="en">Information Society Services Offer</skos:prefLabel>
    <rdf:type rdf:resource="http://www.w3.org/2000/01/rdf-schema#Class"/>
    <rdf:type rdf:resource="https://w3id.org/dpv/owl#Justification"/>
    <rdf:type rdf:resource="http://www.w3.org/2002/07/owl#Class"/>
    <rdfs:isDefinedBy rdf:resource="https://w3id.org/dpv/justifications/owl#"/>
    <dct:contributor rdf:nodeID="person-harshvardhan-j-pandit"/>
    <dct:contributor rdf:nodeID="person-beatriz-esteves"/>
    <sw:term_status xml:lang="en">accepted</sw:term_status>
    <dct:created rdf:datatype="http://www.w3.org/2001/XMLSchema#date">2024-04-21</dct:created>
    <rdfs:subClassOf rdf:resource="https://w3id.org/dpv/justifications/owl#ExerciseJustification"/>
  </rdf:Description>
  <rdf:Description rdf:about="https://w3id.org/dpv/justifications/owl#LegalClaimImpaired">
    <rdf:type rdf:resource="https://w3id.org/dpv/owl#Justification"/>
    <rdf:type rdf:resource="http://www.w3.org/2000/01/rdf-schema#Class"/>
    <rdf:type rdf:resource="http://www.w3.org/2002/07/owl#Class"/>
    <dct:contributor rdf:nodeID="person-harshvardhan-j-pandit"/>
    <skos:definition xml:lang="en">Justification that the process could not be fulfilled or was not successful because it would impair the establishment, exercise, or defence of a legal claim</skos:definition>
    <dct:created rdf:datatype="http://www.w3.org/2001/XMLSchema#date">2024-12-17</dct:created>
    <rdfs:isDefinedBy rdf:resource="https://w3id.org/dpv/justifications/owl#"/>
    <skos:prefLabel xml:lang="en">Legal Claim Impaired</skos:prefLabel>
    <sw:term_status xml:lang="en">accepted</sw:term_status>
    <rdfs:subClassOf rdf:resource="https://w3id.org/dpv/justifications/owl#LegalProcessImpaired"/>
  </rdf:Description>
  <rdf:Description rdf:about="https://w3id.org/dpv/justifications/owl#LegitimateInterestOverride">
    <dct:contributor rdf:nodeID="person-harshvardhan-j-pandit"/>
    <dct:contributor rdf:nodeID="person-beatriz-esteves"/>
    <rdf:type rdf:resource="https://w3id.org/dpv/owl#Justification"/>
    <rdf:type rdf:resource="http://www.w3.org/2000/01/rdf-schema#Class"/>
    <rdf:type rdf:resource="http://www.w3.org/2002/07/owl#Class"/>
    <dct:created rdf:datatype="http://www.w3.org/2001/XMLSchema#date">2024-04-21</dct:created>
    <skos:prefLabel xml:lang="en">Legitimate Interest Override</skos:prefLabel>
    <rdfs:isDefinedBy rdf:resource="https://w3id.org/dpv/justifications/owl#"/>
    <skos:definition xml:lang="en">Justification that the process could not be fulfilled or was not successful because the legitimate interest of the controller overrides the interests or rights of the data subject</skos:definition>
    <sw:term_status xml:lang="en">accepted</sw:term_status>
    <rdfs:subClassOf rdf:resource="https://w3id.org/dpv/justifications/owl#NonFulfilmentJustification"/>
  </rdf:Description>
  <rdf:Description rdf:about="https://w3id.org/dpv/justifications/owl#ThirdPartyRightsImpaired">
    <skos:definition xml:lang="en">Justification that the process could not be fulfilled or was not successful because it would affect the rights and freedoms of others</skos:definition>
    <rdfs:isDefinedBy rdf:resource="https://w3id.org/dpv/justifications/owl#"/>
    <skos:prefLabel xml:lang="en">Third Party Rights Impaired</skos:prefLabel>
    <rdf:type rdf:resource="https://w3id.org/dpv/owl#Justification"/>
    <rdf:type rdf:resource="http://www.w3.org/2000/01/rdf-schema#Class"/>
    <rdf:type rdf:resource="http://www.w3.org/2002/07/owl#Class"/>
    <sw:term_status xml:lang="en">accepted</sw:term_status>
    <dct:contributor rdf:nodeID="person-harshvardhan-j-pandit"/>
    <dct:contributor rdf:nodeID="person-beatriz-esteves"/>
    <dct:created rdf:datatype="http://www.w3.org/2001/XMLSchema#date">2024-04-21</dct:created>
    <rdfs:subClassOf rdf:resource="https://w3id.org/dpv/justifications/owl#LegalProcessImpaired"/>
  </rdf:Description>
  <rdf:Description rdf:about="https://w3id.org/dpv/justifications/owl#FulfilmentImpossible">
    <dct:contributor rdf:nodeID="person-harshvardhan-j-pandit"/>
    <dct:contributor rdf:nodeID="person-beatriz-esteves"/>
    <skos:definition xml:lang="en">Justification that the process could not be fulfilled or was not successful because it is impossible to fulfil</skos:definition>
    <sw:term_status xml:lang="en">accepted</sw:term_status>
    <rdf:type rdf:resource="https://w3id.org/dpv/owl#Justification"/>
    <rdf:type rdf:resource="http://www.w3.org/2000/01/rdf-schema#Class"/>
    <rdf:type rdf:resource="http://www.w3.org/2002/07/owl#Class"/>
    <dct:created rdf:datatype="http://www.w3.org/2001/XMLSchema#date">2024-04-21</dct:created>
    <skos:prefLabel xml:lang="en">Fulfilment Impossible</skos:prefLabel>
    <rdfs:isDefinedBy rdf:resource="https://w3id.org/dpv/justifications/owl#"/>
    <rdfs:subClassOf rdf:resource="https://w3id.org/dpv/justifications/owl#NonFulfilmentJustification"/>
  </rdf:Description>
  <rdf:Description rdf:about="https://w3id.org/dpv/justifications/owl#FreedomOfExpressionImpaired">
    <skos:prefLabel xml:lang="en">Freedom Of Expression Impaired</skos:prefLabel>
    <skos:definition xml:lang="en">Justification that the process could not be fulfilled or was not successful because it would interfere with the right of freedom of expression and information of others</skos:definition>
    <rdf:type rdf:resource="https://w3id.org/dpv/owl#Justification"/>
    <rdf:type rdf:resource="http://www.w3.org/2000/01/rdf-schema#Class"/>
    <rdf:type rdf:resource="http://www.w3.org/2002/07/owl#Class"/>
    <sw:term_status xml:lang="en">accepted</sw:term_status>
    <dct:contributor rdf:nodeID="person-harshvardhan-j-pandit"/>
    <dct:contributor rdf:nodeID="person-beatriz-esteves"/>
    <dct:created rdf:datatype="http://www.w3.org/2001/XMLSchema#date">2024-04-21</dct:created>
    <rdfs:isDefinedBy rdf:resource="https://w3id.org/dpv/justifications/owl#"/>
    <rdfs:subClassOf rdf:resource="https://w3id.org/dpv/justifications/owl#LegalProcessImpaired"/>
  </rdf:Description>
  <rdf:Description rdf:nodeID="person-harshvardhan-j-pandit">
    <foaf:name>Harshvardhan J. Pandit</foaf:name>
    <rdf:type rdf:resource="http://xmlns.com/foaf/0.1/Person"/>
    <rdf:type rdf:resource="http://purl.org/dc/terms/Agent"/>
    <foaf:homepage>https://harshp.com/</foaf:homepage>
    <org:memberOf rdf:nodeID="org-ai-accountability-lab-aial-trinity-college-dublin"/>
    <scoro:hasORCID>0000-0002-5068-3714</scoro:hasORCID>
  </rdf:Description>
  <rdf:Description rdf:nodeID="person-georg-p-krog">
    <org:memberOf rdf:nodeID="org-signatu-as"/>
    <rdf:type rdf:resource="http://xmlns.com/foaf/0.1/Person"/>
    <rdf:type rdf:resource="http://purl.org/dc/terms/Agent"/>
    <foaf:homepage>https://www.linkedin.com/in/georg-philip-krog-a2a278104/</foaf:homepage>
    <foaf:name>Georg P. Krog</foaf:name>
  </rdf:Description>
  <rdf:Description rdf:nodeID="org-uniphar-plc">
    <rdf:type rdf:resource="http://xmlns.com/foaf/0.1/Organization"/>
    <foaf:name>Uniphar PLC</foaf:name>
  </rdf:Description>
  <rdf:Description rdf:nodeID="org-ai-accountability-lab-aial-trinity-college-dublin">
    <foaf:name>AI Accountability Lab (AIAL), Trinity College Dublin</foaf:name>
    <rdf:type rdf:resource="http://xmlns.com/foaf/0.1/Organization"/>
  </rdf:Description>
  <rdf:Description rdf:about="https://w3id.org/dpv/justifications/owl#ProcessExcessive">
    <rdf:type rdf:resource="https://w3id.org/dpv/owl#Justification"/>
    <rdf:type rdf:resource="http://www.w3.org/2000/01/rdf-schema#Class"/>
    <rdf:type rdf:resource="http://www.w3.org/2002/07/owl#Class"/>
    <dct:contributor rdf:nodeID="person-harshvardhan-j-pandit"/>
    <dct:contributor rdf:nodeID="person-beatriz-esteves"/>
    <dct:created rdf:datatype="http://www.w3.org/2001/XMLSchema#date">2024-04-21</dct:created>
    <skos:definition xml:lang="en">Justification that the process could not be fulfilled or was not successful because it was found to be excessive in nature</skos:definition>
    <rdfs:isDefinedBy rdf:resource="https://w3id.org/dpv/justifications/owl#"/>
    <skos:prefLabel xml:lang="en">Process Excessive</skos:prefLabel>
    <sw:term_status xml:lang="en">accepted</sw:term_status>
    <rdfs:subClassOf rdf:resource="https://w3id.org/dpv/justifications/owl#ProcessRejected"/>
  </rdf:Description>
  <rdf:Description rdf:about="https://w3id.org/dpv/justifications/owl#serialisation-n3">
    <dct:conformsTo rdf:resource="https://www.w3.org/TeamSubmission/n3/"/>
    <dct:format rdf:resource="https://www.iana.org/assignments/media-types/text/n3"/>
    <dct:title>Justification Concepts - N3 serialisation</dct:title>
    <profile:hasArtifact rdf:resource="https://w3id.org/dpv/justifications/justifications-owl.n3"/>
    <profile:hasRole rdf:resource="http://www.w3.org/ns/dx/prof/role/vocabulary"/>
    <rdf:type rdf:resource="http://www.w3.org/ns/dx/prof/ResourceDescriptor"/>
  </rdf:Description>
  <rdf:Description rdf:about="https://w3id.org/dpv/justifications/owl#serialisation-ttl">
    <dct:title>Justification Concepts - Turtle serialisation</dct:title>
    <rdf:type rdf:resource="http://www.w3.org/ns/dx/prof/ResourceDescriptor"/>
    <profile:hasArtifact rdf:resource="https://w3id.org/dpv/justifications/justifications-owl.ttl"/>
    <dct:conformsTo rdf:resource="https://www.w3.org/TR/turtle/"/>
    <dct:format rdf:resource="https://www.iana.org/assignments/media-types/text/turtle"/>
    <profile:hasRole rdf:resource="http://www.w3.org/ns/dx/prof/role/vocabulary"/>
  </rdf:Description>
  <rdf:Description rdf:nodeID="person-beatriz-esteves">
    <scoro:hasORCID>0000-0003-0259-7560</scoro:hasORCID>
    <rdf:type rdf:resource="http://xmlns.com/foaf/0.1/Person"/>
    <rdf:type rdf:resource="http://purl.org/dc/terms/Agent"/>
    <org:memberOf rdf:nodeID="org-idlab-imec-ghent-university"/>
    <foaf:name>Beatriz Esteves</foaf:name>
  </rdf:Description>
  <rdf:Description rdf:about="https://w3id.org/dpv/justifications/owl#serialisation-rdf">
    <dct:title>Justification Concepts - RDF/XML serialisation</dct:title>
    <profile:hasRole rdf:resource="http://www.w3.org/ns/dx/prof/role/vocabulary"/>
    <dct:format rdf:resource="https://www.iana.org/assignments/media-types/application/rdf+xml"/>
    <rdf:type rdf:resource="http://www.w3.org/ns/dx/prof/ResourceDescriptor"/>
    <profile:hasArtifact rdf:resource="https://w3id.org/dpv/justifications/justifications-owl.rdf"/>
    <dct:conformsTo rdf:resource="http://www.w3.org/1999/02/22-rdf-syntax-ns#"/>
  </rdf:Description>
  <rdf:Description rdf:nodeID="org-signatu-as">
    <foaf:name>Signatu AS</foaf:name>
    <rdf:type rdf:resource="http://xmlns.com/foaf/0.1/Organization"/>
  </rdf:Description>
  <rdf:Description rdf:nodeID="org-idlab-imec-ghent-university">
    <rdf:type rdf:resource="http://xmlns.com/foaf/0.1/Organization"/>
    <foaf:name>IDLab, IMEC, Ghent University</foaf:name>
  </rdf:Description>
</rdf:RDF>
