@prefix ai: <https://w3id.org/dpv/ai#> .
@prefix bibo: <http://purl.org/ontology/bibo/> .
@prefix dct: <http://purl.org/dc/terms/> .
@prefix foaf: <http://xmlns.com/foaf/0.1/> .
@prefix owl: <http://www.w3.org/2002/07/owl#> .
@prefix profile: <http://www.w3.org/ns/dx/prof/> .
@prefix rdf: <http://www.w3.org/1999/02/22-rdf-syntax-ns#> .
@prefix rdfs: <http://www.w3.org/2000/01/rdf-schema#> .
@prefix risk: <https://w3id.org/dpv/risk#> .
@prefix role: <http://www.w3.org/ns/dx/prof/role/> .
@prefix schema: <https://schema.org/> .
@prefix skos: <http://www.w3.org/2004/02/skos/core#> .
@prefix sw: <http://www.w3.org/2003/06/sw-vocab-status/ns#> .
@prefix vann: <http://purl.org/vocab/vann/> .
@prefix xsd: <http://www.w3.org/2001/XMLSchema#> .

ai:AIBias a rdfs:Class,
        skos:Concept,
        risk:RiskConcept ;
    dct:contributor "Daniel Doherty" ;
    dct:created "2024-09-18"^^xsd:date ;
    rdfs:isDefinedBy ai: ;
    sw:term_status "accepted"@en ;
    skos:broader risk:Bias ;
    skos:definition "Bias associated with development, use, or other activities involving an AI technology or system"@en ;
    skos:inScheme ai:bias-classes ;
    skos:prefLabel "AI Bias"@en .

ai:AlgorithmSelectionBias a rdfs:Class,
        skos:Concept,
        risk:RiskConcept ;
    dct:contributor "Daniel Doherty" ;
    dct:created "2024-09-13"^^xsd:date ;
    dct:source "ISO/IEC 24027:2021"@en ;
    rdfs:isDefinedBy ai: ;
    sw:term_status "accepted"@en ;
    skos:broader ai:EngineeringDecisionBias ;
    skos:definition "Bias that occurs from the selection of machine learning algorithms built into the AI system which introduce unwanted bias in predictions made by the system because the type of algorithm used introduces a variation in the performance of the ML model"@en ;
    skos:inScheme ai:bias-classes ;
    skos:prefLabel "Algorithm Selection Bias"@en .

ai:AutomationBias a rdfs:Class,
        skos:Concept,
        risk:RiskConcept ;
    dct:contributor "Daniel Doherty" ;
    dct:created "2024-09-13"^^xsd:date ;
    dct:source "ISO/IEC 24027:2021"@en ;
    rdfs:isDefinedBy ai: ;
    sw:term_status "accepted"@en ;
    skos:broader risk:CognitiveBias ;
    skos:definition "Bias tha occurs due to propensity for humans to favour suggestions from automated decision-making systems and to ignore contradictory information made without automation, even if it is correct"@en ;
    skos:inScheme ai:bias-classes ;
    skos:prefLabel "Automation Bias"@en .

ai:DataAggregationBias a rdfs:Class,
        skos:Concept,
        risk:RiskConcept ;
    dct:contributor "Daniel Doherty" ;
    dct:created "2024-09-13"^^xsd:date ;
    dct:source "ISO/IEC 24027:2021"@en ;
    rdfs:isDefinedBy ai: ;
    sw:term_status "accepted"@en ;
    skos:broader ai:DataBias ;
    skos:definition "Bias that occurs from aggregating data covering different groups of objects that might have different statistical distributions which introduce bias into the data used to train AI systems"@en ;
    skos:inScheme ai:bias-classes ;
    skos:prefLabel "Data Aggregation Bias"@en .

ai:DataBias a rdfs:Class,
        skos:Concept,
        risk:RiskConcept ;
    dct:contributor "Daniel Doherty" ;
    dct:created "2024-09-13"^^xsd:date ;
    dct:source "ISO/IEC 24027:2021"@en ;
    rdfs:isDefinedBy ai: ;
    sw:term_status "accepted"@en ;
    skos:broader ai:AIBias ;
    skos:definition "Bias that occurs due to unaddressed data properties that lead to AI systems that perform better or worse for different groups"@en ;
    skos:inScheme ai:bias-classes ;
    skos:prefLabel "Data Bias"@en .

ai:DataLabelsAndLabellingProcessBias a rdfs:Class,
        skos:Concept,
        risk:RiskConcept ;
    dct:contributor "Daniel Doherty" ;
    dct:created "2024-09-13"^^xsd:date ;
    dct:source "ISO/IEC 24027:2021"@en ;
    rdfs:isDefinedBy ai: ;
    sw:term_status "accepted"@en ;
    skos:broader ai:DataBias ;
    skos:definition "Bias that occurs due to the labelling process itself introducing societal or cognitive biases"@en ;
    skos:inScheme ai:bias-classes ;
    skos:prefLabel "Data Labels And Labelling Process Bias"@en .

ai:DistributedTrainingBias a rdfs:Class,
        skos:Concept,
        risk:RiskConcept ;
    dct:contributor "Daniel Doherty" ;
    dct:created "2024-09-13"^^xsd:date ;
    dct:source "ISO/IEC 24027:2021"@en ;
    rdfs:isDefinedBy ai: ;
    sw:term_status "accepted"@en ;
    skos:broader ai:DataBias ;
    skos:definition "Bias that occurs due to distributed machine having different sources of data that do not have the same distribution of feature space"@en ;
    skos:inScheme ai:bias-classes ;
    skos:prefLabel "Distributed Training Bias"@en .

ai:EngineeringDecisionBias a rdfs:Class,
        skos:Concept,
        risk:RiskConcept ;
    dct:contributor "Daniel Doherty" ;
    dct:created "2024-09-13"^^xsd:date ;
    dct:source "ISO/IEC 24027:2021"@en ;
    rdfs:isDefinedBy ai: ;
    sw:term_status "accepted"@en ;
    skos:broader ai:AIBias ;
    skos:definition "Bias that occurs due to machine learning model architectures - encompassing all model specifications, parameters and manually designed features"@en ;
    skos:inScheme ai:bias-classes ;
    skos:prefLabel "Engineering Decision Bias"@en ;
    skos:scopeNote "Data bias and human cognitive bias can contribute to such bias"@en .

ai:FeatureEngineeringBias a rdfs:Class,
        skos:Concept,
        risk:RiskConcept ;
    dct:contributor "Daniel Doherty" ;
    dct:created "2024-09-13"^^xsd:date ;
    dct:source "ISO/IEC 24027:2021"@en ;
    rdfs:isDefinedBy ai: ;
    sw:term_status "accepted"@en ;
    skos:broader ai:EngineeringDecisionBias ;
    skos:definition "Bias that occurs from steps such as encoding, data type conversion, dimensionality reduction and feature selection which are subject to choices made by the AI developer and introduce bias in the ML model"@en ;
    skos:inScheme ai:bias-classes ;
    skos:prefLabel "Feature Engineering Bias"@en .

ai:HyperparameterTuningBias a rdfs:Class,
        skos:Concept,
        risk:RiskConcept ;
    dct:contributor "Daniel Doherty" ;
    dct:created "2024-09-13"^^xsd:date ;
    dct:source "ISO/IEC 24027:2021"@en ;
    rdfs:isDefinedBy ai: ;
    sw:term_status "accepted"@en ;
    skos:broader ai:EngineeringDecisionBias ;
    skos:definition "Bias that occurs from hyperparameters defining how the model is structured and which cannot be directly trained from the data like model parameters, where hyperparameters affect the model functioning and accuracy of the model"@en ;
    skos:inScheme ai:bias-classes ;
    skos:prefLabel "Hyperparameter Tuning Bias"@en .

ai:InformativenessBias a rdfs:Class,
        skos:Concept,
        risk:RiskConcept ;
    dct:contributor "Daniel Doherty" ;
    dct:created "2024-09-13"^^xsd:date ;
    dct:source "ISO/IEC 24027:2021"@en ;
    rdfs:isDefinedBy ai: ;
    sw:term_status "accepted"@en ;
    skos:broader ai:EngineeringDecisionBias ;
    skos:definition "Bias that occurs or some groups, the mapping between inputs present in the data and outputs are more difficult to learn and where a model that only has one feature set available, can be biased against the group whose relationships are difficult to learn from available data"@en ;
    skos:inScheme ai:bias-classes ;
    skos:prefLabel "Informativeness Bias"@en ;
    skos:scopeNote "This can happen when some features are highly informative about one group, while a different set of features is highly informative about another group. If this is the case, then a model that only has one feature set available, can be biased against the group whose relationships are difficult to learn from available data"@en .

ai:MissingFeaturesAndLabelsBias a rdfs:Class,
        skos:Concept,
        risk:RiskConcept ;
    dct:contributor "Daniel Doherty" ;
    dct:created "2024-09-13"^^xsd:date ;
    dct:source "ISO/IEC 24027:2021"@en ;
    rdfs:isDefinedBy ai: ;
    sw:term_status "accepted"@en ;
    skos:broader ai:DataBias ;
    skos:definition "Bias that occurs when features are missing from individual training samples"@en ;
    skos:inScheme ai:bias-classes ;
    skos:prefLabel "Missing Features And Labels Bias"@en ;
    skos:scopeNote "If the frequency of missing features is higher for one group than another then this presents another vector for bias"@en .

ai:ModelBias a rdfs:Class,
        skos:Concept,
        risk:RiskConcept ;
    dct:contributor "Daniel Doherty" ;
    dct:created "2024-09-13"^^xsd:date ;
    dct:source "ISO/IEC 24027:2021"@en ;
    rdfs:isDefinedBy ai: ;
    sw:term_status "accepted"@en ;
    skos:broader ai:EngineeringDecisionBias ;
    skos:definition "Bias that occurs when ML uses functions like a maximum likelihood estimator to determine parameters, and there is data skew or under-representation present in the data, where the maximum likelihood estimation tends to amplify any underlying bias in the distribution"@en ;
    skos:inScheme ai:bias-classes ;
    skos:prefLabel "Model Bias"@en .

ai:ModelExpressivenessBias a rdfs:Class,
        skos:Concept,
        risk:RiskConcept ;
    dct:contributor "Daniel Doherty" ;
    dct:created "2024-09-13"^^xsd:date ;
    dct:source "ISO/IEC 24027:2021"@en ;
    rdfs:isDefinedBy ai: ;
    sw:term_status "accepted"@en ;
    skos:broader ai:ModelInteractionBias ;
    skos:definition "Bias that occurs from the number and nature of parameters in a model as well as the neural network topology which affect the expressiveness of the model and any feature that affects model expressiveness differently across groups"@en ;
    skos:inScheme ai:bias-classes ;
    skos:prefLabel "Model Expressiveness Bias"@en .

ai:ModelInteractionBias a rdfs:Class,
        skos:Concept,
        risk:RiskConcept ;
    dct:contributor "Daniel Doherty" ;
    dct:created "2024-09-13"^^xsd:date ;
    dct:source "ISO/IEC 24027:2021"@en ;
    rdfs:isDefinedBy ai: ;
    sw:term_status "accepted"@en ;
    skos:broader ai:EngineeringDecisionBias ;
    skos:definition "Bias that occurs from the structure of a model to create biased predictions"@en ;
    skos:inScheme ai:bias-classes ;
    skos:prefLabel "Model Interaction Bias"@en .

ai:NonRepresentativeSamplingBias a rdfs:Class,
        skos:Concept,
        risk:RiskConcept ;
    dct:contributor "Daniel Doherty" ;
    dct:created "2024-09-13"^^xsd:date ;
    dct:source "ISO/IEC 24027:2021"@en ;
    rdfs:isDefinedBy ai: ;
    sw:term_status "accepted"@en ;
    skos:broader ai:DataBias ;
    skos:definition "Bias that occurs if a dataset is not representative of the intended deployment environment, where the model learns biases based on the ways in which the data is non-representative"@en ;
    skos:inScheme ai:bias-classes ;
    skos:prefLabel "Non-Representative Sampling Bias"@en .

<https://w3id.org/dpv/ai> a owl:Ontology,
        profile:Profile ;
    dct:bibliographicCitation "Data Privacy Vocabulary (DPV) -- Version 2. Harshvardhan J. Pandit, Beatriz Esteves, Georg P. Krog, Paul Ryan, Delaram Golpayegani, Julian Flake https://doi.org/10.48550/arXiv.2404.13426" ;
    dct:conformsTo "http://www.w3.org/2000/01/rdf-schema",
        "http://www.w3.org/2004/02/skos/core" ;
    dct:contributor "Daniel Doherty" ;
    dct:created "2024-05-31"@en ;
    dct:creator "Delaram Golpayegani"@en,
        "Harshvardhan J. Pandit"@en ;
    dct:description "Extension to the Data Privacy Vocabulary (DPV) providing concepts for representing information about AI technologies"@en ;
    dct:identifier "https://w3id.org/dpv/ai" ;
    dct:issued "2024-05-31"@en ;
    dct:license <https://www.w3.org/copyright/document-license-2023/> ;
    dct:modified "2024-10-22"@en ;
    dct:publisher <https://www.w3.org/> ;
    dct:source <https://www.w3.org/groups/cg/dpvcg/> ;
    dct:title "AI Technology Concepts"@en ;
    bibo:doi "10.5281/zenodo.12505841" ;
    bibo:status "http://purl.org/ontology/bibo/status/draft" ;
    vann:preferredNamespacePrefix "ai" ;
    vann:preferredNamespaceUri "https://w3id.org/dpv/ai#" ;
    rdfs:Label "AI"@en ;
    owl:versionIRI <https://w3id.org/dpv/2.1-dev/ai> ;
    owl:versionInfo "2.1-dev" ;
    profile:hasResource ai:serialisation-html,
        ai:serialisation-jsonld,
        ai:serialisation-n3,
        ai:serialisation-rdf,
        ai:serialisation-ttl,
        <https://w3id.org/dpv/examples>,
        <https://w3id.org/dpv/guides>,
        <https://w3id.org/dpv/primer> ;
    profile:isProfileOf rdfs:,
        skos:,
        <https://w3id.org/dpv/tech> ;
    foaf:logo <https://w3id.org/dpv/media/logo.png> ;
    schema:version "2.1-dev" .

ai:serialisation-html a profile:ResourceDescriptor ;
    dct:conformsTo <https://www.w3.org/TR/html/> ;
    dct:format <https://www.iana.org/assignments/media-types/text/html> ;
    dct:title "AI Technology Concepts - HTML serialiation" ;
    profile:hasArtifact <https://w3id.org/dpv/ai/ai.html> ;
    profile:hasRole role:specification .

ai:serialisation-jsonld a profile:ResourceDescriptor ;
    dct:conformsTo <https://www.w3.org/TR/json-ld11/> ;
    dct:format <https://www.iana.org/assignments/media-types/application/ld+json> ;
    dct:title "AI Technology Concepts - JSON-LD serialiation" ;
    profile:hasArtifact <https://w3id.org/dpv/ai/ai.jsonld> ;
    profile:hasRole role:vocabulary .

ai:serialisation-n3 a profile:ResourceDescriptor ;
    dct:conformsTo <https://www.w3.org/TeamSubmission/n3/> ;
    dct:format <https://www.iana.org/assignments/media-types/text/n3> ;
    dct:title "AI Technology Concepts - N3 serialiation" ;
    profile:hasArtifact <https://w3id.org/dpv/ai/ai.n3> ;
    profile:hasRole role:vocabulary .

ai:serialisation-rdf a profile:ResourceDescriptor ;
    dct:conformsTo rdf: ;
    dct:format <https://www.iana.org/assignments/media-types/application/rdf+xml> ;
    dct:title "AI Technology Concepts - RDF/XML serialiation" ;
    profile:hasArtifact <https://w3id.org/dpv/ai/ai.rdf> ;
    profile:hasRole role:vocabulary .

ai:serialisation-ttl a profile:ResourceDescriptor ;
    dct:conformsTo <https://www.w3.org/TR/turtle/> ;
    dct:format <https://www.iana.org/assignments/media-types/text/turtle> ;
    dct:title "AI Technology Concepts - Turtle serialiation" ;
    profile:hasArtifact <https://w3id.org/dpv/ai/ai.ttl> ;
    profile:hasRole role:vocabulary .

<https://w3id.org/dpv/examples> a profile:ResourceDescriptor ;
    dct:conformsTo <https://www.w3.org/TR/html/> ;
    dct:format <https://www.iana.org/assignments/media-types/text/html> ;
    dct:title "Examples for Data Privacy Vocabulary" ;
    profile:hasArtifact <https://w3id.org/dpv/examples> ;
    profile:hasRole role:guidance .

<https://w3id.org/dpv/guides> a profile:ResourceDescriptor ;
    dct:conformsTo <https://www.w3.org/TR/html/> ;
    dct:format <https://www.iana.org/assignments/media-types/text/html> ;
    dct:title "Guides for Data Privacy Vocabulary" ;
    profile:hasArtifact <https://w3id.org/dpv/guides> ;
    profile:hasRole role:guidance .

<https://w3id.org/dpv/primer> a profile:ResourceDescriptor ;
    dct:conformsTo <https://www.w3.org/TR/html/> ;
    dct:format <https://www.iana.org/assignments/media-types/text/html> ;
    dct:title "Primer for Data Privacy Vocabulary" ;
    profile:hasArtifact <https://w3id.org/dpv/primer> ;
    profile:hasRole role:guidance .

ai:bias-classes a skos:ConceptScheme .

