<?xml version="1.0" encoding="utf-8"?>
<rdf:RDF
   xmlns:bibo="http://purl.org/ontology/bibo/"
   xmlns:dcam="http://purl.org/dc/dcam/"
   xmlns:dct="http://purl.org/dc/terms/"
   xmlns:foaf="http://xmlns.com/foaf/0.1/"
   xmlns:org="http://www.w3.org/ns/org#"
   xmlns:owl="http://www.w3.org/2002/07/owl#"
   xmlns:profile="http://www.w3.org/ns/dx/prof/"
   xmlns:rdf="http://www.w3.org/1999/02/22-rdf-syntax-ns#"
   xmlns:rdfs="http://www.w3.org/2000/01/rdf-schema#"
   xmlns:schema="https://schema.org/"
   xmlns:scoro="http://purl.org/spar/scoro/"
   xmlns:skos="http://www.w3.org/2004/02/skos/core#"
   xmlns:sw="http://www.w3.org/2003/06/sw-vocab-status/ns#"
   xmlns:vann="http://purl.org/vocab/vann/"
>
  <rdf:Description rdf:nodeID="Ne22a67b17c7e4a779c30d2864b6a0cee">
    <foaf:name>Harshvardhan J. Pandit</foaf:name>
    <rdf:type rdf:resource="http://purl.org/dc/terms/Agent"/>
    <rdf:type rdf:resource="http://xmlns.com/foaf/0.1/Person"/>
    <foaf:homepage>https://harshp.com/</foaf:homepage>
    <scoro:hasORCID>0000-0002-5068-3714</scoro:hasORCID>
    <org:memberOf rdf:nodeID="N6cd6ef5ec58745369be45f4a23814332"/>
  </rdf:Description>
  <rdf:Description rdf:about="https://w3id.org/dpv/ai/owl#">
    <owl:versionIRI rdf:resource="https://w3id.org/dpv/2.1/ai/owl#"/>
    <profile:hasResource rdf:resource="https://w3id.org/dpv/primer"/>
    <profile:hasResource rdf:resource="https://w3id.org/dpv/guides"/>
    <profile:hasResource rdf:resource="https://w3id.org/dpv/ai/owl#serialisation-jsonld"/>
    <profile:hasResource rdf:resource="https://w3id.org/dpv/ai/owl#serialisation-html"/>
    <profile:hasResource rdf:resource="https://w3id.org/dpv/ai/owl#serialisation-ttl"/>
    <profile:hasResource rdf:resource="https://w3id.org/dpv/ai/owl#serialisation-rdf"/>
    <profile:hasResource rdf:resource="https://w3id.org/dpv/ai/owl#serialisation-n3"/>
    <profile:hasResource rdf:resource="https://w3id.org/dpv/examples"/>
    <dct:bibliographicCitation>Harshvardhan J. Pandit, Beatriz Esteves, Georg P. Krog, Paul Ryan, Delaram Golpayegani, Julian Flake (2025) Data Privacy Vocabulary (DPV) – Version 2.0. In: Demartini, G., et al. The Semantic Web – ISWC 2024. ISWC 2024. Lecture Notes in Computer Science, vol 15233. Springer, Cham. https://doi.org/10.1007/978-3-031-77847-6_10</dct:bibliographicCitation>
    <bibo:status>http://purl.org/ontology/bibo/status/published</bibo:status>
    <dct:hasVersion rdf:resource="https://w3id.org/dpv/ai/owl#"/>
    <dct:issued xml:lang="en">2024-05-31</dct:issued>
    <dct:contributor rdf:nodeID="N9c63c24625fe482386a350b4ea27b4f8"/>
    <dct:conformsTo>http://www.w3.org/2004/02/skos/core</dct:conformsTo>
    <dct:conformsTo>http://www.w3.org/2000/01/rdf-schema</dct:conformsTo>
    <dct:conformsTo rdf:resource="http://www.w3.org/2002/07/owl"/>
    <vann:preferredNamespaceUri>https://w3id.org/dpv/ai#</vann:preferredNamespaceUri>
    <rdf:type rdf:resource="http://www.w3.org/2002/07/owl#Ontology"/>
    <rdf:type rdf:resource="http://www.w3.org/ns/dx/prof/Profile"/>
    <rdfs:Label xml:lang="en">AI</rdfs:Label>
    <dct:title xml:lang="en">AI Technology Concepts</dct:title>
    <dct:creator rdf:nodeID="Ne22a67b17c7e4a779c30d2864b6a0cee"/>
    <dct:creator rdf:nodeID="N9c63c24625fe482386a350b4ea27b4f8"/>
    <owl:versionInfo>2.1</owl:versionInfo>
    <bibo:doi>10.5281/zenodo.12505841</bibo:doi>
    <vann:preferredNamespacePrefix>ai</vann:preferredNamespacePrefix>
    <dct:license rdf:resource="https://www.w3.org/copyright/document-license-2023/"/>
    <dct:identifier>https://w3id.org/dpv/ai</dct:identifier>
    <schema:version>2.1</schema:version>
    <dct:created xml:lang="en">2024-05-31</dct:created>
    <foaf:logo rdf:resource="https://w3id.org/dpv/media/logo.png"/>
    <dct:publisher rdf:resource="https://www.w3.org/"/>
    <profile:isProfileOf rdf:resource="http://www.w3.org/2002/07/owl"/>
    <profile:isProfileOf rdf:resource="https://w3id.org/dpv/tech/owl"/>
    <profile:isProfileOf rdf:resource="https://w3id.org/dpv/ai/owl#"/>
    <dct:modified xml:lang="en">2025-02-01</dct:modified>
    <dct:description xml:lang="en">Extension to the Data Privacy Vocabulary (DPV) providing concepts for representing information about AI technologies</dct:description>
    <dct:source rdf:resource="https://www.w3.org/groups/cg/dpvcg/"/>
  </rdf:Description>
  <rdf:Description rdf:about="https://w3id.org/dpv/ai/owl#hasAI">
    <dcam:rangeIncludes rdf:resource="https://w3id.org/dpv/ai/owl#AI"/>
    <rdfs:isDefinedBy rdf:resource="https://w3id.org/dpv/ai/owl#"/>
    <skos:definition xml:lang="en">Indicates the use of AI for the associated context</skos:definition>
    <skos:prefLabel xml:lang="en">has AI</skos:prefLabel>
    <rdf:type rdf:resource="http://www.w3.org/1999/02/22-rdf-syntax-ns#Property"/>
    <rdf:type rdf:resource="http://www.w3.org/2002/07/owl#ObjectProperty"/>
    <dct:created rdf:datatype="http://www.w3.org/2001/XMLSchema#date">2024-12-01</dct:created>
    <dct:contributor rdf:nodeID="N9c63c24625fe482386a350b4ea27b4f8"/>
    <rdfs:subPropertyOf rdf:resource="https://w3id.org/dpv/owl#isImplementedUsingTechnology"/>
    <schema:rangeIncludes rdf:resource="https://w3id.org/dpv/ai/owl#AI"/>
    <sw:term_status xml:lang="en">accepted</sw:term_status>
  </rdf:Description>
  <rdf:Description rdf:about="https://w3id.org/dpv/ai/owl#hasCapability">
    <rdf:type rdf:resource="http://www.w3.org/1999/02/22-rdf-syntax-ns#Property"/>
    <rdf:type rdf:resource="http://www.w3.org/2002/07/owl#ObjectProperty"/>
    <dct:contributor rdf:nodeID="N9c63c24625fe482386a350b4ea27b4f8"/>
    <schema:rangeIncludes rdf:resource="https://w3id.org/dpv/ai/owl#Capability"/>
    <dct:created rdf:datatype="http://www.w3.org/2001/XMLSchema#date">2024-12-01</dct:created>
    <rdfs:isDefinedBy rdf:resource="https://w3id.org/dpv/ai/owl#"/>
    <sw:term_status xml:lang="en">accepted</sw:term_status>
    <rdfs:subPropertyOf rdf:resource="https://w3id.org/dpv/ai/owl#hasAI"/>
    <skos:prefLabel xml:lang="en">has capability</skos:prefLabel>
    <dcam:rangeIncludes rdf:resource="https://w3id.org/dpv/ai/owl#Capability"/>
    <skos:definition xml:lang="en">Indicates the use of AI capability for the associated context</skos:definition>
  </rdf:Description>
  <rdf:Description rdf:about="https://w3id.org/dpv/ai/owl#Technique">
    <skos:scopeNote xml:lang="en">This concept refers to the foundational computational implementation and is necessary to distinguish the 'algorithm' (ai:Technique) from the 'application' (ai:Capability) and 'goal' (dpv:Purpose)</skos:scopeNote>
    <rdfs:subClassOf rdf:resource="https://w3id.org/dpv/ai/owl#AI"/>
    <skos:definition xml:lang="en">The underlying technological algorithm, method, or process that forms the technique for using or applying AI</skos:definition>
    <rdf:type rdf:resource="http://www.w3.org/2000/01/rdf-schema#Class"/>
    <rdf:type rdf:resource="http://www.w3.org/2002/07/owl#Class"/>
    <skos:prefLabel xml:lang="en">Technique</skos:prefLabel>
    <dct:contributor rdf:nodeID="N9c63c24625fe482386a350b4ea27b4f8"/>
    <dct:created rdf:datatype="http://www.w3.org/2001/XMLSchema#date">2024-04-28</dct:created>
    <sw:term_status xml:lang="en">accepted</sw:term_status>
    <rdfs:isDefinedBy rdf:resource="https://w3id.org/dpv/ai/owl#"/>
  </rdf:Description>
  <rdf:Description rdf:nodeID="N6cd6ef5ec58745369be45f4a23814332">
    <foaf:name>ADAPT Centre, Dublin City University</foaf:name>
    <rdf:type rdf:resource="http://xmlns.com/foaf/0.1/Organization"/>
  </rdf:Description>
  <rdf:Description rdf:about="https://w3id.org/dpv/primer">
    <profile:hasArtifact rdf:resource="https://w3id.org/dpv/primer"/>
    <profile:hasRole rdf:resource="http://www.w3.org/ns/dx/prof/role/guidance"/>
    <dct:format rdf:resource="https://www.iana.org/assignments/media-types/text/html"/>
    <dct:conformsTo rdf:resource="https://www.w3.org/TR/html/"/>
    <rdf:type rdf:resource="http://www.w3.org/ns/dx/prof/ResourceDescriptor"/>
    <dct:title>Primer for Data Privacy Vocabulary</dct:title>
  </rdf:Description>
  <rdf:Description rdf:about="https://w3id.org/dpv/guides">
    <profile:hasArtifact rdf:resource="https://w3id.org/dpv/guides"/>
    <dct:format rdf:resource="https://www.iana.org/assignments/media-types/text/html"/>
    <dct:conformsTo rdf:resource="https://www.w3.org/TR/html/"/>
    <rdf:type rdf:resource="http://www.w3.org/ns/dx/prof/ResourceDescriptor"/>
    <profile:hasRole rdf:resource="http://www.w3.org/ns/dx/prof/role/guidance"/>
    <dct:title>Guides for Data Privacy Vocabulary</dct:title>
  </rdf:Description>
  <rdf:Description rdf:about="https://w3id.org/dpv/ai/owl#serialisation-ttl">
    <dct:title>AI Technology Concepts - Turtle serialiation</dct:title>
    <dct:format rdf:resource="https://www.iana.org/assignments/media-types/text/turtle"/>
    <profile:hasArtifact rdf:resource="https://w3id.org/dpv/ai/ai-owl.ttl"/>
    <rdf:type rdf:resource="http://www.w3.org/ns/dx/prof/ResourceDescriptor"/>
    <dct:conformsTo rdf:resource="https://www.w3.org/TR/turtle/"/>
    <profile:hasRole rdf:resource="http://www.w3.org/ns/dx/prof/role/vocabulary"/>
  </rdf:Description>
  <rdf:Description rdf:about="https://w3id.org/dpv/ai/owl#hasAISystem">
    <rdfs:isDefinedBy rdf:resource="https://w3id.org/dpv/ai/owl#"/>
    <rdf:type rdf:resource="http://www.w3.org/1999/02/22-rdf-syntax-ns#Property"/>
    <rdf:type rdf:resource="http://www.w3.org/2002/07/owl#ObjectProperty"/>
    <skos:prefLabel xml:lang="en">has AI system</skos:prefLabel>
    <dcam:rangeIncludes rdf:resource="https://w3id.org/dpv/ai/owl#AISystem"/>
    <skos:definition xml:lang="en">Indicates the use of AI system for the associated context</skos:definition>
    <dct:contributor rdf:nodeID="N9c63c24625fe482386a350b4ea27b4f8"/>
    <rdfs:subPropertyOf rdf:resource="https://w3id.org/dpv/ai/owl#hasAI"/>
    <sw:term_status xml:lang="en">accepted</sw:term_status>
    <dct:created rdf:datatype="http://www.w3.org/2001/XMLSchema#date">2024-12-01</dct:created>
    <schema:rangeIncludes rdf:resource="https://w3id.org/dpv/ai/owl#AISystem"/>
  </rdf:Description>
  <rdf:Description rdf:about="https://w3id.org/dpv/ai/owl#hasGPAIModel">
    <skos:definition xml:lang="en">Indicates the use of an GPAI model for the associated context</skos:definition>
    <dct:created rdf:datatype="http://www.w3.org/2001/XMLSchema#date">2024-12-01</dct:created>
    <rdf:type rdf:resource="http://www.w3.org/1999/02/22-rdf-syntax-ns#Property"/>
    <rdf:type rdf:resource="http://www.w3.org/2002/07/owl#ObjectProperty"/>
    <sw:term_status xml:lang="en">accepted</sw:term_status>
    <schema:rangeIncludes rdf:resource="https://w3id.org/dpv/ai/owl#GPAIModel"/>
    <skos:prefLabel xml:lang="en">has GPAI model</skos:prefLabel>
    <rdfs:isDefinedBy rdf:resource="https://w3id.org/dpv/ai/owl#"/>
    <dct:contributor rdf:nodeID="N9c63c24625fe482386a350b4ea27b4f8"/>
    <dcam:rangeIncludes rdf:resource="https://w3id.org/dpv/ai/owl#GPAIModel"/>
    <rdfs:subPropertyOf rdf:resource="https://w3id.org/dpv/ai/owl#hasModel"/>
  </rdf:Description>
  <rdf:Description rdf:about="https://w3id.org/dpv/ai/owl#serialisation-jsonld">
    <dct:format rdf:resource="https://www.iana.org/assignments/media-types/application/ld+json"/>
    <dct:conformsTo rdf:resource="https://www.w3.org/TR/json-ld11/"/>
    <rdf:type rdf:resource="http://www.w3.org/ns/dx/prof/ResourceDescriptor"/>
    <profile:hasArtifact rdf:resource="https://w3id.org/dpv/ai/ai-owl.jsonld"/>
    <dct:title>AI Technology Concepts - JSON-LD serialiation</dct:title>
    <profile:hasRole rdf:resource="http://www.w3.org/ns/dx/prof/role/vocabulary"/>
  </rdf:Description>
  <rdf:Description rdf:about="https://w3id.org/dpv/examples">
    <profile:hasRole rdf:resource="http://www.w3.org/ns/dx/prof/role/guidance"/>
    <dct:format rdf:resource="https://www.iana.org/assignments/media-types/text/html"/>
    <rdf:type rdf:resource="http://www.w3.org/ns/dx/prof/ResourceDescriptor"/>
    <dct:conformsTo rdf:resource="https://www.w3.org/TR/html/"/>
    <profile:hasArtifact rdf:resource="https://w3id.org/dpv/examples"/>
    <dct:title>Examples for Data Privacy Vocabulary</dct:title>
  </rdf:Description>
  <rdf:Description rdf:nodeID="N2b218fbf49474a93a5f1d76695037221">
    <rdf:type rdf:resource="http://xmlns.com/foaf/0.1/Organization"/>
    <foaf:name>ADAPT Centre, Trinity College Dublin</foaf:name>
  </rdf:Description>
  <rdf:Description rdf:about="https://w3id.org/dpv/ai/owl#serialisation-n3">
    <rdf:type rdf:resource="http://www.w3.org/ns/dx/prof/ResourceDescriptor"/>
    <profile:hasRole rdf:resource="http://www.w3.org/ns/dx/prof/role/vocabulary"/>
    <profile:hasArtifact rdf:resource="https://w3id.org/dpv/ai/ai-owl.n3"/>
    <dct:format rdf:resource="https://www.iana.org/assignments/media-types/text/n3"/>
    <dct:conformsTo rdf:resource="https://www.w3.org/TeamSubmission/n3/"/>
    <dct:title>AI Technology Concepts - N3 serialiation</dct:title>
  </rdf:Description>
  <rdf:Description rdf:about="https://w3id.org/dpv/ai/owl#AISystem">
    <rdf:type rdf:resource="http://www.w3.org/2000/01/rdf-schema#Class"/>
    <rdf:type rdf:resource="http://www.w3.org/2002/07/owl#Class"/>
    <dct:source xml:lang="en">OECD.AI</dct:source>
    <dct:source xml:lang="en"> ISO/IEC 22989:2023</dct:source>
    <dct:created rdf:datatype="http://www.w3.org/2001/XMLSchema#date">2024-05-17</dct:created>
    <rdfs:isDefinedBy rdf:resource="https://w3id.org/dpv/ai/owl#"/>
    <skos:prefLabel xml:lang="en">AI System</skos:prefLabel>
    <rdfs:subClassOf rdf:resource="https://w3id.org/dpv/ai/owl#AI"/>
    <rdfs:subClassOf rdf:resource="https://w3id.org/dpv/tech/owl#System"/>
    <dct:contributor rdf:nodeID="N9c63c24625fe482386a350b4ea27b4f8"/>
    <sw:term_status xml:lang="en">accepted</sw:term_status>
    <skos:definition xml:lang="en">An engineered system that generates outputs such as content, forecasts, recommendations or decisions for a given set of human-defined objectives (ISO/IEC 22989:2023 definition); or A machine-based system that, for explicit or implicit objectives, infers, from the input it receives, how to generate outputs such as predictions, content, recommendations, or decisions that can influence physical or virtual environments. Different AI systems vary in their levels of autonomy and adaptiveness after deployment (OECD 2024 definition)</skos:definition>
  </rdf:Description>
  <rdf:Description rdf:about="https://w3id.org/dpv/ai/owl#serialisation-rdf">
    <dct:conformsTo rdf:resource="http://www.w3.org/1999/02/22-rdf-syntax-ns#"/>
    <dct:format rdf:resource="https://www.iana.org/assignments/media-types/application/rdf+xml"/>
    <profile:hasRole rdf:resource="http://www.w3.org/ns/dx/prof/role/vocabulary"/>
    <rdf:type rdf:resource="http://www.w3.org/ns/dx/prof/ResourceDescriptor"/>
    <profile:hasArtifact rdf:resource="https://w3id.org/dpv/ai/ai-owl.rdf"/>
    <dct:title>AI Technology Concepts - RDF/XML serialiation</dct:title>
  </rdf:Description>
  <rdf:Description rdf:about="https://w3id.org/dpv/ai/owl#Capability">
    <rdfs:isDefinedBy rdf:resource="https://w3id.org/dpv/ai/owl#"/>
    <sw:term_status xml:lang="en">accepted</sw:term_status>
    <skos:scopeNote xml:lang="en">This concept refers to the application of an AI technique to achieve a technical goal or function, and is necessary to distinguish the 'algorithm' (ai:Technique) from the 'application' (ai:Capability) and 'goal' (dpv:Purpose)</skos:scopeNote>
    <skos:definition xml:lang="en">Capability or use of AI to achieve a technical goal or objective</skos:definition>
    <dct:created rdf:datatype="http://www.w3.org/2001/XMLSchema#date">2024-04-28</dct:created>
    <rdfs:subClassOf rdf:resource="https://w3id.org/dpv/ai/owl#AI"/>
    <rdf:type rdf:resource="http://www.w3.org/2000/01/rdf-schema#Class"/>
    <rdf:type rdf:resource="http://www.w3.org/2002/07/owl#Class"/>
    <skos:prefLabel xml:lang="en">Capability</skos:prefLabel>
    <dct:contributor rdf:nodeID="N9c63c24625fe482386a350b4ea27b4f8"/>
  </rdf:Description>
  <rdf:Description rdf:about="https://w3id.org/dpv/ai/owl#hasModel">
    <rdf:type rdf:resource="http://www.w3.org/1999/02/22-rdf-syntax-ns#Property"/>
    <rdf:type rdf:resource="http://www.w3.org/2002/07/owl#ObjectProperty"/>
    <dct:contributor rdf:nodeID="N9c63c24625fe482386a350b4ea27b4f8"/>
    <skos:prefLabel xml:lang="en">has model</skos:prefLabel>
    <dcam:rangeIncludes rdf:resource="https://w3id.org/dpv/ai/owl#Model"/>
    <sw:term_status xml:lang="en">accepted</sw:term_status>
    <dct:created rdf:datatype="http://www.w3.org/2001/XMLSchema#date">2024-12-01</dct:created>
    <rdfs:subPropertyOf rdf:resource="https://w3id.org/dpv/ai/owl#hasAI"/>
    <skos:definition xml:lang="en">Indicates the use of an AI model for the associated context</skos:definition>
    <rdfs:isDefinedBy rdf:resource="https://w3id.org/dpv/ai/owl#"/>
    <schema:rangeIncludes rdf:resource="https://w3id.org/dpv/ai/owl#Model"/>
  </rdf:Description>
  <rdf:Description rdf:about="https://w3id.org/dpv/ai/owl#AI">
    <skos:definition xml:lang="en">A technical and scientific field devoted to the engineered system that generates outputs such as content, forecasts, recommendations or decisions for a given set of human-defined objectives</skos:definition>
    <dct:created rdf:datatype="http://www.w3.org/2001/XMLSchema#date">2024-04-28</dct:created>
    <rdfs:isDefinedBy rdf:resource="https://w3id.org/dpv/ai/owl#"/>
    <sw:term_status xml:lang="en">accepted</sw:term_status>
    <rdf:type rdf:resource="http://www.w3.org/2000/01/rdf-schema#Class"/>
    <rdf:type rdf:resource="http://www.w3.org/2002/07/owl#Class"/>
    <rdfs:subClassOf rdf:resource="https://w3id.org/dpv/owl#Technology"/>
    <dct:source xml:lang="en">ISO/IEC 22989:2022</dct:source>
    <skos:prefLabel xml:lang="en">Artificial Intelligence (AI)</skos:prefLabel>
    <dct:contributor rdf:nodeID="N9c63c24625fe482386a350b4ea27b4f8"/>
  </rdf:Description>
  <rdf:Description rdf:about="https://w3id.org/dpv/ai/owl#Model">
    <skos:prefLabel xml:lang="en">Model</skos:prefLabel>
    <dct:source xml:lang="en">ISO/IEC 22989:2022</dct:source>
    <dct:source xml:lang="en"> OECD</dct:source>
    <rdf:type rdf:resource="http://www.w3.org/2000/01/rdf-schema#Class"/>
    <rdf:type rdf:resource="http://www.w3.org/2002/07/owl#Class"/>
    <dct:created rdf:datatype="http://www.w3.org/2001/XMLSchema#date">2024-05-17</dct:created>
    <rdfs:isDefinedBy rdf:resource="https://w3id.org/dpv/ai/owl#"/>
    <dct:contributor rdf:nodeID="N9c63c24625fe482386a350b4ea27b4f8"/>
    <rdfs:subClassOf rdf:resource="https://w3id.org/dpv/ai/owl#AI"/>
    <rdfs:subClassOf rdf:resource="https://w3id.org/dpv/tech/owl#Model"/>
    <skos:definition xml:lang="en">Physical, mathematical or otherwise logical representation of a system, entity, phenomenon, process or data involving the use of AI techniques</skos:definition>
    <sw:term_status xml:lang="en">accepted</sw:term_status>
  </rdf:Description>
  <rdf:Description rdf:nodeID="N9c63c24625fe482386a350b4ea27b4f8">
    <rdf:type rdf:resource="http://purl.org/dc/terms/Agent"/>
    <rdf:type rdf:resource="http://xmlns.com/foaf/0.1/Person"/>
    <org:memberOf rdf:nodeID="N2b218fbf49474a93a5f1d76695037221"/>
    <scoro:hasORCID>0000-0002-1208-186X</scoro:hasORCID>
    <foaf:name>Delaram Golpayegani</foaf:name>
  </rdf:Description>
  <rdf:Description rdf:about="https://w3id.org/dpv/ai/owl#hasTechnique">
    <sw:term_status xml:lang="en">accepted</sw:term_status>
    <rdf:type rdf:resource="http://www.w3.org/1999/02/22-rdf-syntax-ns#Property"/>
    <rdf:type rdf:resource="http://www.w3.org/2002/07/owl#ObjectProperty"/>
    <rdfs:isDefinedBy rdf:resource="https://w3id.org/dpv/ai/owl#"/>
    <skos:definition xml:lang="en">Indicates the use of AI technique for the associated context</skos:definition>
    <skos:prefLabel xml:lang="en">has technique</skos:prefLabel>
    <dct:contributor rdf:nodeID="N9c63c24625fe482386a350b4ea27b4f8"/>
    <dct:created rdf:datatype="http://www.w3.org/2001/XMLSchema#date">2024-12-01</dct:created>
    <dcam:rangeIncludes rdf:resource="https://w3id.org/dpv/ai/owl#Technique"/>
    <rdfs:subPropertyOf rdf:resource="https://w3id.org/dpv/ai/owl#hasAI"/>
    <schema:rangeIncludes rdf:resource="https://w3id.org/dpv/ai/owl#Technique"/>
  </rdf:Description>
  <rdf:Description rdf:about="https://w3id.org/dpv/ai/owl#serialisation-html">
    <dct:format rdf:resource="https://www.iana.org/assignments/media-types/text/html"/>
    <dct:conformsTo rdf:resource="https://www.w3.org/TR/html/"/>
    <rdf:type rdf:resource="http://www.w3.org/ns/dx/prof/ResourceDescriptor"/>
    <dct:title>AI Technology Concepts - HTML serialiation</dct:title>
    <profile:hasRole rdf:resource="http://www.w3.org/ns/dx/prof/role/specification"/>
    <profile:hasArtifact rdf:resource="https://w3id.org/dpv/ai/ai-owl.html"/>
  </rdf:Description>
</rdf:RDF>
