@prefix bibo: <http://purl.org/ontology/bibo/> .
@prefix dct: <http://purl.org/dc/terms/> .
@prefix dex: <https://w3id.org/dpv/examples#> .
@prefix dpv: <https://w3id.org/dpv#> .
@prefix foaf: <http://xmlns.com/foaf/0.1/> .
@prefix org: <http://www.w3.org/ns/org#> .
@prefix owl: <http://www.w3.org/2002/07/owl#> .
@prefix profile: <http://www.w3.org/ns/dx/prof/> .
@prefix rdfs: <http://www.w3.org/2000/01/rdf-schema#> .
@prefix role: <http://www.w3.org/ns/dx/prof/role/> .
@prefix schema: <https://schema.org/> .
@prefix scoro: <http://purl.org/spar/scoro/> .
@prefix skos: <http://www.w3.org/2004/02/skos/core#> .
@prefix sw: <http://www.w3.org/2003/06/sw-vocab-status/ns#> .
@prefix vann: <http://purl.org/vocab/vann/> .
@prefix xsd: <http://www.w3.org/2001/XMLSchema#> .

dpv:AcademicScientificOrganisation a rdfs:Class,
        skos:Concept ;
    dct:contributor _:person-harshvardhan-j-pandit ;
    dct:created "2022-02-02"^^xsd:date ;
    dct:modified "2020-10-05"^^xsd:date ;
    dct:source _:0f97484e2a3b06fd9a79bb7fe79ec7aa ;
    rdfs:isDefinedBy dpv: ;
    rdfs:subClassOf dpv:Organisation ;
    sw:term_status "accepted"@en ;
    skos:broader dpv:Organisation ;
    skos:definition "Organisations related to academia or scientific pursuits e.g. Universities, Schools, Research Bodies"@en ;
    skos:inScheme dpv:entities-organisation-classes ;
    skos:prefLabel "Academic or Scientific Organisation"@en .

dpv:AmbulanceProvider a rdfs:Class,
        skos:Concept ;
    dct:contributor _:person-delaram-golpayegani ;
    dct:created "2024-12-01"^^xsd:date ;
    rdfs:isDefinedBy dpv: ;
    rdfs:subClassOf dpv:EmergencyServiceProvider ;
    sw:term_status "accepted"@en ;
    skos:broader dpv:EmergencyServiceProvider ;
    skos:definition "An organisation that that offers transportation and medical care to patients requiring urgent medical attention"@en ;
    skos:inScheme dpv:entities-organisation-classes ;
    skos:prefLabel "Ambulance Provider"@en .

dpv:CharityOrganisation a rdfs:Class,
        skos:Concept ;
    dct:contributor _:person-georg-p-krog ;
    dct:created "2024-12-01"^^xsd:date ;
    rdfs:isDefinedBy dpv: ;
    rdfs:subClassOf dpv:LegalEntity ;
    sw:term_status "accepted"@en ;
    skos:broader dpv:LegalEntity ;
    skos:definition "A nonprofit entity dedicated to providing assistance or raising funds for social, educational, religious, or other philanthropic purposes"@en ;
    skos:inScheme dpv:entities-organisation-classes ;
    skos:prefLabel "Charity Organisation"@en .

dpv:Clinic a rdfs:Class,
        skos:Concept ;
    dct:contributor _:person-delaram-golpayegani ;
    dct:created "2024-12-01"^^xsd:date ;
    rdfs:isDefinedBy dpv: ;
    rdfs:subClassOf dpv:Organisation ;
    sw:term_status "accepted"@en ;
    skos:broader dpv:Organisation ;
    skos:definition "An organisation that is a smaller healthcare facility offering outpatient medical services for diagnosis and treatment"@en ;
    skos:inScheme dpv:entities-organisation-classes ;
    skos:prefLabel "Clinic"@en .

dpv:EducationalOrganisation a rdfs:Class,
        skos:Concept ;
    dct:contributor _:person-delaram-golpayegani ;
    dct:created "2024-12-01"^^xsd:date ;
    rdfs:isDefinedBy dpv: ;
    rdfs:subClassOf dpv:Organisation ;
    sw:term_status "accepted"@en ;
    skos:broader dpv:Organisation ;
    skos:definition "An organisation focused on delivering formal or informal education, training, or research"@en ;
    skos:inScheme dpv:entities-organisation-classes ;
    skos:prefLabel "Educational Organisation"@en .

dpv:EmergencyHealthcareProvider a rdfs:Class,
        skos:Concept ;
    dct:contributor _:person-delaram-golpayegani ;
    dct:created "2024-12-01"^^xsd:date ;
    rdfs:isDefinedBy dpv: ;
    rdfs:subClassOf dpv:EmergencyServiceProvider ;
    sw:term_status "accepted"@en ;
    skos:broader dpv:EmergencyServiceProvider ;
    skos:definition "An organisation that is an emergency service provider focused on delivering immediate medical care to patients in critical or life-threatening situations"@en ;
    skos:inScheme dpv:entities-organisation-classes ;
    skos:prefLabel "Emergency Healthcare Provider"@en .

dpv:EmergencyServiceProvider a rdfs:Class,
        skos:Concept ;
    dct:contributor _:person-delaram-golpayegani ;
    dct:created "2024-12-01"^^xsd:date ;
    rdfs:isDefinedBy dpv: ;
    rdfs:subClassOf dpv:Organisation ;
    sw:term_status "accepted"@en ;
    skos:broader dpv:Organisation ;
    skos:definition "An organisation tasked with providing emergency services such as by responding rapidly to urgent situations to protect lives, property, and the environment"@en ;
    skos:inScheme dpv:entities-organisation-classes ;
    skos:prefLabel "Emergency Service Provider"@en .

dpv:FireDepartment a rdfs:Class,
        skos:Concept ;
    dct:contributor _:person-delaram-golpayegani ;
    dct:created "2024-12-01"^^xsd:date ;
    rdfs:isDefinedBy dpv: ;
    rdfs:subClassOf dpv:EmergencyServiceProvider ;
    sw:term_status "accepted"@en ;
    skos:broader dpv:EmergencyServiceProvider ;
    skos:definition "An organisation that is an emergency service provider for fire prevention, firefighting, and rescue services"@en ;
    skos:inScheme dpv:entities-organisation-classes ;
    skos:prefLabel "Fire Department"@en .

dpv:ForProfitOrganisation a rdfs:Class,
        skos:Concept ;
    dct:contributor _:person-harshvardhan-j-pandit ;
    dct:created "2022-02-02"^^xsd:date ;
    dct:modified "2020-10-05"^^xsd:date ;
    rdfs:isDefinedBy dpv: ;
    rdfs:subClassOf dpv:Organisation ;
    sw:term_status "accepted"@en ;
    skos:broader dpv:Organisation ;
    skos:definition "An organisation that aims to achieve profit as its primary goal"@en ;
    skos:inScheme dpv:entities-organisation-classes ;
    skos:prefLabel "For-Profit Organisation"@en .

dpv:GovernmentalOrganisation a rdfs:Class,
        skos:Concept ;
    dct:contributor _:person-harshvardhan-j-pandit ;
    dct:created "2022-02-02"^^xsd:date ;
    dct:modified "2020-10-05"^^xsd:date ;
    rdfs:isDefinedBy dpv: ;
    rdfs:subClassOf dpv:Organisation ;
    sw:term_status "accepted"@en ;
    skos:broader dpv:Organisation ;
    skos:definition "An organisation managed or part of government"@en ;
    skos:inScheme dpv:entities-organisation-classes ;
    skos:prefLabel "Governmental Organisation"@en .

dpv:HealthcareOrganisation a rdfs:Class,
        skos:Concept ;
    dct:contributor _:person-delaram-golpayegani ;
    dct:created "2024-12-01"^^xsd:date ;
    rdfs:isDefinedBy dpv: ;
    rdfs:subClassOf dpv:Organisation ;
    sw:term_status "accepted"@en ;
    skos:broader dpv:Organisation ;
    skos:definition "An organisation that delivers medical services, promotes health, and provides care for individuals and communities"@en ;
    skos:inScheme dpv:entities-organisation-classes ;
    skos:prefLabel "Healthcare Organisation"@en .

dpv:Hospital a rdfs:Class,
        skos:Concept ;
    dct:contributor _:person-delaram-golpayegani ;
    dct:created "2024-12-01"^^xsd:date ;
    rdfs:isDefinedBy dpv: ;
    rdfs:subClassOf dpv:Organisation ;
    sw:term_status "accepted"@en ;
    skos:broader dpv:Organisation ;
    skos:definition "An organisation that provides comprehensive medical treatment, including emergency care, surgeries, and inpatient services"@en ;
    skos:inScheme dpv:entities-organisation-classes ;
    skos:prefLabel "Hospital"@en .

dpv:IndustryConsortium a rdfs:Class,
        skos:Concept ;
    dct:contributor _:person-harshvardhan-j-pandit ;
    dct:created "2022-02-02"^^xsd:date ;
    dct:modified "2020-10-05"^^xsd:date ;
    dct:source _:0f97484e2a3b06fd9a79bb7fe79ec7aa ;
    rdfs:isDefinedBy dpv: ;
    rdfs:subClassOf dpv:Organisation ;
    sw:term_status "accepted"@en ;
    skos:broader dpv:Organisation ;
    skos:definition "A consortium established and comprising on industry organisations"@en ;
    skos:inScheme dpv:entities-organisation-classes ;
    skos:prefLabel "Industry Consortium"@en .

dpv:InternationalOrganisation a rdfs:Class,
        skos:Concept ;
    dct:contributor _:person-georg-p-krog,
        _:person-julian-flake ;
    dct:created "2022-03-23"^^xsd:date ;
    dct:modified "2020-10-05"^^xsd:date ;
    dct:source [ a schema:WebPage ;
            schema:name "GDPR Art.4-26" ;
            schema:url "https://eur-lex.europa.eu/eli/reg/2016/679/art_4/par_26/oj" ] ;
    rdfs:isDefinedBy dpv: ;
    rdfs:subClassOf dpv:Organisation ;
    sw:term_status "accepted"@en ;
    skos:broader dpv:Organisation ;
    skos:definition "An organisation and its subordinate bodies governed by public international law, or any other body which is set up by, or on the basis of, an agreement between two or more countries"@en ;
    skos:inScheme dpv:entities-organisation-classes ;
    skos:prefLabel "International Organisation"@en .

dpv:JudicialOrganisation a rdfs:Class,
        skos:Concept ;
    dct:contributor _:person-delaram-golpayegani ;
    dct:created "2024-12-01"^^xsd:date ;
    rdfs:isDefinedBy dpv: ;
    rdfs:subClassOf dpv:Organisation ;
    sw:term_status "accepted"@en ;
    skos:broader dpv:Organisation ;
    skos:definition "An organisation involved in interpreting and applying the law, resolving disputes, and administering justice as part of the judicial system"@en ;
    skos:inScheme dpv:entities-organisation-classes ;
    skos:prefLabel "Judicial Organisation"@en .

dpv:LawEnforcementOrganisation a rdfs:Class,
        skos:Concept ;
    dct:contributor _:person-delaram-golpayegani ;
    dct:created "2024-12-01"^^xsd:date ;
    rdfs:isDefinedBy dpv: ;
    rdfs:subClassOf dpv:Organisation ;
    sw:term_status "accepted"@en ;
    skos:broader dpv:Organisation ;
    skos:definition "An organisation that is an agency responsible for enforcing laws, maintaining public order, and ensuring public safety"@en ;
    skos:inScheme dpv:entities-organisation-classes ;
    skos:prefLabel "Law Enforcement Organisation"@en .

dpv:NonGovernmentalOrganisation a rdfs:Class,
        skos:Concept ;
    dct:contributor _:person-harshvardhan-j-pandit ;
    dct:created "2022-02-02"^^xsd:date ;
    dct:modified "2020-10-05"^^xsd:date ;
    dct:source _:0f97484e2a3b06fd9a79bb7fe79ec7aa ;
    rdfs:isDefinedBy dpv: ;
    rdfs:subClassOf dpv:Organisation ;
    sw:term_status "accepted"@en ;
    skos:broader dpv:Organisation ;
    skos:definition "An organisation not part of or independent from the government"@en ;
    skos:inScheme dpv:entities-organisation-classes ;
    skos:prefLabel "Non-Governmental Organisation"@en .

dpv:NonProfitOrganisation a rdfs:Class,
        skos:Concept ;
    dct:contributor _:person-harshvardhan-j-pandit ;
    dct:created "2022-02-02"^^xsd:date ;
    dct:modified "2020-10-05"^^xsd:date ;
    dct:source _:0f97484e2a3b06fd9a79bb7fe79ec7aa ;
    rdfs:isDefinedBy dpv: ;
    rdfs:subClassOf dpv:Organisation ;
    sw:term_status "accepted"@en ;
    skos:broader dpv:Organisation ;
    skos:definition "An organisation that does not aim to achieve profit as its primary goal"@en ;
    skos:inScheme dpv:entities-organisation-classes ;
    skos:prefLabel "Non-Profit Organisation"@en .

dpv:Organisation a rdfs:Class,
        skos:Concept ;
    dct:contributor _:person-harshvardhan-j-pandit ;
    dct:created "2022-02-02"^^xsd:date ;
    rdfs:isDefinedBy dpv: ;
    rdfs:subClassOf dpv:LegalEntity ;
    sw:term_status "accepted"@en ;
    skos:broader dpv:LegalEntity ;
    skos:definition "A general term reflecting a company or a business or a group acting as a unit"@en ;
    skos:inScheme dpv:entities-organisation-classes ;
    skos:prefLabel "Organisation"@en .

dpv:OrganisationalUnit a rdfs:Class,
        skos:Concept ;
    dct:contributor _:person-harshvardhan-j-pandit,
        _:person-paul-ryan ;
    dct:created "2022-03-23"^^xsd:date ;
    vann:example dex:E0037 ;
    rdfs:isDefinedBy dpv: ;
    rdfs:subClassOf dpv:Entity ;
    sw:term_status "accepted"@en ;
    skos:broader dpv:Entity ;
    skos:definition "Entity within an organisation that does not constitute as a separate legal entity"@en ;
    skos:inScheme dpv:entities-organisation-classes ;
    skos:prefLabel "Organisational Unit"@en .

dpv:PrivateSectorBody a rdfs:Class,
        skos:Concept ;
    dct:contributor _:person-georg-p-krog ;
    dct:created "2024-12-01"^^xsd:date ;
    rdfs:isDefinedBy dpv: ;
    rdfs:subClassOf dpv:LegalEntity ;
    sw:term_status "accepted"@en ;
    skos:broader dpv:LegalEntity ;
    skos:definition "An organisation owned and operated by private individuals or companies"@en ;
    skos:inScheme dpv:entities-organisation-classes ;
    skos:prefLabel "Private Sector Body"@en .

dpv:PublicSectorBody a rdfs:Class,
        skos:Concept ;
    dct:contributor _:person-georg-p-krog ;
    dct:created "2024-12-01"^^xsd:date ;
    rdfs:isDefinedBy dpv: ;
    rdfs:subClassOf dpv:LegalEntity ;
    sw:term_status "accepted"@en ;
    skos:broader dpv:LegalEntity ;
    skos:definition "A government-controlled organisation that provides services or goods to the public"@en ;
    skos:inScheme dpv:entities-organisation-classes ;
    skos:prefLabel "Public Sector Body"@en .

dpv:ReligiousAssociations a rdfs:Class,
        skos:Concept ;
    dct:contributor _:person-georg-p-krog ;
    dct:created "2024-12-01"^^xsd:date ;
    rdfs:isDefinedBy dpv: ;
    rdfs:subClassOf dpv:Organisation ;
    sw:term_status "accepted"@en ;
    skos:broader dpv:Organisation ;
    skos:definition "An organisations that supports the practice, promotion, and management of religious activities and beliefs"@en ;
    skos:inScheme dpv:entities-organisation-classes ;
    skos:prefLabel "Religious Associations"@en .

dpv:SMEOrganisation a rdfs:Class,
        skos:Concept ;
    dct:contributor _:person-georg-p-krog ;
    dct:created "2024-12-01"^^xsd:date ;
    rdfs:isDefinedBy dpv: ;
    rdfs:subClassOf dpv:LegalEntity ;
    sw:term_status "accepted"@en ;
    skos:broader dpv:LegalEntity ;
    skos:definition "An organisation that is characterised as a Small or Medium-sized Enterprise based on limited staff and revenue"@en ;
    skos:inScheme dpv:entities-organisation-classes ;
    skos:prefLabel "SME Organisation"@en .

dpv:StartupOrganisation a rdfs:Class,
        skos:Concept ;
    dct:contributor _:person-georg-p-krog ;
    dct:created "2024-12-01"^^xsd:date ;
    rdfs:isDefinedBy dpv: ;
    rdfs:subClassOf dpv:LegalEntity ;
    sw:term_status "accepted"@en ;
    skos:broader dpv:LegalEntity ;
    skos:definition "An organisation that is newly established and is nascent in terms of available resources"@en ;
    skos:inScheme dpv:entities-organisation-classes ;
    skos:prefLabel "Startup Organisation"@en .

<https://w3id.org/dpv> a owl:Ontology,
        profile:Profile ;
    dct:bibliographicCitation "Harshvardhan J. Pandit, Beatriz Esteves, Georg P. Krog, Paul Ryan, Delaram Golpayegani, Julian Flake (2025) Data Privacy Vocabulary (DPV) – Version 2.0. In: Demartini, G., et al. The Semantic Web – ISWC 2024. ISWC 2024. Lecture Notes in Computer Science, vol 15233. Springer, Cham. https://doi.org/10.1007/978-3-031-77847-6_10" ;
    dct:conformsTo "http://www.w3.org/2000/01/rdf-schema",
        "http://www.w3.org/2004/02/skos/core" ;
    dct:contributor _:person-delaram-golpayegani,
        _:person-georg-p-krog,
        _:person-harshvardhan-j-pandit,
        _:person-julian-flake,
        _:person-paul-ryan ;
    dct:created "2022-08-18"@en ;
    dct:creator [ a dct:Agent,
                foaf:Person ;
            scoro:hasORCID "0000-0003-0259-7560" ;
            org:memberOf [ a foaf:Organization ;
                    foaf:name "IDLab, IMEC, Ghent University" ] ;
            foaf:name "Beatriz Esteves" ],
        _:person-delaram-golpayegani,
        _:person-georg-p-krog,
        _:person-harshvardhan-j-pandit,
        _:person-julian-flake,
        _:person-paul-ryan ;
    dct:description "The Data Privacy Vocabulary (DPV) provides terms (classes and properties) to represent information about processing of personal data, for example - purposes, processing operations, personal data, technical and organisational measures."@en ;
    dct:identifier "https://w3id.org/dpv" ;
    dct:issued "2022-08-18"@en ;
    dct:license <https://www.w3.org/copyright/document-license-2023/> ;
    dct:modified "2026-08-01"@en ;
    dct:publisher <https://www.w3.org/> ;
    dct:source <https://www.w3.org/groups/cg/dpvcg/> ;
    dct:title "Data Privacy Vocabulary (DPV)"@en ;
    bibo:doi "10.5281/zenodo.12505841" ;
    bibo:status "http://purl.org/ontology/bibo/status/published" ;
    vann:preferredNamespacePrefix "dpv" ;
    vann:preferredNamespaceUri "https://w3id.org/dpv#" ;
    rdfs:Label "DPV"@en ;
    owl:versionIRI <https://w3id.org/dpv/2.2> ;
    owl:versionInfo "2.2" ;
    profile:hasResource dpv:serialisation-html,
        dpv:serialisation-ttl,
        <https://w3id.org/dpv/examples>,
        <https://w3id.org/dpv/guides>,
        <https://w3id.org/dpv/primer> ;
    profile:isProfileOf rdfs:,
        skos: ;
    foaf:logo <https://w3id.org/dpv/media/logo.png> ;
    schema:version "2.2" .

dpv:serialisation-html a profile:ResourceDescriptor ;
    dct:conformsTo <https://www.w3.org/TR/html/> ;
    dct:format <https://www.iana.org/assignments/media-types/text/html> ;
    dct:title "Data Privacy Vocabulary (DPV) - HTML serialisation" ;
    profile:hasArtifact <https://w3id.org/dpv/dpv.html> ;
    profile:hasRole role:specification .

dpv:serialisation-ttl a profile:ResourceDescriptor ;
    dct:conformsTo <https://www.w3.org/TR/turtle/> ;
    dct:format <https://www.iana.org/assignments/media-types/text/turtle> ;
    dct:title "Data Privacy Vocabulary (DPV) - Turtle serialisation" ;
    profile:hasArtifact <https://w3id.org/dpv/dpv/dpv.ttl> ;
    profile:hasRole role:vocabulary .

<https://w3id.org/dpv/examples> a profile:ResourceDescriptor ;
    dct:conformsTo <https://www.w3.org/TR/html/> ;
    dct:format <https://www.iana.org/assignments/media-types/text/html> ;
    dct:title "Examples for Data Privacy Vocabulary" ;
    profile:hasArtifact <https://w3id.org/dpv/examples> ;
    profile:hasRole role:guidance .

<https://w3id.org/dpv/guides> a profile:ResourceDescriptor ;
    dct:conformsTo <https://www.w3.org/TR/html/> ;
    dct:format <https://www.iana.org/assignments/media-types/text/html> ;
    dct:title "Guides for Data Privacy Vocabulary" ;
    profile:hasArtifact <https://w3id.org/dpv/guides> ;
    profile:hasRole role:guidance .

<https://w3id.org/dpv/primer> a profile:ResourceDescriptor ;
    dct:conformsTo <https://www.w3.org/TR/html/> ;
    dct:format <https://www.iana.org/assignments/media-types/text/html> ;
    dct:title "Primer for Data Privacy Vocabulary" ;
    profile:hasArtifact <https://w3id.org/dpv/primer> ;
    profile:hasRole role:guidance .

dpv:entities-organisation-classes a skos:ConceptScheme .

_:org-adapt-centre-trinity-college-dublin a foaf:Organization ;
    foaf:name "ADAPT Centre, Trinity College Dublin" .

_:org-ai-accountability-lab-aial-trinity-college-dublin a foaf:Organization ;
    foaf:name "AI Accountability Lab (AIAL), Trinity College Dublin" .

_:org-signatu-as a foaf:Organization ;
    foaf:name "Signatu AS" .

_:org-uniphar-plc a foaf:Organization ;
    foaf:name "Uniphar PLC" .

_:org-university-of-koblenz a foaf:Organization ;
    foaf:name "University of Koblenz" .

_:person-julian-flake a dct:Agent,
        foaf:Person ;
    scoro:hasORCID "0009-0006-4623-1463" ;
    org:memberOf _:org-university-of-koblenz ;
    foaf:name "Julian Flake" .

_:person-paul-ryan a dct:Agent,
        foaf:Person ;
    scoro:hasORCID "0000-0003-0770-2737" ;
    org:memberOf _:org-uniphar-plc ;
    foaf:name "Paul Ryan" .

_:0f97484e2a3b06fd9a79bb7fe79ec7aa a schema:WebPage ;
    schema:name "ADMS controlled vocabulary" ;
    schema:url "http://purl.org/adms" .

_:person-georg-p-krog a dct:Agent,
        foaf:Person ;
    org:memberOf _:org-signatu-as ;
    foaf:homepage "https://www.linkedin.com/in/georg-philip-krog-a2a278104/" ;
    foaf:name "Georg P. Krog" .

_:person-harshvardhan-j-pandit a dct:Agent,
        foaf:Person ;
    scoro:hasORCID "0000-0002-5068-3714" ;
    org:memberOf _:org-ai-accountability-lab-aial-trinity-college-dublin ;
    foaf:homepage "https://harshp.com/" ;
    foaf:name "Harshvardhan J. Pandit" .

_:person-delaram-golpayegani a dct:Agent,
        foaf:Person ;
    scoro:hasORCID "0000-0002-1208-186X" ;
    org:memberOf _:org-adapt-centre-trinity-college-dublin ;
    foaf:name "Delaram Golpayegani" .

