@prefix bibo: <http://purl.org/ontology/bibo/> .
@prefix dcam: <http://purl.org/dc/dcam/> .
@prefix dct: <http://purl.org/dc/terms/> .
@prefix dex-owl: <https://w3id.org/dpv/examples/owl#> .
@prefix dpv-owl: <https://w3id.org/dpv/owl#> .
@prefix foaf: <http://xmlns.com/foaf/0.1/> .
@prefix org: <http://www.w3.org/ns/org#> .
@prefix owl: <http://www.w3.org/2002/07/owl#> .
@prefix profile: <http://www.w3.org/ns/dx/prof/> .
@prefix rdf: <http://www.w3.org/1999/02/22-rdf-syntax-ns#> .
@prefix rdfs: <http://www.w3.org/2000/01/rdf-schema#> .
@prefix role: <http://www.w3.org/ns/dx/prof/role/> .
@prefix schema: <https://schema.org/> .
@prefix scoro: <http://purl.org/spar/scoro/> .
@prefix skos: <http://www.w3.org/2004/02/skos/core#> .
@prefix sw: <http://www.w3.org/2003/06/sw-vocab-status/ns#> .
@prefix vann: <http://purl.org/vocab/vann/> .
@prefix xsd: <http://www.w3.org/2001/XMLSchema#> .

dpv-owl:City a rdfs:Class,
        owl:Class ;
    dct:contributor _:person-harshvardhan-j-pandit ;
    dct:created "2022-10-22"^^xsd:date ;
    dct:modified "2025-05-04"^^xsd:date ;
    rdfs:isDefinedBy dpv-owl: ;
    rdfs:subClassOf dpv-owl:Region ;
    sw:term_status "modified"@en ;
    skos:definition "A region consisting of urban population and commerce"@en ;
    skos:prefLabel "City"@en .

dpv-owl:CloudLocation a rdfs:Class,
        owl:Class,
        dpv-owl:Location ;
    dct:contributor _:person-harshvardhan-j-pandit ;
    dct:created "2022-06-15"^^xsd:date ;
    dct:modified "2020-10-05"^^xsd:date ;
    rdfs:isDefinedBy dpv-owl: ;
    rdfs:subClassOf dpv-owl:RemoteLocation ;
    sw:term_status "accepted"@en ;
    skos:definition "Location that is in the 'cloud' i.e. a logical location operated over the internet"@en ;
    skos:prefLabel "Cloud Location"@en .

dpv-owl:Country a rdfs:Class,
        owl:Class ;
    dct:contributor _:person-georg-p-krog,
        _:person-harshvardhan-j-pandit ;
    dct:created "2022-01-19"^^xsd:date ;
    dct:modified "2025-05-04"^^xsd:date ;
    rdfs:isDefinedBy dpv-owl: ;
    rdfs:subClassOf dpv-owl:Jurisdiction ;
    sw:term_status "modified"@en ;
    skos:definition "A political entity indicative of a sovereign or non-sovereign territorial state comprising of distinct geographical areas"@en ;
    skos:prefLabel "Country"@en ;
    skos:scopeNote "The definition of country is not intended for political interpretation. DPVCG welcomes alternate definitions based in existing sources with global scope, such as UN or ISO."@en .

dpv-owl:DecentralisedLocations a rdfs:Class,
        owl:Class,
        dpv-owl:LocationFixture ;
    dct:contributor _:person-harshvardhan-j-pandit ;
    dct:created "2022-06-15"^^xsd:date ;
    dct:modified "2020-10-05"^^xsd:date ;
    rdfs:isDefinedBy dpv-owl: ;
    rdfs:subClassOf dpv-owl:LocationFixture ;
    sw:term_status "accepted"@en ;
    skos:definition "Location that is spread across multiple separate areas with no distinction between their importance"@en ;
    skos:prefLabel "Decentralised Locations"@en .

dpv-owl:EconomicUnion a rdfs:Class,
        owl:Class ;
    dct:contributor _:person-harshvardhan-j-pandit ;
    dct:created "2022-01-19"^^xsd:date ;
    dct:modified "2025-05-04"^^xsd:date ;
    rdfs:isDefinedBy dpv-owl: ;
    rdfs:subClassOf dpv-owl:Jurisdiction ;
    sw:term_status "modified"@en ;
    skos:definition "A political union of two or more countries based on economic or trade agreements"@en ;
    skos:prefLabel "Economic Union"@en .

dpv-owl:FederatedLocations a rdfs:Class,
        owl:Class,
        dpv-owl:LocationFixture ;
    dct:contributor _:person-harshvardhan-j-pandit ;
    dct:created "2022-06-15"^^xsd:date ;
    dct:modified "2020-10-05"^^xsd:date ;
    rdfs:isDefinedBy dpv-owl: ;
    rdfs:subClassOf dpv-owl:LocationFixture ;
    sw:term_status "accepted"@en ;
    skos:definition "Location that is federated across multiple separate areas with designation of a primary or central location"@en ;
    skos:prefLabel "Federated Locations"@en .

dpv-owl:FixedLocation a rdfs:Class,
        owl:Class,
        dpv-owl:LocationFixture ;
    dct:contributor _:person-harshvardhan-j-pandit ;
    dct:created "2022-06-15"^^xsd:date ;
    dct:modified "2020-10-05"^^xsd:date ;
    rdfs:isDefinedBy dpv-owl: ;
    rdfs:subClassOf dpv-owl:LocationFixture ;
    sw:term_status "accepted"@en ;
    skos:definition "Location that is fixed i.e. known to occur at a specific place"@en ;
    skos:prefLabel "Fixed Location"@en .

dpv-owl:FixedMultipleLocations a rdfs:Class,
        owl:Class,
        dpv-owl:LocationFixture ;
    dct:contributor _:person-harshvardhan-j-pandit ;
    dct:created "2022-06-15"^^xsd:date ;
    dct:modified "2020-10-05"^^xsd:date ;
    rdfs:isDefinedBy dpv-owl: ;
    rdfs:subClassOf dpv-owl:FixedLocation ;
    sw:term_status "accepted"@en ;
    skos:definition "Location that is fixed with multiple places e.g. multiple cities"@en ;
    skos:prefLabel "Fixed Multiple Locations"@en .

dpv-owl:FixedSingularLocation a rdfs:Class,
        owl:Class,
        dpv-owl:LocationFixture ;
    dct:contributor _:person-harshvardhan-j-pandit ;
    dct:created "2022-06-15"^^xsd:date ;
    dct:modified "2020-10-05"^^xsd:date ;
    rdfs:isDefinedBy dpv-owl: ;
    rdfs:subClassOf dpv-owl:FixedLocation ;
    sw:term_status "accepted"@en ;
    skos:definition "Location that is fixed at a specific place e.g. a city"@en ;
    skos:prefLabel "Fixed Singular Location"@en .

dpv-owl:HybridPublicPrivateSpace a rdfs:Class,
        owl:Class,
        dpv-owl:Location ;
    dct:contributor _:person-arthit-suriyawongkul,
        _:person-georg-p-krog,
        _:person-harshvardhan-j-pandit,
        _:person-julian-flake ;
    dct:created "2025-04-07"^^xsd:date ;
    rdfs:isDefinedBy dpv-owl: ;
    rdfs:subClassOf dpv-owl:PrivateSpace,
        dpv-owl:PublicSpace ;
    sw:term_status "accepted"@en ;
    skos:definition "A space that is a hybrid space i.e it has both public and private components - such as by having part of it be a private space or which is operated privately"@en ;
    skos:prefLabel "Hybrid Public Private Space"@en .

dpv-owl:InverseJurisdiction a rdfs:Class,
        owl:Class,
        dpv-owl:Jurisdiction ;
    dct:contributor _:person-beatriz-esteves,
        _:person-georg-p-krog,
        _:person-harshvardhan-j-pandit,
        _:person-julian-flake ;
    dct:created "2025-05-04"^^xsd:date ;
    rdfs:isDefinedBy dpv-owl: ;
    rdfs:subClassOf dpv-owl:Jurisdiction ;
    sw:term_status "accepted"@en ;
    skos:definition "An inverse jurisdiction for a specific jurisdiction is the set of all other jurisdictions that are not part of the specific jurisdiction"@en ;
    skos:prefLabel "Inverse Jurisdiction"@en ;
    skos:scopeNote "Inverse Jurisdictions are helpful when asserting and checking rules that involve a concept representing jurisdictions outside of a given jurisdiction. An inverse jurisdiction of an inverse jurisdiction should give back the same original jurisdiction but this is undefined and strongly dissuaded as it could lead to recursive definitions in some use-cases"@en .

dpv-owl:Jurisdiction a rdfs:Class,
        owl:Class ;
    dct:contributor _:person-harshvardhan-j-pandit ;
    dct:created "2025-05-04"^^xsd:date ;
    rdfs:isDefinedBy dpv-owl: ;
    rdfs:subClassOf dpv-owl:Location ;
    sw:term_status "accepted"@en ;
    skos:definition "A jurisdiction represents the locations that define the extent of authority (or control) claimed, granted, or asserted by a legal entity (in particular a legal authority) to govern or enforce rules"@en ;
    skos:prefLabel "Jurisdiction"@en .

dpv-owl:Law a rdfs:Class,
        owl:Class ;
    dct:contributor _:person-harshvardhan-j-pandit ;
    dct:created "2022-01-19"^^xsd:date ;
    rdfs:isDefinedBy dpv-owl: ;
    rdfs:subClassOf rdfs:Class ;
    sw:term_status "accepted"@en ;
    skos:definition "A law is a set of rules created by government or authorities"@en ;
    skos:prefLabel "Law"@en .

dpv-owl:LocalLocation a rdfs:Class,
        owl:Class,
        dpv-owl:Location ;
    dct:contributor _:person-harshvardhan-j-pandit ;
    dct:created "2022-06-15"^^xsd:date ;
    dct:modified "2020-10-05"^^xsd:date ;
    rdfs:isDefinedBy dpv-owl: ;
    rdfs:subClassOf dpv-owl:LocationLocality ;
    sw:term_status "accepted"@en ;
    skos:definition "Location is local"@en ;
    skos:prefLabel "Local Location"@en .

dpv-owl:Location a rdfs:Class,
        owl:Class ;
    dct:contributor _:person-georg-p-krog,
        _:person-harshvardhan-j-pandit ;
    dct:created "2022-01-19"^^xsd:date ;
    vann:example dex-owl:E0060 ;
    rdfs:isDefinedBy dpv-owl: ;
    rdfs:subClassOf rdfs:Class ;
    sw:term_status "accepted"@en ;
    skos:definition "A location is a position, site, or area where something is located"@en ;
    skos:prefLabel "Location"@en ;
    skos:scopeNote "Location may be geographic, physical, or virtual."@en .

dpv-owl:LocationFixture a rdfs:Class,
        owl:Class ;
    dct:contributor _:person-harshvardhan-j-pandit ;
    dct:created "2022-06-15"^^xsd:date ;
    vann:example dex-owl:E0060 ;
    rdfs:isDefinedBy dpv-owl: ;
    rdfs:subClassOf rdfs:Class ;
    sw:term_status "accepted"@en ;
    skos:definition "The fixture of location refers to whether the location is fixed"@en ;
    skos:prefLabel "Location Fixture"@en .

dpv-owl:LocationLocality a rdfs:Class,
        owl:Class,
        dpv-owl:Location ;
    dct:contributor _:person-harshvardhan-j-pandit ;
    dct:created "2022-06-15"^^xsd:date ;
    dct:modified "2022-10-04"^^xsd:date ;
    vann:example dex-owl:E0060 ;
    rdfs:isDefinedBy dpv-owl: ;
    rdfs:subClassOf dpv-owl:Location ;
    sw:term_status "accepted"@en ;
    skos:definition "Locality refers to whether the specified location is local within some context, e.g. for the user"@en ;
    skos:prefLabel "Location Locality"@en .

dpv-owl:PersonalSpace a rdfs:Class,
        owl:Class,
        dpv-owl:Location ;
    dct:contributor _:person-georg-p-krog,
        _:person-harshvardhan-j-pandit,
        _:person-julian-flake ;
    dct:created "2025-04-07"^^xsd:date ;
    rdfs:isDefinedBy dpv-owl: ;
    rdfs:subClassOf dpv-owl:PrivateSpace ;
    sw:term_status "accepted"@en ;
    skos:definition "A private space associated with an individual in a personal capacity - such as their home or the space around their physical person e.g. my home or my room"@en ;
    skos:prefLabel "Personal Space"@en .

dpv-owl:PrivateCommunalSpace a rdfs:Class,
        owl:Class,
        dpv-owl:Location ;
    dct:contributor _:person-arthit-suriyawongkul,
        _:person-georg-p-krog,
        _:person-harshvardhan-j-pandit,
        _:person-julian-flake ;
    dct:created "2025-04-07"^^xsd:date ;
    rdfs:isDefinedBy dpv-owl: ;
    rdfs:subClassOf dpv-owl:PrivateSpace ;
    sw:term_status "accepted"@en ;
    skos:definition "A space that is accessible to a group or a community within a private space and where members of the public do not have access to it e.g. society amenities such as gyms and pools"@en ;
    skos:prefLabel "Private Communal Space"@en .

dpv-owl:PrivateLocation a rdfs:Class,
        owl:Class,
        dpv-owl:Location ;
    dct:contributor _:person-harshvardhan-j-pandit ;
    dct:created "2022-10-22"^^xsd:date ;
    dct:modified "2025-05-04"^^xsd:date ;
    rdfs:isDefinedBy dpv-owl: ;
    rdfs:subClassOf dpv-owl:LocalLocation ;
    sw:term_status "sunset"@en ;
    skos:definition "Location that is not or cannot be accessed by the public and is controlled as a private space"@en ;
    skos:prefLabel "Private Location (deprecated)"@en ;
    skos:scopeNote "This concept will be deprecated in a future DPV release, it is suggested to use the better defined and legally aligned dpv:PrivateSpace instead"@en .

dpv-owl:PrivateSpace a rdfs:Class,
        owl:Class,
        dpv-owl:Location ;
    dct:contributor _:person-arthit-suriyawongkul,
        _:person-georg-p-krog,
        _:person-harshvardhan-j-pandit,
        _:person-julian-flake ;
    dct:created "2025-04-07"^^xsd:date ;
    rdfs:isDefinedBy dpv-owl: ;
    rdfs:subClassOf dpv-owl:Location ;
    sw:term_status "accepted"@en ;
    skos:definition "A space that is owned or controlled by a private entity and where access to members of the public is restricted"@en ;
    skos:prefLabel "Private Space"@en .

dpv-owl:PrivatelyOperatedPublicSpace a rdfs:Class,
        owl:Class,
        dpv-owl:Location ;
    dct:contributor _:person-georg-p-krog,
        _:person-harshvardhan-j-pandit,
        _:person-julian-flake ;
    dct:created "2025-04-07"^^xsd:date ;
    rdfs:isDefinedBy dpv-owl: ;
    rdfs:subClassOf dpv-owl:HybridPublicPrivateSpace,
        dpv-owl:PubliclyAccessibleSpace ;
    sw:term_status "accepted"@en ;
    skos:definition "A space that is operated or managed by a private entity but which is accessible to the public e.g. a public bus station operated by a specific company"@en ;
    skos:prefLabel "Privately Operated Public Space"@en .

dpv-owl:PrivatelyOwnedPublicSpace a rdfs:Class,
        owl:Class,
        dpv-owl:Location ;
    dct:contributor _:person-georg-p-krog,
        _:person-harshvardhan-j-pandit,
        _:person-julian-flake ;
    dct:created "2025-04-07"^^xsd:date ;
    rdfs:isDefinedBy dpv-owl: ;
    rdfs:subClassOf dpv-owl:HybridPublicPrivateSpace,
        dpv-owl:PrivatelyOwnedSpace ;
    sw:term_status "accepted"@en ;
    skos:definition "A space that is privately owned but which is accessible and usable by the public - whether freely or through a process which is open to all members of the public e.g. hotel lobby, shopping mall atriums"@en ;
    skos:prefLabel "Privately Owned Public Space"@en .

dpv-owl:PrivatelyOwnedSpace a rdfs:Class,
        owl:Class,
        dpv-owl:Location ;
    dct:contributor _:person-georg-p-krog,
        _:person-harshvardhan-j-pandit,
        _:person-julian-flake ;
    dct:created "2025-04-07"^^xsd:date ;
    rdfs:isDefinedBy dpv-owl: ;
    rdfs:subClassOf dpv-owl:PrivateSpace ;
    sw:term_status "accepted"@en ;
    skos:definition "A place that is privately owned e.g. offices, malls"@en ;
    skos:prefLabel "Privately Owned Space"@en .

dpv-owl:PublicLocation a rdfs:Class,
        owl:Class,
        dpv-owl:Location ;
    dct:contributor _:person-georg-p-krog ;
    dct:created "2022-10-22"^^xsd:date ;
    dct:modified "2025-05-04"^^xsd:date ;
    rdfs:isDefinedBy dpv-owl: ;
    rdfs:subClassOf dpv-owl:LocalLocation ;
    sw:term_status "sunset"@en ;
    skos:definition "Location that is or can be accessed by the public"@en ;
    skos:prefLabel "Public Location (deprecated)"@en ;
    skos:scopeNote "This concept will be deprecated in a future DPV release, it is suggested to use the better defined and legally aligned dpv:PublicSpace instead"@en .

dpv-owl:PublicSpace a rdfs:Class,
        owl:Class,
        dpv-owl:Location ;
    dct:contributor _:person-arthit-suriyawongkul,
        _:person-georg-p-krog,
        _:person-harshvardhan-j-pandit,
        _:person-julian-flake ;
    dct:created "2025-04-07"^^xsd:date ;
    rdfs:isDefinedBy dpv-owl: ;
    rdfs:subClassOf dpv-owl:Location ;
    sw:term_status "accepted"@en ;
    skos:definition "Any space that is accessible to the public or is owned by the public"@en ;
    skos:prefLabel "Public Space"@en ;
    skos:scopeNote "Public space is distinct from places under (public) government ownership as such places can exclude public from accessing the place e.g. government military installations or reserved land"@en .

dpv-owl:PubliclyAccessibleSpace a rdfs:Class,
        owl:Class,
        dpv-owl:Location ;
    dct:contributor _:person-georg-p-krog,
        _:person-harshvardhan-j-pandit,
        _:person-julian-flake ;
    dct:created "2025-04-07"^^xsd:date ;
    rdfs:isDefinedBy dpv-owl: ;
    rdfs:subClassOf dpv-owl:PublicSpace ;
    sw:term_status "accepted"@en ;
    skos:definition "A space that is accessible to all members of the public e.g. parks, malls, train stations"@en ;
    skos:prefLabel "Publicly Accessible Space"@en .

dpv-owl:PubliclyOwnedSpace a rdfs:Class,
        owl:Class,
        dpv-owl:Location ;
    dct:contributor _:person-arthit-suriyawongkul,
        _:person-georg-p-krog,
        _:person-harshvardhan-j-pandit,
        _:person-julian-flake ;
    dct:created "2025-04-07"^^xsd:date ;
    rdfs:isDefinedBy dpv-owl: ;
    rdfs:subClassOf dpv-owl:PublicSpace ;
    sw:term_status "accepted"@en ;
    skos:definition "A space that is owned by the public e.g. national parks, forests"@en ;
    skos:prefLabel "Publicly Owned Space"@en .

dpv-owl:RandomLocation a rdfs:Class,
        owl:Class,
        dpv-owl:LocationFixture ;
    dct:contributor _:person-harshvardhan-j-pandit ;
    dct:created "2022-06-15"^^xsd:date ;
    dct:modified "2020-10-05"^^xsd:date ;
    rdfs:isDefinedBy dpv-owl: ;
    rdfs:subClassOf dpv-owl:LocationFixture ;
    sw:term_status "accepted"@en ;
    skos:definition "Location that is random or unknown"@en ;
    skos:prefLabel "Random Location"@en .

dpv-owl:Region a rdfs:Class,
        owl:Class ;
    dct:contributor _:person-harshvardhan-j-pandit ;
    dct:created "2022-01-19"^^xsd:date ;
    dct:modified "2025-05-04"^^xsd:date ;
    rdfs:isDefinedBy dpv-owl: ;
    rdfs:subClassOf dpv-owl:Country ;
    sw:term_status "modified"@en ;
    skos:definition "A region is an area or site that is considered a location"@en ;
    skos:prefLabel "Region"@en .

dpv-owl:RemoteLocation a rdfs:Class,
        owl:Class,
        dpv-owl:Location ;
    dct:contributor _:person-harshvardhan-j-pandit ;
    dct:created "2022-06-15"^^xsd:date ;
    dct:modified "2020-10-05"^^xsd:date ;
    rdfs:isDefinedBy dpv-owl: ;
    rdfs:subClassOf dpv-owl:LocationLocality ;
    sw:term_status "accepted"@en ;
    skos:definition "Location is remote i.e. not local"@en ;
    skos:prefLabel "Remote Location"@en .

dpv-owl:SemiPrivateSpace a rdfs:Class,
        owl:Class,
        dpv-owl:Location ;
    dct:contributor _:person-georg-p-krog,
        _:person-harshvardhan-j-pandit,
        _:person-julian-flake ;
    dct:created "2025-04-07"^^xsd:date ;
    rdfs:isDefinedBy dpv-owl: ;
    rdfs:subClassOf dpv-owl:PrivateSpace ;
    sw:term_status "accepted"@en ;
    skos:definition "A private space that acts as a shared space with other entities but which is still essentially private for the individuals e.g. a semi-private hospital room shared with another patient"@en ;
    skos:prefLabel "Semi Private Space"@en .

dpv-owl:SupraNationalUnion a rdfs:Class,
        owl:Class ;
    dct:contributor _:person-harshvardhan-j-pandit ;
    dct:created "2022-01-19"^^xsd:date ;
    dct:modified "2025-05-04"^^xsd:date ;
    rdfs:isDefinedBy dpv-owl: ;
    rdfs:subClassOf dpv-owl:Jurisdiction ;
    sw:term_status "modified"@en ;
    skos:definition "A political union of two or more countries with an establishment of common authority"@en ;
    skos:prefLabel "Supranational Union"@en .

dpv-owl:ThirdCountry a rdfs:Class,
        owl:Class ;
    dct:contributor _:person-harshvardhan-j-pandit ;
    dct:created "2022-02-09"^^xsd:date ;
    dct:modified "2025-05-04"^^xsd:date ;
    rdfs:isDefinedBy dpv-owl: ;
    rdfs:subClassOf dpv-owl:Country ;
    sw:term_status "modified"@en ;
    skos:definition "Represents a country outside applicable or compatible jurisdiction as outlined in law"@en ;
    skos:prefLabel "Third Country"@en .

dpv-owl:VariableLocation a rdfs:Class,
        owl:Class,
        dpv-owl:LocationFixture ;
    dct:contributor _:person-harshvardhan-j-pandit ;
    dct:created "2022-06-15"^^xsd:date ;
    dct:modified "2020-10-05"^^xsd:date ;
    rdfs:isDefinedBy dpv-owl: ;
    rdfs:subClassOf dpv-owl:LocationFixture ;
    sw:term_status "accepted"@en ;
    skos:definition "Location that is known but is variable e.g. somewhere within a given area"@en ;
    skos:prefLabel "Variable Location"@en .

dpv-owl:WithinDevice a rdfs:Class,
        owl:Class,
        dpv-owl:Location ;
    dct:contributor _:person-harshvardhan-j-pandit ;
    dct:created "2022-06-15"^^xsd:date ;
    dct:modified "2025-05-04"^^xsd:date ;
    rdfs:isDefinedBy dpv-owl: ;
    rdfs:subClassOf dpv-owl:LocalLocation ;
    sw:term_status "sunset"@en ;
    skos:definition "Location is local and entirely within a device, such as a smartphone"@en ;
    skos:prefLabel "Within Device (deprecated)"@en ;
    skos:scopeNote "This concept will be deprecated in a future DPV release, it is suggested to use the existing concepts representing device as tech:Device to have parity and consistency between the use of device as a technology and for data storage"@en .

dpv-owl:WithinPhysicalEnvironment a rdfs:Class,
        owl:Class,
        dpv-owl:Location ;
    dct:contributor _:person-harshvardhan-j-pandit ;
    dct:created "2020-10-06"^^xsd:date ;
    dct:modified "2025-05-04"^^xsd:date ;
    rdfs:isDefinedBy dpv-owl: ;
    rdfs:subClassOf dpv-owl:Location ;
    sw:term_status "sunset"@en ;
    skos:definition "Location is local and entirely within a physical environment, such as a room"@en ;
    skos:prefLabel "Within Physical Environment"@en ;
    skos:scopeNote "This concept will be deprecated in a future DPV release, it is suggested to use other concepts that also represent the nature of the location e.g. dpv:PrivateSpace or its accessibility dpv:PubliclyAccessibleSpace"@en .

dpv-owl:WithinVirtualEnvironment a rdfs:Class,
        owl:Class,
        dpv-owl:Location ;
    dct:contributor _:person-harshvardhan-j-pandit ;
    dct:created "2020-10-06"^^xsd:date ;
    dct:modified "2025-05-04"^^xsd:date ;
    rdfs:isDefinedBy dpv-owl: ;
    rdfs:subClassOf dpv-owl:Location ;
    sw:term_status "sunset"@en ;
    skos:definition "Location is local and entirely within a virtual environment, such as a software system"@en ;
    skos:prefLabel "Within Virtual Environment"@en ;
    skos:scopeNote "This concept will be deprecated in a future DPV release, it is suggested to use the existing concepts representing device as tech:Software and its taxonomy to have parity and consistency between the use of software as a technology and as a virtual environment for data storage and operations"@en .

dpv-owl:hasApplicableLaw a rdf:Property,
        owl:ObjectProperty ;
    dcam:rangeIncludes dpv-owl:Law ;
    dct:contributor _:person-harshvardhan-j-pandit ;
    dct:created "2022-01-19"^^xsd:date ;
    rdfs:isDefinedBy dpv-owl: ;
    sw:term_status "accepted"@en ;
    skos:definition "Indicates applicability of a Law"@en ;
    skos:prefLabel "has applicable law"@en ;
    schema:rangeIncludes dpv-owl:Law .

dpv-owl:hasInverseJurisdiction a rdf:Property,
        owl:ObjectProperty ;
    dcam:domainIncludes dpv-owl:Jurisdiction ;
    dcam:rangeIncludes dpv-owl:InverseJurisdiction ;
    dct:contributor _:person-georg-p-krog,
        _:person-harshvardhan-j-pandit,
        _:person-julian-flake ;
    dct:created "2025-05-04"^^xsd:date ;
    rdfs:isDefinedBy dpv-owl: ;
    rdfs:subPropertyOf dpv-owl:hasLocation ;
    sw:term_status "accepted"@en ;
    skos:definition "Indicates the inverse jurisdiction for a given jurisdiction"@en ;
    skos:prefLabel "has inverse jurisdiction"@en ;
    skos:scopeNote "Using this property gives the set of all other jurisdictions that are not part of the jurisdiction e.g. when used with a country, it refers to all other countries"@en ;
    schema:domainIncludes dpv-owl:Jurisdiction ;
    schema:rangeIncludes dpv-owl:InverseJurisdiction .

dpv-owl:hasJurisdiction a rdf:Property,
        owl:ObjectProperty ;
    dcam:rangeIncludes dpv-owl:Location ;
    dct:contributor _:person-harshvardhan-j-pandit ;
    dct:created "2022-01-19"^^xsd:date ;
    rdfs:isDefinedBy dpv-owl: ;
    sw:term_status "accepted"@en ;
    skos:definition "Indicates applicability of specified jurisdiction"@en ;
    skos:prefLabel "has jurisdiction"@en ;
    schema:rangeIncludes dpv-owl:Location .

dpv-owl:hasThirdCountry a rdf:Property,
        owl:ObjectProperty ;
    dcam:rangeIncludes dpv-owl:ThirdCountry ;
    dct:contributor _:person-georg-p-krog,
        _:person-harshvardhan-j-pandit ;
    dct:created "2022-02-09"^^xsd:date ;
    rdfs:isDefinedBy dpv-owl: ;
    rdfs:subPropertyOf dpv-owl:hasCountry ;
    sw:term_status "accepted"@en ;
    skos:definition "Indicates applicability or relevance of a 'third country'"@en ;
    skos:prefLabel "has third country"@en ;
    schema:rangeIncludes dpv-owl:ThirdCountry .

dpv-owl:isOutsideOfLocation a rdf:Property,
        owl:ObjectProperty ;
    dcam:rangeIncludes dpv-owl:Location ;
    dct:contributor _:person-georg-p-krog,
        _:person-harshvardhan-j-pandit,
        _:person-julian-flake ;
    dct:created "2025-05-04"^^xsd:date ;
    rdfs:isDefinedBy dpv-owl: ;
    rdfs:subPropertyOf dpv-owl:hasLocation ;
    sw:term_status "accepted"@en ;
    skos:definition "Indicates the interpretation where the location being referenced is outside of the indicated concept"@en ;
    skos:prefLabel "is outside of location"@en ;
    skos:scopeNote "This property is helpful for cases where a distinction needs to be made between inside/outside of a concept, and the area outside of that concept is to be referenced. For example, using Home with dpv:hasLocation means inside the Home, and using this property along with Home means outside of Home - such as the yard or porch"@en ;
    schema:rangeIncludes dpv-owl:Location .

dpv-owl:hasCountry a rdf:Property,
        owl:ObjectProperty ;
    dcam:rangeIncludes dpv-owl:Country ;
    dct:contributor _:person-georg-p-krog,
        _:person-harshvardhan-j-pandit ;
    dct:created "2022-01-19"^^xsd:date ;
    rdfs:isDefinedBy dpv-owl: ;
    rdfs:subPropertyOf dpv-owl:hasLocation ;
    sw:term_status "accepted"@en ;
    skos:definition "Indicates applicability of specified country"@en ;
    skos:prefLabel "has country"@en ;
    schema:rangeIncludes dpv-owl:Country .

dpv-owl:serialisation-html a profile:ResourceDescriptor ;
    dct:conformsTo <https://www.w3.org/TR/html/> ;
    dct:format <https://www.iana.org/assignments/media-types/text/html> ;
    dct:title "Data Privacy Vocabulary (DPV) - HTML serialisation" ;
    profile:hasArtifact <https://w3id.org/dpv/dpv-owl.html> ;
    profile:hasRole role:specification .

dpv-owl:serialisation-jsonld a profile:ResourceDescriptor ;
    dct:conformsTo <https://www.w3.org/TR/json-ld11/> ;
    dct:format <https://www.iana.org/assignments/media-types/application/ld+json> ;
    dct:title "Data Privacy Vocabulary (DPV) - JSON-LD serialisation" ;
    profile:hasArtifact <https://w3id.org/dpv/dpv/dpv-owl.jsonld> ;
    profile:hasRole role:vocabulary .

dpv-owl:serialisation-n3 a profile:ResourceDescriptor ;
    dct:conformsTo <https://www.w3.org/TeamSubmission/n3/> ;
    dct:format <https://www.iana.org/assignments/media-types/text/n3> ;
    dct:title "Data Privacy Vocabulary (DPV) - N3 serialisation" ;
    profile:hasArtifact <https://w3id.org/dpv/dpv/dpv-owl.n3> ;
    profile:hasRole role:vocabulary .

dpv-owl:serialisation-rdf a profile:ResourceDescriptor ;
    dct:conformsTo rdf: ;
    dct:format <https://www.iana.org/assignments/media-types/application/rdf+xml> ;
    dct:title "Data Privacy Vocabulary (DPV) - RDF/XML serialisation" ;
    profile:hasArtifact <https://w3id.org/dpv/dpv/dpv-owl.rdf> ;
    profile:hasRole role:vocabulary .

dpv-owl:serialisation-ttl a profile:ResourceDescriptor ;
    dct:conformsTo <https://www.w3.org/TR/turtle/> ;
    dct:format <https://www.iana.org/assignments/media-types/text/turtle> ;
    dct:title "Data Privacy Vocabulary (DPV) - Turtle serialisation" ;
    profile:hasArtifact <https://w3id.org/dpv/dpv/dpv-owl.ttl> ;
    profile:hasRole role:vocabulary .

<https://w3id.org/dpv/examples> a profile:ResourceDescriptor ;
    dct:conformsTo <https://www.w3.org/TR/html/> ;
    dct:format <https://www.iana.org/assignments/media-types/text/html> ;
    dct:title "Examples" ;
    profile:hasArtifact <https://w3id.org/dpv/examples> ;
    profile:hasRole role:guidance .

<https://w3id.org/dpv/guides> a profile:ResourceDescriptor ;
    dct:conformsTo <https://www.w3.org/TR/html/> ;
    dct:format <https://www.iana.org/assignments/media-types/text/html> ;
    dct:title "Guides for Data Privacy Vocabulary" ;
    profile:hasArtifact <https://w3id.org/dpv/guides> ;
    profile:hasRole role:guidance .

<https://w3id.org/dpv/primer> a profile:ResourceDescriptor ;
    dct:conformsTo <https://www.w3.org/TR/html/> ;
    dct:format <https://www.iana.org/assignments/media-types/text/html> ;
    dct:title "Primer for Data Privacy Vocabulary" ;
    profile:hasArtifact <https://w3id.org/dpv/primer> ;
    profile:hasRole role:guidance .

dpv-owl:hasLocation a rdf:Property,
        owl:ObjectProperty ;
    dcam:rangeIncludes dpv-owl:Location ;
    dct:contributor _:person-axel-polleres,
        _:person-harshvardhan-j-pandit,
        _:person-mark-lizar,
        _:person-rob-brennan ;
    dct:created "2019-04-05"^^xsd:date ;
    dct:source [ a schema:WebPage ;
            schema:name "SPECIAL Project" ;
            schema:url "https://specialprivacy.ercim.eu/" ] ;
    vann:example dex-owl:E0060 ;
    rdfs:isDefinedBy dpv-owl: ;
    sw:term_status "accepted"@en ;
    skos:definition "Indicates information about location"@en ;
    skos:prefLabel "has location"@en ;
    schema:rangeIncludes dpv-owl:Location .

dpv-owl: a owl:Ontology,
        profile:Profile ;
    dct:bibliographicCitation "Harshvardhan J. Pandit, Beatriz Esteves, Georg P. Krog, Paul Ryan, Delaram Golpayegani, Julian Flake (2025) Data Privacy Vocabulary (DPV) – Version 2.0. In: Demartini, G., et al. The Semantic Web – ISWC 2024. ISWC 2024. Lecture Notes in Computer Science, vol 15233. Springer, Cham. https://doi.org/10.1007/978-3-031-77847-6_10" ;
    dct:conformsTo <http://www.w3.org/2002/07/owl>,
        "http://www.w3.org/2000/01/rdf-schema",
        "http://www.w3.org/2004/02/skos/core" ;
    dct:contributor _:person-arthit-suriyawongkul,
        _:person-axel-polleres,
        _:person-beatriz-esteves,
        _:person-georg-p-krog,
        _:person-harshvardhan-j-pandit,
        _:person-julian-flake,
        _:person-mark-lizar,
        _:person-rob-brennan ;
    dct:created "2022-08-18"@en ;
    dct:creator _:person-beatriz-esteves,
        [ a dct:Agent,
                foaf:Person ;
            scoro:hasORCID "0000-0002-1208-186X" ;
            org:memberOf _:org-adapt-centre-trinity-college-dublin ;
            foaf:name "Delaram Golpayegani" ],
        _:person-georg-p-krog,
        _:person-harshvardhan-j-pandit,
        _:person-julian-flake,
        [ a dct:Agent,
                foaf:Person ;
            scoro:hasORCID "0000-0003-0770-2737" ;
            org:memberOf [ a foaf:Organization ;
                    foaf:name "Uniphar PLC" ] ;
            foaf:name "Paul Ryan" ] ;
    dct:description "The Data Privacy Vocabulary (DPV) provides terms (classes and properties) to represent information about processing of personal data, for example - purposes, processing operations, personal data, technical and organisational measures."@en ;
    dct:hasVersion dpv-owl: ;
    dct:identifier "https://w3id.org/dpv" ;
    dct:issued "2022-08-18"@en ;
    dct:license <https://www.w3.org/copyright/document-license-2023/> ;
    dct:modified "2025-08-01"@en ;
    dct:publisher <https://www.w3.org/> ;
    dct:source <https://www.w3.org/groups/cg/dpvcg/> ;
    dct:title "Data Privacy Vocabulary (DPV)"@en ;
    bibo:doi "10.5281/zenodo.12505841" ;
    bibo:status "http://purl.org/ontology/bibo/status/published" ;
    vann:preferredNamespacePrefix "dpv" ;
    vann:preferredNamespaceUri "https://w3id.org/dpv#" ;
    rdfs:Label "DPV"@en ;
    owl:versionIRI <https://w3id.org/dpv/2.2/owl#> ;
    owl:versionInfo "2.2" ;
    profile:hasResource <https://w3id.org/dpv/examples>,
        <https://w3id.org/dpv/guides>,
        dpv-owl:serialisation-html,
        dpv-owl:serialisation-jsonld,
        dpv-owl:serialisation-n3,
        dpv-owl:serialisation-rdf,
        dpv-owl:serialisation-ttl,
        <https://w3id.org/dpv/primer> ;
    profile:isProfileOf <http://www.w3.org/2002/07/owl>,
        dpv-owl: ;
    foaf:logo <https://w3id.org/dpv/media/logo.png> ;
    schema:version "2.2" .

_:org-ai-accountability-lab-aial-trinity-college-dublin a foaf:Organization ;
    foaf:name "AI Accountability Lab (AIAL), Trinity College Dublin" .

_:org-idlab-imec-ghent-university a foaf:Organization ;
    foaf:name "IDLab, IMEC, Ghent University" .

_:org-openconsent-kantara-initiative a foaf:Organization ;
    foaf:name "OpenConsent/Kantara Initiative" .

_:org-signatu-as a foaf:Organization ;
    foaf:name "Signatu AS" .

_:org-university-college-dublin a foaf:Organization ;
    foaf:name "University College Dublin" .

_:org-university-of-koblenz a foaf:Organization ;
    foaf:name "University of Koblenz" .

_:org-vienna-university-of-economics-and-business a foaf:Organization ;
    foaf:name "Vienna University of Economics and Business" .

_:org-adapt-centre-trinity-college-dublin a foaf:Organization ;
    foaf:name "ADAPT Centre, Trinity College Dublin" .

_:person-axel-polleres a dct:Agent,
        foaf:Person ;
    org:memberOf _:org-vienna-university-of-economics-and-business ;
    foaf:name "Axel Polleres" .

_:person-mark-lizar a dct:Agent,
        foaf:Person ;
    org:memberOf _:org-openconsent-kantara-initiative ;
    foaf:name "Mark Lizar" .

_:person-rob-brennan a dct:Agent,
        foaf:Person ;
    scoro:hasORCID "0000-0001-8236-362X" ;
    org:memberOf _:org-university-college-dublin ;
    foaf:name "Rob Brennan" .

_:person-beatriz-esteves a dct:Agent,
        foaf:Person ;
    scoro:hasORCID "0000-0003-0259-7560" ;
    org:memberOf _:org-idlab-imec-ghent-university ;
    foaf:name "Beatriz Esteves" .

_:person-arthit-suriyawongkul a dct:Agent,
        foaf:Person ;
    scoro:hasORCID "0000-0002-9698-1899" ;
    org:memberOf _:org-adapt-centre-trinity-college-dublin ;
    foaf:name "Arthit Suriyawongkul" .

_:person-julian-flake a dct:Agent,
        foaf:Person ;
    scoro:hasORCID "0009-0006-4623-1463" ;
    org:memberOf _:org-university-of-koblenz ;
    foaf:name "Julian Flake" .

_:person-georg-p-krog a dct:Agent,
        foaf:Person ;
    org:memberOf _:org-signatu-as ;
    foaf:homepage "https://www.linkedin.com/in/georg-philip-krog-a2a278104/" ;
    foaf:name "Georg P. Krog" .

_:person-harshvardhan-j-pandit a dct:Agent,
        foaf:Person ;
    scoro:hasORCID "0000-0002-5068-3714" ;
    org:memberOf _:org-ai-accountability-lab-aial-trinity-college-dublin ;
    foaf:homepage "https://harshp.com/" ;
    foaf:name "Harshvardhan J. Pandit" .

