<?xml version="1.0" encoding="utf-8"?>
<rdf:RDF
   xmlns:bibo="http://purl.org/ontology/bibo/"
   xmlns:dct="http://purl.org/dc/terms/"
   xmlns:foaf="http://xmlns.com/foaf/0.1/"
   xmlns:org="http://www.w3.org/ns/org#"
   xmlns:owl="http://www.w3.org/2002/07/owl#"
   xmlns:profile="http://www.w3.org/ns/dx/prof/"
   xmlns:rdf="http://www.w3.org/1999/02/22-rdf-syntax-ns#"
   xmlns:rdfs="http://www.w3.org/2000/01/rdf-schema#"
   xmlns:schema="https://schema.org/"
   xmlns:scoro="http://purl.org/spar/scoro/"
   xmlns:skos="http://www.w3.org/2004/02/skos/core#"
   xmlns:sw="http://www.w3.org/2003/06/sw-vocab-status/ns#"
   xmlns:vann="http://purl.org/vocab/vann/"
>
  <rdf:Description rdf:about="https://w3id.org/dpv/sector/education/owl#StudentAssignmentAssessment">
    <rdf:type rdf:resource="https://w3id.org/dpv/owl#Purpose"/>
    <rdf:type rdf:resource="http://www.w3.org/2000/01/rdf-schema#Class"/>
    <rdf:type rdf:resource="http://www.w3.org/2002/07/owl#Class"/>
    <skos:definition xml:lang="en">Purposes associated with assessment of student performance in the context of an educational assignment or task or other processes where the student is required to perform an activity which is then assessed</skos:definition>
    <sw:term_status xml:lang="en">accepted</sw:term_status>
    <skos:prefLabel xml:lang="en">Student Assignment Assessment</skos:prefLabel>
    <rdfs:isDefinedBy rdf:resource="https://w3id.org/dpv/sector/education/owl#"/>
    <dct:created rdf:datatype="http://www.w3.org/2001/XMLSchema#date">2024-12-01</dct:created>
    <rdfs:subClassOf rdf:resource="https://w3id.org/dpv/sector/education/owl#StudentLearningOutcomeAssessment"/>
  </rdf:Description>
  <rdf:Description rdf:about="https://w3id.org/dpv/sector/education/owl#StudentPerformanceManagement">
    <dct:created rdf:datatype="http://www.w3.org/2001/XMLSchema#date">2024-12-01</dct:created>
    <rdfs:isDefinedBy rdf:resource="https://w3id.org/dpv/sector/education/owl#"/>
    <rdf:type rdf:resource="http://www.w3.org/2000/01/rdf-schema#Class"/>
    <rdf:type rdf:resource="https://w3id.org/dpv/owl#Purpose"/>
    <rdf:type rdf:resource="http://www.w3.org/2002/07/owl#Class"/>
    <skos:prefLabel xml:lang="en">Student Performance Management</skos:prefLabel>
    <sw:term_status xml:lang="en">accepted</sw:term_status>
    <skos:definition xml:lang="en">Purposes associated with management of student performance in educational contexts</skos:definition>
    <rdfs:subClassOf rdf:resource="https://w3id.org/dpv/sector/education/owl#StudentManagement"/>
  </rdf:Description>
  <rdf:Description rdf:about="https://w3id.org/dpv/sector/education/owl#StudentOnlineProctoring">
    <rdfs:isDefinedBy rdf:resource="https://w3id.org/dpv/sector/education/owl#"/>
    <rdf:type rdf:resource="http://www.w3.org/2000/01/rdf-schema#Class"/>
    <rdf:type rdf:resource="https://w3id.org/dpv/owl#Purpose"/>
    <rdf:type rdf:resource="http://www.w3.org/2002/07/owl#Class"/>
    <skos:prefLabel xml:lang="en">Student Online Proctoring</skos:prefLabel>
    <dct:created rdf:datatype="http://www.w3.org/2001/XMLSchema#date">2024-12-01</dct:created>
    <sw:term_status xml:lang="en">accepted</sw:term_status>
    <skos:definition xml:lang="en">Purposes associated with online or virtual or remote proctoring i.e. monitoring of students present virtually over an online platform or within their remote physical location during an assessment with the aim of ensuring they do not cheat</skos:definition>
    <rdfs:subClassOf rdf:resource="https://w3id.org/dpv/sector/education/owl#StudentProctoring"/>
  </rdf:Description>
  <rdf:Description rdf:about="https://w3id.org/dpv/sector/education/owl#">
    <owl:versionIRI rdf:resource="https://w3id.org/dpv/2.2/sector/education/owl#"/>
    <vann:preferredNamespacePrefix>sector-education</vann:preferredNamespacePrefix>
    <profile:hasResource rdf:resource="https://w3id.org/dpv/guides"/>
    <profile:hasResource rdf:resource="https://w3id.org/dpv/sector/education/owl#serialisation-ttl"/>
    <profile:hasResource rdf:resource="https://w3id.org/dpv/sector/education/owl#serialisation-html"/>
    <profile:hasResource rdf:resource="https://w3id.org/dpv/sector/education/owl#serialisation-jsonld"/>
    <profile:hasResource rdf:resource="https://w3id.org/dpv/sector/education/owl#serialisation-n3"/>
    <profile:hasResource rdf:resource="https://w3id.org/dpv/sector/education/owl#serialisation-rdf"/>
    <profile:hasResource rdf:resource="https://w3id.org/dpv/primer"/>
    <profile:hasResource rdf:resource="https://w3id.org/dpv/examples"/>
    <dct:description xml:lang="en">Extension to the Data Privacy Vocabulary (DPV) providing concepts for the education sector</dct:description>
    <dct:created xml:lang="en">2024-12-01</dct:created>
    <dct:conformsTo>http://www.w3.org/2000/01/rdf-schema</dct:conformsTo>
    <dct:conformsTo>http://www.w3.org/2004/02/skos/core</dct:conformsTo>
    <dct:conformsTo rdf:resource="http://www.w3.org/2002/07/owl"/>
    <dct:bibliographicCitation>Harshvardhan J. Pandit, Beatriz Esteves, Georg P. Krog, Paul Ryan, Delaram Golpayegani, Julian Flake (2025) Data Privacy Vocabulary (DPV) – Version 2.0. In: Demartini, G., et al. The Semantic Web – ISWC 2024. ISWC 2024. Lecture Notes in Computer Science, vol 15233. Springer, Cham. https://doi.org/10.1007/978-3-031-77847-6_10</dct:bibliographicCitation>
    <profile:isProfileOf rdf:resource="https://w3id.org/dpv/owl"/>
    <profile:isProfileOf rdf:resource="http://www.w3.org/2002/07/owl"/>
    <profile:isProfileOf rdf:resource="https://w3id.org/dpv/sector/education/owl#"/>
    <dct:creator rdf:nodeID="person-harshvardhan-j-pandit"/>
    <dct:issued xml:lang="en">2024-12-01</dct:issued>
    <rdfs:Label xml:lang="en">SECTOR-EDUCATION</rdfs:Label>
    <dct:license rdf:resource="https://www.w3.org/copyright/document-license-2023/"/>
    <foaf:logo rdf:resource="https://w3id.org/dpv/media/logo.png"/>
    <dct:contributor rdf:nodeID="person-harshvardhan-j-pandit"/>
    <dct:contributor rdf:nodeID="person-arthit-suriyawongkul"/>
    <dct:identifier>https://w3id.org/dpv/sector/education</dct:identifier>
    <rdf:type rdf:resource="http://www.w3.org/2002/07/owl#Ontology"/>
    <rdf:type rdf:resource="http://www.w3.org/ns/dx/prof/Profile"/>
    <dct:title xml:lang="en">Education Sector Concepts</dct:title>
    <dct:source rdf:resource="https://www.w3.org/groups/cg/dpvcg/"/>
    <dct:hasVersion rdf:resource="https://w3id.org/dpv/sector/education/owl#"/>
    <schema:version>2.2</schema:version>
    <bibo:doi>10.5281/zenodo.12505841</bibo:doi>
    <dct:publisher rdf:resource="https://www.w3.org/"/>
    <vann:preferredNamespaceUri>https://w3id.org/dpv/sector/education#</vann:preferredNamespaceUri>
    <owl:versionInfo>2.2</owl:versionInfo>
    <dct:modified xml:lang="en">2025-08-01</dct:modified>
    <bibo:status>http://purl.org/ontology/bibo/status/draft</bibo:status>
  </rdf:Description>
  <rdf:Description rdf:about="https://w3id.org/dpv/sector/education/owl#StudentMisconductInvestigation">
    <dct:created rdf:datatype="http://www.w3.org/2001/XMLSchema#date">2024-12-01</dct:created>
    <rdfs:isDefinedBy rdf:resource="https://w3id.org/dpv/sector/education/owl#"/>
    <rdf:type rdf:resource="http://www.w3.org/2000/01/rdf-schema#Class"/>
    <rdf:type rdf:resource="https://w3id.org/dpv/owl#Purpose"/>
    <rdf:type rdf:resource="http://www.w3.org/2002/07/owl#Class"/>
    <sw:term_status xml:lang="en">accepted</sw:term_status>
    <skos:prefLabel xml:lang="en">Student Misconduct Investigation</skos:prefLabel>
    <skos:definition xml:lang="en">Purposes associated with investigating and assessing potential misconduct by or on a student or a group of students in an educational context</skos:definition>
    <rdfs:subClassOf rdf:resource="https://w3id.org/dpv/sector/education/owl#StudentIntegrityManagement"/>
  </rdf:Description>
  <rdf:Description rdf:about="https://w3id.org/dpv/sector/education/owl#StudentInstituteAllocation">
    <rdf:type rdf:resource="https://w3id.org/dpv/owl#Purpose"/>
    <rdf:type rdf:resource="http://www.w3.org/2000/01/rdf-schema#Class"/>
    <rdf:type rdf:resource="http://www.w3.org/2002/07/owl#Class"/>
    <sw:term_status xml:lang="en">accepted</sw:term_status>
    <skos:prefLabel xml:lang="en">Student Institute Allocation</skos:prefLabel>
    <skos:definition xml:lang="en">Purposes associated with allocation of students to specific educational or other institutes in the context of educational services</skos:definition>
    <dct:created rdf:datatype="http://www.w3.org/2001/XMLSchema#date">2024-12-01</dct:created>
    <rdfs:isDefinedBy rdf:resource="https://w3id.org/dpv/sector/education/owl#"/>
    <rdfs:subClassOf rdf:resource="https://w3id.org/dpv/sector/education/owl#StudentAllocation"/>
  </rdf:Description>
  <rdf:Description rdf:about="https://w3id.org/dpv/sector/education/owl#StudentManagement">
    <skos:prefLabel xml:lang="en">Student Management</skos:prefLabel>
    <rdfs:isDefinedBy rdf:resource="https://w3id.org/dpv/sector/education/owl#"/>
    <skos:definition xml:lang="en">Purposes associated with management of current and prospective students</skos:definition>
    <dct:created rdf:datatype="http://www.w3.org/2001/XMLSchema#date">2024-12-01</dct:created>
    <rdf:type rdf:resource="http://www.w3.org/2000/01/rdf-schema#Class"/>
    <rdf:type rdf:resource="https://w3id.org/dpv/owl#Purpose"/>
    <rdf:type rdf:resource="http://www.w3.org/2002/07/owl#Class"/>
    <sw:term_status xml:lang="en">accepted</sw:term_status>
    <rdfs:subClassOf rdf:resource="https://w3id.org/dpv/sector/education/owl#EducationManagement"/>
  </rdf:Description>
  <rdf:Description rdf:nodeID="person-arthit-suriyawongkul">
    <foaf:name>Arthit Suriyawongkul</foaf:name>
    <scoro:hasORCID>0000-0002-9698-1899</scoro:hasORCID>
    <org:memberOf rdf:nodeID="org-adapt-centre-trinity-college-dublin"/>
    <rdf:type rdf:resource="http://purl.org/dc/terms/Agent"/>
    <rdf:type rdf:resource="http://xmlns.com/foaf/0.1/Person"/>
  </rdf:Description>
  <rdf:Description rdf:about="https://w3id.org/dpv/sector/education/owl#StudentProgramAllocation">
    <rdf:type rdf:resource="https://w3id.org/dpv/owl#Purpose"/>
    <rdf:type rdf:resource="http://www.w3.org/2000/01/rdf-schema#Class"/>
    <rdf:type rdf:resource="http://www.w3.org/2002/07/owl#Class"/>
    <sw:term_status xml:lang="en">accepted</sw:term_status>
    <rdfs:isDefinedBy rdf:resource="https://w3id.org/dpv/sector/education/owl#"/>
    <skos:definition xml:lang="en">Purposes associated with allocation of students to specific programs in the context of educational services</skos:definition>
    <skos:prefLabel xml:lang="en">Student Program Allocation</skos:prefLabel>
    <dct:created rdf:datatype="http://www.w3.org/2001/XMLSchema#date">2024-12-01</dct:created>
    <rdfs:subClassOf rdf:resource="https://w3id.org/dpv/sector/education/owl#StudentAllocation"/>
  </rdf:Description>
  <rdf:Description rdf:about="https://w3id.org/dpv/sector/education/owl#StudentExamAssessment">
    <rdf:type rdf:resource="http://www.w3.org/2000/01/rdf-schema#Class"/>
    <rdf:type rdf:resource="https://w3id.org/dpv/owl#Purpose"/>
    <rdf:type rdf:resource="http://www.w3.org/2002/07/owl#Class"/>
    <skos:definition xml:lang="en">Purposes associated with assessment of student performance in the context of an educational exam</skos:definition>
    <sw:term_status xml:lang="en">accepted</sw:term_status>
    <skos:prefLabel xml:lang="en">Student Exam Assessment</skos:prefLabel>
    <rdfs:isDefinedBy rdf:resource="https://w3id.org/dpv/sector/education/owl#"/>
    <dct:created rdf:datatype="http://www.w3.org/2001/XMLSchema#date">2024-12-01</dct:created>
    <rdfs:subClassOf rdf:resource="https://w3id.org/dpv/sector/education/owl#StudentLearningOutcomeAssessment"/>
  </rdf:Description>
  <rdf:Description rdf:about="https://w3id.org/dpv/sector/education/owl#AccessManagement">
    <rdfs:isDefinedBy rdf:resource="https://w3id.org/dpv/sector/education/owl#"/>
    <dct:created rdf:datatype="http://www.w3.org/2001/XMLSchema#date">2024-12-01</dct:created>
    <rdf:type rdf:resource="http://www.w3.org/2000/01/rdf-schema#Class"/>
    <rdf:type rdf:resource="https://w3id.org/dpv/owl#Purpose"/>
    <rdf:type rdf:resource="http://www.w3.org/2002/07/owl#Class"/>
    <sw:term_status xml:lang="en">accepted</sw:term_status>
    <skos:prefLabel xml:lang="en">AccessManagement</skos:prefLabel>
    <skos:definition xml:lang="en">Purposes associated with determination and management of access to educational programs, resources, and services</skos:definition>
    <rdfs:subClassOf rdf:resource="https://w3id.org/dpv/sector/education/owl#EducationManagement"/>
  </rdf:Description>
  <rdf:Description rdf:about="https://w3id.org/dpv/sector/education/owl#StudentPersonalisedContentDelivery">
    <rdfs:isDefinedBy rdf:resource="https://w3id.org/dpv/sector/education/owl#"/>
    <rdf:type rdf:resource="http://www.w3.org/2000/01/rdf-schema#Class"/>
    <rdf:type rdf:resource="https://w3id.org/dpv/owl#Purpose"/>
    <rdf:type rdf:resource="http://www.w3.org/2002/07/owl#Class"/>
    <skos:prefLabel xml:lang="en">Student Personalised Content Delivery</skos:prefLabel>
    <dct:created rdf:datatype="http://www.w3.org/2001/XMLSchema#date">2024-12-01</dct:created>
    <sw:term_status xml:lang="en">accepted</sw:term_status>
    <skos:definition xml:lang="en">Purposes associated with personalisation of the content delivery for an individual student or a group of students in the context of educational services</skos:definition>
    <rdfs:subClassOf rdf:resource="https://w3id.org/dpv/sector/education/owl#ServiceProvision"/>
    <rdfs:subClassOf rdf:resource="https://w3id.org/dpv/owl#Personalisation"/>
  </rdf:Description>
  <rdf:Description rdf:about="https://w3id.org/dpv/sector/education/owl#ResearchIntegrityManagement">
    <rdf:type rdf:resource="http://www.w3.org/2000/01/rdf-schema#Class"/>
    <rdf:type rdf:resource="https://w3id.org/dpv/owl#Purpose"/>
    <rdf:type rdf:resource="http://www.w3.org/2002/07/owl#Class"/>
    <sw:term_status xml:lang="en">accepted</sw:term_status>
    <dct:created rdf:datatype="http://www.w3.org/2001/XMLSchema#date">2024-12-01</dct:created>
    <rdfs:isDefinedBy rdf:resource="https://w3id.org/dpv/sector/education/owl#"/>
    <skos:prefLabel xml:lang="en">Research Integrity Management</skos:prefLabel>
    <skos:definition xml:lang="en">Purposes associated with assessment, determination, and management of integrity for or of research activities and outputs in an educational or academic research context</skos:definition>
    <rdfs:subClassOf rdf:resource="https://w3id.org/dpv/sector/education/owl#ResearchManagement"/>
    <rdfs:subClassOf rdf:resource="https://w3id.org/dpv/owl#OrganisationRiskManagement"/>
  </rdf:Description>
  <rdf:Description rdf:about="https://w3id.org/dpv/sector/education/owl#StudentAttendanceManagement">
    <rdf:type rdf:resource="http://www.w3.org/2000/01/rdf-schema#Class"/>
    <rdf:type rdf:resource="https://w3id.org/dpv/owl#Purpose"/>
    <rdf:type rdf:resource="http://www.w3.org/2002/07/owl#Class"/>
    <sw:term_status xml:lang="en">accepted</sw:term_status>
    <rdfs:isDefinedBy rdf:resource="https://w3id.org/dpv/sector/education/owl#"/>
    <dct:created rdf:datatype="http://www.w3.org/2001/XMLSchema#date">2024-12-01</dct:created>
    <skos:definition xml:lang="en">Purposes associated with undertaking and management of attendance of students within an educational context</skos:definition>
    <skos:prefLabel xml:lang="en">Student Attendance Management</skos:prefLabel>
    <rdfs:subClassOf rdf:resource="https://w3id.org/dpv/sector/education/owl#ServiceProvision"/>
  </rdf:Description>
  <rdf:Description rdf:about="https://w3id.org/dpv/sector/education/owl#StudentEnrolmentManagement">
    <dct:created rdf:datatype="http://www.w3.org/2001/XMLSchema#date">2024-12-01</dct:created>
    <rdfs:isDefinedBy rdf:resource="https://w3id.org/dpv/sector/education/owl#"/>
    <rdf:type rdf:resource="http://www.w3.org/2000/01/rdf-schema#Class"/>
    <rdf:type rdf:resource="https://w3id.org/dpv/owl#Purpose"/>
    <rdf:type rdf:resource="http://www.w3.org/2002/07/owl#Class"/>
    <dct:contributor rdf:nodeID="person-harshvardhan-j-pandit"/>
    <dct:contributor rdf:nodeID="person-arthit-suriyawongkul"/>
    <dct:modified rdf:datatype="http://www.w3.org/2001/XMLSchema#date">2025-08-06</dct:modified>
    <skos:definition xml:lang="en">Purposes associated with enrolment of students and prospective students in educational courses, programs, and institutes</skos:definition>
    <skos:prefLabel xml:lang="en">Student Enrolment Management</skos:prefLabel>
    <sw:term_status xml:lang="en">modified</sw:term_status>
    <rdfs:subClassOf rdf:resource="https://w3id.org/dpv/sector/education/owl#StudentAdmissionManagement"/>
  </rdf:Description>
  <rdf:Description rdf:about="https://w3id.org/dpv/sector/education/owl#StudentIdentityVerification">
    <rdfs:isDefinedBy rdf:resource="https://w3id.org/dpv/sector/education/owl#"/>
    <rdf:type rdf:resource="http://www.w3.org/2000/01/rdf-schema#Class"/>
    <rdf:type rdf:resource="https://w3id.org/dpv/owl#Purpose"/>
    <rdf:type rdf:resource="http://www.w3.org/2002/07/owl#Class"/>
    <skos:prefLabel xml:lang="en">Student Identity Verification</skos:prefLabel>
    <sw:term_status xml:lang="en">accepted</sw:term_status>
    <skos:definition xml:lang="en">Purposes associated with verification of a student's identity in an educational context, such as for exams or access to resources</skos:definition>
    <dct:created rdf:datatype="http://www.w3.org/2001/XMLSchema#date">2024-12-01</dct:created>
    <rdfs:subClassOf rdf:resource="https://w3id.org/dpv/sector/education/owl#StudentIntegrityManagement"/>
    <rdfs:subClassOf rdf:resource="https://w3id.org/dpv/owl#IdentityVerification"/>
  </rdf:Description>
  <rdf:Description rdf:about="https://w3id.org/dpv/sector/education/owl#StudentPerformanceMonitoring">
    <rdf:type rdf:resource="http://www.w3.org/2000/01/rdf-schema#Class"/>
    <rdf:type rdf:resource="https://w3id.org/dpv/owl#Purpose"/>
    <rdf:type rdf:resource="http://www.w3.org/2002/07/owl#Class"/>
    <sw:term_status xml:lang="en">accepted</sw:term_status>
    <skos:prefLabel xml:lang="en">Student Performance Monitoring</skos:prefLabel>
    <dct:created rdf:datatype="http://www.w3.org/2001/XMLSchema#date">2024-12-01</dct:created>
    <rdfs:isDefinedBy rdf:resource="https://w3id.org/dpv/sector/education/owl#"/>
    <skos:definition xml:lang="en">Purposes associated with monitoring of student performance in educational contexts</skos:definition>
    <rdfs:subClassOf rdf:resource="https://w3id.org/dpv/sector/education/owl#StudentManagement"/>
  </rdf:Description>
  <rdf:Description rdf:about="https://w3id.org/dpv/sector/education/owl#ResearchManagement">
    <sw:term_status xml:lang="en">accepted</sw:term_status>
    <rdfs:isDefinedBy rdf:resource="https://w3id.org/dpv/sector/education/owl#"/>
    <skos:definition xml:lang="en">Purposes associated with research activities and management of research activities within an educational context e.g. within university departments or research groups</skos:definition>
    <skos:prefLabel xml:lang="en">Research Management</skos:prefLabel>
    <dct:created rdf:datatype="http://www.w3.org/2001/XMLSchema#date">2024-12-01</dct:created>
    <rdf:type rdf:resource="http://www.w3.org/2000/01/rdf-schema#Class"/>
    <rdf:type rdf:resource="https://w3id.org/dpv/owl#Purpose"/>
    <rdf:type rdf:resource="http://www.w3.org/2002/07/owl#Class"/>
    <rdfs:subClassOf rdf:resource="https://w3id.org/dpv/owl#AcademicResearch"/>
    <rdfs:subClassOf rdf:resource="https://w3id.org/dpv/sector/education/owl#EducationManagement"/>
  </rdf:Description>
  <rdf:Description rdf:about="https://w3id.org/dpv/sector/education/owl#StudentResourceAccessManagement">
    <sw:term_status xml:lang="en">accepted</sw:term_status>
    <rdfs:isDefinedBy rdf:resource="https://w3id.org/dpv/sector/education/owl#"/>
    <skos:prefLabel xml:lang="en">Student Resource Access Management</skos:prefLabel>
    <dct:created rdf:datatype="http://www.w3.org/2001/XMLSchema#date">2024-12-01</dct:created>
    <rdf:type rdf:resource="http://www.w3.org/2000/01/rdf-schema#Class"/>
    <rdf:type rdf:resource="https://w3id.org/dpv/owl#Purpose"/>
    <rdf:type rdf:resource="http://www.w3.org/2002/07/owl#Class"/>
    <skos:definition xml:lang="en">Purposes associated with determining and managing access to students to specific resources within an educational context, such as laboratory equipment or library resources</skos:definition>
    <rdfs:subClassOf rdf:resource="https://w3id.org/dpv/sector/education/owl#ServiceProvision"/>
  </rdf:Description>
  <rdf:Description rdf:about="https://w3id.org/dpv/sector/education/owl#StudentSocialActivitiesManagement">
    <skos:prefLabel xml:lang="en">Student Social Activities Management</skos:prefLabel>
    <rdfs:isDefinedBy rdf:resource="https://w3id.org/dpv/sector/education/owl#"/>
    <skos:definition xml:lang="en">Purposes associated with promotion, admission, and management of social activities for students within an educational context</skos:definition>
    <rdf:type rdf:resource="http://www.w3.org/2000/01/rdf-schema#Class"/>
    <rdf:type rdf:resource="https://w3id.org/dpv/owl#Purpose"/>
    <rdf:type rdf:resource="http://www.w3.org/2002/07/owl#Class"/>
    <dct:created rdf:datatype="http://www.w3.org/2001/XMLSchema#date">2024-12-01</dct:created>
    <sw:term_status xml:lang="en">accepted</sw:term_status>
    <rdfs:subClassOf rdf:resource="https://w3id.org/dpv/sector/education/owl#StudentManagement"/>
  </rdf:Description>
  <rdf:Description rdf:about="https://w3id.org/dpv/guides">
    <dct:format rdf:resource="https://www.iana.org/assignments/media-types/text/html"/>
    <profile:hasRole rdf:resource="http://www.w3.org/ns/dx/prof/role/guidance"/>
    <dct:title>Guides for Data Privacy Vocabulary</dct:title>
    <rdf:type rdf:resource="http://www.w3.org/ns/dx/prof/ResourceDescriptor"/>
    <dct:conformsTo rdf:resource="https://www.w3.org/TR/html/"/>
    <profile:hasArtifact rdf:resource="https://w3id.org/dpv/guides"/>
  </rdf:Description>
  <rdf:Description rdf:about="https://w3id.org/dpv/sector/education/owl#StudentIntegrityManagement">
    <dct:created rdf:datatype="http://www.w3.org/2001/XMLSchema#date">2024-12-01</dct:created>
    <rdfs:isDefinedBy rdf:resource="https://w3id.org/dpv/sector/education/owl#"/>
    <skos:definition xml:lang="en">Purposes associated with integrity assessment and management of students and activities by students in an educational context</skos:definition>
    <rdf:type rdf:resource="http://www.w3.org/2000/01/rdf-schema#Class"/>
    <rdf:type rdf:resource="https://w3id.org/dpv/owl#Purpose"/>
    <rdf:type rdf:resource="http://www.w3.org/2002/07/owl#Class"/>
    <skos:prefLabel xml:lang="en">Student Integrity Management</skos:prefLabel>
    <sw:term_status xml:lang="en">accepted</sw:term_status>
    <rdfs:subClassOf rdf:resource="https://w3id.org/dpv/owl#OrganisationRiskManagement"/>
    <rdfs:subClassOf rdf:resource="https://w3id.org/dpv/sector/education/owl#StudentManagement"/>
  </rdf:Description>
  <rdf:Description rdf:about="https://w3id.org/dpv/examples">
    <rdf:type rdf:resource="http://www.w3.org/ns/dx/prof/ResourceDescriptor"/>
    <dct:title>Examples</dct:title>
    <dct:conformsTo rdf:resource="https://www.w3.org/TR/html/"/>
    <dct:format rdf:resource="https://www.iana.org/assignments/media-types/text/html"/>
    <profile:hasRole rdf:resource="http://www.w3.org/ns/dx/prof/role/guidance"/>
    <profile:hasArtifact rdf:resource="https://w3id.org/dpv/examples"/>
  </rdf:Description>
  <rdf:Description rdf:about="https://w3id.org/dpv/sector/education/owl#StudentIntegrityTraining">
    <dct:created rdf:datatype="http://www.w3.org/2001/XMLSchema#date">2024-12-01</dct:created>
    <rdf:type rdf:resource="http://www.w3.org/2000/01/rdf-schema#Class"/>
    <rdf:type rdf:resource="https://w3id.org/dpv/owl#Purpose"/>
    <rdf:type rdf:resource="http://www.w3.org/2002/07/owl#Class"/>
    <sw:term_status xml:lang="en">accepted</sw:term_status>
    <skos:prefLabel xml:lang="en">Student Integrity Training</skos:prefLabel>
    <skos:definition xml:lang="en">Purposes associated with providing, assessing, and managing training for students regarding integrity in an educational context</skos:definition>
    <rdfs:isDefinedBy rdf:resource="https://w3id.org/dpv/sector/education/owl#"/>
    <rdfs:subClassOf rdf:resource="https://w3id.org/dpv/sector/education/owl#StudentIntegrityManagement"/>
  </rdf:Description>
  <rdf:Description rdf:about="https://w3id.org/dpv/sector/education/owl#StudentLearningFeedbackManagement">
    <rdf:type rdf:resource="http://www.w3.org/2000/01/rdf-schema#Class"/>
    <rdf:type rdf:resource="https://w3id.org/dpv/owl#Purpose"/>
    <rdf:type rdf:resource="http://www.w3.org/2002/07/owl#Class"/>
    <sw:term_status xml:lang="en">accepted</sw:term_status>
    <skos:prefLabel xml:lang="en">Student Learning Feedback Management</skos:prefLabel>
    <skos:definition xml:lang="en">Purposes associated with creating, providing, and managing feedback for students regarding their learning potential and outcomes in the context of educational services</skos:definition>
    <dct:created rdf:datatype="http://www.w3.org/2001/XMLSchema#date">2024-12-01</dct:created>
    <rdfs:isDefinedBy rdf:resource="https://w3id.org/dpv/sector/education/owl#"/>
    <rdfs:subClassOf rdf:resource="https://w3id.org/dpv/sector/education/owl#ServiceProvision"/>
  </rdf:Description>
  <rdf:Description rdf:about="https://w3id.org/dpv/sector/education/owl#StudentAcademicPotentialAssessment">
    <dct:created rdf:datatype="http://www.w3.org/2001/XMLSchema#date">2024-12-01</dct:created>
    <rdfs:isDefinedBy rdf:resource="https://w3id.org/dpv/sector/education/owl#"/>
    <rdf:type rdf:resource="http://www.w3.org/2000/01/rdf-schema#Class"/>
    <rdf:type rdf:resource="https://w3id.org/dpv/owl#Purpose"/>
    <rdf:type rdf:resource="http://www.w3.org/2002/07/owl#Class"/>
    <skos:prefLabel xml:lang="en">Student Academic Potential Assessment</skos:prefLabel>
    <skos:definition xml:lang="en">Purposes associated with assessment of academic potential as a measure of the capability of the student for specific academic or educational courses, programs, or services</skos:definition>
    <sw:term_status xml:lang="en">accepted</sw:term_status>
    <rdfs:subClassOf rdf:resource="https://w3id.org/dpv/sector/education/owl#StudentPerformanceAssessment"/>
  </rdf:Description>
  <rdf:Description rdf:about="https://w3id.org/dpv/primer">
    <dct:title>Primer for Data Privacy Vocabulary</dct:title>
    <rdf:type rdf:resource="http://www.w3.org/ns/dx/prof/ResourceDescriptor"/>
    <dct:conformsTo rdf:resource="https://www.w3.org/TR/html/"/>
    <dct:format rdf:resource="https://www.iana.org/assignments/media-types/text/html"/>
    <profile:hasRole rdf:resource="http://www.w3.org/ns/dx/prof/role/guidance"/>
    <profile:hasArtifact rdf:resource="https://w3id.org/dpv/primer"/>
  </rdf:Description>
  <rdf:Description rdf:about="https://w3id.org/dpv/sector/education/owl#ResearchDataManagement">
    <dct:created rdf:datatype="http://www.w3.org/2001/XMLSchema#date">2024-12-01</dct:created>
    <skos:definition xml:lang="en">Purposes associated with management of data in an educational or academic research context</skos:definition>
    <rdfs:isDefinedBy rdf:resource="https://w3id.org/dpv/sector/education/owl#"/>
    <rdf:type rdf:resource="http://www.w3.org/2000/01/rdf-schema#Class"/>
    <rdf:type rdf:resource="https://w3id.org/dpv/owl#Purpose"/>
    <rdf:type rdf:resource="http://www.w3.org/2002/07/owl#Class"/>
    <sw:term_status xml:lang="en">accepted</sw:term_status>
    <skos:prefLabel xml:lang="en">Research Data Management</skos:prefLabel>
    <rdfs:subClassOf rdf:resource="https://w3id.org/dpv/sector/education/owl#ResearchManagement"/>
  </rdf:Description>
  <rdf:Description rdf:about="https://w3id.org/dpv/sector/education/owl#StudentLearningNeedsAssessment">
    <skos:prefLabel xml:lang="en">Student Learning Needs Assessment</skos:prefLabel>
    <rdf:type rdf:resource="https://w3id.org/dpv/owl#Purpose"/>
    <rdf:type rdf:resource="http://www.w3.org/2000/01/rdf-schema#Class"/>
    <rdf:type rdf:resource="http://www.w3.org/2002/07/owl#Class"/>
    <sw:term_status xml:lang="en">accepted</sw:term_status>
    <skos:definition xml:lang="en">Purposes associated with assessment of learning needs or a measure of what resources, services, and approaches are needed for a student to learn and gain specific knowledge or group of knowledge within an educational context</skos:definition>
    <rdfs:isDefinedBy rdf:resource="https://w3id.org/dpv/sector/education/owl#"/>
    <dct:created rdf:datatype="http://www.w3.org/2001/XMLSchema#date">2024-12-01</dct:created>
    <rdfs:subClassOf rdf:resource="https://w3id.org/dpv/sector/education/owl#StudentPerformanceAssessment"/>
  </rdf:Description>
  <rdf:Description rdf:about="https://w3id.org/dpv/sector/education/owl#StudentInPersonProctoring">
    <skos:prefLabel xml:lang="en">Student In Person Proctoring</skos:prefLabel>
    <rdfs:isDefinedBy rdf:resource="https://w3id.org/dpv/sector/education/owl#"/>
    <rdf:type rdf:resource="http://www.w3.org/2000/01/rdf-schema#Class"/>
    <rdf:type rdf:resource="https://w3id.org/dpv/owl#Purpose"/>
    <rdf:type rdf:resource="http://www.w3.org/2002/07/owl#Class"/>
    <skos:definition xml:lang="en">Purposes associated with in-person or physical proctoring i.e. monitoring of students physically present within a particular location during an assessment with the aim of ensuring they do not cheat</skos:definition>
    <dct:created rdf:datatype="http://www.w3.org/2001/XMLSchema#date">2024-12-01</dct:created>
    <sw:term_status xml:lang="en">accepted</sw:term_status>
    <rdfs:subClassOf rdf:resource="https://w3id.org/dpv/sector/education/owl#StudentProctoring"/>
  </rdf:Description>
  <rdf:Description rdf:about="https://w3id.org/dpv/sector/education/owl#StudentPerformanceAssessment">
    <skos:definition xml:lang="en">Purposes associated with assessment of student performance, including through exams and assignments, in educational contexts</skos:definition>
    <skos:prefLabel xml:lang="en">Student Performance Assessment</skos:prefLabel>
    <rdf:type rdf:resource="http://www.w3.org/2000/01/rdf-schema#Class"/>
    <rdf:type rdf:resource="https://w3id.org/dpv/owl#Purpose"/>
    <rdf:type rdf:resource="http://www.w3.org/2002/07/owl#Class"/>
    <sw:term_status xml:lang="en">accepted</sw:term_status>
    <dct:created rdf:datatype="http://www.w3.org/2001/XMLSchema#date">2024-12-01</dct:created>
    <rdfs:isDefinedBy rdf:resource="https://w3id.org/dpv/sector/education/owl#"/>
    <rdfs:subClassOf rdf:resource="https://w3id.org/dpv/sector/education/owl#StudentManagement"/>
  </rdf:Description>
  <rdf:Description rdf:about="https://w3id.org/dpv/sector/education/owl#StudentCourseAllocation">
    <sw:term_status xml:lang="en">accepted</sw:term_status>
    <rdf:type rdf:resource="https://w3id.org/dpv/owl#Purpose"/>
    <rdf:type rdf:resource="http://www.w3.org/2000/01/rdf-schema#Class"/>
    <rdf:type rdf:resource="http://www.w3.org/2002/07/owl#Class"/>
    <skos:definition xml:lang="en">Purposes associated with allocation of students to specific courses in the context of educational services</skos:definition>
    <skos:prefLabel xml:lang="en">Student Course Allocation</skos:prefLabel>
    <rdfs:isDefinedBy rdf:resource="https://w3id.org/dpv/sector/education/owl#"/>
    <dct:created rdf:datatype="http://www.w3.org/2001/XMLSchema#date">2024-12-01</dct:created>
    <rdfs:subClassOf rdf:resource="https://w3id.org/dpv/sector/education/owl#StudentAllocation"/>
  </rdf:Description>
  <rdf:Description rdf:about="https://w3id.org/dpv/sector/education/owl#StudentAdmissionScreening">
    <dct:created rdf:datatype="http://www.w3.org/2001/XMLSchema#date">2024-12-01</dct:created>
    <sw:term_status xml:lang="en">accepted</sw:term_status>
    <rdf:type rdf:resource="https://w3id.org/dpv/owl#Purpose"/>
    <rdf:type rdf:resource="http://www.w3.org/2000/01/rdf-schema#Class"/>
    <rdf:type rdf:resource="http://www.w3.org/2002/07/owl#Class"/>
    <skos:definition xml:lang="en">Purposes associated with screening and filtering students and prospective students for the purposes of admission to educational organisations, resources, and services</skos:definition>
    <skos:prefLabel xml:lang="en">Student Admission Screening</skos:prefLabel>
    <rdfs:isDefinedBy rdf:resource="https://w3id.org/dpv/sector/education/owl#"/>
    <rdfs:subClassOf rdf:resource="https://w3id.org/dpv/sector/education/owl#StudentAdmissionManagement"/>
  </rdf:Description>
  <rdf:Description rdf:about="https://w3id.org/dpv/sector/education/owl#serialisation-rdf">
    <profile:hasRole rdf:resource="http://www.w3.org/ns/dx/prof/role/vocabulary"/>
    <rdf:type rdf:resource="http://www.w3.org/ns/dx/prof/ResourceDescriptor"/>
    <dct:format rdf:resource="https://www.iana.org/assignments/media-types/application/rdf+xml"/>
    <profile:hasArtifact rdf:resource="https://w3id.org/dpv/sector/education/sector-education-owl.rdf"/>
    <dct:conformsTo rdf:resource="http://www.w3.org/1999/02/22-rdf-syntax-ns#"/>
    <dct:title>Education Sector Concepts - RDF/XML serialisation</dct:title>
  </rdf:Description>
  <rdf:Description rdf:about="https://w3id.org/dpv/sector/education/owl#StaffManagement">
    <rdf:type rdf:resource="http://www.w3.org/2000/01/rdf-schema#Class"/>
    <rdf:type rdf:resource="https://w3id.org/dpv/owl#Purpose"/>
    <rdf:type rdf:resource="http://www.w3.org/2002/07/owl#Class"/>
    <skos:prefLabel xml:lang="en">Staff Management</skos:prefLabel>
    <sw:term_status xml:lang="en">accepted</sw:term_status>
    <rdfs:isDefinedBy rdf:resource="https://w3id.org/dpv/sector/education/owl#"/>
    <skos:definition xml:lang="en">Purposes associated with management of staff and related personnel in educational organisations</skos:definition>
    <dct:created rdf:datatype="http://www.w3.org/2001/XMLSchema#date">2024-12-01</dct:created>
    <rdfs:subClassOf rdf:resource="https://w3id.org/dpv/sector/education/owl#EducationManagement"/>
  </rdf:Description>
  <rdf:Description rdf:about="https://w3id.org/dpv/sector/education/owl#StudentLearningOutcomeAssessment">
    <dct:created rdf:datatype="http://www.w3.org/2001/XMLSchema#date">2024-12-01</dct:created>
    <rdf:type rdf:resource="http://www.w3.org/2000/01/rdf-schema#Class"/>
    <rdf:type rdf:resource="https://w3id.org/dpv/owl#Purpose"/>
    <rdf:type rdf:resource="http://www.w3.org/2002/07/owl#Class"/>
    <sw:term_status xml:lang="en">accepted</sw:term_status>
    <skos:prefLabel xml:lang="en">Student Learning Outcome Assessment</skos:prefLabel>
    <skos:definition xml:lang="en">Purposes associated with assessment of student performance in the context of meeting learning outcomes as set within the educational course or program</skos:definition>
    <rdfs:isDefinedBy rdf:resource="https://w3id.org/dpv/sector/education/owl#"/>
    <rdfs:subClassOf rdf:resource="https://w3id.org/dpv/sector/education/owl#StudentPerformanceAssessment"/>
  </rdf:Description>
  <rdf:Description rdf:about="https://w3id.org/dpv/sector/education/owl#StudentGuidanceManagement">
    <dct:created rdf:datatype="http://www.w3.org/2001/XMLSchema#date">2024-12-01</dct:created>
    <rdfs:isDefinedBy rdf:resource="https://w3id.org/dpv/sector/education/owl#"/>
    <rdf:type rdf:resource="http://www.w3.org/2000/01/rdf-schema#Class"/>
    <rdf:type rdf:resource="https://w3id.org/dpv/owl#Purpose"/>
    <rdf:type rdf:resource="http://www.w3.org/2002/07/owl#Class"/>
    <skos:definition xml:lang="en">Purposes associated with providing and managing guidance, counselling, and other related services within the context of educational services</skos:definition>
    <sw:term_status xml:lang="en">accepted</sw:term_status>
    <skos:prefLabel xml:lang="en">Student Guidance Management</skos:prefLabel>
    <rdfs:subClassOf rdf:resource="https://w3id.org/dpv/sector/education/owl#StudentWellbeingManagement"/>
  </rdf:Description>
  <rdf:Description rdf:about="https://w3id.org/dpv/sector/education/owl#StudentPlagiarismDetection">
    <dct:created rdf:datatype="http://www.w3.org/2001/XMLSchema#date">2024-12-01</dct:created>
    <skos:definition xml:lang="en">Purposes associated with determination of plagiarism demonstrated by a student or students or present within the work submitted by a student or students in an educational context</skos:definition>
    <rdf:type rdf:resource="http://www.w3.org/2000/01/rdf-schema#Class"/>
    <rdf:type rdf:resource="https://w3id.org/dpv/owl#Purpose"/>
    <rdf:type rdf:resource="http://www.w3.org/2002/07/owl#Class"/>
    <sw:term_status xml:lang="en">accepted</sw:term_status>
    <skos:prefLabel xml:lang="en">Student Plagiarism Detection</skos:prefLabel>
    <rdfs:isDefinedBy rdf:resource="https://w3id.org/dpv/sector/education/owl#"/>
    <rdfs:subClassOf rdf:resource="https://w3id.org/dpv/owl#FraudPreventionAndDetection"/>
    <rdfs:subClassOf rdf:resource="https://w3id.org/dpv/sector/education/owl#StudentIntegrityManagement"/>
  </rdf:Description>
  <rdf:Description rdf:about="https://w3id.org/dpv/sector/education/owl#StudentFeesManagement">
    <skos:definition xml:lang="en">Purposes associated with management of fees from or for students in the context of educational resources and services</skos:definition>
    <rdf:type rdf:resource="http://www.w3.org/2000/01/rdf-schema#Class"/>
    <rdf:type rdf:resource="https://w3id.org/dpv/owl#Purpose"/>
    <rdf:type rdf:resource="http://www.w3.org/2002/07/owl#Class"/>
    <skos:prefLabel xml:lang="en">Student Fees Management</skos:prefLabel>
    <dct:created rdf:datatype="http://www.w3.org/2001/XMLSchema#date">2024-12-01</dct:created>
    <rdfs:isDefinedBy rdf:resource="https://w3id.org/dpv/sector/education/owl#"/>
    <sw:term_status xml:lang="en">accepted</sw:term_status>
    <rdfs:subClassOf rdf:resource="https://w3id.org/dpv/sector/education/owl#StudentAdmissionManagement"/>
  </rdf:Description>
  <rdf:Description rdf:about="https://w3id.org/dpv/sector/education/owl#StudentAdmissionManagement">
    <dct:created rdf:datatype="http://www.w3.org/2001/XMLSchema#date">2024-12-01</dct:created>
    <rdfs:isDefinedBy rdf:resource="https://w3id.org/dpv/sector/education/owl#"/>
    <skos:prefLabel xml:lang="en">Student Admission Management</skos:prefLabel>
    <rdf:type rdf:resource="http://www.w3.org/2000/01/rdf-schema#Class"/>
    <rdf:type rdf:resource="https://w3id.org/dpv/owl#Purpose"/>
    <rdf:type rdf:resource="http://www.w3.org/2002/07/owl#Class"/>
    <skos:definition xml:lang="en">Purposes associated with management of admission process for current and prospective students</skos:definition>
    <sw:term_status xml:lang="en">accepted</sw:term_status>
    <rdfs:subClassOf rdf:resource="https://w3id.org/dpv/sector/education/owl#StudentManagement"/>
    <rdfs:subClassOf rdf:resource="https://w3id.org/dpv/sector/education/owl#AccessManagement"/>
  </rdf:Description>
  <rdf:Description rdf:about="https://w3id.org/dpv/sector/education/owl#StudentProctoring">
    <dct:created rdf:datatype="http://www.w3.org/2001/XMLSchema#date">2024-12-01</dct:created>
    <rdfs:isDefinedBy rdf:resource="https://w3id.org/dpv/sector/education/owl#"/>
    <rdf:type rdf:resource="http://www.w3.org/2000/01/rdf-schema#Class"/>
    <rdf:type rdf:resource="https://w3id.org/dpv/owl#Purpose"/>
    <rdf:type rdf:resource="http://www.w3.org/2002/07/owl#Class"/>
    <sw:term_status xml:lang="en">accepted</sw:term_status>
    <skos:definition xml:lang="en">Purposes associated with proctoring i.e. monitoring of students during an assessment with the aim of ensuring they do not cheat</skos:definition>
    <skos:prefLabel xml:lang="en">Student Proctoring</skos:prefLabel>
    <rdfs:subClassOf rdf:resource="https://w3id.org/dpv/sector/education/owl#StudentCheatingAssessment"/>
  </rdf:Description>
  <rdf:Description rdf:about="https://w3id.org/dpv/sector/education/owl#ServiceProvision">
    <rdf:type rdf:resource="http://www.w3.org/2000/01/rdf-schema#Class"/>
    <rdf:type rdf:resource="https://w3id.org/dpv/owl#Purpose"/>
    <rdf:type rdf:resource="http://www.w3.org/2002/07/owl#Class"/>
    <skos:prefLabel xml:lang="en">Service Provision</skos:prefLabel>
    <skos:definition xml:lang="en">Purposes associated with provision of educational services, including lectures, seminars, laboratory work, and other similar activities within the context of provision of education</skos:definition>
    <rdfs:isDefinedBy rdf:resource="https://w3id.org/dpv/sector/education/owl#"/>
    <dct:created rdf:datatype="http://www.w3.org/2001/XMLSchema#date">2024-12-01</dct:created>
    <sw:term_status xml:lang="en">accepted</sw:term_status>
    <rdfs:subClassOf rdf:resource="https://w3id.org/dpv/sector/education/owl#EducationManagement"/>
    <rdfs:subClassOf rdf:resource="https://w3id.org/dpv/owl#ServiceProvision"/>
  </rdf:Description>
  <rdf:Description rdf:about="https://w3id.org/dpv/sector/education/owl#StudentWellbeingManagement">
    <rdf:type rdf:resource="http://www.w3.org/2000/01/rdf-schema#Class"/>
    <rdf:type rdf:resource="https://w3id.org/dpv/owl#Purpose"/>
    <rdf:type rdf:resource="http://www.w3.org/2002/07/owl#Class"/>
    <sw:term_status xml:lang="en">accepted</sw:term_status>
    <skos:prefLabel xml:lang="en">Student Wellbeing Management</skos:prefLabel>
    <skos:definition xml:lang="en">Purposes associated with management of student wellbeing in an educational context</skos:definition>
    <rdfs:isDefinedBy rdf:resource="https://w3id.org/dpv/sector/education/owl#"/>
    <dct:created rdf:datatype="http://www.w3.org/2001/XMLSchema#date">2024-12-01</dct:created>
    <rdfs:subClassOf rdf:resource="https://w3id.org/dpv/sector/education/owl#StudentManagement"/>
  </rdf:Description>
  <rdf:Description rdf:about="https://w3id.org/dpv/sector/education/owl#serialisation-n3">
    <rdf:type rdf:resource="http://www.w3.org/ns/dx/prof/ResourceDescriptor"/>
    <dct:conformsTo rdf:resource="https://www.w3.org/TeamSubmission/n3/"/>
    <dct:format rdf:resource="https://www.iana.org/assignments/media-types/text/n3"/>
    <profile:hasArtifact rdf:resource="https://w3id.org/dpv/sector/education/sector-education-owl.n3"/>
    <dct:title>Education Sector Concepts - N3 serialisation</dct:title>
    <profile:hasRole rdf:resource="http://www.w3.org/ns/dx/prof/role/vocabulary"/>
  </rdf:Description>
  <rdf:Description rdf:about="https://w3id.org/dpv/sector/education/owl#StudentProgramRecommendation">
    <sw:term_status xml:lang="en">accepted</sw:term_status>
    <skos:prefLabel xml:lang="en">Student Program Recommendation</skos:prefLabel>
    <rdf:type rdf:resource="https://w3id.org/dpv/owl#Purpose"/>
    <rdf:type rdf:resource="http://www.w3.org/2000/01/rdf-schema#Class"/>
    <rdf:type rdf:resource="http://www.w3.org/2002/07/owl#Class"/>
    <rdfs:isDefinedBy rdf:resource="https://w3id.org/dpv/sector/education/owl#"/>
    <skos:definition xml:lang="en">Purposes associated with providing recommendations to students regarding prospective programs for education</skos:definition>
    <dct:created rdf:datatype="http://www.w3.org/2001/XMLSchema#date">2024-12-01</dct:created>
    <rdfs:subClassOf rdf:resource="https://w3id.org/dpv/sector/education/owl#StudentAdmissionManagement"/>
  </rdf:Description>
  <rdf:Description rdf:about="https://w3id.org/dpv/sector/education/owl#StudentCheatingAssessment">
    <skos:definition xml:lang="en">Purposes associated with detection, assessment, and management of activities considered as cheating or other activities considered to subvert rules or to obtain unfair advantage in the context of educational services and assessments</skos:definition>
    <skos:prefLabel xml:lang="en">Student Cheating Assessment</skos:prefLabel>
    <rdfs:isDefinedBy rdf:resource="https://w3id.org/dpv/sector/education/owl#"/>
    <rdf:type rdf:resource="http://www.w3.org/2000/01/rdf-schema#Class"/>
    <rdf:type rdf:resource="https://w3id.org/dpv/owl#Purpose"/>
    <rdf:type rdf:resource="http://www.w3.org/2002/07/owl#Class"/>
    <dct:created rdf:datatype="http://www.w3.org/2001/XMLSchema#date">2024-12-01</dct:created>
    <sw:term_status xml:lang="en">accepted</sw:term_status>
    <rdfs:subClassOf rdf:resource="https://w3id.org/dpv/owl#FraudPreventionAndDetection"/>
    <rdfs:subClassOf rdf:resource="https://w3id.org/dpv/sector/education/owl#StudentIntegrityManagement"/>
  </rdf:Description>
  <rdf:Description rdf:about="https://w3id.org/dpv/sector/education/owl#EducationManagement">
    <rdfs:isDefinedBy rdf:resource="https://w3id.org/dpv/sector/education/owl#"/>
    <dct:created rdf:datatype="http://www.w3.org/2001/XMLSchema#date">2024-12-01</dct:created>
    <skos:definition xml:lang="en">Purposes associated with running and management of educational organisations and services</skos:definition>
    <rdf:type rdf:resource="http://www.w3.org/2000/01/rdf-schema#Class"/>
    <rdf:type rdf:resource="https://w3id.org/dpv/owl#Purpose"/>
    <rdf:type rdf:resource="http://www.w3.org/2002/07/owl#Class"/>
    <skos:prefLabel xml:lang="en">Education Management</skos:prefLabel>
    <sw:term_status xml:lang="en">accepted</sw:term_status>
    <rdfs:subClassOf rdf:resource="https://w3id.org/dpv/owl#Purpose"/>
  </rdf:Description>
  <rdf:Description rdf:about="https://w3id.org/dpv/sector/education/owl#ResearchUserStudyManagement">
    <skos:definition xml:lang="en">Purposes associated with conducting and assessing studies involving people (as user studies) in an educational or academic research context</skos:definition>
    <rdf:type rdf:resource="http://www.w3.org/2000/01/rdf-schema#Class"/>
    <rdf:type rdf:resource="https://w3id.org/dpv/owl#Purpose"/>
    <rdf:type rdf:resource="http://www.w3.org/2002/07/owl#Class"/>
    <sw:term_status xml:lang="en">accepted</sw:term_status>
    <dct:created rdf:datatype="http://www.w3.org/2001/XMLSchema#date">2024-12-01</dct:created>
    <skos:prefLabel xml:lang="en">Research User Study Management</skos:prefLabel>
    <rdfs:isDefinedBy rdf:resource="https://w3id.org/dpv/sector/education/owl#"/>
    <rdfs:subClassOf rdf:resource="https://w3id.org/dpv/sector/education/owl#ResearchManagement"/>
  </rdf:Description>
  <rdf:Description rdf:nodeID="person-harshvardhan-j-pandit">
    <foaf:name>Harshvardhan J. Pandit</foaf:name>
    <rdf:type rdf:resource="http://xmlns.com/foaf/0.1/Person"/>
    <rdf:type rdf:resource="http://purl.org/dc/terms/Agent"/>
    <foaf:homepage>https://harshp.com/</foaf:homepage>
    <org:memberOf rdf:nodeID="org-ai-accountability-lab-aial-trinity-college-dublin"/>
    <scoro:hasORCID>0000-0002-5068-3714</scoro:hasORCID>
  </rdf:Description>
  <rdf:Description rdf:about="https://w3id.org/dpv/sector/education/owl#StudentFinancialBenefitsManagement">
    <rdfs:isDefinedBy rdf:resource="https://w3id.org/dpv/sector/education/owl#"/>
    <skos:prefLabel xml:lang="en">Student Financial Benefits Management</skos:prefLabel>
    <rdf:type rdf:resource="http://www.w3.org/2000/01/rdf-schema#Class"/>
    <rdf:type rdf:resource="https://w3id.org/dpv/owl#Purpose"/>
    <rdf:type rdf:resource="http://www.w3.org/2002/07/owl#Class"/>
    <skos:definition xml:lang="en">Purposes associated with management of financial benefits for students in the context of educational resources and services</skos:definition>
    <dct:created rdf:datatype="http://www.w3.org/2001/XMLSchema#date">2024-12-01</dct:created>
    <sw:term_status xml:lang="en">accepted</sw:term_status>
    <rdfs:subClassOf rdf:resource="https://w3id.org/dpv/sector/education/owl#StudentAdmissionManagement"/>
  </rdf:Description>
  <rdf:Description rdf:about="https://w3id.org/dpv/sector/education/owl#StudentInstituteRecommendation">
    <sw:term_status xml:lang="en">accepted</sw:term_status>
    <rdf:type rdf:resource="http://www.w3.org/2000/01/rdf-schema#Class"/>
    <rdf:type rdf:resource="https://w3id.org/dpv/owl#Purpose"/>
    <rdf:type rdf:resource="http://www.w3.org/2002/07/owl#Class"/>
    <dct:created rdf:datatype="http://www.w3.org/2001/XMLSchema#date">2024-12-01</dct:created>
    <rdfs:isDefinedBy rdf:resource="https://w3id.org/dpv/sector/education/owl#"/>
    <skos:definition xml:lang="en">Purposes associated with providing recommendations to students regarding prospective institutes for education</skos:definition>
    <skos:prefLabel xml:lang="en">Student Institute Recommendation</skos:prefLabel>
    <rdfs:subClassOf rdf:resource="https://w3id.org/dpv/sector/education/owl#StudentAdmissionManagement"/>
  </rdf:Description>
  <rdf:Description rdf:about="https://w3id.org/dpv/sector/education/owl#StudentEligibilityAssessment">
    <dct:created rdf:datatype="http://www.w3.org/2001/XMLSchema#date">2024-12-01</dct:created>
    <skos:prefLabel xml:lang="en">Student Eligibility Assessment</skos:prefLabel>
    <rdf:type rdf:resource="https://w3id.org/dpv/owl#Purpose"/>
    <rdf:type rdf:resource="http://www.w3.org/2000/01/rdf-schema#Class"/>
    <rdf:type rdf:resource="http://www.w3.org/2002/07/owl#Class"/>
    <sw:term_status xml:lang="en">accepted</sw:term_status>
    <rdfs:isDefinedBy rdf:resource="https://w3id.org/dpv/sector/education/owl#"/>
    <skos:definition xml:lang="en">Purposes associated with eligibility assessment of students and prospective students for the purposes of admission and access to educational institutes, resources, and services</skos:definition>
    <rdfs:subClassOf rdf:resource="https://w3id.org/dpv/sector/education/owl#StudentAdmissionManagement"/>
  </rdf:Description>
  <rdf:Description rdf:about="https://w3id.org/dpv/sector/education/owl#StudentCourseRecommendation">
    <rdfs:isDefinedBy rdf:resource="https://w3id.org/dpv/sector/education/owl#"/>
    <rdf:type rdf:resource="http://www.w3.org/2000/01/rdf-schema#Class"/>
    <rdf:type rdf:resource="https://w3id.org/dpv/owl#Purpose"/>
    <rdf:type rdf:resource="http://www.w3.org/2002/07/owl#Class"/>
    <skos:definition xml:lang="en">Purposes associated with providing recommendations to students regarding prospective courses for education</skos:definition>
    <dct:created rdf:datatype="http://www.w3.org/2001/XMLSchema#date">2024-12-01</dct:created>
    <skos:prefLabel xml:lang="en">Student Course Recommendation</skos:prefLabel>
    <sw:term_status xml:lang="en">accepted</sw:term_status>
    <rdfs:subClassOf rdf:resource="https://w3id.org/dpv/sector/education/owl#StudentAdmissionManagement"/>
  </rdf:Description>
  <rdf:Description rdf:nodeID="org-ai-accountability-lab-aial-trinity-college-dublin">
    <foaf:name>AI Accountability Lab (AIAL), Trinity College Dublin</foaf:name>
    <rdf:type rdf:resource="http://xmlns.com/foaf/0.1/Organization"/>
  </rdf:Description>
  <rdf:Description rdf:about="https://w3id.org/dpv/sector/education/owl#StudentContentDelivery">
    <rdfs:isDefinedBy rdf:resource="https://w3id.org/dpv/sector/education/owl#"/>
    <skos:definition xml:lang="en">Purposes associated with delivery of content to student or group of students in the context of educational services</skos:definition>
    <dct:created rdf:datatype="http://www.w3.org/2001/XMLSchema#date">2024-12-01</dct:created>
    <rdf:type rdf:resource="http://www.w3.org/2000/01/rdf-schema#Class"/>
    <rdf:type rdf:resource="https://w3id.org/dpv/owl#Purpose"/>
    <rdf:type rdf:resource="http://www.w3.org/2002/07/owl#Class"/>
    <sw:term_status xml:lang="en">accepted</sw:term_status>
    <skos:prefLabel xml:lang="en">Student Content Delivery</skos:prefLabel>
    <rdfs:subClassOf rdf:resource="https://w3id.org/dpv/sector/education/owl#ServiceProvision"/>
  </rdf:Description>
  <rdf:Description rdf:about="https://w3id.org/dpv/sector/education/owl#serialisation-jsonld">
    <dct:title>Education Sector Concepts - JSON-LD serialisation</dct:title>
    <profile:hasArtifact rdf:resource="https://w3id.org/dpv/sector/education/sector-education-owl.jsonld"/>
    <dct:format rdf:resource="https://www.iana.org/assignments/media-types/application/ld+json"/>
    <profile:hasRole rdf:resource="http://www.w3.org/ns/dx/prof/role/vocabulary"/>
    <rdf:type rdf:resource="http://www.w3.org/ns/dx/prof/ResourceDescriptor"/>
    <dct:conformsTo rdf:resource="https://www.w3.org/TR/json-ld11/"/>
  </rdf:Description>
  <rdf:Description rdf:about="https://w3id.org/dpv/sector/education/owl#StaffPerformanceAssessment">
    <rdf:type rdf:resource="https://w3id.org/dpv/owl#Purpose"/>
    <rdf:type rdf:resource="http://www.w3.org/2000/01/rdf-schema#Class"/>
    <rdf:type rdf:resource="http://www.w3.org/2002/07/owl#Class"/>
    <skos:definition xml:lang="en">Purposes associated with assessment of performance of staff and related personnel in the context of an educational organisation</skos:definition>
    <sw:term_status xml:lang="en">accepted</sw:term_status>
    <skos:prefLabel xml:lang="en">Staff Performance Assessment</skos:prefLabel>
    <dct:created rdf:datatype="http://www.w3.org/2001/XMLSchema#date">2024-12-01</dct:created>
    <rdfs:isDefinedBy rdf:resource="https://w3id.org/dpv/sector/education/owl#"/>
    <rdfs:subClassOf rdf:resource="https://w3id.org/dpv/sector/education/owl#StaffManagement"/>
    <rdfs:subClassOf rdf:resource="https://w3id.org/dpv/owl#PersonnelPerformanceMonitoring"/>
  </rdf:Description>
  <rdf:Description rdf:about="https://w3id.org/dpv/sector/education/owl#serialisation-html">
    <dct:format rdf:resource="https://www.iana.org/assignments/media-types/text/html"/>
    <rdf:type rdf:resource="http://www.w3.org/ns/dx/prof/ResourceDescriptor"/>
    <profile:hasArtifact rdf:resource="https://w3id.org/dpv/sector/education/sector-education-owl.html"/>
    <profile:hasRole rdf:resource="http://www.w3.org/ns/dx/prof/role/specification"/>
    <dct:title>Education Sector Concepts - HTML serialisation</dct:title>
    <dct:conformsTo rdf:resource="https://www.w3.org/TR/html/"/>
  </rdf:Description>
  <rdf:Description rdf:about="https://w3id.org/dpv/sector/education/owl#serialisation-ttl">
    <profile:hasArtifact rdf:resource="https://w3id.org/dpv/sector/education/sector-education-owl.ttl"/>
    <dct:format rdf:resource="https://www.iana.org/assignments/media-types/text/turtle"/>
    <dct:conformsTo rdf:resource="https://www.w3.org/TR/turtle/"/>
    <profile:hasRole rdf:resource="http://www.w3.org/ns/dx/prof/role/vocabulary"/>
    <dct:title>Education Sector Concepts - Turtle serialisation</dct:title>
    <rdf:type rdf:resource="http://www.w3.org/ns/dx/prof/ResourceDescriptor"/>
  </rdf:Description>
  <rdf:Description rdf:about="https://w3id.org/dpv/sector/education/owl#StudentSpecialNeedsManagement">
    <skos:definition xml:lang="en">Purposes associated with determination and management of special needs of students and prospective students in the context of educational services and resources</skos:definition>
    <rdf:type rdf:resource="http://www.w3.org/2000/01/rdf-schema#Class"/>
    <rdf:type rdf:resource="https://w3id.org/dpv/owl#Purpose"/>
    <rdf:type rdf:resource="http://www.w3.org/2002/07/owl#Class"/>
    <sw:term_status xml:lang="en">accepted</sw:term_status>
    <dct:created rdf:datatype="http://www.w3.org/2001/XMLSchema#date">2024-12-01</dct:created>
    <rdfs:isDefinedBy rdf:resource="https://w3id.org/dpv/sector/education/owl#"/>
    <skos:prefLabel xml:lang="en">Student Special Needs Management</skos:prefLabel>
    <rdfs:subClassOf rdf:resource="https://w3id.org/dpv/sector/education/owl#StudentAdmissionManagement"/>
  </rdf:Description>
  <rdf:Description rdf:about="https://w3id.org/dpv/sector/education/owl#StudentAllocation">
    <rdfs:isDefinedBy rdf:resource="https://w3id.org/dpv/sector/education/owl#"/>
    <skos:definition xml:lang="en">Purposes associated with allocation of students to educational institutes, resources, and services</skos:definition>
    <rdf:type rdf:resource="http://www.w3.org/2000/01/rdf-schema#Class"/>
    <rdf:type rdf:resource="https://w3id.org/dpv/owl#Purpose"/>
    <rdf:type rdf:resource="http://www.w3.org/2002/07/owl#Class"/>
    <skos:prefLabel xml:lang="en">StudentAllocation</skos:prefLabel>
    <dct:created rdf:datatype="http://www.w3.org/2001/XMLSchema#date">2024-12-01</dct:created>
    <sw:term_status xml:lang="en">accepted</sw:term_status>
    <rdfs:subClassOf rdf:resource="https://w3id.org/dpv/sector/education/owl#StudentManagement"/>
  </rdf:Description>
  <rdf:Description rdf:nodeID="org-adapt-centre-trinity-college-dublin">
    <foaf:name>ADAPT Centre, Trinity College Dublin</foaf:name>
    <rdf:type rdf:resource="http://xmlns.com/foaf/0.1/Organization"/>
  </rdf:Description>
</rdf:RDF>
