<?xml version="1.0" encoding="utf-8"?>
<rdf:RDF
   xmlns:bibo="http://purl.org/ontology/bibo/"
   xmlns:dcam="http://purl.org/dc/dcam/"
   xmlns:dct="http://purl.org/dc/terms/"
   xmlns:foaf="http://xmlns.com/foaf/0.1/"
   xmlns:org="http://www.w3.org/ns/org#"
   xmlns:owl="http://www.w3.org/2002/07/owl#"
   xmlns:profile="http://www.w3.org/ns/dx/prof/"
   xmlns:rdf="http://www.w3.org/1999/02/22-rdf-syntax-ns#"
   xmlns:rdfs="http://www.w3.org/2000/01/rdf-schema#"
   xmlns:schema="https://schema.org/"
   xmlns:scoro="http://purl.org/spar/scoro/"
   xmlns:skos="http://www.w3.org/2004/02/skos/core#"
   xmlns:sw="http://www.w3.org/2003/06/sw-vocab-status/ns#"
   xmlns:vann="http://purl.org/vocab/vann/"
>
  <rdf:Description rdf:nodeID="Ne84980f7db76425ca367742d2085d8c9">
    <org:memberOf rdf:nodeID="N1179325f3fdc440ea7096a5f4b108a44"/>
    <scoro:hasORCID>0009-0006-4623-1463</scoro:hasORCID>
    <rdf:type rdf:resource="http://xmlns.com/foaf/0.1/Person"/>
    <rdf:type rdf:resource="http://purl.org/dc/terms/Agent"/>
    <foaf:name>Julian Flake</foaf:name>
  </rdf:Description>
  <rdf:Description rdf:about="https://w3id.org/dpv/risk/owl#shares">
    <rdfs:subPropertyOf rdf:resource="https://w3id.org/dpv/risk/owl#controls"/>
    <rdf:type rdf:resource="http://www.w3.org/1999/02/22-rdf-syntax-ns#Property"/>
    <rdf:type rdf:resource="http://www.w3.org/2002/07/owl#ObjectProperty"/>
    <rdfs:isDefinedBy rdf:resource="https://w3id.org/dpv/risk/owl#"/>
    <dct:created rdf:datatype="http://www.w3.org/2001/XMLSchema#date">2025-01-06</dct:created>
    <skos:definition xml:lang="en">Indicates the specified event or action is shared with another context or entity by this control</skos:definition>
    <skos:prefLabel xml:lang="en">shares</skos:prefLabel>
    <dct:contributor rdf:nodeID="Ne22a67b17c7e4a779c30d2864b6a0cee"/>
    <dcam:domainIncludes rdf:resource="https://w3id.org/dpv/risk/owl#ShareControl"/>
    <sw:term_status xml:lang="en">accepted</sw:term_status>
    <schema:rangeIncludes rdf:resource="https://w3id.org/dpv/owl#RiskConcept"/>
    <dcam:rangeIncludes rdf:resource="https://w3id.org/dpv/owl#RiskConcept"/>
    <schema:domainIncludes rdf:resource="https://w3id.org/dpv/risk/owl#ShareControl"/>
  </rdf:Description>
  <rdf:Description rdf:about="https://w3id.org/dpv/risk/owl#resolves">
    <rdfs:isDefinedBy rdf:resource="https://w3id.org/dpv/risk/owl#"/>
    <rdf:type rdf:resource="http://www.w3.org/1999/02/22-rdf-syntax-ns#Property"/>
    <rdf:type rdf:resource="http://www.w3.org/2002/07/owl#ObjectProperty"/>
    <schema:rangeIncludes rdf:resource="https://w3id.org/dpv/owl#RiskConcept"/>
    <dcam:domainIncludes rdf:resource="https://w3id.org/dpv/risk/owl#ResolutionControl"/>
    <skos:definition xml:lang="en">Indicates the specified event or action is resolved by this control</skos:definition>
    <dct:contributor rdf:nodeID="Ne22a67b17c7e4a779c30d2864b6a0cee"/>
    <dct:created rdf:datatype="http://www.w3.org/2001/XMLSchema#date">2025-01-06</dct:created>
    <sw:term_status xml:lang="en">accepted</sw:term_status>
    <dcam:rangeIncludes rdf:resource="https://w3id.org/dpv/owl#RiskConcept"/>
    <schema:domainIncludes rdf:resource="https://w3id.org/dpv/risk/owl#ResolutionControl"/>
    <rdfs:subPropertyOf rdf:resource="https://w3id.org/dpv/risk/owl#controls"/>
    <skos:prefLabel xml:lang="en">resolves</skos:prefLabel>
  </rdf:Description>
  <rdf:Description rdf:about="https://w3id.org/dpv/risk/owl#RemeditationControl">
    <rdf:type rdf:resource="http://www.w3.org/2000/01/rdf-schema#Class"/>
    <rdf:type rdf:resource="https://w3id.org/dpv/risk/owl#RiskControl"/>
    <rdf:type rdf:resource="http://www.w3.org/2002/07/owl#Class"/>
    <skos:prefLabel xml:lang="en">Remeditation Control</skos:prefLabel>
    <dct:modified rdf:datatype="http://www.w3.org/2001/XMLSchema#date">2025-01-06</dct:modified>
    <sw:term_status xml:lang="en">modified</sw:term_status>
    <dct:created rdf:datatype="http://www.w3.org/2001/XMLSchema#date">2024-05-19</dct:created>
    <rdfs:isDefinedBy rdf:resource="https://w3id.org/dpv/risk/owl#"/>
    <skos:scopeNote xml:lang="en">Remediation involves making changes in the context to avoid further events and effects, which may be for the specific event or for other similar events and effects. As such, remediation can also be undertaken as a proactive measure in the risk management lifecycle following an incident</skos:scopeNote>
    <dct:contributor rdf:nodeID="N9c63c24625fe482386a350b4ea27b4f8"/>
    <dct:contributor rdf:nodeID="Ne22a67b17c7e4a779c30d2864b6a0cee"/>
    <skos:definition xml:lang="en">Control that aims to fix or remedy the causes of an event to prevent further occurences</skos:definition>
    <rdfs:subClassOf rdf:resource="https://w3id.org/dpv/risk/owl#ResolutionControl"/>
  </rdf:Description>
  <rdf:Description rdf:about="https://w3id.org/dpv/risk/owl#ProactiveControl">
    <rdf:type rdf:resource="https://w3id.org/dpv/risk/owl#RiskControl"/>
    <rdf:type rdf:resource="http://www.w3.org/2000/01/rdf-schema#Class"/>
    <rdf:type rdf:resource="http://www.w3.org/2002/07/owl#Class"/>
    <sw:term_status xml:lang="en">accepted</sw:term_status>
    <skos:prefLabel xml:lang="en">Proactive Control</skos:prefLabel>
    <skos:scopeNote xml:lang="en">The use of 'proactive' here refers to this control being established to address events before they occur. It does not indicate putting in place controls before the event such as planning ahead for potential use of controls to respond to an incident</skos:scopeNote>
    <rdfs:isDefinedBy rdf:resource="https://w3id.org/dpv/risk/owl#"/>
    <dct:created rdf:datatype="http://www.w3.org/2001/XMLSchema#date">2025-01-06</dct:created>
    <skos:definition xml:lang="en">Control that is established or functions before an event occurs</skos:definition>
    <dct:contributor rdf:nodeID="Ne22a67b17c7e4a779c30d2864b6a0cee"/>
    <rdfs:subClassOf rdf:resource="https://w3id.org/dpv/risk/owl#RiskControl"/>
  </rdf:Description>
  <rdf:Description rdf:about="https://w3id.org/dpv/risk/owl#overrides">
    <rdf:type rdf:resource="http://www.w3.org/1999/02/22-rdf-syntax-ns#Property"/>
    <rdf:type rdf:resource="http://www.w3.org/2002/07/owl#ObjectProperty"/>
    <skos:definition xml:lang="en">Indicates the specified event or action is overridden by this control</skos:definition>
    <dct:contributor rdf:nodeID="Ne22a67b17c7e4a779c30d2864b6a0cee"/>
    <sw:term_status xml:lang="en">accepted</sw:term_status>
    <rdfs:isDefinedBy rdf:resource="https://w3id.org/dpv/risk/owl#"/>
    <schema:rangeIncludes rdf:resource="https://w3id.org/dpv/owl#RiskConcept"/>
    <dcam:rangeIncludes rdf:resource="https://w3id.org/dpv/owl#RiskConcept"/>
    <dct:created rdf:datatype="http://www.w3.org/2001/XMLSchema#date">2025-01-06</dct:created>
    <rdfs:subPropertyOf rdf:resource="https://w3id.org/dpv/risk/owl#controls"/>
    <schema:domainIncludes rdf:resource="https://w3id.org/dpv/risk/owl#OverrideControl"/>
    <dcam:domainIncludes rdf:resource="https://w3id.org/dpv/risk/owl#OverrideControl"/>
    <skos:prefLabel xml:lang="en">overrides</skos:prefLabel>
  </rdf:Description>
  <rdf:Description rdf:about="https://w3id.org/dpv/risk/owl#controls">
    <skos:definition xml:lang="en">Indicates this control manages specified risk concept event or action, such as for risk sources, risks, consequences, and impacts</skos:definition>
    <rdfs:isDefinedBy rdf:resource="https://w3id.org/dpv/risk/owl#"/>
    <dct:contributor rdf:nodeID="Ne22a67b17c7e4a779c30d2864b6a0cee"/>
    <rdf:type rdf:resource="http://www.w3.org/1999/02/22-rdf-syntax-ns#Property"/>
    <rdf:type rdf:resource="http://www.w3.org/2002/07/owl#ObjectProperty"/>
    <dcam:domainIncludes rdf:resource="https://w3id.org/dpv/risk/owl#RiskControl"/>
    <dct:created rdf:datatype="http://www.w3.org/2001/XMLSchema#date">2025-01-06</dct:created>
    <sw:term_status xml:lang="en">accepted</sw:term_status>
    <vann:example rdf:resource="https://w3id.org/dpv/examples/owl#E0086"/>
    <dcam:rangeIncludes rdf:resource="https://w3id.org/dpv/owl#RiskConcept"/>
    <skos:prefLabel xml:lang="en">control</skos:prefLabel>
    <schema:domainIncludes rdf:resource="https://w3id.org/dpv/risk/owl#RiskControl"/>
    <schema:rangeIncludes rdf:resource="https://w3id.org/dpv/owl#RiskConcept"/>
  </rdf:Description>
  <rdf:Description rdf:about="https://w3id.org/dpv/risk/owl#detects">
    <dct:contributor rdf:nodeID="Ne22a67b17c7e4a779c30d2864b6a0cee"/>
    <dct:contributor rdf:nodeID="N9c63c24625fe482386a350b4ea27b4f8"/>
    <skos:definition xml:lang="en">Indicates the specified event or action is detected by this control</skos:definition>
    <schema:domainIncludes rdf:resource="https://w3id.org/dpv/risk/owl#DetectionControl"/>
    <dct:created rdf:datatype="http://www.w3.org/2001/XMLSchema#date">2024-12-01</dct:created>
    <dcam:domainIncludes rdf:resource="https://w3id.org/dpv/risk/owl#DetectionControl"/>
    <rdfs:isDefinedBy rdf:resource="https://w3id.org/dpv/risk/owl#"/>
    <schema:rangeIncludes rdf:resource="https://w3id.org/dpv/owl#RiskConcept"/>
    <skos:prefLabel xml:lang="en">detects</skos:prefLabel>
    <dcam:rangeIncludes rdf:resource="https://w3id.org/dpv/owl#RiskConcept"/>
    <rdfs:subPropertyOf rdf:resource="https://w3id.org/dpv/risk/owl#monitors"/>
    <rdf:type rdf:resource="http://www.w3.org/1999/02/22-rdf-syntax-ns#Property"/>
    <rdf:type rdf:resource="http://www.w3.org/2002/07/owl#ObjectProperty"/>
    <sw:term_status xml:lang="en">modified</sw:term_status>
    <dct:modified rdf:datatype="http://www.w3.org/2001/XMLSchema#date">2025-01-06</dct:modified>
  </rdf:Description>
  <rdf:Description rdf:about="https://w3id.org/dpv/risk/owl#AvoidanceControl">
    <skos:prefLabel xml:lang="en">Avoidance Control</skos:prefLabel>
    <dct:contributor rdf:nodeID="Ne22a67b17c7e4a779c30d2864b6a0cee"/>
    <rdf:type rdf:resource="https://w3id.org/dpv/risk/owl#RiskControl"/>
    <rdf:type rdf:resource="http://www.w3.org/2000/01/rdf-schema#Class"/>
    <rdf:type rdf:resource="http://www.w3.org/2002/07/owl#Class"/>
    <sw:term_status xml:lang="en">accepted</sw:term_status>
    <rdfs:isDefinedBy rdf:resource="https://w3id.org/dpv/risk/owl#"/>
    <skos:definition xml:lang="en">Control that avoids an event with the goal of removing it completely</skos:definition>
    <skos:scopeNote xml:lang="en">Avoiding is distinct from Mitigation and Modification as the goal to avoid an event is to prevent it from occuring at all, whereas mitigation and modification accept an event will occur and focus on managing it</skos:scopeNote>
    <dct:created rdf:datatype="http://www.w3.org/2001/XMLSchema#date">2025-01-06</dct:created>
    <rdfs:subClassOf rdf:resource="https://w3id.org/dpv/risk/owl#ProactiveControl"/>
  </rdf:Description>
  <rdf:Description rdf:about="https://w3id.org/dpv/risk/owl#TransferControl">
    <dct:contributor rdf:nodeID="Ne22a67b17c7e4a779c30d2864b6a0cee"/>
    <rdf:type rdf:resource="https://w3id.org/dpv/risk/owl#RiskControl"/>
    <rdf:type rdf:resource="http://www.w3.org/2000/01/rdf-schema#Class"/>
    <rdf:type rdf:resource="http://www.w3.org/2002/07/owl#Class"/>
    <dct:created rdf:datatype="http://www.w3.org/2001/XMLSchema#date">2025-01-06</dct:created>
    <sw:term_status xml:lang="en">accepted</sw:term_status>
    <rdfs:isDefinedBy rdf:resource="https://w3id.org/dpv/risk/owl#"/>
    <skos:prefLabel xml:lang="en">Transfer Control</skos:prefLabel>
    <skos:scopeNote xml:lang="en">Transfer implies moving (physically or logically) the event to another context or entity. While Risk Management methods indicate risk transfer as occuring between entities, this concept is defined more broadly by including 'context or entity' so as to enable modelling cases where the transfer takes place between processes - which may be managed by the same or different entity. Additionally, typical use of 'Transfer' implies a formal mechanism such as an agreement, which is absent from this concept. If only partial responsibility is tranferred, such as for a specific measure, then this can be considered as an instance of sharing the risk - for which risk:ShareControl is provided</skos:scopeNote>
    <skos:definition xml:lang="en">Control that aims to transfer the event (or risk) to another context or entity</skos:definition>
    <rdfs:subClassOf rdf:resource="https://w3id.org/dpv/risk/owl#RiskControl"/>
  </rdf:Description>
  <rdf:Description rdf:about="https://w3id.org/dpv/risk/owl#RecoveryControl">
    <skos:scopeNote xml:lang="en">Recovery implies taking steps to correct the effects which may not be the same as the initial conditions before the event, whereas risk:ReversalControl refers to undoing the effects such that the initial condition is restored</skos:scopeNote>
    <dct:created rdf:datatype="http://www.w3.org/2001/XMLSchema#date">2024-05-19</dct:created>
    <rdf:type rdf:resource="http://www.w3.org/2000/01/rdf-schema#Class"/>
    <rdf:type rdf:resource="https://w3id.org/dpv/risk/owl#RiskControl"/>
    <rdf:type rdf:resource="http://www.w3.org/2002/07/owl#Class"/>
    <skos:prefLabel xml:lang="en">Recovery Control</skos:prefLabel>
    <sw:term_status xml:lang="en">modified</sw:term_status>
    <dct:modified rdf:datatype="http://www.w3.org/2001/XMLSchema#date">2025-01-06</dct:modified>
    <dct:contributor rdf:nodeID="N9c63c24625fe482386a350b4ea27b4f8"/>
    <dct:contributor rdf:nodeID="Ne22a67b17c7e4a779c30d2864b6a0cee"/>
    <rdfs:isDefinedBy rdf:resource="https://w3id.org/dpv/risk/owl#"/>
    <skos:definition xml:lang="en">Control that aims to restore the context following an event</skos:definition>
    <rdfs:subClassOf rdf:resource="https://w3id.org/dpv/risk/owl#ResolutionControl"/>
  </rdf:Description>
  <rdf:Description rdf:nodeID="N0c4f26726681494f8f9054328c810c07">
    <rdf:type rdf:resource="http://xmlns.com/foaf/0.1/Organization"/>
    <foaf:name>University College Dublin</foaf:name>
  </rdf:Description>
  <rdf:Description rdf:about="https://w3id.org/dpv/risk/owl#MonitorRiskControl">
    <skos:prefLabel xml:lang="en">Monitor Control</skos:prefLabel>
    <rdfs:isDefinedBy rdf:resource="https://w3id.org/dpv/risk/owl#"/>
    <rdf:type rdf:resource="https://w3id.org/dpv/risk/owl#RiskControl"/>
    <rdf:type rdf:resource="http://www.w3.org/2000/01/rdf-schema#Class"/>
    <rdf:type rdf:resource="http://www.w3.org/2002/07/owl#Class"/>
    <dct:contributor rdf:nodeID="Ne22a67b17c7e4a779c30d2864b6a0cee"/>
    <dct:modified rdf:datatype="http://www.w3.org/2001/XMLSchema#date">2025-01-06</dct:modified>
    <skos:definition xml:lang="en">Control that monitors another Control</skos:definition>
    <sw:term_status xml:lang="en">modified</sw:term_status>
    <dct:created rdf:datatype="http://www.w3.org/2001/XMLSchema#date">2024-05-19</dct:created>
    <rdfs:subClassOf rdf:resource="https://w3id.org/dpv/risk/owl#MonitorControl"/>
  </rdf:Description>
  <rdf:Description rdf:about="https://w3id.org/dpv/risk/owl#recovers">
    <skos:prefLabel xml:lang="en">recovers</skos:prefLabel>
    <sw:term_status xml:lang="en">accepted</sw:term_status>
    <rdfs:isDefinedBy rdf:resource="https://w3id.org/dpv/risk/owl#"/>
    <dcam:domainIncludes rdf:resource="https://w3id.org/dpv/risk/owl#RecoveryControl"/>
    <schema:rangeIncludes rdf:resource="https://w3id.org/dpv/owl#RiskConcept"/>
    <skos:definition xml:lang="en">Indicates the specified event or action is recovered from by this control</skos:definition>
    <rdf:type rdf:resource="http://www.w3.org/1999/02/22-rdf-syntax-ns#Property"/>
    <rdf:type rdf:resource="http://www.w3.org/2002/07/owl#ObjectProperty"/>
    <dct:contributor rdf:nodeID="Ne22a67b17c7e4a779c30d2864b6a0cee"/>
    <dct:created rdf:datatype="http://www.w3.org/2001/XMLSchema#date">2025-01-06</dct:created>
    <schema:domainIncludes rdf:resource="https://w3id.org/dpv/risk/owl#RecoveryControl"/>
    <dcam:rangeIncludes rdf:resource="https://w3id.org/dpv/owl#RiskConcept"/>
    <rdfs:subPropertyOf rdf:resource="https://w3id.org/dpv/risk/owl#resolves"/>
  </rdf:Description>
  <rdf:Description rdf:about="https://w3id.org/dpv/risk/owl#RiskControl">
    <skos:prefLabel xml:lang="en">Risk Control</skos:prefLabel>
    <sw:term_status xml:lang="en">accepted</sw:term_status>
    <rdf:type rdf:resource="http://www.w3.org/2000/01/rdf-schema#Class"/>
    <rdf:type rdf:resource="http://www.w3.org/2002/07/owl#Class"/>
    <vann:example rdf:resource="https://w3id.org/dpv/examples/owl#E0086"/>
    <vann:example rdf:resource="https://w3id.org/dpv/examples/owl#E0071"/>
    <dct:created rdf:datatype="http://www.w3.org/2001/XMLSchema#date">2024-05-19</dct:created>
    <skos:definition xml:lang="en">Control that modifies risk</skos:definition>
    <rdfs:subClassOf rdf:resource="https://w3id.org/dpv/owl#RiskMitigationMeasure"/>
    <dct:modified rdf:datatype="http://www.w3.org/2001/XMLSchema#date">2025-01-06</dct:modified>
    <rdfs:isDefinedBy rdf:resource="https://w3id.org/dpv/risk/owl#"/>
  </rdf:Description>
  <rdf:Description rdf:about="https://w3id.org/dpv/risk/owl#DetectionControl">
    <skos:prefLabel xml:lang="en">Detection Control</skos:prefLabel>
    <rdf:type rdf:resource="https://w3id.org/dpv/risk/owl#RiskControl"/>
    <rdf:type rdf:resource="http://www.w3.org/2000/01/rdf-schema#Class"/>
    <rdf:type rdf:resource="http://www.w3.org/2002/07/owl#Class"/>
    <sw:term_status xml:lang="en">modified</sw:term_status>
    <dct:modified rdf:datatype="http://www.w3.org/2001/XMLSchema#date">2025-01-06</dct:modified>
    <dct:contributor rdf:nodeID="N9c63c24625fe482386a350b4ea27b4f8"/>
    <dct:contributor rdf:nodeID="Ne22a67b17c7e4a779c30d2864b6a0cee"/>
    <skos:definition xml:lang="en">Control that detects an event</skos:definition>
    <rdfs:isDefinedBy rdf:resource="https://w3id.org/dpv/risk/owl#"/>
    <dct:created rdf:datatype="http://www.w3.org/2001/XMLSchema#date">2024-05-19</dct:created>
    <skos:scopeNote xml:lang="en">Detection refers to the observation, derivation, inference, or any other method for drawing conclusions that an event has occurred or is likely to occur with a given certainty. For controls that identify information about the event in terms of metrics or characteristics, see risk:IdentificationControl</skos:scopeNote>
    <rdfs:subClassOf rdf:resource="https://w3id.org/dpv/risk/owl#MonitorControl"/>
  </rdf:Description>
  <rdf:Description rdf:about="https://w3id.org/dpv/risk/owl#transfers">
    <dct:contributor rdf:nodeID="Ne22a67b17c7e4a779c30d2864b6a0cee"/>
    <sw:term_status xml:lang="en">accepted</sw:term_status>
    <rdfs:isDefinedBy rdf:resource="https://w3id.org/dpv/risk/owl#"/>
    <schema:rangeIncludes rdf:resource="https://w3id.org/dpv/owl#RiskConcept"/>
    <dcam:rangeIncludes rdf:resource="https://w3id.org/dpv/owl#RiskConcept"/>
    <rdfs:subPropertyOf rdf:resource="https://w3id.org/dpv/risk/owl#controls"/>
    <schema:domainIncludes rdf:resource="https://w3id.org/dpv/risk/owl#TransferControl"/>
    <rdf:type rdf:resource="http://www.w3.org/1999/02/22-rdf-syntax-ns#Property"/>
    <rdf:type rdf:resource="http://www.w3.org/2002/07/owl#ObjectProperty"/>
    <skos:prefLabel xml:lang="en">transfers</skos:prefLabel>
    <dct:created rdf:datatype="http://www.w3.org/2001/XMLSchema#date">2025-01-06</dct:created>
    <skos:definition xml:lang="en">Indicates the specified event or action is transfered to another context or entity by this control</skos:definition>
    <dcam:domainIncludes rdf:resource="https://w3id.org/dpv/risk/owl#TransferControl"/>
  </rdf:Description>
  <rdf:Description rdf:about="https://w3id.org/dpv/primer">
    <profile:hasArtifact rdf:resource="https://w3id.org/dpv/primer"/>
    <dct:conformsTo rdf:resource="https://www.w3.org/TR/html/"/>
    <rdf:type rdf:resource="http://www.w3.org/ns/dx/prof/ResourceDescriptor"/>
    <dct:format rdf:resource="https://www.iana.org/assignments/media-types/text/html"/>
    <profile:hasRole rdf:resource="http://www.w3.org/ns/dx/prof/role/guidance"/>
    <dct:title>Primer for Data Privacy Vocabulary</dct:title>
  </rdf:Description>
  <rdf:Description rdf:about="https://w3id.org/dpv/guides">
    <profile:hasArtifact rdf:resource="https://w3id.org/dpv/guides"/>
    <dct:title>Guides for Data Privacy Vocabulary</dct:title>
    <dct:conformsTo rdf:resource="https://www.w3.org/TR/html/"/>
    <rdf:type rdf:resource="http://www.w3.org/ns/dx/prof/ResourceDescriptor"/>
    <profile:hasRole rdf:resource="http://www.w3.org/ns/dx/prof/role/guidance"/>
    <dct:format rdf:resource="https://www.iana.org/assignments/media-types/text/html"/>
  </rdf:Description>
  <rdf:Description rdf:about="https://w3id.org/dpv/risk/owl#OversightControl">
    <skos:scopeNote xml:lang="en">Oversight can be ambigiously used in terms of having knowledge about an event (see risk:TransparencyControl instead), or being able to identify when it occurs (see risk:DetectionControl instead). The control defined by this concept includes the ability to act on the event as part of the 'oversight' term used in management</skos:scopeNote>
    <skos:definition xml:lang="en">Control that provides oversight for an event in terms of having information about it and being able to supervise or manage it</skos:definition>
    <rdf:type rdf:resource="https://w3id.org/dpv/risk/owl#RiskControl"/>
    <rdf:type rdf:resource="http://www.w3.org/2000/01/rdf-schema#Class"/>
    <rdf:type rdf:resource="http://www.w3.org/2002/07/owl#Class"/>
    <dct:contributor rdf:nodeID="Ne22a67b17c7e4a779c30d2864b6a0cee"/>
    <dct:created rdf:datatype="http://www.w3.org/2001/XMLSchema#date">2025-01-06</dct:created>
    <skos:prefLabel xml:lang="en">Oversight Control</skos:prefLabel>
    <sw:term_status xml:lang="en">accepted</sw:term_status>
    <rdfs:isDefinedBy rdf:resource="https://w3id.org/dpv/risk/owl#"/>
    <rdfs:subClassOf rdf:resource="https://w3id.org/dpv/risk/owl#MonitorControl"/>
  </rdf:Description>
  <rdf:Description rdf:about="https://w3id.org/dpv/risk/owl#monitors">
    <rdf:type rdf:resource="http://www.w3.org/1999/02/22-rdf-syntax-ns#Property"/>
    <rdf:type rdf:resource="http://www.w3.org/2002/07/owl#ObjectProperty"/>
    <sw:term_status xml:lang="en">accepted</sw:term_status>
    <schema:rangeIncludes rdf:resource="https://w3id.org/dpv/owl#RiskConcept"/>
    <dcam:domainIncludes rdf:resource="https://w3id.org/dpv/risk/owl#MonitorControl"/>
    <skos:definition xml:lang="en">Indicates the specified event or action is monitored by this control</skos:definition>
    <rdfs:subPropertyOf rdf:resource="https://w3id.org/dpv/risk/owl#controls"/>
    <schema:domainIncludes rdf:resource="https://w3id.org/dpv/risk/owl#MonitorControl"/>
    <rdfs:isDefinedBy rdf:resource="https://w3id.org/dpv/risk/owl#"/>
    <dct:contributor rdf:nodeID="Ne22a67b17c7e4a779c30d2864b6a0cee"/>
    <skos:prefLabel xml:lang="en">monitors</skos:prefLabel>
    <dct:created rdf:datatype="http://www.w3.org/2001/XMLSchema#date">2025-01-06</dct:created>
    <dcam:rangeIncludes rdf:resource="https://w3id.org/dpv/owl#RiskConcept"/>
  </rdf:Description>
  <rdf:Description rdf:about="https://w3id.org/dpv/risk/owl#ImpactControl">
    <dct:contributor rdf:nodeID="Ne22a67b17c7e4a779c30d2864b6a0cee"/>
    <skos:prefLabel xml:lang="en">Impact Control</skos:prefLabel>
    <rdf:type rdf:resource="https://w3id.org/dpv/risk/owl#RiskControl"/>
    <rdf:type rdf:resource="http://www.w3.org/2000/01/rdf-schema#Class"/>
    <rdf:type rdf:resource="http://www.w3.org/2002/07/owl#Class"/>
    <dct:modified rdf:datatype="http://www.w3.org/2001/XMLSchema#date">2025-01-06</dct:modified>
    <dct:created rdf:datatype="http://www.w3.org/2001/XMLSchema#date">2024-05-19</dct:created>
    <skos:definition xml:lang="en">Risk Mitigation Measure that controls Impacts</skos:definition>
    <rdfs:isDefinedBy rdf:resource="https://w3id.org/dpv/risk/owl#"/>
    <sw:term_status xml:lang="en">modified</sw:term_status>
    <rdfs:subClassOf rdf:resource="https://w3id.org/dpv/risk/owl#RiskControl"/>
  </rdf:Description>
  <rdf:Description rdf:about="https://w3id.org/dpv/risk/owl#investigates">
    <schema:rangeIncludes rdf:resource="https://w3id.org/dpv/owl#RiskConcept"/>
    <rdf:type rdf:resource="http://www.w3.org/1999/02/22-rdf-syntax-ns#Property"/>
    <rdf:type rdf:resource="http://www.w3.org/2002/07/owl#ObjectProperty"/>
    <dct:created rdf:datatype="http://www.w3.org/2001/XMLSchema#date">2025-01-06</dct:created>
    <sw:term_status xml:lang="en">accepted</sw:term_status>
    <skos:prefLabel xml:lang="en">investigates</skos:prefLabel>
    <rdfs:subPropertyOf rdf:resource="https://w3id.org/dpv/risk/owl#controls"/>
    <dct:contributor rdf:nodeID="Ne22a67b17c7e4a779c30d2864b6a0cee"/>
    <dcam:domainIncludes rdf:resource="https://w3id.org/dpv/risk/owl#InvestigationControl"/>
    <schema:domainIncludes rdf:resource="https://w3id.org/dpv/risk/owl#InvestigationControl"/>
    <dcam:rangeIncludes rdf:resource="https://w3id.org/dpv/owl#RiskConcept"/>
    <skos:definition xml:lang="en">Indicates the specified event or action is investigated by this control</skos:definition>
    <rdfs:isDefinedBy rdf:resource="https://w3id.org/dpv/risk/owl#"/>
  </rdf:Description>
  <rdf:Description rdf:about="https://w3id.org/dpv/risk/owl#HaltImpact">
    <rdf:type rdf:resource="https://w3id.org/dpv/risk/owl#RiskControl"/>
    <rdf:type rdf:resource="http://www.w3.org/2000/01/rdf-schema#Class"/>
    <rdf:type rdf:resource="http://www.w3.org/2002/07/owl#Class"/>
    <dct:contributor rdf:nodeID="Ne22a67b17c7e4a779c30d2864b6a0cee"/>
    <dct:created rdf:datatype="http://www.w3.org/2001/XMLSchema#date">2025-01-06</dct:created>
    <skos:definition xml:lang="en">Control that halts the (ongoing) impact event or process such that it no longer takes place or is applicable in the context</skos:definition>
    <sw:term_status xml:lang="en">accepted</sw:term_status>
    <rdfs:isDefinedBy rdf:resource="https://w3id.org/dpv/risk/owl#"/>
    <skos:prefLabel xml:lang="en">Halt Impact</skos:prefLabel>
    <rdfs:subClassOf rdf:resource="https://w3id.org/dpv/risk/owl#InterruptionControl"/>
    <rdfs:subClassOf rdf:resource="https://w3id.org/dpv/risk/owl#ImpactControl"/>
  </rdf:Description>
  <rdf:Description rdf:about="https://w3id.org/dpv/risk/owl#MonitorRisk">
    <dct:created rdf:datatype="http://www.w3.org/2001/XMLSchema#date">2024-05-19</dct:created>
    <rdf:type rdf:resource="http://www.w3.org/2000/01/rdf-schema#Class"/>
    <rdf:type rdf:resource="https://w3id.org/dpv/risk/owl#RiskControl"/>
    <rdf:type rdf:resource="http://www.w3.org/2002/07/owl#Class"/>
    <dct:modified rdf:datatype="http://www.w3.org/2001/XMLSchema#date">2025-01-06</dct:modified>
    <skos:definition xml:lang="en">Control that monitors a Risk</skos:definition>
    <rdfs:isDefinedBy rdf:resource="https://w3id.org/dpv/risk/owl#"/>
    <sw:term_status xml:lang="en">modified</sw:term_status>
    <skos:prefLabel xml:lang="en">Monitor Risk</skos:prefLabel>
    <dct:contributor rdf:nodeID="Ne22a67b17c7e4a779c30d2864b6a0cee"/>
    <rdfs:subClassOf rdf:resource="https://w3id.org/dpv/risk/owl#MonitorControl"/>
  </rdf:Description>
  <rdf:Description rdf:about="https://w3id.org/dpv/risk/owl#TransparencyControl">
    <dct:contributor rdf:nodeID="Ne22a67b17c7e4a779c30d2864b6a0cee"/>
    <dct:contributor rdf:nodeID="N9c63c24625fe482386a350b4ea27b4f8"/>
    <skos:prefLabel xml:lang="en">Transparency Control</skos:prefLabel>
    <rdf:type rdf:resource="https://w3id.org/dpv/risk/owl#RiskControl"/>
    <rdf:type rdf:resource="http://www.w3.org/2000/01/rdf-schema#Class"/>
    <rdf:type rdf:resource="http://www.w3.org/2002/07/owl#Class"/>
    <sw:term_status xml:lang="en">accepted</sw:term_status>
    <rdfs:isDefinedBy rdf:resource="https://w3id.org/dpv/risk/owl#"/>
    <skos:scopeNote xml:lang="en">Transparency refers to the availability of information, whether for the same or different entity in relation to who establishes and operates the control, and where transparency implies having the means to obtain and use information about an event</skos:scopeNote>
    <skos:definition xml:lang="en">Control that provides information about an event</skos:definition>
    <dct:created rdf:datatype="http://www.w3.org/2001/XMLSchema#date">2025-01-06</dct:created>
    <rdfs:subClassOf rdf:resource="https://w3id.org/dpv/risk/owl#MonitorControl"/>
  </rdf:Description>
  <rdf:Description rdf:about="https://w3id.org/dpv/risk/owl#modifies">
    <rdf:type rdf:resource="http://www.w3.org/1999/02/22-rdf-syntax-ns#Property"/>
    <rdf:type rdf:resource="http://www.w3.org/2002/07/owl#ObjectProperty"/>
    <dct:contributor rdf:nodeID="N9c63c24625fe482386a350b4ea27b4f8"/>
    <dct:contributor rdf:nodeID="Ne22a67b17c7e4a779c30d2864b6a0cee"/>
    <sw:term_status xml:lang="en">modified</sw:term_status>
    <dct:modified rdf:datatype="http://www.w3.org/2001/XMLSchema#date">2025-01-06</dct:modified>
    <dcam:rangeIncludes rdf:resource="https://w3id.org/dpv/owl#RiskConcept"/>
    <skos:prefLabel xml:lang="en">modifies</skos:prefLabel>
    <dct:created rdf:datatype="http://www.w3.org/2001/XMLSchema#date">2024-12-01</dct:created>
    <rdfs:isDefinedBy rdf:resource="https://w3id.org/dpv/risk/owl#"/>
    <rdfs:subPropertyOf rdf:resource="https://w3id.org/dpv/risk/owl#avoids"/>
    <schema:rangeIncludes rdf:resource="https://w3id.org/dpv/owl#RiskConcept"/>
    <schema:domainIncludes rdf:resource="https://w3id.org/dpv/risk/owl#ModificationControl"/>
    <dcam:domainIncludes rdf:resource="https://w3id.org/dpv/risk/owl#ModificationControl"/>
    <skos:definition xml:lang="en">Indicates the specified event or action is modified by this control</skos:definition>
  </rdf:Description>
  <rdf:Description rdf:about="https://w3id.org/dpv/risk/owl#">
    <owl:versionIRI rdf:resource="https://w3id.org/dpv/2.1/risk/owl#"/>
    <dct:title xml:lang="en">Risk Concepts</dct:title>
    <profile:hasResource rdf:resource="https://w3id.org/dpv/primer"/>
    <profile:hasResource rdf:resource="https://w3id.org/dpv/guides"/>
    <profile:hasResource rdf:resource="https://w3id.org/dpv/risk/owl#serialisation-n3"/>
    <profile:hasResource rdf:resource="https://w3id.org/dpv/risk/owl#serialisation-html"/>
    <profile:hasResource rdf:resource="https://w3id.org/dpv/risk/owl#serialisation-jsonld"/>
    <profile:hasResource rdf:resource="https://w3id.org/dpv/risk/owl#serialisation-ttl"/>
    <profile:hasResource rdf:resource="https://w3id.org/dpv/examples"/>
    <profile:hasResource rdf:resource="https://w3id.org/dpv/risk/owl#serialisation-rdf"/>
    <dct:bibliographicCitation>Harshvardhan J. Pandit, Beatriz Esteves, Georg P. Krog, Paul Ryan, Delaram Golpayegani, Julian Flake (2025) Data Privacy Vocabulary (DPV) – Version 2.0. In: Demartini, G., et al. The Semantic Web – ISWC 2024. ISWC 2024. Lecture Notes in Computer Science, vol 15233. Springer, Cham. https://doi.org/10.1007/978-3-031-77847-6_10</dct:bibliographicCitation>
    <bibo:status>http://purl.org/ontology/bibo/status/published</bibo:status>
    <rdfs:Label xml:lang="en">RISK</rdfs:Label>
    <dct:contributor rdf:nodeID="N9c63c24625fe482386a350b4ea27b4f8"/>
    <dct:contributor rdf:nodeID="Ne22a67b17c7e4a779c30d2864b6a0cee"/>
    <dct:conformsTo>http://www.w3.org/2004/02/skos/core</dct:conformsTo>
    <dct:conformsTo>http://www.w3.org/2000/01/rdf-schema</dct:conformsTo>
    <dct:conformsTo rdf:resource="http://www.w3.org/2002/07/owl"/>
    <dct:creator rdf:nodeID="N59852c09189e47bd989757f1615f7bdf"/>
    <dct:creator rdf:nodeID="N7d9b5ee7f31f4f2ba5951e30b49ec7c0"/>
    <dct:creator rdf:nodeID="Ne22a67b17c7e4a779c30d2864b6a0cee"/>
    <dct:creator rdf:nodeID="Ndedfd6f107a441f99c7268556c8aca81"/>
    <dct:creator rdf:nodeID="N9c63c24625fe482386a350b4ea27b4f8"/>
    <dct:creator rdf:nodeID="Ne84980f7db76425ca367742d2085d8c9"/>
    <dct:creator rdf:nodeID="N75641c194b3f4973ab2abfb33aed55d3"/>
    <dct:created xml:lang="en">2022-08-14</dct:created>
    <profile:isProfileOf rdf:resource="https://w3id.org/dpv/owl"/>
    <profile:isProfileOf rdf:resource="http://www.w3.org/2002/07/owl"/>
    <profile:isProfileOf rdf:resource="https://w3id.org/dpv/risk/owl#"/>
    <rdf:type rdf:resource="http://www.w3.org/2002/07/owl#Ontology"/>
    <rdf:type rdf:resource="http://www.w3.org/ns/dx/prof/Profile"/>
    <dct:identifier>https://w3id.org/dpv/risk</dct:identifier>
    <owl:versionInfo>2.1</owl:versionInfo>
    <dct:description xml:lang="en">Extension to the Data Privacy Vocabulary (DPV) providing concepts for representing information about risk assessment and risk management</dct:description>
    <bibo:doi>10.5281/zenodo.12505841</bibo:doi>
    <dct:license rdf:resource="https://www.w3.org/copyright/document-license-2023/"/>
    <schema:version>2.1</schema:version>
    <foaf:logo rdf:resource="https://w3id.org/dpv/media/logo.png"/>
    <dct:publisher rdf:resource="https://www.w3.org/"/>
    <dct:issued xml:lang="en">2022-08-14</dct:issued>
    <dct:modified xml:lang="en">2025-02-01</dct:modified>
    <dct:hasVersion rdf:resource="https://w3id.org/dpv/risk/owl#"/>
    <vann:preferredNamespacePrefix>risk</vann:preferredNamespacePrefix>
    <dct:source rdf:resource="https://www.w3.org/groups/cg/dpvcg/"/>
    <vann:preferredNamespaceUri>https://w3id.org/dpv/risk#</vann:preferredNamespaceUri>
  </rdf:Description>
  <rdf:Description rdf:about="https://w3id.org/dpv/risk/owl#MonitorVulnerabilities">
    <dct:contributor rdf:nodeID="Ne22a67b17c7e4a779c30d2864b6a0cee"/>
    <rdf:type rdf:resource="https://w3id.org/dpv/risk/owl#RiskControl"/>
    <rdf:type rdf:resource="http://www.w3.org/2000/01/rdf-schema#Class"/>
    <rdf:type rdf:resource="http://www.w3.org/2002/07/owl#Class"/>
    <rdfs:isDefinedBy rdf:resource="https://w3id.org/dpv/risk/owl#"/>
    <dct:created rdf:datatype="http://www.w3.org/2001/XMLSchema#date">2024-05-19</dct:created>
    <skos:prefLabel xml:lang="en">Monitor Vulnerabilities</skos:prefLabel>
    <sw:term_status xml:lang="en">modified</sw:term_status>
    <skos:definition xml:lang="en">Control that monitors a Risk Vulnerability</skos:definition>
    <dct:modified rdf:datatype="http://www.w3.org/2001/XMLSchema#date">2025-01-06</dct:modified>
    <rdfs:subClassOf rdf:resource="https://w3id.org/dpv/risk/owl#MonitorControl"/>
  </rdf:Description>
  <rdf:Description rdf:about="https://w3id.org/dpv/examples">
    <profile:hasRole rdf:resource="http://www.w3.org/ns/dx/prof/role/guidance"/>
    <profile:hasArtifact rdf:resource="https://w3id.org/dpv/examples"/>
    <dct:title>Examples for Data Privacy Vocabulary</dct:title>
    <rdf:type rdf:resource="http://www.w3.org/ns/dx/prof/ResourceDescriptor"/>
    <dct:format rdf:resource="https://www.iana.org/assignments/media-types/text/html"/>
    <dct:conformsTo rdf:resource="https://www.w3.org/TR/html/"/>
  </rdf:Description>
  <rdf:Description rdf:about="https://w3id.org/dpv/risk/owl#InterventionControl">
    <dct:created rdf:datatype="http://www.w3.org/2001/XMLSchema#date">2025-01-06</dct:created>
    <skos:definition xml:lang="en">Control that intervenes in the operations of the event to change some context with the aim of changing the event or the effects</skos:definition>
    <dct:contributor rdf:nodeID="Ne22a67b17c7e4a779c30d2864b6a0cee"/>
    <rdf:type rdf:resource="https://w3id.org/dpv/risk/owl#RiskControl"/>
    <rdf:type rdf:resource="http://www.w3.org/2000/01/rdf-schema#Class"/>
    <rdf:type rdf:resource="http://www.w3.org/2002/07/owl#Class"/>
    <skos:scopeNote xml:lang="en">Intervention implies taking steps to resolve the effects or to prevent further escalation while the event is still ongoing. For halting the event, see risk:InterruptionControl, for recovering and undoing the effects, see risk:RecoveryControl and risk:ReversalControl. Intervention is a temporary or stop-gap measure which is used while the event is ongoing to prevent it from escalating or creating additional issues</skos:scopeNote>
    <sw:term_status xml:lang="en">accepted</sw:term_status>
    <skos:prefLabel xml:lang="en">Intervention Control</skos:prefLabel>
    <rdfs:isDefinedBy rdf:resource="https://w3id.org/dpv/risk/owl#"/>
    <rdfs:subClassOf rdf:resource="https://w3id.org/dpv/risk/owl#ReductionControl"/>
  </rdf:Description>
  <rdf:Description rdf:about="https://w3id.org/dpv/risk/owl#intervenes">
    <dct:contributor rdf:nodeID="Ne22a67b17c7e4a779c30d2864b6a0cee"/>
    <skos:definition xml:lang="en">Indicates the specified event or action is intervened by this control</skos:definition>
    <dct:created rdf:datatype="http://www.w3.org/2001/XMLSchema#date">2025-01-06</dct:created>
    <sw:term_status xml:lang="en">accepted</sw:term_status>
    <rdfs:isDefinedBy rdf:resource="https://w3id.org/dpv/risk/owl#"/>
    <rdfs:subPropertyOf rdf:resource="https://w3id.org/dpv/risk/owl#reduces"/>
    <schema:rangeIncludes rdf:resource="https://w3id.org/dpv/owl#RiskConcept"/>
    <skos:prefLabel xml:lang="en">intervenes</skos:prefLabel>
    <dcam:rangeIncludes rdf:resource="https://w3id.org/dpv/owl#RiskConcept"/>
    <schema:domainIncludes rdf:resource="https://w3id.org/dpv/risk/owl#InterventionControl"/>
    <dcam:domainIncludes rdf:resource="https://w3id.org/dpv/risk/owl#InterventionControl"/>
    <rdf:type rdf:resource="http://www.w3.org/1999/02/22-rdf-syntax-ns#Property"/>
    <rdf:type rdf:resource="http://www.w3.org/2002/07/owl#ObjectProperty"/>
  </rdf:Description>
  <rdf:Description rdf:about="https://w3id.org/dpv/risk/owl#reverses">
    <sw:term_status xml:lang="en">accepted</sw:term_status>
    <rdfs:isDefinedBy rdf:resource="https://w3id.org/dpv/risk/owl#"/>
    <schema:rangeIncludes rdf:resource="https://w3id.org/dpv/owl#RiskConcept"/>
    <dcam:rangeIncludes rdf:resource="https://w3id.org/dpv/owl#RiskConcept"/>
    <dct:created rdf:datatype="http://www.w3.org/2001/XMLSchema#date">2025-01-06</dct:created>
    <rdfs:subPropertyOf rdf:resource="https://w3id.org/dpv/risk/owl#resolves"/>
    <rdf:type rdf:resource="http://www.w3.org/1999/02/22-rdf-syntax-ns#Property"/>
    <rdf:type rdf:resource="http://www.w3.org/2002/07/owl#ObjectProperty"/>
    <skos:prefLabel xml:lang="en">reverses</skos:prefLabel>
    <dcam:domainIncludes rdf:resource="https://w3id.org/dpv/risk/owl#ReversalControl"/>
    <schema:domainIncludes rdf:resource="https://w3id.org/dpv/risk/owl#ReversalControl"/>
    <skos:definition xml:lang="en">Indicates the specified event or action is reversed by this control</skos:definition>
    <dct:contributor rdf:nodeID="Ne22a67b17c7e4a779c30d2864b6a0cee"/>
  </rdf:Description>
  <rdf:Description rdf:about="https://w3id.org/dpv/risk/owl#ReduceSeverity">
    <rdf:type rdf:resource="http://www.w3.org/2000/01/rdf-schema#Class"/>
    <rdf:type rdf:resource="https://w3id.org/dpv/risk/owl#RiskControl"/>
    <rdf:type rdf:resource="http://www.w3.org/2002/07/owl#Class"/>
    <skos:definition xml:lang="en">Control that reduces the severity of an event's effects</skos:definition>
    <dct:modified rdf:datatype="http://www.w3.org/2001/XMLSchema#date">2025-01-06</dct:modified>
    <dct:created rdf:datatype="http://www.w3.org/2001/XMLSchema#date">2024-05-19</dct:created>
    <skos:prefLabel xml:lang="en">Reduce Severity</skos:prefLabel>
    <rdfs:isDefinedBy rdf:resource="https://w3id.org/dpv/risk/owl#"/>
    <dct:contributor rdf:nodeID="Ne22a67b17c7e4a779c30d2864b6a0cee"/>
    <sw:term_status xml:lang="en">modified</sw:term_status>
    <rdfs:subClassOf rdf:resource="https://w3id.org/dpv/risk/owl#ReductionControl"/>
  </rdf:Description>
  <rdf:Description rdf:about="https://w3id.org/dpv/risk/owl#MonitorImpact">
    <skos:prefLabel xml:lang="en">Monitor Impact</skos:prefLabel>
    <dct:modified rdf:datatype="http://www.w3.org/2001/XMLSchema#date">2025-01-06</dct:modified>
    <dct:created rdf:datatype="http://www.w3.org/2001/XMLSchema#date">2024-05-19</dct:created>
    <rdf:type rdf:resource="https://w3id.org/dpv/risk/owl#RiskControl"/>
    <rdf:type rdf:resource="http://www.w3.org/2000/01/rdf-schema#Class"/>
    <rdf:type rdf:resource="http://www.w3.org/2002/07/owl#Class"/>
    <rdfs:isDefinedBy rdf:resource="https://w3id.org/dpv/risk/owl#"/>
    <sw:term_status xml:lang="en">modified</sw:term_status>
    <skos:definition xml:lang="en">Control that monitors a Risk Impact</skos:definition>
    <dct:contributor rdf:nodeID="Ne22a67b17c7e4a779c30d2864b6a0cee"/>
    <rdfs:subClassOf rdf:resource="https://w3id.org/dpv/risk/owl#MonitorControl"/>
  </rdf:Description>
  <rdf:Description rdf:about="https://w3id.org/dpv/risk/owl#AvoidConsequence">
    <rdf:type rdf:resource="http://www.w3.org/2000/01/rdf-schema#Class"/>
    <rdf:type rdf:resource="https://w3id.org/dpv/risk/owl#RiskControl"/>
    <rdf:type rdf:resource="http://www.w3.org/2002/07/owl#Class"/>
    <skos:definition xml:lang="en">Control that proactively avoids the consequence such that it has a reduced exposure or applicability in the context</skos:definition>
    <sw:term_status xml:lang="en">accepted</sw:term_status>
    <skos:prefLabel xml:lang="en">Avoid Consequence</skos:prefLabel>
    <rdfs:isDefinedBy rdf:resource="https://w3id.org/dpv/risk/owl#"/>
    <dct:contributor rdf:nodeID="Ne22a67b17c7e4a779c30d2864b6a0cee"/>
    <dct:created rdf:datatype="http://www.w3.org/2001/XMLSchema#date">2025-01-06</dct:created>
    <rdfs:subClassOf rdf:resource="https://w3id.org/dpv/risk/owl#ConsequenceControl"/>
    <rdfs:subClassOf rdf:resource="https://w3id.org/dpv/risk/owl#AvoidanceControl"/>
  </rdf:Description>
  <rdf:Description rdf:about="https://w3id.org/dpv/risk/owl#InterruptionControl">
    <rdf:type rdf:resource="https://w3id.org/dpv/risk/owl#RiskControl"/>
    <rdf:type rdf:resource="http://www.w3.org/2000/01/rdf-schema#Class"/>
    <rdf:type rdf:resource="http://www.w3.org/2002/07/owl#Class"/>
    <skos:prefLabel xml:lang="en">Interruption Control</skos:prefLabel>
    <rdfs:isDefinedBy rdf:resource="https://w3id.org/dpv/risk/owl#"/>
    <skos:scopeNote xml:lang="en">Interruption refers to the event being temporarily halted, such as an emergency measure while further suitable measures are identified and put in place. To indicate stopping the event completely rather than a temporary interruption, see risk:RemediationControl which fixes the underlying issue and risk:EliminationEvent which prevents the event from occuring</skos:scopeNote>
    <dct:created rdf:datatype="http://www.w3.org/2001/XMLSchema#date">2025-01-06</dct:created>
    <dct:contributor rdf:nodeID="N9c63c24625fe482386a350b4ea27b4f8"/>
    <dct:contributor rdf:nodeID="Ne22a67b17c7e4a779c30d2864b6a0cee"/>
    <skos:definition xml:lang="en">Control that interrupts an event without removing the possibility for it to be resumed and where the aim is to stop the event</skos:definition>
    <sw:term_status xml:lang="en">accepted</sw:term_status>
    <rdfs:subClassOf rdf:resource="https://w3id.org/dpv/risk/owl#ReductionControl"/>
  </rdf:Description>
  <rdf:Description rdf:about="https://w3id.org/dpv/risk/owl#ChangeConsequence">
    <rdf:type rdf:resource="https://w3id.org/dpv/risk/owl#RiskControl"/>
    <rdf:type rdf:resource="http://www.w3.org/2000/01/rdf-schema#Class"/>
    <rdf:type rdf:resource="http://www.w3.org/2002/07/owl#Class"/>
    <dct:modified rdf:datatype="http://www.w3.org/2001/XMLSchema#date">2025-01-06</dct:modified>
    <sw:term_status xml:lang="en">modified</sw:term_status>
    <skos:definition xml:lang="en">Control that proactively changes the consequence event such that one event is replaced with the occurence or applicability of another event in the context</skos:definition>
    <rdfs:isDefinedBy rdf:resource="https://w3id.org/dpv/risk/owl#"/>
    <dct:contributor rdf:nodeID="Ne22a67b17c7e4a779c30d2864b6a0cee"/>
    <skos:prefLabel xml:lang="en">Change Consequence</skos:prefLabel>
    <dct:created rdf:datatype="http://www.w3.org/2001/XMLSchema#date">2024-05-19</dct:created>
    <rdfs:subClassOf rdf:resource="https://w3id.org/dpv/risk/owl#SubstitutionControl"/>
    <rdfs:subClassOf rdf:resource="https://w3id.org/dpv/risk/owl#ConsequenceControl"/>
  </rdf:Description>
  <rdf:Description rdf:about="https://w3id.org/dpv/risk/owl#remedies">
    <dct:created rdf:datatype="http://www.w3.org/2001/XMLSchema#date">2025-01-06</dct:created>
    <skos:definition xml:lang="en">Indicates the specified event or action is remedied by this control</skos:definition>
    <rdfs:subPropertyOf rdf:resource="https://w3id.org/dpv/risk/owl#resolves"/>
    <dct:contributor rdf:nodeID="Ne22a67b17c7e4a779c30d2864b6a0cee"/>
    <rdf:type rdf:resource="http://www.w3.org/1999/02/22-rdf-syntax-ns#Property"/>
    <rdf:type rdf:resource="http://www.w3.org/2002/07/owl#ObjectProperty"/>
    <skos:prefLabel xml:lang="en">remedies</skos:prefLabel>
    <sw:term_status xml:lang="en">accepted</sw:term_status>
    <schema:rangeIncludes rdf:resource="https://w3id.org/dpv/owl#RiskConcept"/>
    <dcam:rangeIncludes rdf:resource="https://w3id.org/dpv/owl#RiskConcept"/>
    <schema:domainIncludes rdf:resource="https://w3id.org/dpv/risk/owl#RemediationControl"/>
    <dcam:domainIncludes rdf:resource="https://w3id.org/dpv/risk/owl#RemediationControl"/>
    <rdfs:isDefinedBy rdf:resource="https://w3id.org/dpv/risk/owl#"/>
  </rdf:Description>
  <rdf:Description rdf:about="https://w3id.org/dpv/risk/owl#MitigationControl">
    <sw:term_status xml:lang="en">accepted</sw:term_status>
    <rdfs:isDefinedBy rdf:resource="https://w3id.org/dpv/risk/owl#"/>
    <dct:created rdf:datatype="http://www.w3.org/2001/XMLSchema#date">2025-01-06</dct:created>
    <rdf:type rdf:resource="http://www.w3.org/2000/01/rdf-schema#Class"/>
    <rdf:type rdf:resource="https://w3id.org/dpv/risk/owl#RiskControl"/>
    <rdf:type rdf:resource="http://www.w3.org/2002/07/owl#Class"/>
    <skos:definition xml:lang="en">Control that aims to reduce the likelihood or effect of an event with the goal of managing an event accepted to occur</skos:definition>
    <skos:prefLabel xml:lang="en">Mitigation Control</skos:prefLabel>
    <dct:contributor rdf:nodeID="N9c63c24625fe482386a350b4ea27b4f8"/>
    <dct:contributor rdf:nodeID="Ne22a67b17c7e4a779c30d2864b6a0cee"/>
    <skos:scopeNote xml:lang="en">Mitigation requires accepting that an event will occur, and thereby focusing on managing it by reducing its likelihood or effects by adding additional processes to specifically address the event or its effects</skos:scopeNote>
    <rdfs:subClassOf rdf:resource="https://w3id.org/dpv/risk/owl#ProactiveControl"/>
  </rdf:Description>
  <rdf:Description rdf:about="https://w3id.org/dpv/risk/owl#ReactiveControl">
    <dct:created rdf:datatype="http://www.w3.org/2001/XMLSchema#date">2025-01-06</dct:created>
    <skos:prefLabel xml:lang="en">Reactive Control</skos:prefLabel>
    <skos:scopeNote xml:lang="en">The use of 'reactive' here refers to this control being established i.e. becoming active to address the effects of an event after they occur. It does not imply that the controls are put in place after the event or that there is no planned procedure for handling an incident</skos:scopeNote>
    <dct:contributor rdf:nodeID="Ne22a67b17c7e4a779c30d2864b6a0cee"/>
    <rdf:type rdf:resource="https://w3id.org/dpv/risk/owl#RiskControl"/>
    <rdf:type rdf:resource="http://www.w3.org/2000/01/rdf-schema#Class"/>
    <rdf:type rdf:resource="http://www.w3.org/2002/07/owl#Class"/>
    <sw:term_status xml:lang="en">accepted</sw:term_status>
    <rdfs:isDefinedBy rdf:resource="https://w3id.org/dpv/risk/owl#"/>
    <skos:definition xml:lang="en">Control that is established or functions after an event occurs</skos:definition>
    <rdfs:subClassOf rdf:resource="https://w3id.org/dpv/risk/owl#RiskControl"/>
  </rdf:Description>
  <rdf:Description rdf:about="https://w3id.org/dpv/risk/owl#eliminates">
    <dcam:domainIncludes rdf:resource="https://w3id.org/dpv/risk/owl#EliminationControl"/>
    <dct:created rdf:datatype="http://www.w3.org/2001/XMLSchema#date">2024-12-01</dct:created>
    <rdfs:isDefinedBy rdf:resource="https://w3id.org/dpv/risk/owl#"/>
    <rdfs:subPropertyOf rdf:resource="https://w3id.org/dpv/risk/owl#avoids"/>
    <schema:rangeIncludes rdf:resource="https://w3id.org/dpv/owl#RiskConcept"/>
    <dcam:rangeIncludes rdf:resource="https://w3id.org/dpv/owl#RiskConcept"/>
    <skos:definition xml:lang="en">Indicates the specified event or action is eliminated by this control</skos:definition>
    <rdf:type rdf:resource="http://www.w3.org/1999/02/22-rdf-syntax-ns#Property"/>
    <rdf:type rdf:resource="http://www.w3.org/2002/07/owl#ObjectProperty"/>
    <sw:term_status xml:lang="en">modified</sw:term_status>
    <skos:prefLabel xml:lang="en">eliminates</skos:prefLabel>
    <dct:modified rdf:datatype="http://www.w3.org/2001/XMLSchema#date">2025-01-06</dct:modified>
    <dct:contributor rdf:nodeID="N9c63c24625fe482386a350b4ea27b4f8"/>
    <dct:contributor rdf:nodeID="Ne22a67b17c7e4a779c30d2864b6a0cee"/>
    <schema:domainIncludes rdf:resource="https://w3id.org/dpv/risk/owl#EliminationControl"/>
  </rdf:Description>
  <rdf:Description rdf:about="https://w3id.org/dpv/risk/owl#ReduceLikelihood">
    <rdf:type rdf:resource="https://w3id.org/dpv/risk/owl#RiskControl"/>
    <rdf:type rdf:resource="http://www.w3.org/2000/01/rdf-schema#Class"/>
    <rdf:type rdf:resource="http://www.w3.org/2002/07/owl#Class"/>
    <sw:term_status xml:lang="en">modified</sw:term_status>
    <skos:definition xml:lang="en">Control that reduces the likelihood of an event to occur</skos:definition>
    <dct:modified rdf:datatype="http://www.w3.org/2001/XMLSchema#date">2025-01-06</dct:modified>
    <dct:created rdf:datatype="http://www.w3.org/2001/XMLSchema#date">2024-05-19</dct:created>
    <dct:contributor rdf:nodeID="Ne22a67b17c7e4a779c30d2864b6a0cee"/>
    <rdfs:isDefinedBy rdf:resource="https://w3id.org/dpv/risk/owl#"/>
    <skos:prefLabel xml:lang="en">Reduce Likelihood</skos:prefLabel>
    <rdfs:subClassOf rdf:resource="https://w3id.org/dpv/risk/owl#ReductionControl"/>
  </rdf:Description>
  <rdf:Description rdf:about="https://w3id.org/dpv/risk/owl#ShareRisk">
    <rdf:type rdf:resource="https://w3id.org/dpv/risk/owl#RiskControl"/>
    <rdf:type rdf:resource="http://www.w3.org/2000/01/rdf-schema#Class"/>
    <rdf:type rdf:resource="http://www.w3.org/2002/07/owl#Class"/>
    <rdfs:isDefinedBy rdf:resource="https://w3id.org/dpv/risk/owl#"/>
    <sw:term_status xml:lang="en">modified</sw:term_status>
    <skos:definition xml:lang="en">Risk Mitigation Measure that shares Risk e.g. amongst stakeholders</skos:definition>
    <skos:prefLabel xml:lang="en">Share Risk</skos:prefLabel>
    <dct:contributor rdf:nodeID="Ne22a67b17c7e4a779c30d2864b6a0cee"/>
    <dct:modified rdf:datatype="http://www.w3.org/2001/XMLSchema#date">2025-01-06</dct:modified>
    <dct:created rdf:datatype="http://www.w3.org/2001/XMLSchema#date">2024-05-19</dct:created>
    <rdfs:subClassOf rdf:resource="https://w3id.org/dpv/risk/owl#ShareControl"/>
  </rdf:Description>
  <rdf:Description rdf:about="https://w3id.org/dpv/risk/owl#contains">
    <sw:term_status xml:lang="en">accepted</sw:term_status>
    <rdfs:isDefinedBy rdf:resource="https://w3id.org/dpv/risk/owl#"/>
    <schema:rangeIncludes rdf:resource="https://w3id.org/dpv/owl#RiskConcept"/>
    <dcam:rangeIncludes rdf:resource="https://w3id.org/dpv/owl#RiskConcept"/>
    <dcam:domainIncludes rdf:resource="https://w3id.org/dpv/risk/owl#ContainmentControl"/>
    <rdfs:subPropertyOf rdf:resource="https://w3id.org/dpv/risk/owl#controls"/>
    <rdf:type rdf:resource="http://www.w3.org/1999/02/22-rdf-syntax-ns#Property"/>
    <rdf:type rdf:resource="http://www.w3.org/2002/07/owl#ObjectProperty"/>
    <skos:prefLabel xml:lang="en">contains</skos:prefLabel>
    <dct:contributor rdf:nodeID="Ne22a67b17c7e4a779c30d2864b6a0cee"/>
    <dct:created rdf:datatype="http://www.w3.org/2001/XMLSchema#date">2025-01-06</dct:created>
    <schema:domainIncludes rdf:resource="https://w3id.org/dpv/risk/owl#ContainmentControl"/>
    <skos:definition xml:lang="en">Indicates the specified event or action is contained by this control</skos:definition>
  </rdf:Description>
  <rdf:Description rdf:about="https://w3id.org/dpv/risk/owl#EliminationControl">
    <dct:contributor rdf:nodeID="N9c63c24625fe482386a350b4ea27b4f8"/>
    <dct:contributor rdf:nodeID="Ne22a67b17c7e4a779c30d2864b6a0cee"/>
    <skos:definition xml:lang="en">Control that eliminates an event entirely such that the event does not occur</skos:definition>
    <dct:created rdf:datatype="http://www.w3.org/2001/XMLSchema#date">2025-01-06</dct:created>
    <rdf:type rdf:resource="http://www.w3.org/2000/01/rdf-schema#Class"/>
    <rdf:type rdf:resource="https://w3id.org/dpv/risk/owl#RiskControl"/>
    <rdf:type rdf:resource="http://www.w3.org/2002/07/owl#Class"/>
    <sw:term_status xml:lang="en">accepted</sw:term_status>
    <skos:scopeNote xml:lang="en">Elimination requires the event's likelihood to be reduced to zero such that the event cannot occur in the context. This can be done by establishing methods to prevent the event from occuring (e.g. gatekeeping filters) or by changing the underlying context context (e.g. replacing faulty device). The difference between risk:ModificationControl and risk:EliminationControl is that modification works to change the event characteristics whereas elimination works on the context to prevent the event</skos:scopeNote>
    <skos:prefLabel xml:lang="en">Elimination Control</skos:prefLabel>
    <rdfs:isDefinedBy rdf:resource="https://w3id.org/dpv/risk/owl#"/>
    <rdfs:subClassOf rdf:resource="https://w3id.org/dpv/risk/owl#AvoidanceControl"/>
  </rdf:Description>
  <rdf:Description rdf:about="https://w3id.org/dpv/risk/owl#RemoveImpact">
    <rdfs:isDefinedBy rdf:resource="https://w3id.org/dpv/risk/owl#"/>
    <rdf:type rdf:resource="http://www.w3.org/2000/01/rdf-schema#Class"/>
    <rdf:type rdf:resource="https://w3id.org/dpv/risk/owl#RiskControl"/>
    <rdf:type rdf:resource="http://www.w3.org/2002/07/owl#Class"/>
    <skos:definition xml:lang="en">Control that proactively removes the impact event such that the event does not occur in the context</skos:definition>
    <dct:contributor rdf:nodeID="Ne22a67b17c7e4a779c30d2864b6a0cee"/>
    <sw:term_status xml:lang="en">modified</sw:term_status>
    <dct:modified rdf:datatype="http://www.w3.org/2001/XMLSchema#date">2025-01-06</dct:modified>
    <skos:prefLabel xml:lang="en">Remove Impact</skos:prefLabel>
    <dct:created rdf:datatype="http://www.w3.org/2001/XMLSchema#date">2024-05-19</dct:created>
    <rdfs:subClassOf rdf:resource="https://w3id.org/dpv/risk/owl#ImpactControl"/>
    <rdfs:subClassOf rdf:resource="https://w3id.org/dpv/risk/owl#EliminationControl"/>
  </rdf:Description>
  <rdf:Description rdf:about="https://w3id.org/dpv/risk/owl#interrupts">
    <schema:domainIncludes rdf:resource="https://w3id.org/dpv/risk/owl#InterruptionControl"/>
    <skos:prefLabel xml:lang="en">interrupts</skos:prefLabel>
    <dct:contributor rdf:nodeID="Ne22a67b17c7e4a779c30d2864b6a0cee"/>
    <dcam:domainIncludes rdf:resource="https://w3id.org/dpv/risk/owl#InterruptionControl"/>
    <dct:created rdf:datatype="http://www.w3.org/2001/XMLSchema#date">2025-01-06</dct:created>
    <sw:term_status xml:lang="en">accepted</sw:term_status>
    <rdfs:isDefinedBy rdf:resource="https://w3id.org/dpv/risk/owl#"/>
    <rdfs:subPropertyOf rdf:resource="https://w3id.org/dpv/risk/owl#reduces"/>
    <dcam:rangeIncludes rdf:resource="https://w3id.org/dpv/owl#RiskConcept"/>
    <skos:definition xml:lang="en">Indicates the specified event or action is interrupted by this control</skos:definition>
    <rdf:type rdf:resource="http://www.w3.org/1999/02/22-rdf-syntax-ns#Property"/>
    <rdf:type rdf:resource="http://www.w3.org/2002/07/owl#ObjectProperty"/>
    <schema:rangeIncludes rdf:resource="https://w3id.org/dpv/owl#RiskConcept"/>
  </rdf:Description>
  <rdf:Description rdf:about="https://w3id.org/dpv/risk/owl#ShareControl">
    <rdfs:isDefinedBy rdf:resource="https://w3id.org/dpv/risk/owl#"/>
    <skos:prefLabel xml:lang="en">Share Control</skos:prefLabel>
    <dct:created rdf:datatype="http://www.w3.org/2001/XMLSchema#date">2025-01-06</dct:created>
    <skos:scopeNote xml:lang="en">Sharing implies a combined responsibility or sharing of effects from an event - which can be between entities or procesess (or other contexts). The use of 'event' here broadly refers to any event, which may be a risk event or could also be specific measures being adopted in response to an event. For specifically indicating sharing of risk per typical risk management processes, see risk:ShareRisk</skos:scopeNote>
    <rdf:type rdf:resource="http://www.w3.org/2000/01/rdf-schema#Class"/>
    <rdf:type rdf:resource="https://w3id.org/dpv/risk/owl#RiskControl"/>
    <rdf:type rdf:resource="http://www.w3.org/2002/07/owl#Class"/>
    <dct:contributor rdf:nodeID="Ne22a67b17c7e4a779c30d2864b6a0cee"/>
    <skos:definition xml:lang="en">Control that aims to share or distribute the event (or risk) with another context or entity</skos:definition>
    <sw:term_status xml:lang="en">accepted</sw:term_status>
    <rdfs:subClassOf rdf:resource="https://w3id.org/dpv/risk/owl#TransferControl"/>
  </rdf:Description>
  <rdf:Description rdf:about="https://w3id.org/dpv/risk/owl#RemoveSource">
    <skos:definition xml:lang="en">Control that proactively removes the risk source such that it is no longer present or applicable in the context</skos:definition>
    <rdf:type rdf:resource="https://w3id.org/dpv/risk/owl#RiskControl"/>
    <rdf:type rdf:resource="http://www.w3.org/2000/01/rdf-schema#Class"/>
    <rdf:type rdf:resource="http://www.w3.org/2002/07/owl#Class"/>
    <dct:modified rdf:datatype="http://www.w3.org/2001/XMLSchema#date">2025-01-06</dct:modified>
    <sw:term_status xml:lang="en">modified</sw:term_status>
    <dct:created rdf:datatype="http://www.w3.org/2001/XMLSchema#date">2024-05-19</dct:created>
    <skos:prefLabel xml:lang="en">Remove Source</skos:prefLabel>
    <rdfs:isDefinedBy rdf:resource="https://w3id.org/dpv/risk/owl#"/>
    <dct:contributor rdf:nodeID="Ne22a67b17c7e4a779c30d2864b6a0cee"/>
    <rdfs:subClassOf rdf:resource="https://w3id.org/dpv/risk/owl#EliminationControl"/>
    <rdfs:subClassOf rdf:resource="https://w3id.org/dpv/risk/owl#SourceControl"/>
  </rdf:Description>
  <rdf:Description rdf:about="https://w3id.org/dpv/risk/owl#reduces">
    <rdfs:isDefinedBy rdf:resource="https://w3id.org/dpv/risk/owl#"/>
    <skos:prefLabel xml:lang="en">reduces</skos:prefLabel>
    <dct:contributor rdf:nodeID="Ne22a67b17c7e4a779c30d2864b6a0cee"/>
    <dct:created rdf:datatype="http://www.w3.org/2001/XMLSchema#date">2025-01-06</dct:created>
    <skos:definition xml:lang="en">Indicates the specified event or action is reduced by this control</skos:definition>
    <dcam:rangeIncludes rdf:resource="https://w3id.org/dpv/owl#RiskConcept"/>
    <rdf:type rdf:resource="http://www.w3.org/1999/02/22-rdf-syntax-ns#Property"/>
    <rdf:type rdf:resource="http://www.w3.org/2002/07/owl#ObjectProperty"/>
    <sw:term_status xml:lang="en">accepted</sw:term_status>
    <dcam:domainIncludes rdf:resource="https://w3id.org/dpv/risk/owl#ReductionControl"/>
    <schema:rangeIncludes rdf:resource="https://w3id.org/dpv/owl#RiskConcept"/>
    <schema:domainIncludes rdf:resource="https://w3id.org/dpv/risk/owl#ReductionControl"/>
    <rdfs:subPropertyOf rdf:resource="https://w3id.org/dpv/risk/owl#controls"/>
  </rdf:Description>
  <rdf:Description rdf:about="https://w3id.org/dpv/risk/owl#MonitorControl">
    <skos:definition xml:lang="en">Control that monitors for the occurence of an event</skos:definition>
    <dct:created rdf:datatype="http://www.w3.org/2001/XMLSchema#date">2024-05-19</dct:created>
    <rdf:type rdf:resource="http://www.w3.org/2000/01/rdf-schema#Class"/>
    <rdf:type rdf:resource="https://w3id.org/dpv/risk/owl#RiskControl"/>
    <rdf:type rdf:resource="http://www.w3.org/2002/07/owl#Class"/>
    <dct:contributor rdf:nodeID="Ne22a67b17c7e4a779c30d2864b6a0cee"/>
    <sw:term_status xml:lang="en">modified</sw:term_status>
    <skos:prefLabel xml:lang="en">Monitor Control</skos:prefLabel>
    <skos:scopeNote xml:lang="en">Monitoring is a broad term that refers to identifying information about an event, including its occurence, characteristics such as severity or specific contextual metrics, affected things and entities, and having the ability to obtain and use this information to address the event. Monitoring is also used to refer to the activities associated with ensuring controls are active and effective. For this reason, specific concepts are defined which extend this control to express explicit actions included in the general use of 'monitoring' in risk management</skos:scopeNote>
    <dct:modified rdf:datatype="http://www.w3.org/2001/XMLSchema#date">2025-01-06</dct:modified>
    <rdfs:isDefinedBy rdf:resource="https://w3id.org/dpv/risk/owl#"/>
    <rdfs:subClassOf rdf:resource="https://w3id.org/dpv/risk/owl#ProactiveControl"/>
  </rdf:Description>
  <rdf:Description rdf:about="https://w3id.org/dpv/risk/owl#ReductionControl">
    <skos:prefLabel xml:lang="en">Reduction Control</skos:prefLabel>
    <rdf:type rdf:resource="https://w3id.org/dpv/risk/owl#RiskControl"/>
    <rdf:type rdf:resource="http://www.w3.org/2000/01/rdf-schema#Class"/>
    <rdf:type rdf:resource="http://www.w3.org/2002/07/owl#Class"/>
    <sw:term_status xml:lang="en">modified</sw:term_status>
    <dct:modified rdf:datatype="http://www.w3.org/2001/XMLSchema#date">2025-01-06</dct:modified>
    <rdfs:isDefinedBy rdf:resource="https://w3id.org/dpv/risk/owl#"/>
    <skos:definition xml:lang="en">Control that reduces the effects of an event</skos:definition>
    <dct:created rdf:datatype="http://www.w3.org/2001/XMLSchema#date">2024-05-19</dct:created>
    <skos:scopeNote xml:lang="en">Reduction here refers to a lessening of the effects after the event has occured by either reducing their likelihood or their severity in the context. This can involve changing the underlying context such that the effects have a reduced chance of occuring, or to create additional measures such that the effects do not have the initial severity for an entity</skos:scopeNote>
    <rdfs:subClassOf rdf:resource="https://w3id.org/dpv/risk/owl#ReactiveControl"/>
  </rdf:Description>
  <rdf:Description rdf:about="https://w3id.org/dpv/risk/owl#RemoveConsequence">
    <rdfs:isDefinedBy rdf:resource="https://w3id.org/dpv/risk/owl#"/>
    <skos:definition xml:lang="en">Control that proactively removes the consequence event such that the event does not occur in the context</skos:definition>
    <dct:created rdf:datatype="http://www.w3.org/2001/XMLSchema#date">2024-05-19</dct:created>
    <rdf:type rdf:resource="http://www.w3.org/2000/01/rdf-schema#Class"/>
    <rdf:type rdf:resource="https://w3id.org/dpv/risk/owl#RiskControl"/>
    <rdf:type rdf:resource="http://www.w3.org/2002/07/owl#Class"/>
    <skos:prefLabel xml:lang="en">Remove Consequence</skos:prefLabel>
    <sw:term_status xml:lang="en">modified</sw:term_status>
    <dct:contributor rdf:nodeID="Ne22a67b17c7e4a779c30d2864b6a0cee"/>
    <dct:modified rdf:datatype="http://www.w3.org/2001/XMLSchema#date">2025-01-06</dct:modified>
    <rdfs:subClassOf rdf:resource="https://w3id.org/dpv/risk/owl#ConsequenceControl"/>
    <rdfs:subClassOf rdf:resource="https://w3id.org/dpv/risk/owl#EliminationControl"/>
  </rdf:Description>
  <rdf:Description rdf:about="https://w3id.org/dpv/risk/owl#logs">
    <dcam:domainIncludes rdf:resource="https://w3id.org/dpv/risk/owl#LoggingControl"/>
    <dct:created rdf:datatype="http://www.w3.org/2001/XMLSchema#date">2025-01-06</dct:created>
    <rdfs:isDefinedBy rdf:resource="https://w3id.org/dpv/risk/owl#"/>
    <dct:contributor rdf:nodeID="Ne22a67b17c7e4a779c30d2864b6a0cee"/>
    <rdf:type rdf:resource="http://www.w3.org/1999/02/22-rdf-syntax-ns#Property"/>
    <rdf:type rdf:resource="http://www.w3.org/2002/07/owl#ObjectProperty"/>
    <skos:prefLabel xml:lang="en">logs</skos:prefLabel>
    <sw:term_status xml:lang="en">accepted</sw:term_status>
    <schema:rangeIncludes rdf:resource="https://w3id.org/dpv/owl#RiskConcept"/>
    <dcam:rangeIncludes rdf:resource="https://w3id.org/dpv/owl#RiskConcept"/>
    <skos:definition xml:lang="en">Indicates the specified event or action is logged by this control</skos:definition>
    <schema:domainIncludes rdf:resource="https://w3id.org/dpv/risk/owl#LoggingControl"/>
    <rdfs:subPropertyOf rdf:resource="https://w3id.org/dpv/risk/owl#monitors"/>
  </rdf:Description>
  <rdf:Description rdf:about="https://w3id.org/dpv/risk/owl#HaltSource">
    <skos:definition xml:lang="en">Control that halts the (ongoing) risk source event or process such that it no longer takes place or is applicable in the context</skos:definition>
    <skos:prefLabel xml:lang="en">Halt Source</skos:prefLabel>
    <rdf:type rdf:resource="https://w3id.org/dpv/risk/owl#RiskControl"/>
    <rdf:type rdf:resource="http://www.w3.org/2000/01/rdf-schema#Class"/>
    <rdf:type rdf:resource="http://www.w3.org/2002/07/owl#Class"/>
    <dct:modified rdf:datatype="http://www.w3.org/2001/XMLSchema#date">2025-01-06</dct:modified>
    <sw:term_status xml:lang="en">modified</sw:term_status>
    <rdfs:isDefinedBy rdf:resource="https://w3id.org/dpv/risk/owl#"/>
    <dct:contributor rdf:nodeID="Ne22a67b17c7e4a779c30d2864b6a0cee"/>
    <dct:created rdf:datatype="http://www.w3.org/2001/XMLSchema#date">2024-05-19</dct:created>
    <rdfs:subClassOf rdf:resource="https://w3id.org/dpv/risk/owl#SourceControl"/>
    <rdfs:subClassOf rdf:resource="https://w3id.org/dpv/risk/owl#InterruptionControl"/>
  </rdf:Description>
  <rdf:Description rdf:nodeID="N7d9b5ee7f31f4f2ba5951e30b49ec7c0">
    <rdf:type rdf:resource="http://xmlns.com/foaf/0.1/Person"/>
    <rdf:type rdf:resource="http://purl.org/dc/terms/Agent"/>
    <foaf:name>Georg P. Krog</foaf:name>
    <foaf:homepage>https://www.linkedin.com/in/georg-philip-krog-a2a278104/</foaf:homepage>
    <org:memberOf rdf:nodeID="N93888206f03d482f86db2078dc52e4da"/>
  </rdf:Description>
  <rdf:Description rdf:about="https://w3id.org/dpv/risk/owl#mitigates">
    <rdfs:isDefinedBy rdf:resource="https://w3id.org/dpv/risk/owl#"/>
    <dct:contributor rdf:nodeID="N9c63c24625fe482386a350b4ea27b4f8"/>
    <dct:contributor rdf:nodeID="Ne22a67b17c7e4a779c30d2864b6a0cee"/>
    <sw:term_status xml:lang="en">modified</sw:term_status>
    <schema:rangeIncludes rdf:resource="https://w3id.org/dpv/owl#RiskConcept"/>
    <skos:definition xml:lang="en">Indicates the specified event or action is mitigated by this control</skos:definition>
    <dcam:domainIncludes rdf:resource="https://w3id.org/dpv/risk/owl#MitigationControl"/>
    <skos:prefLabel xml:lang="en">mitigates</skos:prefLabel>
    <rdf:type rdf:resource="http://www.w3.org/1999/02/22-rdf-syntax-ns#Property"/>
    <rdf:type rdf:resource="http://www.w3.org/2002/07/owl#ObjectProperty"/>
    <dct:created rdf:datatype="http://www.w3.org/2001/XMLSchema#date">2024-12-01</dct:created>
    <schema:domainIncludes rdf:resource="https://w3id.org/dpv/risk/owl#MitigationControl"/>
    <rdfs:subPropertyOf rdf:resource="https://w3id.org/dpv/risk/owl#avoids"/>
    <dct:modified rdf:datatype="http://www.w3.org/2001/XMLSchema#date">2025-01-06</dct:modified>
    <dcam:rangeIncludes rdf:resource="https://w3id.org/dpv/owl#RiskConcept"/>
  </rdf:Description>
  <rdf:Description rdf:about="https://w3id.org/dpv/risk/owl#SourceControl">
    <rdf:type rdf:resource="https://w3id.org/dpv/risk/owl#RiskControl"/>
    <rdf:type rdf:resource="http://www.w3.org/2000/01/rdf-schema#Class"/>
    <rdf:type rdf:resource="http://www.w3.org/2002/07/owl#Class"/>
    <skos:definition xml:lang="en">Risk control for managing risk sources</skos:definition>
    <rdfs:isDefinedBy rdf:resource="https://w3id.org/dpv/risk/owl#"/>
    <sw:term_status xml:lang="en">modified</sw:term_status>
    <dct:contributor rdf:nodeID="Ne22a67b17c7e4a779c30d2864b6a0cee"/>
    <skos:prefLabel xml:lang="en">Source Control</skos:prefLabel>
    <dct:modified rdf:datatype="http://www.w3.org/2001/XMLSchema#date">2025-01-06</dct:modified>
    <dct:created rdf:datatype="http://www.w3.org/2001/XMLSchema#date">2024-05-19</dct:created>
    <rdfs:subClassOf rdf:resource="https://w3id.org/dpv/risk/owl#RiskControl"/>
  </rdf:Description>
  <rdf:Description rdf:about="https://w3id.org/dpv/risk/owl#AvoidSource">
    <rdfs:isDefinedBy rdf:resource="https://w3id.org/dpv/risk/owl#"/>
    <dct:created rdf:datatype="http://www.w3.org/2001/XMLSchema#date">2024-05-19</dct:created>
    <rdf:type rdf:resource="http://www.w3.org/2000/01/rdf-schema#Class"/>
    <rdf:type rdf:resource="https://w3id.org/dpv/risk/owl#RiskControl"/>
    <rdf:type rdf:resource="http://www.w3.org/2002/07/owl#Class"/>
    <skos:prefLabel xml:lang="en">Avoid Source</skos:prefLabel>
    <sw:term_status xml:lang="en">modified</sw:term_status>
    <skos:definition xml:lang="en">Control that proactively avoids the risk source such that it has a reduced exposure or applicability in the context</skos:definition>
    <dct:modified rdf:datatype="http://www.w3.org/2001/XMLSchema#date">2025-01-06</dct:modified>
    <dct:contributor rdf:nodeID="Ne22a67b17c7e4a779c30d2864b6a0cee"/>
    <rdfs:subClassOf rdf:resource="https://w3id.org/dpv/risk/owl#SourceControl"/>
    <rdfs:subClassOf rdf:resource="https://w3id.org/dpv/risk/owl#AvoidanceControl"/>
  </rdf:Description>
  <rdf:Description rdf:about="https://w3id.org/dpv/risk/owl#SubstitutionControl">
    <sw:term_status xml:lang="en">accepted</sw:term_status>
    <rdfs:isDefinedBy rdf:resource="https://w3id.org/dpv/risk/owl#"/>
    <skos:prefLabel xml:lang="en">Substitution Control</skos:prefLabel>
    <skos:scopeNote xml:lang="en">Substitution implies that the replacement event is less risky or is more safe than the replaced event, which is distinct from elimination where no event occurs and thus there is an elimination of risk entirely</skos:scopeNote>
    <rdf:type rdf:resource="http://www.w3.org/2000/01/rdf-schema#Class"/>
    <rdf:type rdf:resource="https://w3id.org/dpv/risk/owl#RiskControl"/>
    <rdf:type rdf:resource="http://www.w3.org/2002/07/owl#Class"/>
    <dct:contributor rdf:nodeID="N9c63c24625fe482386a350b4ea27b4f8"/>
    <dct:contributor rdf:nodeID="Ne22a67b17c7e4a779c30d2864b6a0cee"/>
    <skos:definition xml:lang="en">Control that substitutes an event with another such that the initial event no longer takes place while the substituted event takes place in place of it</skos:definition>
    <dct:created rdf:datatype="http://www.w3.org/2001/XMLSchema#date">2025-01-06</dct:created>
    <rdfs:subClassOf rdf:resource="https://w3id.org/dpv/risk/owl#AvoidanceControl"/>
  </rdf:Description>
  <rdf:Description rdf:about="https://w3id.org/dpv/risk/owl#identifies">
    <dct:contributor rdf:nodeID="Ne22a67b17c7e4a779c30d2864b6a0cee"/>
    <dct:contributor rdf:nodeID="N9c63c24625fe482386a350b4ea27b4f8"/>
    <schema:rangeIncludes rdf:resource="https://w3id.org/dpv/owl#RiskConcept"/>
    <rdf:type rdf:resource="http://www.w3.org/1999/02/22-rdf-syntax-ns#Property"/>
    <rdf:type rdf:resource="http://www.w3.org/2002/07/owl#ObjectProperty"/>
    <skos:prefLabel xml:lang="en">identifies</skos:prefLabel>
    <dct:created rdf:datatype="http://www.w3.org/2001/XMLSchema#date">2024-12-01</dct:created>
    <dcam:rangeIncludes rdf:resource="https://w3id.org/dpv/owl#RiskConcept"/>
    <rdfs:subPropertyOf rdf:resource="https://w3id.org/dpv/risk/owl#monitors"/>
    <dct:modified rdf:datatype="http://www.w3.org/2001/XMLSchema#date">2025-01-06</dct:modified>
    <rdfs:isDefinedBy rdf:resource="https://w3id.org/dpv/risk/owl#"/>
    <sw:term_status xml:lang="en">modified</sw:term_status>
    <dcam:domainIncludes rdf:resource="https://w3id.org/dpv/risk/owl#IdentificationControl"/>
    <skos:definition xml:lang="en">Indicates the specified event or action is identified by this control</skos:definition>
    <schema:domainIncludes rdf:resource="https://w3id.org/dpv/risk/owl#IdentificationControl"/>
  </rdf:Description>
  <rdf:Description rdf:about="https://w3id.org/dpv/risk/owl#MonitorConsequence">
    <dct:created rdf:datatype="http://www.w3.org/2001/XMLSchema#date">2024-05-19</dct:created>
    <rdf:type rdf:resource="http://www.w3.org/2000/01/rdf-schema#Class"/>
    <rdf:type rdf:resource="https://w3id.org/dpv/risk/owl#RiskControl"/>
    <rdf:type rdf:resource="http://www.w3.org/2002/07/owl#Class"/>
    <dct:contributor rdf:nodeID="Ne22a67b17c7e4a779c30d2864b6a0cee"/>
    <sw:term_status xml:lang="en">modified</sw:term_status>
    <skos:prefLabel xml:lang="en">Monitor Consequence</skos:prefLabel>
    <dct:modified rdf:datatype="http://www.w3.org/2001/XMLSchema#date">2025-01-06</dct:modified>
    <skos:definition xml:lang="en">Control that monitors a Risk Consequence</skos:definition>
    <rdfs:isDefinedBy rdf:resource="https://w3id.org/dpv/risk/owl#"/>
    <rdfs:subClassOf rdf:resource="https://w3id.org/dpv/risk/owl#MonitorControl"/>
  </rdf:Description>
  <rdf:Description rdf:about="https://w3id.org/dpv/risk/owl#ModificationControl">
    <rdf:type rdf:resource="http://www.w3.org/2000/01/rdf-schema#Class"/>
    <rdf:type rdf:resource="https://w3id.org/dpv/risk/owl#RiskControl"/>
    <rdf:type rdf:resource="http://www.w3.org/2002/07/owl#Class"/>
    <dct:contributor rdf:nodeID="N9c63c24625fe482386a350b4ea27b4f8"/>
    <dct:contributor rdf:nodeID="Ne22a67b17c7e4a779c30d2864b6a0cee"/>
    <skos:prefLabel xml:lang="en">Modification Control</skos:prefLabel>
    <skos:definition xml:lang="en">Control that modifies the context to change the event's characteristics such that the event still occurs but with the modified characteristics with the goal of managing an event that is accepted to occur</skos:definition>
    <skos:scopeNote xml:lang="en">Modification necessitates a change in the context to result in a change in the event's characteristics. Where such changes reduce the likelihood or effects of the event, the modification also works as a mitigation for the event</skos:scopeNote>
    <sw:term_status xml:lang="en">accepted</sw:term_status>
    <rdfs:isDefinedBy rdf:resource="https://w3id.org/dpv/risk/owl#"/>
    <dct:created rdf:datatype="http://www.w3.org/2001/XMLSchema#date">2025-01-06</dct:created>
    <rdfs:subClassOf rdf:resource="https://w3id.org/dpv/risk/owl#ProactiveControl"/>
  </rdf:Description>
  <rdf:Description rdf:about="https://w3id.org/dpv/risk/owl#hasControl">
    <dct:contributor rdf:nodeID="Ne22a67b17c7e4a779c30d2864b6a0cee"/>
    <schema:rangeIncludes rdf:resource="https://w3id.org/dpv/risk/owl#RiskControl"/>
    <dcam:rangeIncludes rdf:resource="https://w3id.org/dpv/risk/owl#RiskControl"/>
    <rdfs:isDefinedBy rdf:resource="https://w3id.org/dpv/risk/owl#"/>
    <skos:prefLabel xml:lang="en">has control</skos:prefLabel>
    <rdf:type rdf:resource="http://www.w3.org/1999/02/22-rdf-syntax-ns#Property"/>
    <rdf:type rdf:resource="http://www.w3.org/2002/07/owl#ObjectProperty"/>
    <vann:example rdf:resource="https://w3id.org/dpv/examples/owl#E0071"/>
    <sw:term_status xml:lang="en">modified</sw:term_status>
    <skos:definition xml:lang="en">Indicates the use of specified control</skos:definition>
    <dct:modified rdf:datatype="http://www.w3.org/2001/XMLSchema#date">2025-01-06</dct:modified>
    <dct:created rdf:datatype="http://www.w3.org/2001/XMLSchema#date">2024-02-14</dct:created>
  </rdf:Description>
  <rdf:Description rdf:about="https://w3id.org/dpv/risk/owl#ChangeImpact">
    <skos:prefLabel xml:lang="en">Change Impact</skos:prefLabel>
    <rdfs:isDefinedBy rdf:resource="https://w3id.org/dpv/risk/owl#"/>
    <skos:definition xml:lang="en">Control that proactively changes the impact event such that one event is replaced with the occurence or applicability of another event in the context</skos:definition>
    <rdf:type rdf:resource="http://www.w3.org/2000/01/rdf-schema#Class"/>
    <rdf:type rdf:resource="https://w3id.org/dpv/risk/owl#RiskControl"/>
    <rdf:type rdf:resource="http://www.w3.org/2002/07/owl#Class"/>
    <dct:created rdf:datatype="http://www.w3.org/2001/XMLSchema#date">2024-05-19</dct:created>
    <sw:term_status xml:lang="en">modified</sw:term_status>
    <dct:contributor rdf:nodeID="Ne22a67b17c7e4a779c30d2864b6a0cee"/>
    <dct:modified rdf:datatype="http://www.w3.org/2001/XMLSchema#date">2025-01-06</dct:modified>
    <rdfs:subClassOf rdf:resource="https://w3id.org/dpv/risk/owl#ImpactControl"/>
    <rdfs:subClassOf rdf:resource="https://w3id.org/dpv/risk/owl#SubstitutionControl"/>
  </rdf:Description>
  <rdf:Description rdf:nodeID="N75641c194b3f4973ab2abfb33aed55d3">
    <scoro:hasORCID>0000-0003-0259-7560</scoro:hasORCID>
    <foaf:name>Beatriz Esteves</foaf:name>
    <org:memberOf rdf:nodeID="Nb10f7ca597f946ef8f976f1681fc0421"/>
    <rdf:type rdf:resource="http://xmlns.com/foaf/0.1/Person"/>
    <rdf:type rdf:resource="http://purl.org/dc/terms/Agent"/>
  </rdf:Description>
  <rdf:Description rdf:nodeID="N9c63c24625fe482386a350b4ea27b4f8">
    <rdf:type rdf:resource="http://purl.org/dc/terms/Agent"/>
    <rdf:type rdf:resource="http://xmlns.com/foaf/0.1/Person"/>
    <scoro:hasORCID>0000-0002-1208-186X</scoro:hasORCID>
    <foaf:name>Delaram Golpayegani</foaf:name>
    <org:memberOf rdf:nodeID="N2b218fbf49474a93a5f1d76695037221"/>
  </rdf:Description>
  <rdf:Description rdf:about="https://w3id.org/dpv/risk/owl#substitutes">
    <rdfs:isDefinedBy rdf:resource="https://w3id.org/dpv/risk/owl#"/>
    <schema:rangeIncludes rdf:resource="https://w3id.org/dpv/owl#RiskConcept"/>
    <dcam:rangeIncludes rdf:resource="https://w3id.org/dpv/owl#RiskConcept"/>
    <dcam:domainIncludes rdf:resource="https://w3id.org/dpv/risk/owl#SubstitutionControl"/>
    <dct:created rdf:datatype="http://www.w3.org/2001/XMLSchema#date">2025-01-06</dct:created>
    <skos:definition xml:lang="en">Indicates the specified event or action is substituted by this control</skos:definition>
    <skos:prefLabel xml:lang="en">substitutes</skos:prefLabel>
    <schema:domainIncludes rdf:resource="https://w3id.org/dpv/risk/owl#SubstitutionControl"/>
    <rdf:type rdf:resource="http://www.w3.org/1999/02/22-rdf-syntax-ns#Property"/>
    <rdf:type rdf:resource="http://www.w3.org/2002/07/owl#ObjectProperty"/>
    <sw:term_status xml:lang="en">accepted</sw:term_status>
    <rdfs:subPropertyOf rdf:resource="https://w3id.org/dpv/risk/owl#avoids"/>
    <dct:contributor rdf:nodeID="Ne22a67b17c7e4a779c30d2864b6a0cee"/>
  </rdf:Description>
  <rdf:Description rdf:about="https://w3id.org/dpv/risk/owl#ConsequenceControl">
    <dct:created rdf:datatype="http://www.w3.org/2001/XMLSchema#date">2024-05-19</dct:created>
    <rdf:type rdf:resource="http://www.w3.org/2000/01/rdf-schema#Class"/>
    <rdf:type rdf:resource="https://w3id.org/dpv/risk/owl#RiskControl"/>
    <rdf:type rdf:resource="http://www.w3.org/2002/07/owl#Class"/>
    <dct:contributor rdf:nodeID="Ne22a67b17c7e4a779c30d2864b6a0cee"/>
    <sw:term_status xml:lang="en">modified</sw:term_status>
    <dct:modified rdf:datatype="http://www.w3.org/2001/XMLSchema#date">2025-01-06</dct:modified>
    <skos:prefLabel xml:lang="en">Consequence Control</skos:prefLabel>
    <skos:definition xml:lang="en">Risk control for managing consequences</skos:definition>
    <rdfs:isDefinedBy rdf:resource="https://w3id.org/dpv/risk/owl#"/>
    <rdfs:subClassOf rdf:resource="https://w3id.org/dpv/risk/owl#RiskControl"/>
  </rdf:Description>
  <rdf:Description rdf:about="https://w3id.org/dpv/risk/owl#IdentificationControl">
    <rdfs:isDefinedBy rdf:resource="https://w3id.org/dpv/risk/owl#"/>
    <dct:contributor rdf:nodeID="N9c63c24625fe482386a350b4ea27b4f8"/>
    <dct:contributor rdf:nodeID="Ne22a67b17c7e4a779c30d2864b6a0cee"/>
    <skos:scopeNote xml:lang="en">Identification in the context of an event refers to its characteristics such as likelihood, severity, as well as contextual metrics such as amount of data or power being used, or affected entities or things, and which can be used to categorise the event in terms of risk level or other contextual groupings</skos:scopeNote>
    <rdf:type rdf:resource="http://www.w3.org/2000/01/rdf-schema#Class"/>
    <rdf:type rdf:resource="https://w3id.org/dpv/risk/owl#RiskControl"/>
    <rdf:type rdf:resource="http://www.w3.org/2002/07/owl#Class"/>
    <skos:definition xml:lang="en">Control that identifies the characteristics of an event</skos:definition>
    <dct:created rdf:datatype="http://www.w3.org/2001/XMLSchema#date">2024-05-19</dct:created>
    <skos:prefLabel xml:lang="en">Identification Control</skos:prefLabel>
    <dct:modified rdf:datatype="http://www.w3.org/2001/XMLSchema#date">2025-01-06</dct:modified>
    <sw:term_status xml:lang="en">modified</sw:term_status>
    <rdfs:subClassOf rdf:resource="https://w3id.org/dpv/risk/owl#MonitorControl"/>
  </rdf:Description>
  <rdf:Description rdf:nodeID="N59852c09189e47bd989757f1615f7bdf">
    <rdf:type rdf:resource="http://xmlns.com/foaf/0.1/Person"/>
    <rdf:type rdf:resource="http://purl.org/dc/terms/Agent"/>
    <org:memberOf rdf:nodeID="N0c4f26726681494f8f9054328c810c07"/>
    <foaf:name>Rob Brennan</foaf:name>
  </rdf:Description>
  <rdf:Description rdf:about="https://w3id.org/dpv/risk/owl#MonitorRiskSource">
    <skos:prefLabel xml:lang="en">Monitor Risk Source</skos:prefLabel>
    <skos:definition xml:lang="en">Control that monitors a Risk Source</skos:definition>
    <dct:contributor rdf:nodeID="Ne22a67b17c7e4a779c30d2864b6a0cee"/>
    <rdf:type rdf:resource="https://w3id.org/dpv/risk/owl#RiskControl"/>
    <rdf:type rdf:resource="http://www.w3.org/2000/01/rdf-schema#Class"/>
    <rdf:type rdf:resource="http://www.w3.org/2002/07/owl#Class"/>
    <rdfs:isDefinedBy rdf:resource="https://w3id.org/dpv/risk/owl#"/>
    <sw:term_status xml:lang="en">modified</sw:term_status>
    <dct:modified rdf:datatype="http://www.w3.org/2001/XMLSchema#date">2025-01-06</dct:modified>
    <dct:created rdf:datatype="http://www.w3.org/2001/XMLSchema#date">2024-05-19</dct:created>
    <rdfs:subClassOf rdf:resource="https://w3id.org/dpv/risk/owl#MonitorControl"/>
  </rdf:Description>
  <rdf:Description rdf:about="https://w3id.org/dpv/risk/owl#AvoidImpact">
    <skos:prefLabel xml:lang="en">Avoid Impact</skos:prefLabel>
    <rdf:type rdf:resource="http://www.w3.org/2000/01/rdf-schema#Class"/>
    <rdf:type rdf:resource="https://w3id.org/dpv/risk/owl#RiskControl"/>
    <rdf:type rdf:resource="http://www.w3.org/2002/07/owl#Class"/>
    <skos:definition xml:lang="en">Control that proactively avoids the impact such that it has a reduced exposure or applicability in the context</skos:definition>
    <dct:contributor rdf:nodeID="Ne22a67b17c7e4a779c30d2864b6a0cee"/>
    <dct:created rdf:datatype="http://www.w3.org/2001/XMLSchema#date">2025-01-06</dct:created>
    <sw:term_status xml:lang="en">accepted</sw:term_status>
    <rdfs:isDefinedBy rdf:resource="https://w3id.org/dpv/risk/owl#"/>
    <rdfs:subClassOf rdf:resource="https://w3id.org/dpv/risk/owl#ImpactControl"/>
    <rdfs:subClassOf rdf:resource="https://w3id.org/dpv/risk/owl#AvoidanceControl"/>
  </rdf:Description>
  <rdf:Description rdf:about="https://w3id.org/dpv/risk/owl#InvestigationControl">
    <rdf:type rdf:resource="http://www.w3.org/2000/01/rdf-schema#Class"/>
    <rdf:type rdf:resource="https://w3id.org/dpv/risk/owl#RiskControl"/>
    <rdf:type rdf:resource="http://www.w3.org/2002/07/owl#Class"/>
    <skos:definition xml:lang="en">Control that identifies information through an investigative process about an event and its effects after it has occured</skos:definition>
    <dct:contributor rdf:nodeID="Ne22a67b17c7e4a779c30d2864b6a0cee"/>
    <sw:term_status xml:lang="en">accepted</sw:term_status>
    <skos:prefLabel xml:lang="en">Investigation Control</skos:prefLabel>
    <skos:scopeNote xml:lang="en">Investigative controls are used to identify information about an event and its effects which can be used to identify further effective measures to address them, and to identify processes to remedy and recover from it. Investigation control therefore is focused on analysis of an event after its occurence with the goal of identifying applicability and effectiveness of other controls to address it</skos:scopeNote>
    <rdfs:isDefinedBy rdf:resource="https://w3id.org/dpv/risk/owl#"/>
    <dct:created rdf:datatype="http://www.w3.org/2001/XMLSchema#date">2025-01-06</dct:created>
    <rdfs:subClassOf rdf:resource="https://w3id.org/dpv/risk/owl#ReactiveControl"/>
  </rdf:Description>
  <rdf:Description rdf:about="https://w3id.org/dpv/risk/owl#avoids">
    <skos:prefLabel xml:lang="en">avoids</skos:prefLabel>
    <dcam:domainIncludes rdf:resource="https://w3id.org/dpv/risk/owl#AvoidanceControl"/>
    <skos:definition xml:lang="en">Indicates the event or action is avoided by the specified control</skos:definition>
    <dct:created rdf:datatype="http://www.w3.org/2001/XMLSchema#date">2025-01-06</dct:created>
    <schema:domainIncludes rdf:resource="https://w3id.org/dpv/risk/owl#AvoidanceControl"/>
    <rdfs:isDefinedBy rdf:resource="https://w3id.org/dpv/risk/owl#"/>
    <dct:contributor rdf:nodeID="Ne22a67b17c7e4a779c30d2864b6a0cee"/>
    <rdf:type rdf:resource="http://www.w3.org/1999/02/22-rdf-syntax-ns#Property"/>
    <rdf:type rdf:resource="http://www.w3.org/2002/07/owl#ObjectProperty"/>
    <sw:term_status xml:lang="en">accepted</sw:term_status>
    <rdfs:subPropertyOf rdf:resource="https://w3id.org/dpv/risk/owl#reduces"/>
    <schema:rangeIncludes rdf:resource="https://w3id.org/dpv/owl#RiskConcept"/>
    <dcam:rangeIncludes rdf:resource="https://w3id.org/dpv/owl#RiskConcept"/>
  </rdf:Description>
  <rdf:Description rdf:about="https://w3id.org/dpv/risk/owl#serialisation-html">
    <profile:hasArtifact rdf:resource="https://w3id.org/dpv/risk/risk-owl.html"/>
    <profile:hasRole rdf:resource="http://www.w3.org/ns/dx/prof/role/specification"/>
    <rdf:type rdf:resource="http://www.w3.org/ns/dx/prof/ResourceDescriptor"/>
    <dct:title>Risk Concepts - HTML serialiation</dct:title>
    <dct:conformsTo rdf:resource="https://www.w3.org/TR/html/"/>
    <dct:format rdf:resource="https://www.iana.org/assignments/media-types/text/html"/>
  </rdf:Description>
  <rdf:Description rdf:nodeID="N6cd6ef5ec58745369be45f4a23814332">
    <rdf:type rdf:resource="http://xmlns.com/foaf/0.1/Organization"/>
    <foaf:name>ADAPT Centre, Dublin City University</foaf:name>
  </rdf:Description>
  <rdf:Description rdf:about="https://w3id.org/dpv/risk/owl#LoggingControl">
    <rdfs:isDefinedBy rdf:resource="https://w3id.org/dpv/risk/owl#"/>
    <dct:contributor rdf:nodeID="N9c63c24625fe482386a350b4ea27b4f8"/>
    <dct:contributor rdf:nodeID="Ne22a67b17c7e4a779c30d2864b6a0cee"/>
    <rdf:type rdf:resource="https://w3id.org/dpv/risk/owl#RiskControl"/>
    <rdf:type rdf:resource="http://www.w3.org/2000/01/rdf-schema#Class"/>
    <rdf:type rdf:resource="http://www.w3.org/2002/07/owl#Class"/>
    <dct:created rdf:datatype="http://www.w3.org/2001/XMLSchema#date">2025-01-06</dct:created>
    <skos:definition xml:lang="en">Control that logs an event</skos:definition>
    <skos:prefLabel xml:lang="en">Logging Control</skos:prefLabel>
    <skos:scopeNote xml:lang="en">Log refers to a record of information regarding the event, including whether it has occured, was prevented from occuring, and any actions or processes taken in response to it or resulting from it</skos:scopeNote>
    <sw:term_status xml:lang="en">accepted</sw:term_status>
    <rdfs:subClassOf rdf:resource="https://w3id.org/dpv/risk/owl#MonitorControl"/>
  </rdf:Description>
  <rdf:Description rdf:about="https://w3id.org/dpv/risk/owl#ReversalControl">
    <dct:created rdf:datatype="http://www.w3.org/2001/XMLSchema#date">2025-01-06</dct:created>
    <sw:term_status xml:lang="en">accepted</sw:term_status>
    <rdfs:isDefinedBy rdf:resource="https://w3id.org/dpv/risk/owl#"/>
    <skos:scopeNote xml:lang="en">Reversal can be achieved through measures such as restoring information from a backup or replacing things such that the initial context not containing the event's effects is restored</skos:scopeNote>
    <rdf:type rdf:resource="http://www.w3.org/2000/01/rdf-schema#Class"/>
    <rdf:type rdf:resource="https://w3id.org/dpv/risk/owl#RiskControl"/>
    <rdf:type rdf:resource="http://www.w3.org/2002/07/owl#Class"/>
    <skos:prefLabel xml:lang="en">Reversal Control</skos:prefLabel>
    <skos:definition xml:lang="en">Control that aims to reverse or undo the effects of an event</skos:definition>
    <dct:contributor rdf:nodeID="N9c63c24625fe482386a350b4ea27b4f8"/>
    <dct:contributor rdf:nodeID="Ne22a67b17c7e4a779c30d2864b6a0cee"/>
    <rdfs:subClassOf rdf:resource="https://w3id.org/dpv/risk/owl#ResolutionControl"/>
  </rdf:Description>
  <rdf:Description rdf:about="https://w3id.org/dpv/risk/owl#ContainmentControl">
    <rdf:type rdf:resource="http://www.w3.org/2000/01/rdf-schema#Class"/>
    <rdf:type rdf:resource="https://w3id.org/dpv/risk/owl#RiskControl"/>
    <rdf:type rdf:resource="http://www.w3.org/2002/07/owl#Class"/>
    <dct:created rdf:datatype="http://www.w3.org/2001/XMLSchema#date">2024-05-19</dct:created>
    <dct:modified rdf:datatype="http://www.w3.org/2001/XMLSchema#date">2025-01-06</dct:modified>
    <sw:term_status xml:lang="en">modified</sw:term_status>
    <skos:scopeNote xml:lang="en">Containment implies either changing the event or the context such that the event's effects are restricted, such as by establishing a physical or digital boundary within which the effects can occur or to prevent the effects from affecting things inside the boundary</skos:scopeNote>
    <skos:prefLabel xml:lang="en">Containment Control</skos:prefLabel>
    <skos:definition xml:lang="en">Control that aims to contain the event in terms of limiting its occurence or effects</skos:definition>
    <rdfs:isDefinedBy rdf:resource="https://w3id.org/dpv/risk/owl#"/>
    <dct:contributor rdf:nodeID="N9c63c24625fe482386a350b4ea27b4f8"/>
    <dct:contributor rdf:nodeID="Ne22a67b17c7e4a779c30d2864b6a0cee"/>
    <rdfs:subClassOf rdf:resource="https://w3id.org/dpv/risk/owl#ReductionControl"/>
  </rdf:Description>
  <rdf:Description rdf:about="https://w3id.org/dpv/risk/owl#ResolutionControl">
    <dct:contributor rdf:nodeID="Ne22a67b17c7e4a779c30d2864b6a0cee"/>
    <skos:prefLabel xml:lang="en">Resolution Control</skos:prefLabel>
    <skos:definition xml:lang="en">Control that aims to resolve an event's effects with the goal of fixing or recovering from it</skos:definition>
    <rdf:type rdf:resource="https://w3id.org/dpv/risk/owl#RiskControl"/>
    <rdf:type rdf:resource="http://www.w3.org/2000/01/rdf-schema#Class"/>
    <rdf:type rdf:resource="http://www.w3.org/2002/07/owl#Class"/>
    <dct:created rdf:datatype="http://www.w3.org/2001/XMLSchema#date">2025-01-06</dct:created>
    <sw:term_status xml:lang="en">accepted</sw:term_status>
    <rdfs:isDefinedBy rdf:resource="https://w3id.org/dpv/risk/owl#"/>
    <rdfs:subClassOf rdf:resource="https://w3id.org/dpv/risk/owl#ReactiveControl"/>
  </rdf:Description>
  <rdf:Description rdf:about="https://w3id.org/dpv/risk/owl#HaltConsequence">
    <rdfs:isDefinedBy rdf:resource="https://w3id.org/dpv/risk/owl#"/>
    <dct:contributor rdf:nodeID="Ne22a67b17c7e4a779c30d2864b6a0cee"/>
    <dct:created rdf:datatype="http://www.w3.org/2001/XMLSchema#date">2025-01-06</dct:created>
    <sw:term_status xml:lang="en">accepted</sw:term_status>
    <rdf:type rdf:resource="http://www.w3.org/2000/01/rdf-schema#Class"/>
    <rdf:type rdf:resource="https://w3id.org/dpv/risk/owl#RiskControl"/>
    <rdf:type rdf:resource="http://www.w3.org/2002/07/owl#Class"/>
    <skos:definition xml:lang="en">Control that halts the (ongoing) consequence event or process such that it no longer takes place or is applicable in the context</skos:definition>
    <skos:prefLabel xml:lang="en">Halt Consequence</skos:prefLabel>
    <rdfs:subClassOf rdf:resource="https://w3id.org/dpv/risk/owl#InterruptionControl"/>
    <rdfs:subClassOf rdf:resource="https://w3id.org/dpv/risk/owl#ConsequenceControl"/>
  </rdf:Description>
  <rdf:Description rdf:about="https://w3id.org/dpv/risk/owl#OverrideControl">
    <rdf:type rdf:resource="https://w3id.org/dpv/risk/owl#RiskControl"/>
    <rdf:type rdf:resource="http://www.w3.org/2000/01/rdf-schema#Class"/>
    <rdf:type rdf:resource="http://www.w3.org/2002/07/owl#Class"/>
    <skos:definition xml:lang="en">Control that aims to override the event with the goal of avoiding its further effects</skos:definition>
    <skos:prefLabel xml:lang="en">Override Control</skos:prefLabel>
    <dct:contributor rdf:nodeID="N9c63c24625fe482386a350b4ea27b4f8"/>
    <dct:contributor rdf:nodeID="Ne22a67b17c7e4a779c30d2864b6a0cee"/>
    <rdfs:isDefinedBy rdf:resource="https://w3id.org/dpv/risk/owl#"/>
    <dct:created rdf:datatype="http://www.w3.org/2001/XMLSchema#date">2025-01-06</dct:created>
    <skos:scopeNote xml:lang="en">Override indicates a (temporary) change or bypassing of usual processes, controls, and measures in response to an event</skos:scopeNote>
    <sw:term_status xml:lang="en">accepted</sw:term_status>
    <rdfs:subClassOf rdf:resource="https://w3id.org/dpv/risk/owl#ReactiveControl"/>
  </rdf:Description>
  <rdf:Description rdf:about="https://w3id.org/dpv/risk/owl#serialisation-ttl">
    <profile:hasArtifact rdf:resource="https://w3id.org/dpv/risk/risk-owl.ttl"/>
    <rdf:type rdf:resource="http://www.w3.org/ns/dx/prof/ResourceDescriptor"/>
    <dct:format rdf:resource="https://www.iana.org/assignments/media-types/text/turtle"/>
    <profile:hasRole rdf:resource="http://www.w3.org/ns/dx/prof/role/vocabulary"/>
    <dct:conformsTo rdf:resource="https://www.w3.org/TR/turtle/"/>
    <dct:title>Risk Concepts - Turtle serialiation</dct:title>
  </rdf:Description>
  <rdf:Description rdf:nodeID="Nb10f7ca597f946ef8f976f1681fc0421">
    <foaf:name>IDLab, IMEC, Ghent University</foaf:name>
    <rdf:type rdf:resource="http://xmlns.com/foaf/0.1/Organization"/>
  </rdf:Description>
  <rdf:Description rdf:about="https://w3id.org/dpv/risk/owl#serialisation-jsonld">
    <profile:hasRole rdf:resource="http://www.w3.org/ns/dx/prof/role/vocabulary"/>
    <profile:hasArtifact rdf:resource="https://w3id.org/dpv/risk/risk-owl.jsonld"/>
    <rdf:type rdf:resource="http://www.w3.org/ns/dx/prof/ResourceDescriptor"/>
    <dct:format rdf:resource="https://www.iana.org/assignments/media-types/application/ld+json"/>
    <dct:title>Risk Concepts - JSON-LD serialiation</dct:title>
    <dct:conformsTo rdf:resource="https://www.w3.org/TR/json-ld11/"/>
  </rdf:Description>
  <rdf:Description rdf:about="https://w3id.org/dpv/risk/owl#serialisation-n3">
    <dct:format rdf:resource="https://www.iana.org/assignments/media-types/text/n3"/>
    <dct:conformsTo rdf:resource="https://www.w3.org/TeamSubmission/n3/"/>
    <dct:title>Risk Concepts - N3 serialiation</dct:title>
    <profile:hasArtifact rdf:resource="https://w3id.org/dpv/risk/risk-owl.n3"/>
    <rdf:type rdf:resource="http://www.w3.org/ns/dx/prof/ResourceDescriptor"/>
    <profile:hasRole rdf:resource="http://www.w3.org/ns/dx/prof/role/vocabulary"/>
  </rdf:Description>
  <rdf:Description rdf:nodeID="Ndedfd6f107a441f99c7268556c8aca81">
    <org:memberOf rdf:nodeID="N7212af5ee4254bd389ed10151fe479fe"/>
    <rdf:type rdf:resource="http://xmlns.com/foaf/0.1/Person"/>
    <rdf:type rdf:resource="http://purl.org/dc/terms/Agent"/>
    <scoro:hasORCID>0000-0003-0770-2737</scoro:hasORCID>
    <foaf:name>Paul Ryan</foaf:name>
  </rdf:Description>
  <rdf:Description rdf:nodeID="N93888206f03d482f86db2078dc52e4da">
    <foaf:name>Signatu AS</foaf:name>
    <rdf:type rdf:resource="http://xmlns.com/foaf/0.1/Organization"/>
  </rdf:Description>
  <rdf:Description rdf:about="https://w3id.org/dpv/risk/owl#serialisation-rdf">
    <profile:hasRole rdf:resource="http://www.w3.org/ns/dx/prof/role/vocabulary"/>
    <dct:format rdf:resource="https://www.iana.org/assignments/media-types/application/rdf+xml"/>
    <rdf:type rdf:resource="http://www.w3.org/ns/dx/prof/ResourceDescriptor"/>
    <dct:title>Risk Concepts - RDF/XML serialiation</dct:title>
    <dct:conformsTo rdf:resource="http://www.w3.org/1999/02/22-rdf-syntax-ns#"/>
    <profile:hasArtifact rdf:resource="https://w3id.org/dpv/risk/risk-owl.rdf"/>
  </rdf:Description>
  <rdf:Description rdf:nodeID="N2b218fbf49474a93a5f1d76695037221">
    <foaf:name>ADAPT Centre, Trinity College Dublin</foaf:name>
    <rdf:type rdf:resource="http://xmlns.com/foaf/0.1/Organization"/>
  </rdf:Description>
  <rdf:Description rdf:nodeID="Ne22a67b17c7e4a779c30d2864b6a0cee">
    <rdf:type rdf:resource="http://xmlns.com/foaf/0.1/Person"/>
    <rdf:type rdf:resource="http://purl.org/dc/terms/Agent"/>
    <org:memberOf rdf:nodeID="N6cd6ef5ec58745369be45f4a23814332"/>
    <foaf:name>Harshvardhan J. Pandit</foaf:name>
    <foaf:homepage>https://harshp.com/</foaf:homepage>
    <scoro:hasORCID>0000-0002-5068-3714</scoro:hasORCID>
  </rdf:Description>
  <rdf:Description rdf:nodeID="N1179325f3fdc440ea7096a5f4b108a44">
    <rdf:type rdf:resource="http://xmlns.com/foaf/0.1/Organization"/>
    <foaf:name>University of Koblenz</foaf:name>
  </rdf:Description>
  <rdf:Description rdf:nodeID="N7212af5ee4254bd389ed10151fe479fe">
    <rdf:type rdf:resource="http://xmlns.com/foaf/0.1/Organization"/>
    <foaf:name>Uniphar PLC</foaf:name>
  </rdf:Description>
</rdf:RDF>
