<?xml version="1.0" encoding="utf-8"?>
<rdf:RDF
   xmlns:bibo="http://purl.org/ontology/bibo/"
   xmlns:dct="http://purl.org/dc/terms/"
   xmlns:foaf="http://xmlns.com/foaf/0.1/"
   xmlns:org="http://www.w3.org/ns/org#"
   xmlns:owl="http://www.w3.org/2002/07/owl#"
   xmlns:profile="http://www.w3.org/ns/dx/prof/"
   xmlns:rdf="http://www.w3.org/1999/02/22-rdf-syntax-ns#"
   xmlns:rdfs="http://www.w3.org/2000/01/rdf-schema#"
   xmlns:schema="https://schema.org/"
   xmlns:scoro="http://purl.org/spar/scoro/"
   xmlns:skos="http://www.w3.org/2004/02/skos/core#"
   xmlns:sw="http://www.w3.org/2003/06/sw-vocab-status/ns#"
   xmlns:vann="http://purl.org/vocab/vann/"
>
  <rdf:Description rdf:about="https://w3id.org/dpv/sector/law/owl#LegalOffencePatternAnalysis">
    <rdfs:isDefinedBy rdf:resource="https://w3id.org/dpv/sector/law/owl#"/>
    <dct:created rdf:datatype="http://www.w3.org/2001/XMLSchema#date">2024-12-01</dct:created>
    <rdf:type rdf:resource="http://www.w3.org/2000/01/rdf-schema#Class"/>
    <rdf:type rdf:resource="https://w3id.org/dpv/owl#Purpose"/>
    <rdf:type rdf:resource="http://www.w3.org/2002/07/owl#Class"/>
    <sw:term_status xml:lang="en">accepted</sw:term_status>
    <skos:prefLabel xml:lang="en">Legal Offence Pattern Analysis</skos:prefLabel>
    <skos:definition xml:lang="en">Purposes associated with identifying and analysing patterns and trends related to offences, violations, crime, or other activities of interest within the legal system</skos:definition>
    <rdfs:subClassOf rdf:resource="https://w3id.org/dpv/sector/law/owl#LegalResearchDevelopment"/>
  </rdf:Description>
  <rdf:Description rdf:about="https://w3id.org/dpv/sector/law/owl#LegalComplaintManagement">
    <rdf:type rdf:resource="http://www.w3.org/2000/01/rdf-schema#Class"/>
    <rdf:type rdf:resource="https://w3id.org/dpv/owl#Purpose"/>
    <rdf:type rdf:resource="http://www.w3.org/2002/07/owl#Class"/>
    <sw:term_status xml:lang="en">accepted</sw:term_status>
    <dct:created rdf:datatype="http://www.w3.org/2001/XMLSchema#date">2024-12-01</dct:created>
    <skos:definition xml:lang="en">Purposes associated with management of complaints within the judicial system</skos:definition>
    <skos:prefLabel xml:lang="en">Legal Complaint Management</skos:prefLabel>
    <rdfs:isDefinedBy rdf:resource="https://w3id.org/dpv/sector/law/owl#"/>
    <rdfs:subClassOf rdf:resource="https://w3id.org/dpv/sector/law/owl#JudicialSystemManagement"/>
  </rdf:Description>
  <rdf:Description rdf:about="https://w3id.org/dpv/sector/law/owl#TransportLawEnforcement">
    <sw:term_status xml:lang="en">accepted</sw:term_status>
    <rdf:type rdf:resource="https://w3id.org/dpv/owl#Purpose"/>
    <rdf:type rdf:resource="http://www.w3.org/2000/01/rdf-schema#Class"/>
    <rdf:type rdf:resource="http://www.w3.org/2002/07/owl#Class"/>
    <dct:created rdf:datatype="http://www.w3.org/2001/XMLSchema#date">2024-12-01</dct:created>
    <skos:definition xml:lang="en">Purposes associated with law enforcement related to transportation infrastructure and services</skos:definition>
    <skos:prefLabel xml:lang="en">Transport Law Enforcement</skos:prefLabel>
    <rdfs:isDefinedBy rdf:resource="https://w3id.org/dpv/sector/law/owl#"/>
    <rdfs:subClassOf rdf:resource="https://w3id.org/dpv/sector/law/owl#LawEnforcement"/>
  </rdf:Description>
  <rdf:Description rdf:about="https://w3id.org/dpv/sector/law/owl#ImmigrationIdentityVerification">
    <dct:created rdf:datatype="http://www.w3.org/2001/XMLSchema#date">2024-12-01</dct:created>
    <skos:prefLabel xml:lang="en">Immigration Identity Verification</skos:prefLabel>
    <skos:definition xml:lang="en">Purposes associated with verificiation of identity related to immigration within the legal system</skos:definition>
    <rdf:type rdf:resource="http://www.w3.org/2000/01/rdf-schema#Class"/>
    <rdf:type rdf:resource="https://w3id.org/dpv/owl#Purpose"/>
    <rdf:type rdf:resource="http://www.w3.org/2002/07/owl#Class"/>
    <sw:term_status xml:lang="en">accepted</sw:term_status>
    <rdfs:isDefinedBy rdf:resource="https://w3id.org/dpv/sector/law/owl#"/>
    <rdfs:subClassOf rdf:resource="https://w3id.org/dpv/owl#IdentityVerification"/>
    <rdfs:subClassOf rdf:resource="https://w3id.org/dpv/sector/law/owl#ImmigrationRequestManagement"/>
  </rdf:Description>
  <rdf:Description rdf:about="https://w3id.org/dpv/sector/law/owl#CrimeDetection">
    <rdf:type rdf:resource="http://www.w3.org/2000/01/rdf-schema#Class"/>
    <rdf:type rdf:resource="https://w3id.org/dpv/owl#Purpose"/>
    <rdf:type rdf:resource="http://www.w3.org/2002/07/owl#Class"/>
    <skos:definition xml:lang="en">Purposes associated with detection of crimes within the legal system</skos:definition>
    <rdfs:isDefinedBy rdf:resource="https://w3id.org/dpv/sector/law/owl#"/>
    <dct:created rdf:datatype="http://www.w3.org/2001/XMLSchema#date">2024-12-01</dct:created>
    <skos:prefLabel xml:lang="en">Crime Detection</skos:prefLabel>
    <sw:term_status xml:lang="en">accepted</sw:term_status>
    <rdfs:subClassOf rdf:resource="https://w3id.org/dpv/sector/law/owl#LegalOffenceDetection"/>
    <rdfs:subClassOf rdf:resource="https://w3id.org/dpv/sector/law/owl#CriminalLawEnforcement"/>
  </rdf:Description>
  <rdf:Description rdf:about="https://w3id.org/dpv/sector/law/owl#JudicialSystemManagement">
    <rdf:type rdf:resource="https://w3id.org/dpv/owl#Purpose"/>
    <rdf:type rdf:resource="http://www.w3.org/2000/01/rdf-schema#Class"/>
    <rdf:type rdf:resource="http://www.w3.org/2002/07/owl#Class"/>
    <dct:created rdf:datatype="http://www.w3.org/2001/XMLSchema#date">2024-12-01</dct:created>
    <skos:prefLabel xml:lang="en">Judicial System Management</skos:prefLabel>
    <skos:definition xml:lang="en">Purposes associated with administration and coordination of the operations, processes, and resources within the judicial system</skos:definition>
    <sw:term_status xml:lang="en">accepted</sw:term_status>
    <rdfs:isDefinedBy rdf:resource="https://w3id.org/dpv/sector/law/owl#"/>
    <rdfs:subClassOf rdf:resource="https://w3id.org/dpv/sector/law/owl#JusticeManagement"/>
  </rdf:Description>
  <rdf:Description rdf:about="https://w3id.org/dpv/sector/law/owl#RoadTrafficLawViolationDetection">
    <rdfs:isDefinedBy rdf:resource="https://w3id.org/dpv/sector/law/owl#"/>
    <skos:definition xml:lang="en">Purposes associated with detection of violations related to road traffic law</skos:definition>
    <sw:term_status xml:lang="en">accepted</sw:term_status>
    <rdf:type rdf:resource="https://w3id.org/dpv/owl#Purpose"/>
    <rdf:type rdf:resource="http://www.w3.org/2000/01/rdf-schema#Class"/>
    <rdf:type rdf:resource="http://www.w3.org/2002/07/owl#Class"/>
    <dct:created rdf:datatype="http://www.w3.org/2001/XMLSchema#date">2024-12-01</dct:created>
    <skos:prefLabel xml:lang="en">Road Traffic Law Violation Detection</skos:prefLabel>
    <rdfs:subClassOf rdf:resource="https://w3id.org/dpv/sector/law/owl#RoadTrafficLawEnforcement"/>
  </rdf:Description>
  <rdf:Description rdf:about="https://w3id.org/dpv/sector/law/owl#RoadTrafficSignalEnforcement">
    <sw:term_status xml:lang="en">accepted</sw:term_status>
    <skos:definition xml:lang="en">Purposes associated with detection and enforcement of traffic signals on roads</skos:definition>
    <rdf:type rdf:resource="https://w3id.org/dpv/owl#Purpose"/>
    <rdf:type rdf:resource="http://www.w3.org/2000/01/rdf-schema#Class"/>
    <rdf:type rdf:resource="http://www.w3.org/2002/07/owl#Class"/>
    <skos:prefLabel xml:lang="en">Road Traffic Signal Enforcement</skos:prefLabel>
    <dct:created rdf:datatype="http://www.w3.org/2001/XMLSchema#date">2024-12-01</dct:created>
    <rdfs:isDefinedBy rdf:resource="https://w3id.org/dpv/sector/law/owl#"/>
    <rdfs:subClassOf rdf:resource="https://w3id.org/dpv/sector/law/owl#RoadTrafficRuleEnforcement"/>
  </rdf:Description>
  <rdf:Description rdf:about="https://w3id.org/dpv/sector/law/owl#serialisation-n3">
    <profile:hasRole rdf:resource="http://www.w3.org/ns/dx/prof/role/vocabulary"/>
    <dct:format rdf:resource="https://www.iana.org/assignments/media-types/text/n3"/>
    <dct:conformsTo rdf:resource="https://www.w3.org/TeamSubmission/n3/"/>
    <rdf:type rdf:resource="http://www.w3.org/ns/dx/prof/ResourceDescriptor"/>
    <dct:title>Law Enforcement &amp; Justice Sector Concepts - N3 serialiation</dct:title>
    <profile:hasArtifact rdf:resource="https://w3id.org/dpv/sector/law/sector-law-owl.n3"/>
  </rdf:Description>
  <rdf:Description rdf:about="https://w3id.org/dpv/sector/law/owl#CriminalBehaviourDetection">
    <skos:prefLabel xml:lang="en">Criminal Behaviour Detection</skos:prefLabel>
    <rdfs:isDefinedBy rdf:resource="https://w3id.org/dpv/sector/law/owl#"/>
    <rdf:type rdf:resource="http://www.w3.org/2000/01/rdf-schema#Class"/>
    <rdf:type rdf:resource="https://w3id.org/dpv/owl#Purpose"/>
    <rdf:type rdf:resource="http://www.w3.org/2002/07/owl#Class"/>
    <sw:term_status xml:lang="en">accepted</sw:term_status>
    <skos:definition xml:lang="en">Purposes associated with detection of criminal behaviour within the legal system</skos:definition>
    <dct:created rdf:datatype="http://www.w3.org/2001/XMLSchema#date">2024-12-01</dct:created>
    <rdfs:subClassOf rdf:resource="https://w3id.org/dpv/sector/law/owl#CrimeDetection"/>
  </rdf:Description>
  <rdf:Description rdf:about="https://w3id.org/dpv/sector/law/owl#ImmigrationDecisionCommunication">
    <skos:prefLabel xml:lang="en">Immigration Decision Communication</skos:prefLabel>
    <rdf:type rdf:resource="https://w3id.org/dpv/owl#Purpose"/>
    <rdf:type rdf:resource="http://www.w3.org/2000/01/rdf-schema#Class"/>
    <rdf:type rdf:resource="http://www.w3.org/2002/07/owl#Class"/>
    <rdfs:isDefinedBy rdf:resource="https://w3id.org/dpv/sector/law/owl#"/>
    <skos:definition xml:lang="en">Purposes associated with communicating decisions for applications related to immigration within the legal system</skos:definition>
    <dct:created rdf:datatype="http://www.w3.org/2001/XMLSchema#date">2024-12-01</dct:created>
    <sw:term_status xml:lang="en">accepted</sw:term_status>
    <rdfs:subClassOf rdf:resource="https://w3id.org/dpv/sector/law/owl#ImmigrationRequestManagement"/>
  </rdf:Description>
  <rdf:Description rdf:about="https://w3id.org/dpv/sector/law/owl#ImmigrationApplicationScreening">
    <rdf:type rdf:resource="https://w3id.org/dpv/owl#Purpose"/>
    <rdf:type rdf:resource="http://www.w3.org/2000/01/rdf-schema#Class"/>
    <rdf:type rdf:resource="http://www.w3.org/2002/07/owl#Class"/>
    <dct:created rdf:datatype="http://www.w3.org/2001/XMLSchema#date">2024-12-01</dct:created>
    <skos:definition xml:lang="en">Purposes associated with screening or filtering applications related to immigration within the legal system</skos:definition>
    <skos:prefLabel xml:lang="en">Immigration Application Screening</skos:prefLabel>
    <rdfs:isDefinedBy rdf:resource="https://w3id.org/dpv/sector/law/owl#"/>
    <sw:term_status xml:lang="en">accepted</sw:term_status>
    <rdfs:subClassOf rdf:resource="https://w3id.org/dpv/sector/law/owl#ImmigrationApplicationManagement"/>
  </rdf:Description>
  <rdf:Description rdf:about="https://w3id.org/dpv/sector/law/owl#">
    <owl:versionIRI rdf:resource="https://w3id.org/dpv/2.1/sector/law/owl#"/>
    <profile:isProfileOf rdf:resource="https://w3id.org/dpv/owl"/>
    <profile:isProfileOf rdf:resource="http://www.w3.org/2002/07/owl"/>
    <profile:isProfileOf rdf:resource="https://w3id.org/dpv/sector/law/owl#"/>
    <profile:hasResource rdf:resource="https://w3id.org/dpv/sector/law/owl#serialisation-html"/>
    <profile:hasResource rdf:resource="https://w3id.org/dpv/examples"/>
    <profile:hasResource rdf:resource="https://w3id.org/dpv/guides"/>
    <profile:hasResource rdf:resource="https://w3id.org/dpv/sector/law/owl#serialisation-ttl"/>
    <profile:hasResource rdf:resource="https://w3id.org/dpv/sector/law/owl#serialisation-n3"/>
    <profile:hasResource rdf:resource="https://w3id.org/dpv/sector/law/owl#serialisation-jsonld"/>
    <profile:hasResource rdf:resource="https://w3id.org/dpv/sector/law/owl#serialisation-rdf"/>
    <profile:hasResource rdf:resource="https://w3id.org/dpv/primer"/>
    <dct:modified xml:lang="en">2025-02-01</dct:modified>
    <rdfs:Label xml:lang="en">SECTOR-LAW</rdfs:Label>
    <vann:preferredNamespacePrefix>sector-law</vann:preferredNamespacePrefix>
    <bibo:doi>10.5281/zenodo.12505841</bibo:doi>
    <dct:publisher rdf:resource="https://www.w3.org/"/>
    <bibo:status>http://purl.org/ontology/bibo/status/draft</bibo:status>
    <dct:issued xml:lang="en">2024-12-01</dct:issued>
    <dct:title xml:lang="en">Law Enforcement &amp; Justice Sector Concepts</dct:title>
    <dct:description xml:lang="en">Extension to the Data Privacy Vocabulary (DPV) providing concepts for the law enforcement and justice sector</dct:description>
    <owl:versionInfo>2.1</owl:versionInfo>
    <schema:version>2.1</schema:version>
    <dct:conformsTo>http://www.w3.org/2000/01/rdf-schema</dct:conformsTo>
    <dct:conformsTo>http://www.w3.org/2004/02/skos/core</dct:conformsTo>
    <dct:conformsTo rdf:resource="http://www.w3.org/2002/07/owl"/>
    <dct:identifier>https://w3id.org/dpv/sector/law</dct:identifier>
    <dct:source rdf:resource="https://www.w3.org/groups/cg/dpvcg/"/>
    <dct:creator rdf:nodeID="N2fe5586a82794e5a99ff2b47c1f2175e"/>
    <vann:preferredNamespaceUri>https://w3id.org/dpv/sector/law#</vann:preferredNamespaceUri>
    <dct:bibliographicCitation>Data Privacy Vocabulary (DPV) -- Version 2. Harshvardhan J. Pandit, Beatriz Esteves, Georg P. Krog, Paul Ryan, Delaram Golpayegani, Julian Flake https://doi.org/10.48550/arXiv.2404.13426</dct:bibliographicCitation>
    <dct:hasVersion rdf:resource="https://w3id.org/dpv/sector/law/owl#"/>
    <dct:license rdf:resource="https://www.w3.org/copyright/document-license-2023/"/>
    <dct:created xml:lang="en">2024-12-01</dct:created>
    <rdf:type rdf:resource="http://www.w3.org/2002/07/owl#Ontology"/>
    <rdf:type rdf:resource="http://www.w3.org/ns/dx/prof/Profile"/>
    <foaf:logo rdf:resource="https://w3id.org/dpv/media/logo.png"/>
  </rdf:Description>
  <rdf:Description rdf:about="https://w3id.org/dpv/sector/law/owl#JusticeManagement">
    <rdfs:isDefinedBy rdf:resource="https://w3id.org/dpv/sector/law/owl#"/>
    <rdf:type rdf:resource="http://www.w3.org/2000/01/rdf-schema#Class"/>
    <rdf:type rdf:resource="https://w3id.org/dpv/owl#Purpose"/>
    <rdf:type rdf:resource="http://www.w3.org/2002/07/owl#Class"/>
    <sw:term_status xml:lang="en">accepted</sw:term_status>
    <skos:prefLabel xml:lang="en">Justice Management</skos:prefLabel>
    <dct:created rdf:datatype="http://www.w3.org/2001/XMLSchema#date">2024-12-01</dct:created>
    <skos:definition xml:lang="en">Purposes associated with administration of justice within the legal system</skos:definition>
    <rdfs:subClassOf rdf:resource="https://w3id.org/dpv/owl#Purpose"/>
  </rdf:Description>
  <rdf:Description rdf:about="https://w3id.org/dpv/sector/law/owl#ImmigrationFraudManagement">
    <sw:term_status xml:lang="en">accepted</sw:term_status>
    <rdf:type rdf:resource="https://w3id.org/dpv/owl#Purpose"/>
    <rdf:type rdf:resource="http://www.w3.org/2000/01/rdf-schema#Class"/>
    <rdf:type rdf:resource="http://www.w3.org/2002/07/owl#Class"/>
    <skos:prefLabel xml:lang="en">Immigration Fraud Management</skos:prefLabel>
    <skos:definition xml:lang="en">Purposes associated with detection and prevention of fraud related to immigration within the legal system</skos:definition>
    <rdfs:isDefinedBy rdf:resource="https://w3id.org/dpv/sector/law/owl#"/>
    <dct:created rdf:datatype="http://www.w3.org/2001/XMLSchema#date">2024-12-01</dct:created>
    <rdfs:subClassOf rdf:resource="https://w3id.org/dpv/sector/law/owl#ImmigrationSecurityManagement"/>
  </rdf:Description>
  <rdf:Description rdf:about="https://w3id.org/dpv/sector/law/owl#ImmigrationEligibilityAssessment">
    <sw:term_status xml:lang="en">accepted</sw:term_status>
    <skos:definition xml:lang="en">Purposes associated with assessment of eligibility related to immigration within the legal system</skos:definition>
    <skos:prefLabel xml:lang="en">Immigration Eligibility Assessment</skos:prefLabel>
    <rdf:type rdf:resource="https://w3id.org/dpv/owl#Purpose"/>
    <rdf:type rdf:resource="http://www.w3.org/2000/01/rdf-schema#Class"/>
    <rdf:type rdf:resource="http://www.w3.org/2002/07/owl#Class"/>
    <rdfs:isDefinedBy rdf:resource="https://w3id.org/dpv/sector/law/owl#"/>
    <dct:created rdf:datatype="http://www.w3.org/2001/XMLSchema#date">2024-12-01</dct:created>
    <rdfs:subClassOf rdf:resource="https://w3id.org/dpv/sector/law/owl#ImmigrationRequestManagement"/>
  </rdf:Description>
  <rdf:Description rdf:about="https://w3id.org/dpv/sector/law/owl#ImmigrationApplicationCollection">
    <sw:term_status xml:lang="en">accepted</sw:term_status>
    <rdfs:isDefinedBy rdf:resource="https://w3id.org/dpv/sector/law/owl#"/>
    <dct:created rdf:datatype="http://www.w3.org/2001/XMLSchema#date">2024-12-01</dct:created>
    <skos:definition xml:lang="en">xPurposes associated with collection of applications related to immigration within the legal system</skos:definition>
    <rdf:type rdf:resource="https://w3id.org/dpv/owl#Purpose"/>
    <rdf:type rdf:resource="http://www.w3.org/2000/01/rdf-schema#Class"/>
    <rdf:type rdf:resource="http://www.w3.org/2002/07/owl#Class"/>
    <skos:prefLabel xml:lang="en">Immigration Application Collection</skos:prefLabel>
    <rdfs:subClassOf rdf:resource="https://w3id.org/dpv/sector/law/owl#ImmigrationApplicationManagement"/>
  </rdf:Description>
  <rdf:Description rdf:about="https://w3id.org/dpv/sector/law/owl#ImmigrationHealthRiskPrediction">
    <dct:created rdf:datatype="http://www.w3.org/2001/XMLSchema#date">2024-12-01</dct:created>
    <skos:prefLabel xml:lang="en">Immigration Health Risk Prediction</skos:prefLabel>
    <rdf:type rdf:resource="http://www.w3.org/2000/01/rdf-schema#Class"/>
    <rdf:type rdf:resource="https://w3id.org/dpv/owl#Purpose"/>
    <rdf:type rdf:resource="http://www.w3.org/2002/07/owl#Class"/>
    <rdfs:isDefinedBy rdf:resource="https://w3id.org/dpv/sector/law/owl#"/>
    <sw:term_status xml:lang="en">accepted</sw:term_status>
    <skos:definition xml:lang="en">Purposes related to predicting health risks as part of security related to immigration within the legal system</skos:definition>
    <rdfs:subClassOf rdf:resource="https://w3id.org/dpv/sector/law/owl#ImmigrationHealthRiskManagement"/>
  </rdf:Description>
  <rdf:Description rdf:about="https://w3id.org/dpv/sector/law/owl#PublicTransportSafetyMonitoring">
    <rdf:type rdf:resource="https://w3id.org/dpv/owl#Purpose"/>
    <rdf:type rdf:resource="http://www.w3.org/2000/01/rdf-schema#Class"/>
    <rdf:type rdf:resource="http://www.w3.org/2002/07/owl#Class"/>
    <dct:created rdf:datatype="http://www.w3.org/2001/XMLSchema#date">2024-12-01</dct:created>
    <skos:definition xml:lang="en">Purposes associated with monitoring public transport infrastructure and services for the purposes of public safety</skos:definition>
    <skos:prefLabel xml:lang="en">Public Transport Safety Monitoring</skos:prefLabel>
    <sw:term_status xml:lang="en">accepted</sw:term_status>
    <rdfs:isDefinedBy rdf:resource="https://w3id.org/dpv/sector/law/owl#"/>
    <rdfs:subClassOf rdf:resource="https://w3id.org/dpv/sector/law/owl#PublicTransportLawEnforcement"/>
  </rdf:Description>
  <rdf:Description rdf:about="https://w3id.org/dpv/sector/law/owl#ImmigrationApplicationAssessment">
    <skos:prefLabel xml:lang="en">Immigration Application Assessment</skos:prefLabel>
    <sw:term_status xml:lang="en">accepted</sw:term_status>
    <rdf:type rdf:resource="https://w3id.org/dpv/owl#Purpose"/>
    <rdf:type rdf:resource="http://www.w3.org/2000/01/rdf-schema#Class"/>
    <rdf:type rdf:resource="http://www.w3.org/2002/07/owl#Class"/>
    <skos:definition xml:lang="en">Purposes associated with assessment of applications for validity, determination of outcomes such as visa durations, and determining decisions such as visa approved related to immigration within the legal system</skos:definition>
    <dct:created rdf:datatype="http://www.w3.org/2001/XMLSchema#date">2024-12-01</dct:created>
    <rdfs:isDefinedBy rdf:resource="https://w3id.org/dpv/sector/law/owl#"/>
    <rdfs:subClassOf rdf:resource="https://w3id.org/dpv/sector/law/owl#ImmigrationApplicationManagement"/>
  </rdf:Description>
  <rdf:Description rdf:about="https://w3id.org/dpv/sector/law/owl#ImmigrationHealthRiskManagement">
    <sw:term_status xml:lang="en">accepted</sw:term_status>
    <skos:prefLabel xml:lang="en">Immigration Health Risk Management</skos:prefLabel>
    <skos:definition xml:lang="en">Purposes related to management of health risks as part of security related to immigration within the legal system</skos:definition>
    <rdf:type rdf:resource="https://w3id.org/dpv/owl#Purpose"/>
    <rdf:type rdf:resource="http://www.w3.org/2000/01/rdf-schema#Class"/>
    <rdf:type rdf:resource="http://www.w3.org/2002/07/owl#Class"/>
    <rdfs:isDefinedBy rdf:resource="https://w3id.org/dpv/sector/law/owl#"/>
    <dct:created rdf:datatype="http://www.w3.org/2001/XMLSchema#date">2024-12-01</dct:created>
    <rdfs:subClassOf rdf:resource="https://w3id.org/dpv/sector/law/owl#ImmigrationSecurityManagement"/>
  </rdf:Description>
  <rdf:Description rdf:about="https://w3id.org/dpv/sector/law/owl#CrimeVictimPrediction">
    <sw:term_status xml:lang="en">accepted</sw:term_status>
    <skos:prefLabel xml:lang="en">Crime Victim Prediction</skos:prefLabel>
    <rdf:type rdf:resource="https://w3id.org/dpv/owl#Purpose"/>
    <rdf:type rdf:resource="http://www.w3.org/2000/01/rdf-schema#Class"/>
    <rdf:type rdf:resource="http://www.w3.org/2002/07/owl#Class"/>
    <dct:created rdf:datatype="http://www.w3.org/2001/XMLSchema#date">2024-12-01</dct:created>
    <rdfs:isDefinedBy rdf:resource="https://w3id.org/dpv/sector/law/owl#"/>
    <skos:definition xml:lang="en">Purposes associated with predicting safety concerns or threats for victims of criminal activities within the legal system</skos:definition>
    <rdfs:subClassOf rdf:resource="https://w3id.org/dpv/sector/law/owl#CrimeVictimSafetyManagement"/>
  </rdf:Description>
  <rdf:Description rdf:about="https://w3id.org/dpv/sector/law/owl#ImmigrationBorderDocumentVerification">
    <dct:created rdf:datatype="http://www.w3.org/2001/XMLSchema#date">2024-12-01</dct:created>
    <rdf:type rdf:resource="https://w3id.org/dpv/owl#Purpose"/>
    <rdf:type rdf:resource="http://www.w3.org/2000/01/rdf-schema#Class"/>
    <rdf:type rdf:resource="http://www.w3.org/2002/07/owl#Class"/>
    <skos:definition xml:lang="en">Purposes associated with verification of documents and information at the border as defined in the legal system</skos:definition>
    <rdfs:isDefinedBy rdf:resource="https://w3id.org/dpv/sector/law/owl#"/>
    <skos:prefLabel xml:lang="en">Immigration Border Document Verification</skos:prefLabel>
    <sw:term_status xml:lang="en">accepted</sw:term_status>
    <rdfs:subClassOf rdf:resource="https://w3id.org/dpv/sector/law/owl#ImmigrationBorderControlManagement"/>
  </rdf:Description>
  <rdf:Description rdf:about="https://w3id.org/dpv/sector/law/owl#RoadTrafficRuleEnforcement">
    <rdf:type rdf:resource="https://w3id.org/dpv/owl#Purpose"/>
    <rdf:type rdf:resource="http://www.w3.org/2000/01/rdf-schema#Class"/>
    <rdf:type rdf:resource="http://www.w3.org/2002/07/owl#Class"/>
    <dct:created rdf:datatype="http://www.w3.org/2001/XMLSchema#date">2024-12-01</dct:created>
    <skos:prefLabel xml:lang="en">Road Traffic Rule Enforcement</skos:prefLabel>
    <rdfs:isDefinedBy rdf:resource="https://w3id.org/dpv/sector/law/owl#"/>
    <skos:definition xml:lang="en">Purposes associated with detection and enforcement of traffic rules on roads</skos:definition>
    <sw:term_status xml:lang="en">accepted</sw:term_status>
    <rdfs:subClassOf rdf:resource="https://w3id.org/dpv/sector/law/owl#RoadTrafficLawEnforcement"/>
  </rdf:Description>
  <rdf:Description rdf:nodeID="Nfbd61e1f087d467e81291e0c311268a5">
    <foaf:name>ADAPT Centre, Dublin City University</foaf:name>
    <rdf:type rdf:resource="http://xmlns.com/foaf/0.1/Organization"/>
  </rdf:Description>
  <rdf:Description rdf:about="https://w3id.org/dpv/sector/law/owl#RoadVehicleRegistrationEnforcement">
    <rdf:type rdf:resource="https://w3id.org/dpv/owl#Purpose"/>
    <rdf:type rdf:resource="http://www.w3.org/2000/01/rdf-schema#Class"/>
    <rdf:type rdf:resource="http://www.w3.org/2002/07/owl#Class"/>
    <dct:created rdf:datatype="http://www.w3.org/2001/XMLSchema#date">2024-12-01</dct:created>
    <rdfs:isDefinedBy rdf:resource="https://w3id.org/dpv/sector/law/owl#"/>
    <sw:term_status xml:lang="en">accepted</sw:term_status>
    <skos:definition xml:lang="en">Purposes associated with detection and enforcement of road vehicle registration</skos:definition>
    <skos:prefLabel xml:lang="en">Road Vehicle Registration Enforcement</skos:prefLabel>
    <rdfs:subClassOf rdf:resource="https://w3id.org/dpv/sector/law/owl#RoadTrafficLawEnforcement"/>
  </rdf:Description>
  <rdf:Description rdf:about="https://w3id.org/dpv/sector/law/owl#CrimeArrestDetention">
    <skos:prefLabel xml:lang="en">Crime Arrest Detention</skos:prefLabel>
    <sw:term_status xml:lang="en">accepted</sw:term_status>
    <rdf:type rdf:resource="https://w3id.org/dpv/owl#Purpose"/>
    <rdf:type rdf:resource="http://www.w3.org/2000/01/rdf-schema#Class"/>
    <rdf:type rdf:resource="http://www.w3.org/2002/07/owl#Class"/>
    <skos:definition xml:lang="en">Purposes associated with arresting and detention of individuals in relation to criminal activities within the legal system</skos:definition>
    <rdfs:isDefinedBy rdf:resource="https://w3id.org/dpv/sector/law/owl#"/>
    <dct:created rdf:datatype="http://www.w3.org/2001/XMLSchema#date">2024-12-01</dct:created>
    <rdfs:subClassOf rdf:resource="https://w3id.org/dpv/sector/law/owl#CriminalLawEnforcement"/>
  </rdf:Description>
  <rdf:Description rdf:about="https://w3id.org/dpv/sector/law/owl#ImmigrationMigrationManagement">
    <skos:prefLabel xml:lang="en">Immigration Migration Management</skos:prefLabel>
    <sw:term_status xml:lang="en">accepted</sw:term_status>
    <rdf:type rdf:resource="https://w3id.org/dpv/owl#Purpose"/>
    <rdf:type rdf:resource="http://www.w3.org/2000/01/rdf-schema#Class"/>
    <rdf:type rdf:resource="http://www.w3.org/2002/07/owl#Class"/>
    <skos:definition xml:lang="en">Purposes associated with management of requests or petitions for migration including collecting and processing of applications, determining elibility, making and communicating decisions, and enforcing the limits as related to immigration within the legal system</skos:definition>
    <rdfs:isDefinedBy rdf:resource="https://w3id.org/dpv/sector/law/owl#"/>
    <dct:created rdf:datatype="http://www.w3.org/2001/XMLSchema#date">2024-12-01</dct:created>
    <rdfs:subClassOf rdf:resource="https://w3id.org/dpv/sector/law/owl#ImmigrationManagement"/>
  </rdf:Description>
  <rdf:Description rdf:about="https://w3id.org/dpv/sector/law/owl#UnauthorisedMigrationDetection">
    <dct:created rdf:datatype="http://www.w3.org/2001/XMLSchema#date">2024-12-01</dct:created>
    <skos:prefLabel xml:lang="en">Unauthorised Migration Detection</skos:prefLabel>
    <rdf:type rdf:resource="https://w3id.org/dpv/owl#Purpose"/>
    <rdf:type rdf:resource="http://www.w3.org/2000/01/rdf-schema#Class"/>
    <rdf:type rdf:resource="http://www.w3.org/2002/07/owl#Class"/>
    <rdfs:isDefinedBy rdf:resource="https://w3id.org/dpv/sector/law/owl#"/>
    <sw:term_status xml:lang="en">accepted</sw:term_status>
    <skos:definition xml:lang="en">Puposes associated with detecting unauthorised migration within the legal system</skos:definition>
    <rdfs:subClassOf rdf:resource="https://w3id.org/dpv/sector/law/owl#UnauthorisedMigrationManagement"/>
  </rdf:Description>
  <rdf:Description rdf:about="https://w3id.org/dpv/sector/law/owl#ImmigrationSecurityManagement">
    <rdf:type rdf:resource="https://w3id.org/dpv/owl#Purpose"/>
    <rdf:type rdf:resource="http://www.w3.org/2000/01/rdf-schema#Class"/>
    <rdf:type rdf:resource="http://www.w3.org/2002/07/owl#Class"/>
    <skos:prefLabel xml:lang="en">Immigration Security Management</skos:prefLabel>
    <skos:definition xml:lang="en">Purposes related to management of security related to immigration within the legal system</skos:definition>
    <sw:term_status xml:lang="en">accepted</sw:term_status>
    <rdfs:isDefinedBy rdf:resource="https://w3id.org/dpv/sector/law/owl#"/>
    <dct:created rdf:datatype="http://www.w3.org/2001/XMLSchema#date">2024-12-01</dct:created>
    <rdfs:subClassOf rdf:resource="https://w3id.org/dpv/sector/law/owl#ImmigrationManagement"/>
  </rdf:Description>
  <rdf:Description rdf:about="https://w3id.org/dpv/sector/law/owl#LawEnforcement">
    <skos:prefLabel xml:lang="en">Law Enforcement</skos:prefLabel>
    <rdf:type rdf:resource="http://www.w3.org/2000/01/rdf-schema#Class"/>
    <rdf:type rdf:resource="https://w3id.org/dpv/owl#Purpose"/>
    <rdf:type rdf:resource="http://www.w3.org/2002/07/owl#Class"/>
    <rdfs:isDefinedBy rdf:resource="https://w3id.org/dpv/sector/law/owl#"/>
    <dct:created rdf:datatype="http://www.w3.org/2001/XMLSchema#date">2024-12-01</dct:created>
    <sw:term_status xml:lang="en">accepted</sw:term_status>
    <skos:definition xml:lang="en">Purposes associated with law enforcement within the legal system</skos:definition>
    <rdfs:subClassOf rdf:resource="https://w3id.org/dpv/sector/law/owl#JusticeManagement"/>
  </rdf:Description>
  <rdf:Description rdf:about="https://w3id.org/dpv/sector/law/owl#ImmigrationManagement">
    <rdf:type rdf:resource="https://w3id.org/dpv/owl#Purpose"/>
    <rdf:type rdf:resource="http://www.w3.org/2000/01/rdf-schema#Class"/>
    <rdf:type rdf:resource="http://www.w3.org/2002/07/owl#Class"/>
    <skos:prefLabel xml:lang="en">Immigration Management</skos:prefLabel>
    <dct:created rdf:datatype="http://www.w3.org/2001/XMLSchema#date">2024-12-01</dct:created>
    <skos:definition xml:lang="en">Purposes associated with management of immigration within the legal system</skos:definition>
    <sw:term_status xml:lang="en">accepted</sw:term_status>
    <rdfs:isDefinedBy rdf:resource="https://w3id.org/dpv/sector/law/owl#"/>
    <rdfs:subClassOf rdf:resource="https://w3id.org/dpv/sector/law/owl#JusticeManagement"/>
  </rdf:Description>
  <rdf:Description rdf:about="https://w3id.org/dpv/sector/law/owl#serialisation-rdf">
    <rdf:type rdf:resource="http://www.w3.org/ns/dx/prof/ResourceDescriptor"/>
    <dct:format rdf:resource="https://www.iana.org/assignments/media-types/application/rdf+xml"/>
    <dct:conformsTo rdf:resource="http://www.w3.org/1999/02/22-rdf-syntax-ns#"/>
    <dct:title>Law Enforcement &amp; Justice Sector Concepts - RDF/XML serialiation</dct:title>
    <profile:hasArtifact rdf:resource="https://w3id.org/dpv/sector/law/sector-law-owl.rdf"/>
    <profile:hasRole rdf:resource="http://www.w3.org/ns/dx/prof/role/vocabulary"/>
  </rdf:Description>
  <rdf:Description rdf:about="https://w3id.org/dpv/sector/law/owl#JudicialCaseManagement">
    <dct:created rdf:datatype="http://www.w3.org/2001/XMLSchema#date">2024-12-01</dct:created>
    <skos:definition xml:lang="en">Purposes associated with management of cases within the judicial system</skos:definition>
    <sw:term_status xml:lang="en">accepted</sw:term_status>
    <rdf:type rdf:resource="https://w3id.org/dpv/owl#Purpose"/>
    <rdf:type rdf:resource="http://www.w3.org/2000/01/rdf-schema#Class"/>
    <rdf:type rdf:resource="http://www.w3.org/2002/07/owl#Class"/>
    <skos:prefLabel xml:lang="en">Judicial Case Management</skos:prefLabel>
    <rdfs:isDefinedBy rdf:resource="https://w3id.org/dpv/sector/law/owl#"/>
    <rdfs:subClassOf rdf:resource="https://w3id.org/dpv/sector/law/owl#JudicialSystemManagement"/>
  </rdf:Description>
  <rdf:Description rdf:about="https://w3id.org/dpv/sector/law/owl#RoadParkingEnforcement">
    <rdf:type rdf:resource="https://w3id.org/dpv/owl#Purpose"/>
    <rdf:type rdf:resource="http://www.w3.org/2000/01/rdf-schema#Class"/>
    <rdf:type rdf:resource="http://www.w3.org/2002/07/owl#Class"/>
    <skos:definition xml:lang="en">Purposes associated with detection and enforcement of parking rules on roads</skos:definition>
    <rdfs:isDefinedBy rdf:resource="https://w3id.org/dpv/sector/law/owl#"/>
    <skos:prefLabel xml:lang="en">Road Parking Enforcement</skos:prefLabel>
    <dct:created rdf:datatype="http://www.w3.org/2001/XMLSchema#date">2024-12-01</dct:created>
    <sw:term_status xml:lang="en">accepted</sw:term_status>
    <rdfs:subClassOf rdf:resource="https://w3id.org/dpv/sector/law/owl#RoadTrafficRuleEnforcement"/>
  </rdf:Description>
  <rdf:Description rdf:about="https://w3id.org/dpv/sector/law/owl#CrimeSurveillance">
    <skos:definition xml:lang="en">Purposes associated with monitoring or observing to detect or deter potential or ongoing criminal activities within the legal system</skos:definition>
    <rdf:type rdf:resource="http://www.w3.org/2000/01/rdf-schema#Class"/>
    <rdf:type rdf:resource="https://w3id.org/dpv/owl#Purpose"/>
    <rdf:type rdf:resource="http://www.w3.org/2002/07/owl#Class"/>
    <skos:prefLabel xml:lang="en">Crime Surveillance</skos:prefLabel>
    <sw:term_status xml:lang="en">accepted</sw:term_status>
    <rdfs:isDefinedBy rdf:resource="https://w3id.org/dpv/sector/law/owl#"/>
    <dct:created rdf:datatype="http://www.w3.org/2001/XMLSchema#date">2024-12-01</dct:created>
    <rdfs:subClassOf rdf:resource="https://w3id.org/dpv/sector/law/owl#CriminalLawEnforcement"/>
    <rdfs:subClassOf rdf:resource="https://w3id.org/dpv/sector/law/owl#LegalOffenceSurveillance"/>
  </rdf:Description>
  <rdf:Description rdf:about="https://w3id.org/dpv/sector/law/owl#ImmigrationResidencyPermitManagement">
    <rdfs:isDefinedBy rdf:resource="https://w3id.org/dpv/sector/law/owl#"/>
    <skos:prefLabel xml:lang="en">Immigration Residency Permit Management</skos:prefLabel>
    <rdf:type rdf:resource="http://www.w3.org/2000/01/rdf-schema#Class"/>
    <rdf:type rdf:resource="https://w3id.org/dpv/owl#Purpose"/>
    <rdf:type rdf:resource="http://www.w3.org/2002/07/owl#Class"/>
    <sw:term_status xml:lang="en">accepted</sw:term_status>
    <skos:definition xml:lang="en">Purposes associated with management of residency permits, including collecting and processing of applications, determining elibility, making and communicating decisions, and enforcing the limits as related to immigration within the legal system</skos:definition>
    <dct:created rdf:datatype="http://www.w3.org/2001/XMLSchema#date">2024-12-01</dct:created>
    <rdfs:subClassOf rdf:resource="https://w3id.org/dpv/sector/law/owl#ImmigrationManagement"/>
  </rdf:Description>
  <rdf:Description rdf:about="https://w3id.org/dpv/sector/law/owl#LegalOffenceProsecution">
    <rdfs:isDefinedBy rdf:resource="https://w3id.org/dpv/sector/law/owl#"/>
    <dct:created rdf:datatype="http://www.w3.org/2001/XMLSchema#date">2024-12-01</dct:created>
    <rdf:type rdf:resource="http://www.w3.org/2000/01/rdf-schema#Class"/>
    <rdf:type rdf:resource="https://w3id.org/dpv/owl#Purpose"/>
    <rdf:type rdf:resource="http://www.w3.org/2002/07/owl#Class"/>
    <sw:term_status xml:lang="en">accepted</sw:term_status>
    <skos:definition xml:lang="en">Purposes associated with prosecution of illegal activities or violations or offences within the legal system</skos:definition>
    <skos:prefLabel xml:lang="en">Legal Offence Prosecution</skos:prefLabel>
    <rdfs:subClassOf rdf:resource="https://w3id.org/dpv/sector/law/owl#LawEnforcement"/>
  </rdf:Description>
  <rdf:Description rdf:about="https://w3id.org/dpv/sector/law/owl#UnauthorisedMigrationPrediction">
    <rdfs:isDefinedBy rdf:resource="https://w3id.org/dpv/sector/law/owl#"/>
    <skos:prefLabel xml:lang="en">Unauthorised Migration Prediction</skos:prefLabel>
    <sw:term_status xml:lang="en">accepted</sw:term_status>
    <rdf:type rdf:resource="https://w3id.org/dpv/owl#Purpose"/>
    <rdf:type rdf:resource="http://www.w3.org/2000/01/rdf-schema#Class"/>
    <rdf:type rdf:resource="http://www.w3.org/2002/07/owl#Class"/>
    <dct:created rdf:datatype="http://www.w3.org/2001/XMLSchema#date">2024-12-01</dct:created>
    <skos:definition xml:lang="en">Puposes associated with predicting unauthorised migration within the legal system</skos:definition>
    <rdfs:subClassOf rdf:resource="https://w3id.org/dpv/sector/law/owl#UnauthorisedMigrationManagement"/>
  </rdf:Description>
  <rdf:Description rdf:about="https://w3id.org/dpv/sector/law/owl#CrimeVictimSafetyProvision">
    <rdf:type rdf:resource="http://www.w3.org/2000/01/rdf-schema#Class"/>
    <rdf:type rdf:resource="https://w3id.org/dpv/owl#Purpose"/>
    <rdf:type rdf:resource="http://www.w3.org/2002/07/owl#Class"/>
    <skos:definition xml:lang="en">Purposes associated with managing and providing safety for victims of criminal activities within the legal system</skos:definition>
    <rdfs:isDefinedBy rdf:resource="https://w3id.org/dpv/sector/law/owl#"/>
    <sw:term_status xml:lang="en">accepted</sw:term_status>
    <skos:prefLabel xml:lang="en">Crime Victim Safety Provision</skos:prefLabel>
    <dct:created rdf:datatype="http://www.w3.org/2001/XMLSchema#date">2024-12-01</dct:created>
    <rdfs:subClassOf rdf:resource="https://w3id.org/dpv/sector/law/owl#CrimeVictimSafetyManagement"/>
  </rdf:Description>
  <rdf:Description rdf:about="https://w3id.org/dpv/sector/law/owl#LegalInterrogation">
    <sw:term_status xml:lang="en">accepted</sw:term_status>
    <rdfs:isDefinedBy rdf:resource="https://w3id.org/dpv/sector/law/owl#"/>
    <rdf:type rdf:resource="https://w3id.org/dpv/owl#Purpose"/>
    <rdf:type rdf:resource="http://www.w3.org/2000/01/rdf-schema#Class"/>
    <rdf:type rdf:resource="http://www.w3.org/2002/07/owl#Class"/>
    <dct:created rdf:datatype="http://www.w3.org/2001/XMLSchema#date">2024-12-01</dct:created>
    <skos:definition xml:lang="en">Purposes associated with questioning of individuals in relation to an investigation or other matters within the legal system</skos:definition>
    <skos:prefLabel xml:lang="en">Legal Interrogation</skos:prefLabel>
    <rdfs:subClassOf rdf:resource="https://w3id.org/dpv/sector/law/owl#LegalInvestigation"/>
  </rdf:Description>
  <rdf:Description rdf:about="https://w3id.org/dpv/sector/law/owl#ImmigrationClaimVerification">
    <rdf:type rdf:resource="http://www.w3.org/2000/01/rdf-schema#Class"/>
    <rdf:type rdf:resource="https://w3id.org/dpv/owl#Purpose"/>
    <rdf:type rdf:resource="http://www.w3.org/2002/07/owl#Class"/>
    <skos:definition xml:lang="en">Purposes associated with verification of claims, such as background, history, and past life related to immigration within the legal system</skos:definition>
    <sw:term_status xml:lang="en">accepted</sw:term_status>
    <rdfs:isDefinedBy rdf:resource="https://w3id.org/dpv/sector/law/owl#"/>
    <skos:prefLabel xml:lang="en">Immigration Claim Verification</skos:prefLabel>
    <dct:created rdf:datatype="http://www.w3.org/2001/XMLSchema#date">2024-12-01</dct:created>
    <rdfs:subClassOf rdf:resource="https://w3id.org/dpv/sector/law/owl#ImmigrationRequestManagement"/>
  </rdf:Description>
  <rdf:Description rdf:about="https://w3id.org/dpv/sector/law/owl#UnauthorisedMigrationManagement">
    <rdf:type rdf:resource="http://www.w3.org/2000/01/rdf-schema#Class"/>
    <rdf:type rdf:resource="https://w3id.org/dpv/owl#Purpose"/>
    <rdf:type rdf:resource="http://www.w3.org/2002/07/owl#Class"/>
    <sw:term_status xml:lang="en">accepted</sw:term_status>
    <skos:definition xml:lang="en">Puposes associated with detection, prevention, and management of unauthorised migration within the legal system</skos:definition>
    <dct:created rdf:datatype="http://www.w3.org/2001/XMLSchema#date">2024-12-01</dct:created>
    <rdfs:isDefinedBy rdf:resource="https://w3id.org/dpv/sector/law/owl#"/>
    <skos:prefLabel xml:lang="en">Unauthorised Migration Management</skos:prefLabel>
    <rdfs:subClassOf rdf:resource="https://w3id.org/dpv/sector/law/owl#ImmigrationSecurityManagement"/>
  </rdf:Description>
  <rdf:Description rdf:about="https://w3id.org/dpv/sector/law/owl#serialisation-ttl">
    <dct:title>Law Enforcement &amp; Justice Sector Concepts - Turtle serialiation</dct:title>
    <profile:hasArtifact rdf:resource="https://w3id.org/dpv/sector/law/sector-law-owl.ttl"/>
    <dct:format rdf:resource="https://www.iana.org/assignments/media-types/text/turtle"/>
    <profile:hasRole rdf:resource="http://www.w3.org/ns/dx/prof/role/vocabulary"/>
    <dct:conformsTo rdf:resource="https://www.w3.org/TR/turtle/"/>
    <rdf:type rdf:resource="http://www.w3.org/ns/dx/prof/ResourceDescriptor"/>
  </rdf:Description>
  <rdf:Description rdf:about="https://w3id.org/dpv/sector/law/owl#RoadTrafficLawEnforcement">
    <rdf:type rdf:resource="https://w3id.org/dpv/owl#Purpose"/>
    <rdf:type rdf:resource="http://www.w3.org/2000/01/rdf-schema#Class"/>
    <rdf:type rdf:resource="http://www.w3.org/2002/07/owl#Class"/>
    <skos:prefLabel xml:lang="en">Road Traffic Law Enforcement</skos:prefLabel>
    <dct:created rdf:datatype="http://www.w3.org/2001/XMLSchema#date">2024-12-01</dct:created>
    <rdfs:isDefinedBy rdf:resource="https://w3id.org/dpv/sector/law/owl#"/>
    <skos:definition xml:lang="en">Purposes associated with law enforcement related to road infrastructure and services</skos:definition>
    <sw:term_status xml:lang="en">accepted</sw:term_status>
    <rdfs:subClassOf rdf:resource="https://w3id.org/dpv/sector/law/owl#TransportLawEnforcement"/>
  </rdf:Description>
  <rdf:Description rdf:about="https://w3id.org/dpv/sector/law/owl#CrimeInvestigation">
    <rdf:type rdf:resource="http://www.w3.org/2000/01/rdf-schema#Class"/>
    <rdf:type rdf:resource="https://w3id.org/dpv/owl#Purpose"/>
    <rdf:type rdf:resource="http://www.w3.org/2002/07/owl#Class"/>
    <rdfs:isDefinedBy rdf:resource="https://w3id.org/dpv/sector/law/owl#"/>
    <dct:created rdf:datatype="http://www.w3.org/2001/XMLSchema#date">2024-12-01</dct:created>
    <sw:term_status xml:lang="en">accepted</sw:term_status>
    <skos:definition xml:lang="en">Purposes associated with investigation of crimes within the legal system</skos:definition>
    <skos:prefLabel xml:lang="en">Crime Investigation</skos:prefLabel>
    <rdfs:subClassOf rdf:resource="https://w3id.org/dpv/sector/law/owl#CriminalLawEnforcement"/>
    <rdfs:subClassOf rdf:resource="https://w3id.org/dpv/sector/law/owl#LegalInvestigation"/>
  </rdf:Description>
  <rdf:Description rdf:about="https://w3id.org/dpv/sector/law/owl#ImmigrationExpiredPermitManagement">
    <rdf:type rdf:resource="https://w3id.org/dpv/owl#Purpose"/>
    <rdf:type rdf:resource="http://www.w3.org/2000/01/rdf-schema#Class"/>
    <rdf:type rdf:resource="http://www.w3.org/2002/07/owl#Class"/>
    <dct:created rdf:datatype="http://www.w3.org/2001/XMLSchema#date">2024-12-01</dct:created>
    <rdfs:isDefinedBy rdf:resource="https://w3id.org/dpv/sector/law/owl#"/>
    <skos:definition xml:lang="en">Purposes associated with management of expired visas, authorisations, and other permits related to immigration within the legal system</skos:definition>
    <skos:prefLabel xml:lang="en">Immigration Expired Permit Management</skos:prefLabel>
    <sw:term_status xml:lang="en">accepted</sw:term_status>
    <rdfs:subClassOf rdf:resource="https://w3id.org/dpv/sector/law/owl#ImmigrationSecurityManagement"/>
  </rdf:Description>
  <rdf:Description rdf:about="https://w3id.org/dpv/sector/law/owl#PublicTransportFraudManagement">
    <skos:definition xml:lang="en">Purposes associated with fraud prevention and detection and management related to public transport infrastructure and services</skos:definition>
    <dct:created rdf:datatype="http://www.w3.org/2001/XMLSchema#date">2024-12-01</dct:created>
    <rdf:type rdf:resource="http://www.w3.org/2000/01/rdf-schema#Class"/>
    <rdf:type rdf:resource="https://w3id.org/dpv/owl#Purpose"/>
    <rdf:type rdf:resource="http://www.w3.org/2002/07/owl#Class"/>
    <skos:prefLabel xml:lang="en">Public Transport Fraud Management</skos:prefLabel>
    <rdfs:isDefinedBy rdf:resource="https://w3id.org/dpv/sector/law/owl#"/>
    <sw:term_status xml:lang="en">accepted</sw:term_status>
    <rdfs:subClassOf rdf:resource="https://w3id.org/dpv/sector/law/owl#PublicTransportLawEnforcement"/>
  </rdf:Description>
  <rdf:Description rdf:about="https://w3id.org/dpv/sector/law/owl#LegalEvidenceInterpretation">
    <rdf:type rdf:resource="http://www.w3.org/2000/01/rdf-schema#Class"/>
    <rdf:type rdf:resource="https://w3id.org/dpv/owl#Purpose"/>
    <rdf:type rdf:resource="http://www.w3.org/2002/07/owl#Class"/>
    <rdfs:isDefinedBy rdf:resource="https://w3id.org/dpv/sector/law/owl#"/>
    <skos:prefLabel xml:lang="en">Legal Evidence Interpretation</skos:prefLabel>
    <sw:term_status xml:lang="en">accepted</sw:term_status>
    <skos:definition xml:lang="en">Purposes associated with interpretation of evidence for investigation within the legal system</skos:definition>
    <dct:created rdf:datatype="http://www.w3.org/2001/XMLSchema#date">2024-12-01</dct:created>
    <rdfs:subClassOf rdf:resource="https://w3id.org/dpv/sector/law/owl#LegalInvestigation"/>
  </rdf:Description>
  <rdf:Description rdf:about="https://w3id.org/dpv/sector/law/owl#PrisonManagement">
    <skos:definition xml:lang="en">Purposes associated with management of prison institutions part of the legal system</skos:definition>
    <rdf:type rdf:resource="https://w3id.org/dpv/owl#Purpose"/>
    <rdf:type rdf:resource="http://www.w3.org/2000/01/rdf-schema#Class"/>
    <rdf:type rdf:resource="http://www.w3.org/2002/07/owl#Class"/>
    <rdfs:isDefinedBy rdf:resource="https://w3id.org/dpv/sector/law/owl#"/>
    <skos:prefLabel xml:lang="en">Prison Management</skos:prefLabel>
    <dct:created rdf:datatype="http://www.w3.org/2001/XMLSchema#date">2024-12-01</dct:created>
    <sw:term_status xml:lang="en">accepted</sw:term_status>
    <rdfs:subClassOf rdf:resource="https://w3id.org/dpv/sector/law/owl#LegalInstitutionalManagement"/>
  </rdf:Description>
  <rdf:Description rdf:about="https://w3id.org/dpv/sector/law/owl#RoadTrafficLawViolationFineCollection">
    <rdfs:isDefinedBy rdf:resource="https://w3id.org/dpv/sector/law/owl#"/>
    <dct:created rdf:datatype="http://www.w3.org/2001/XMLSchema#date">2024-12-01</dct:created>
    <skos:definition xml:lang="en">Purposes associated with managing payment and collection of fines related to violations of road traffic law</skos:definition>
    <sw:term_status xml:lang="en">accepted</sw:term_status>
    <rdf:type rdf:resource="https://w3id.org/dpv/owl#Purpose"/>
    <rdf:type rdf:resource="http://www.w3.org/2000/01/rdf-schema#Class"/>
    <rdf:type rdf:resource="http://www.w3.org/2002/07/owl#Class"/>
    <skos:prefLabel xml:lang="en">Road Traffic Law Violation Fine Collection</skos:prefLabel>
    <rdfs:subClassOf rdf:resource="https://w3id.org/dpv/sector/law/owl#RoadTrafficLawEnforcement"/>
  </rdf:Description>
  <rdf:Description rdf:about="https://w3id.org/dpv/sector/law/owl#CrimeVictimSafetyManagement">
    <rdf:type rdf:resource="https://w3id.org/dpv/owl#Purpose"/>
    <rdf:type rdf:resource="http://www.w3.org/2000/01/rdf-schema#Class"/>
    <rdf:type rdf:resource="http://www.w3.org/2002/07/owl#Class"/>
    <rdfs:isDefinedBy rdf:resource="https://w3id.org/dpv/sector/law/owl#"/>
    <dct:created rdf:datatype="http://www.w3.org/2001/XMLSchema#date">2024-12-01</dct:created>
    <skos:definition xml:lang="en">Purposes associated with management of safety for victims of criminal activities within the legal system</skos:definition>
    <sw:term_status xml:lang="en">accepted</sw:term_status>
    <skos:prefLabel xml:lang="en">Crime Victim Safety Management</skos:prefLabel>
    <rdfs:subClassOf rdf:resource="https://w3id.org/dpv/sector/law/owl#CriminalLawEnforcement"/>
  </rdf:Description>
  <rdf:Description rdf:about="https://w3id.org/dpv/sector/law/owl#LegalInstitutionalManagement">
    <sw:term_status xml:lang="en">accepted</sw:term_status>
    <skos:definition xml:lang="en">Purposes associated with management of institutions part of the legal system</skos:definition>
    <rdf:type rdf:resource="https://w3id.org/dpv/owl#Purpose"/>
    <rdf:type rdf:resource="http://www.w3.org/2000/01/rdf-schema#Class"/>
    <rdf:type rdf:resource="http://www.w3.org/2002/07/owl#Class"/>
    <skos:prefLabel xml:lang="en">Legal Institutional Management</skos:prefLabel>
    <rdfs:isDefinedBy rdf:resource="https://w3id.org/dpv/sector/law/owl#"/>
    <dct:created rdf:datatype="http://www.w3.org/2001/XMLSchema#date">2024-12-01</dct:created>
    <rdfs:subClassOf rdf:resource="https://w3id.org/dpv/sector/law/owl#JusticeManagement"/>
  </rdf:Description>
  <rdf:Description rdf:about="https://w3id.org/dpv/sector/law/owl#JudicialRecordKeeping">
    <rdf:type rdf:resource="http://www.w3.org/2000/01/rdf-schema#Class"/>
    <rdf:type rdf:resource="https://w3id.org/dpv/owl#Purpose"/>
    <rdf:type rdf:resource="http://www.w3.org/2002/07/owl#Class"/>
    <skos:definition xml:lang="en">Purposes associated with record keeping within the judicial system</skos:definition>
    <rdfs:isDefinedBy rdf:resource="https://w3id.org/dpv/sector/law/owl#"/>
    <dct:created rdf:datatype="http://www.w3.org/2001/XMLSchema#date">2024-12-01</dct:created>
    <sw:term_status xml:lang="en">accepted</sw:term_status>
    <skos:prefLabel xml:lang="en">Judicial Record Keeping</skos:prefLabel>
    <rdfs:subClassOf rdf:resource="https://w3id.org/dpv/sector/law/owl#JudicialSystemManagement"/>
  </rdf:Description>
  <rdf:Description rdf:about="https://w3id.org/dpv/sector/law/owl#LegalResearchDevelopment">
    <dct:created rdf:datatype="http://www.w3.org/2001/XMLSchema#date">2024-12-01</dct:created>
    <rdfs:isDefinedBy rdf:resource="https://w3id.org/dpv/sector/law/owl#"/>
    <skos:prefLabel xml:lang="en">Legal Research Development</skos:prefLabel>
    <rdf:type rdf:resource="http://www.w3.org/2000/01/rdf-schema#Class"/>
    <rdf:type rdf:resource="https://w3id.org/dpv/owl#Purpose"/>
    <rdf:type rdf:resource="http://www.w3.org/2002/07/owl#Class"/>
    <sw:term_status xml:lang="en">accepted</sw:term_status>
    <skos:definition xml:lang="en">Purposes associated with research and development within the legal system</skos:definition>
    <rdfs:subClassOf rdf:resource="https://w3id.org/dpv/sector/law/owl#LawEnforcement"/>
  </rdf:Description>
  <rdf:Description rdf:about="https://w3id.org/dpv/sector/law/owl#SuspectedCrimeInvestigation">
    <rdf:type rdf:resource="http://www.w3.org/2000/01/rdf-schema#Class"/>
    <rdf:type rdf:resource="https://w3id.org/dpv/owl#Purpose"/>
    <rdf:type rdf:resource="http://www.w3.org/2002/07/owl#Class"/>
    <sw:term_status xml:lang="en">accepted</sw:term_status>
    <skos:definition xml:lang="en">Purposes associated with investigation of suspected crimes within the legal system</skos:definition>
    <skos:prefLabel xml:lang="en">Suspected Crime Investigation</skos:prefLabel>
    <rdfs:isDefinedBy rdf:resource="https://w3id.org/dpv/sector/law/owl#"/>
    <dct:created rdf:datatype="http://www.w3.org/2001/XMLSchema#date">2024-12-01</dct:created>
    <rdfs:subClassOf rdf:resource="https://w3id.org/dpv/sector/law/owl#CriminalLawEnforcement"/>
    <rdfs:subClassOf rdf:resource="https://w3id.org/dpv/sector/law/owl#LegalSuspectedOffenceInvestigation"/>
  </rdf:Description>
  <rdf:Description rdf:about="https://w3id.org/dpv/sector/law/owl#RoadDUIEnforcement">
    <skos:definition xml:lang="en">Purposes associated with detection and enforcement of DUI (driving under influence) rules on roads</skos:definition>
    <rdf:type rdf:resource="http://www.w3.org/2000/01/rdf-schema#Class"/>
    <rdf:type rdf:resource="https://w3id.org/dpv/owl#Purpose"/>
    <rdf:type rdf:resource="http://www.w3.org/2002/07/owl#Class"/>
    <rdfs:isDefinedBy rdf:resource="https://w3id.org/dpv/sector/law/owl#"/>
    <dct:created rdf:datatype="http://www.w3.org/2001/XMLSchema#date">2024-12-01</dct:created>
    <sw:term_status xml:lang="en">accepted</sw:term_status>
    <skos:prefLabel xml:lang="en">Road DUIEnforcement</skos:prefLabel>
    <rdfs:subClassOf rdf:resource="https://w3id.org/dpv/sector/law/owl#RoadTrafficRuleEnforcement"/>
  </rdf:Description>
  <rdf:Description rdf:about="https://w3id.org/dpv/sector/law/owl#LegalEvidenceCollection">
    <dct:created rdf:datatype="http://www.w3.org/2001/XMLSchema#date">2024-12-01</dct:created>
    <rdf:type rdf:resource="http://www.w3.org/2000/01/rdf-schema#Class"/>
    <rdf:type rdf:resource="https://w3id.org/dpv/owl#Purpose"/>
    <rdf:type rdf:resource="http://www.w3.org/2002/07/owl#Class"/>
    <sw:term_status xml:lang="en">accepted</sw:term_status>
    <skos:prefLabel xml:lang="en">Legal Evidence Collection</skos:prefLabel>
    <skos:definition xml:lang="en">Purposes associated with collection and management of evidence for investigation within the legal system</skos:definition>
    <rdfs:isDefinedBy rdf:resource="https://w3id.org/dpv/sector/law/owl#"/>
    <rdfs:subClassOf rdf:resource="https://w3id.org/dpv/sector/law/owl#LegalInvestigation"/>
  </rdf:Description>
  <rdf:Description rdf:about="https://w3id.org/dpv/sector/law/owl#CrimeVictimRestitutionSupport">
    <rdf:type rdf:resource="http://www.w3.org/2000/01/rdf-schema#Class"/>
    <rdf:type rdf:resource="https://w3id.org/dpv/owl#Purpose"/>
    <rdf:type rdf:resource="http://www.w3.org/2002/07/owl#Class"/>
    <skos:prefLabel xml:lang="en">Crime Victim Restitution Support</skos:prefLabel>
    <skos:definition xml:lang="en">Purposes associated with supporting victims of criminal activities through restitution or providing restoration or compensation of goods and services within the legal system</skos:definition>
    <rdfs:isDefinedBy rdf:resource="https://w3id.org/dpv/sector/law/owl#"/>
    <dct:created rdf:datatype="http://www.w3.org/2001/XMLSchema#date">2024-12-01</dct:created>
    <sw:term_status xml:lang="en">accepted</sw:term_status>
    <rdfs:subClassOf rdf:resource="https://w3id.org/dpv/sector/law/owl#CrimeVictimSafetyManagement"/>
  </rdf:Description>
  <rdf:Description rdf:about="https://w3id.org/dpv/sector/law/owl#LegalOffencePrediction">
    <sw:term_status xml:lang="en">accepted</sw:term_status>
    <rdfs:isDefinedBy rdf:resource="https://w3id.org/dpv/sector/law/owl#"/>
    <dct:created rdf:datatype="http://www.w3.org/2001/XMLSchema#date">2024-12-01</dct:created>
    <rdf:type rdf:resource="https://w3id.org/dpv/owl#Purpose"/>
    <rdf:type rdf:resource="http://www.w3.org/2000/01/rdf-schema#Class"/>
    <rdf:type rdf:resource="http://www.w3.org/2002/07/owl#Class"/>
    <skos:definition xml:lang="en">Purposes associated with predicting occurences or patterns related to offences, violations, crime, or other activities of interest within the legal system</skos:definition>
    <skos:prefLabel xml:lang="en">Legal Offence Prediction</skos:prefLabel>
    <rdfs:subClassOf rdf:resource="https://w3id.org/dpv/sector/law/owl#LegalResearchDevelopment"/>
  </rdf:Description>
  <rdf:Description rdf:about="https://w3id.org/dpv/sector/law/owl#ImmigrationComplaintManagement">
    <dct:created rdf:datatype="http://www.w3.org/2001/XMLSchema#date">2024-12-01</dct:created>
    <skos:definition xml:lang="en">Purposes associated with management of complaints related to immigration within the legal system</skos:definition>
    <sw:term_status xml:lang="en">accepted</sw:term_status>
    <rdf:type rdf:resource="https://w3id.org/dpv/owl#Purpose"/>
    <rdf:type rdf:resource="http://www.w3.org/2000/01/rdf-schema#Class"/>
    <rdf:type rdf:resource="http://www.w3.org/2002/07/owl#Class"/>
    <skos:prefLabel xml:lang="en">Immigration Complaint Management</skos:prefLabel>
    <rdfs:isDefinedBy rdf:resource="https://w3id.org/dpv/sector/law/owl#"/>
    <rdfs:subClassOf rdf:resource="https://w3id.org/dpv/sector/law/owl#ImmigrationManagement"/>
  </rdf:Description>
  <rdf:Description rdf:about="https://w3id.org/dpv/guides">
    <rdf:type rdf:resource="http://www.w3.org/ns/dx/prof/ResourceDescriptor"/>
    <profile:hasRole rdf:resource="http://www.w3.org/ns/dx/prof/role/guidance"/>
    <dct:title>Guides for Data Privacy Vocabulary</dct:title>
    <dct:conformsTo rdf:resource="https://www.w3.org/TR/html/"/>
    <profile:hasArtifact rdf:resource="https://w3id.org/dpv/guides"/>
    <dct:format rdf:resource="https://www.iana.org/assignments/media-types/text/html"/>
  </rdf:Description>
  <rdf:Description rdf:about="https://w3id.org/dpv/sector/law/owl#ImmigrationBorderControlManagement">
    <rdf:type rdf:resource="https://w3id.org/dpv/owl#Purpose"/>
    <rdf:type rdf:resource="http://www.w3.org/2000/01/rdf-schema#Class"/>
    <rdf:type rdf:resource="http://www.w3.org/2002/07/owl#Class"/>
    <dct:created rdf:datatype="http://www.w3.org/2001/XMLSchema#date">2024-12-01</dct:created>
    <skos:definition xml:lang="en">Purposes associated with border control within the legal system</skos:definition>
    <rdfs:isDefinedBy rdf:resource="https://w3id.org/dpv/sector/law/owl#"/>
    <skos:prefLabel xml:lang="en">Immigration Border Control Management</skos:prefLabel>
    <sw:term_status xml:lang="en">accepted</sw:term_status>
    <rdfs:subClassOf rdf:resource="https://w3id.org/dpv/sector/law/owl#ImmigrationSecurityManagement"/>
  </rdf:Description>
  <rdf:Description rdf:about="https://w3id.org/dpv/sector/law/owl#ImmigrationVisaManagement">
    <sw:term_status xml:lang="en">accepted</sw:term_status>
    <rdfs:isDefinedBy rdf:resource="https://w3id.org/dpv/sector/law/owl#"/>
    <dct:created rdf:datatype="http://www.w3.org/2001/XMLSchema#date">2024-12-01</dct:created>
    <skos:definition xml:lang="en">Purposes associated with management of visas, including collecting and processing of applications, determining elibility, making and communicating decisions, and enforcing the limits as related to immigration within the legal system</skos:definition>
    <skos:prefLabel xml:lang="en">Immigration Visa Management</skos:prefLabel>
    <rdf:type rdf:resource="https://w3id.org/dpv/owl#Purpose"/>
    <rdf:type rdf:resource="http://www.w3.org/2000/01/rdf-schema#Class"/>
    <rdf:type rdf:resource="http://www.w3.org/2002/07/owl#Class"/>
    <rdfs:subClassOf rdf:resource="https://w3id.org/dpv/sector/law/owl#ImmigrationManagement"/>
  </rdf:Description>
  <rdf:Description rdf:about="https://w3id.org/dpv/sector/law/owl#RoadVehicleInsuranceEnforcement">
    <rdf:type rdf:resource="https://w3id.org/dpv/owl#Purpose"/>
    <rdf:type rdf:resource="http://www.w3.org/2000/01/rdf-schema#Class"/>
    <rdf:type rdf:resource="http://www.w3.org/2002/07/owl#Class"/>
    <skos:prefLabel xml:lang="en">Road Vehicle Insurance Enforcement</skos:prefLabel>
    <rdfs:isDefinedBy rdf:resource="https://w3id.org/dpv/sector/law/owl#"/>
    <dct:created rdf:datatype="http://www.w3.org/2001/XMLSchema#date">2024-12-01</dct:created>
    <skos:definition xml:lang="en">Purposes associated with detection and enforcement of road vehicle insurance</skos:definition>
    <sw:term_status xml:lang="en">accepted</sw:term_status>
    <rdfs:subClassOf rdf:resource="https://w3id.org/dpv/sector/law/owl#RoadTrafficLawEnforcement"/>
  </rdf:Description>
  <rdf:Description rdf:about="https://w3id.org/dpv/sector/law/owl#RoadVehicleEmissionEnforcement">
    <rdf:type rdf:resource="http://www.w3.org/2000/01/rdf-schema#Class"/>
    <rdf:type rdf:resource="https://w3id.org/dpv/owl#Purpose"/>
    <rdf:type rdf:resource="http://www.w3.org/2002/07/owl#Class"/>
    <skos:prefLabel xml:lang="en">Road Vehicle Emission Enforcement</skos:prefLabel>
    <sw:term_status xml:lang="en">accepted</sw:term_status>
    <rdfs:isDefinedBy rdf:resource="https://w3id.org/dpv/sector/law/owl#"/>
    <skos:definition xml:lang="en">Purposes associated with detection and enforcement of road vehicle emissions</skos:definition>
    <dct:created rdf:datatype="http://www.w3.org/2001/XMLSchema#date">2024-12-01</dct:created>
    <rdfs:subClassOf rdf:resource="https://w3id.org/dpv/sector/law/owl#RoadTrafficLawEnforcement"/>
  </rdf:Description>
  <rdf:Description rdf:about="https://w3id.org/dpv/sector/law/owl#CrimeVictimSafetyAssessment">
    <skos:prefLabel xml:lang="en">Crime Victim Safety Assessment</skos:prefLabel>
    <sw:term_status xml:lang="en">accepted</sw:term_status>
    <rdf:type rdf:resource="https://w3id.org/dpv/owl#Purpose"/>
    <rdf:type rdf:resource="http://www.w3.org/2000/01/rdf-schema#Class"/>
    <rdf:type rdf:resource="http://www.w3.org/2002/07/owl#Class"/>
    <dct:created rdf:datatype="http://www.w3.org/2001/XMLSchema#date">2024-12-01</dct:created>
    <rdfs:isDefinedBy rdf:resource="https://w3id.org/dpv/sector/law/owl#"/>
    <skos:definition xml:lang="en">Purposes associated with safety assessment of victims of criminal activities within the legal system</skos:definition>
    <rdfs:subClassOf rdf:resource="https://w3id.org/dpv/sector/law/owl#CrimeVictimSafetyManagement"/>
  </rdf:Description>
  <rdf:Description rdf:about="https://w3id.org/dpv/sector/law/owl#RecidivismPrediction">
    <skos:definition xml:lang="en">Purposes associated with prediction of recidivism as the repeating of an undesirable behaviours or offences or violations by an entity after they have experienced negative consequences of that behaviour or have been informed or trained on how to avoid repeating it</skos:definition>
    <skos:prefLabel xml:lang="en">Recidivism Prediction</skos:prefLabel>
    <rdf:type rdf:resource="https://w3id.org/dpv/owl#Purpose"/>
    <rdf:type rdf:resource="http://www.w3.org/2000/01/rdf-schema#Class"/>
    <rdf:type rdf:resource="http://www.w3.org/2002/07/owl#Class"/>
    <rdfs:isDefinedBy rdf:resource="https://w3id.org/dpv/sector/law/owl#"/>
    <dct:created rdf:datatype="http://www.w3.org/2001/XMLSchema#date">2024-12-01</dct:created>
    <sw:term_status xml:lang="en">accepted</sw:term_status>
    <rdfs:subClassOf rdf:resource="https://w3id.org/dpv/sector/law/owl#LegalRepeatOffencePrediction"/>
  </rdf:Description>
  <rdf:Description rdf:about="https://w3id.org/dpv/sector/law/owl#ImmigrationDocumentVerficiation">
    <rdf:type rdf:resource="https://w3id.org/dpv/owl#Purpose"/>
    <rdf:type rdf:resource="http://www.w3.org/2000/01/rdf-schema#Class"/>
    <rdf:type rdf:resource="http://www.w3.org/2002/07/owl#Class"/>
    <dct:created rdf:datatype="http://www.w3.org/2001/XMLSchema#date">2024-12-01</dct:created>
    <skos:definition xml:lang="en">Purposes associated with verification of documents and information related to immigration within the legal system</skos:definition>
    <rdfs:isDefinedBy rdf:resource="https://w3id.org/dpv/sector/law/owl#"/>
    <skos:prefLabel xml:lang="en">Immigration Document Verficiation</skos:prefLabel>
    <sw:term_status xml:lang="en">accepted</sw:term_status>
    <rdfs:subClassOf rdf:resource="https://w3id.org/dpv/sector/law/owl#ImmigrationRequestManagement"/>
  </rdf:Description>
  <rdf:Description rdf:about="https://w3id.org/dpv/sector/law/owl#RoadSpeedLimitEnforcement">
    <dct:created rdf:datatype="http://www.w3.org/2001/XMLSchema#date">2024-12-01</dct:created>
    <rdf:type rdf:resource="http://www.w3.org/2000/01/rdf-schema#Class"/>
    <rdf:type rdf:resource="https://w3id.org/dpv/owl#Purpose"/>
    <rdf:type rdf:resource="http://www.w3.org/2002/07/owl#Class"/>
    <sw:term_status xml:lang="en">accepted</sw:term_status>
    <skos:definition xml:lang="en">Purposes associated with detection and enforcement of speed limits on roads</skos:definition>
    <skos:prefLabel xml:lang="en">Road Speed Limit Enforcement</skos:prefLabel>
    <rdfs:isDefinedBy rdf:resource="https://w3id.org/dpv/sector/law/owl#"/>
    <rdfs:subClassOf rdf:resource="https://w3id.org/dpv/sector/law/owl#RoadTrafficRuleEnforcement"/>
  </rdf:Description>
  <rdf:Description rdf:about="https://w3id.org/dpv/sector/law/owl#JudicialDisputeManagement">
    <rdf:type rdf:resource="https://w3id.org/dpv/owl#Purpose"/>
    <rdf:type rdf:resource="http://www.w3.org/2000/01/rdf-schema#Class"/>
    <rdf:type rdf:resource="http://www.w3.org/2002/07/owl#Class"/>
    <skos:prefLabel xml:lang="en">Judicial Dispute Management</skos:prefLabel>
    <rdfs:isDefinedBy rdf:resource="https://w3id.org/dpv/sector/law/owl#"/>
    <dct:created rdf:datatype="http://www.w3.org/2001/XMLSchema#date">2024-12-01</dct:created>
    <skos:definition xml:lang="en">Purposes associated with detection, assessment, identifying resolutions, and other activities related to management of disputes within the judicial system</skos:definition>
    <sw:term_status xml:lang="en">accepted</sw:term_status>
    <rdfs:subClassOf rdf:resource="https://w3id.org/dpv/sector/law/owl#JudicialSystemManagement"/>
  </rdf:Description>
  <rdf:Description rdf:about="https://w3id.org/dpv/sector/law/owl#CrimeProsecution">
    <skos:definition xml:lang="en">Purposes associated with prosecution of criminal activities within the legal system</skos:definition>
    <rdf:type rdf:resource="https://w3id.org/dpv/owl#Purpose"/>
    <rdf:type rdf:resource="http://www.w3.org/2000/01/rdf-schema#Class"/>
    <rdf:type rdf:resource="http://www.w3.org/2002/07/owl#Class"/>
    <rdfs:isDefinedBy rdf:resource="https://w3id.org/dpv/sector/law/owl#"/>
    <skos:prefLabel xml:lang="en">Crime Prosecution</skos:prefLabel>
    <dct:created rdf:datatype="http://www.w3.org/2001/XMLSchema#date">2024-12-01</dct:created>
    <sw:term_status xml:lang="en">accepted</sw:term_status>
    <rdfs:subClassOf rdf:resource="https://w3id.org/dpv/sector/law/owl#LegalOffenceProsecution"/>
    <rdfs:subClassOf rdf:resource="https://w3id.org/dpv/sector/law/owl#CriminalLawEnforcement"/>
  </rdf:Description>
  <rdf:Description rdf:about="https://w3id.org/dpv/sector/law/owl#ImmigrationWorkAuthorisationManagement">
    <rdf:type rdf:resource="http://www.w3.org/2000/01/rdf-schema#Class"/>
    <rdf:type rdf:resource="https://w3id.org/dpv/owl#Purpose"/>
    <rdf:type rdf:resource="http://www.w3.org/2002/07/owl#Class"/>
    <sw:term_status xml:lang="en">accepted</sw:term_status>
    <rdfs:isDefinedBy rdf:resource="https://w3id.org/dpv/sector/law/owl#"/>
    <skos:prefLabel xml:lang="en">Immigration Work Authorisation Management</skos:prefLabel>
    <skos:definition xml:lang="en">Purposes associated with management of work authorisations, including collecting and processing of applications, determining elibility, making and communicating decisions, and enforcing the limits as related to immigration within the legal system</skos:definition>
    <dct:created rdf:datatype="http://www.w3.org/2001/XMLSchema#date">2024-12-01</dct:created>
    <rdfs:subClassOf rdf:resource="https://w3id.org/dpv/sector/law/owl#ImmigrationManagement"/>
  </rdf:Description>
  <rdf:Description rdf:about="https://w3id.org/dpv/sector/law/owl#JudicialLegalInterpretation">
    <skos:definition xml:lang="en">Purposes associated with interpretation of laws, arguments, and facts and other related information within the judicial system</skos:definition>
    <rdf:type rdf:resource="https://w3id.org/dpv/owl#Purpose"/>
    <rdf:type rdf:resource="http://www.w3.org/2000/01/rdf-schema#Class"/>
    <rdf:type rdf:resource="http://www.w3.org/2002/07/owl#Class"/>
    <rdfs:isDefinedBy rdf:resource="https://w3id.org/dpv/sector/law/owl#"/>
    <dct:created rdf:datatype="http://www.w3.org/2001/XMLSchema#date">2024-12-01</dct:created>
    <sw:term_status xml:lang="en">accepted</sw:term_status>
    <skos:prefLabel xml:lang="en">Judicial Legal Interpretation</skos:prefLabel>
    <rdfs:subClassOf rdf:resource="https://w3id.org/dpv/sector/law/owl#JudicialSystemManagement"/>
  </rdf:Description>
  <rdf:Description rdf:about="https://w3id.org/dpv/sector/law/owl#PublicTransportViolationDetection">
    <rdfs:isDefinedBy rdf:resource="https://w3id.org/dpv/sector/law/owl#"/>
    <rdf:type rdf:resource="http://www.w3.org/2000/01/rdf-schema#Class"/>
    <rdf:type rdf:resource="https://w3id.org/dpv/owl#Purpose"/>
    <rdf:type rdf:resource="http://www.w3.org/2002/07/owl#Class"/>
    <sw:term_status xml:lang="en">accepted</sw:term_status>
    <dct:created rdf:datatype="http://www.w3.org/2001/XMLSchema#date">2024-12-01</dct:created>
    <skos:definition xml:lang="en">Purposes associated with detection of violations  related to road traffic law within or including public transport</skos:definition>
    <skos:prefLabel xml:lang="en">Public Transport Violation Detection</skos:prefLabel>
    <rdfs:subClassOf rdf:resource="https://w3id.org/dpv/sector/law/owl#PublicTransportLawEnforcement"/>
  </rdf:Description>
  <rdf:Description rdf:about="https://w3id.org/dpv/sector/law/owl#ImmigrationHealthRiskDetection">
    <skos:prefLabel xml:lang="en">Immigration Health Risk Detection</skos:prefLabel>
    <rdfs:isDefinedBy rdf:resource="https://w3id.org/dpv/sector/law/owl#"/>
    <dct:created rdf:datatype="http://www.w3.org/2001/XMLSchema#date">2024-12-01</dct:created>
    <rdf:type rdf:resource="http://www.w3.org/2000/01/rdf-schema#Class"/>
    <rdf:type rdf:resource="https://w3id.org/dpv/owl#Purpose"/>
    <rdf:type rdf:resource="http://www.w3.org/2002/07/owl#Class"/>
    <sw:term_status xml:lang="en">accepted</sw:term_status>
    <skos:definition xml:lang="en">Purposes related to detecting health risks as part of security related to immigration within the legal system</skos:definition>
    <rdfs:subClassOf rdf:resource="https://w3id.org/dpv/sector/law/owl#ImmigrationHealthRiskManagement"/>
  </rdf:Description>
  <rdf:Description rdf:about="https://w3id.org/dpv/sector/law/owl#PublicTransportLawEnforcement">
    <rdf:type rdf:resource="https://w3id.org/dpv/owl#Purpose"/>
    <rdf:type rdf:resource="http://www.w3.org/2000/01/rdf-schema#Class"/>
    <rdf:type rdf:resource="http://www.w3.org/2002/07/owl#Class"/>
    <skos:prefLabel xml:lang="en">Public Transport Law Enforcement</skos:prefLabel>
    <rdfs:isDefinedBy rdf:resource="https://w3id.org/dpv/sector/law/owl#"/>
    <dct:created rdf:datatype="http://www.w3.org/2001/XMLSchema#date">2024-12-01</dct:created>
    <sw:term_status xml:lang="en">accepted</sw:term_status>
    <skos:definition xml:lang="en">Purposes associated with enforcement of road traffic law for public transport infrastructure and services</skos:definition>
    <rdfs:subClassOf rdf:resource="https://w3id.org/dpv/sector/law/owl#RoadTrafficLawEnforcement"/>
  </rdf:Description>
  <rdf:Description rdf:about="https://w3id.org/dpv/sector/law/owl#RoadTrafficLawViolationFineAssessment">
    <rdf:type rdf:resource="https://w3id.org/dpv/owl#Purpose"/>
    <rdf:type rdf:resource="http://www.w3.org/2000/01/rdf-schema#Class"/>
    <rdf:type rdf:resource="http://www.w3.org/2002/07/owl#Class"/>
    <rdfs:isDefinedBy rdf:resource="https://w3id.org/dpv/sector/law/owl#"/>
    <dct:created rdf:datatype="http://www.w3.org/2001/XMLSchema#date">2024-12-01</dct:created>
    <skos:prefLabel xml:lang="en">Road Traffic Law Violation Fine Assessment</skos:prefLabel>
    <sw:term_status xml:lang="en">accepted</sw:term_status>
    <skos:definition xml:lang="en">Purposes associated with determination and calculation related to assessment of fines for violaitions of road traffic law</skos:definition>
    <rdfs:subClassOf rdf:resource="https://w3id.org/dpv/sector/law/owl#RoadTrafficLawEnforcement"/>
  </rdf:Description>
  <rdf:Description rdf:about="https://w3id.org/dpv/sector/law/owl#ImmigrationTransitPermitManagement">
    <rdfs:isDefinedBy rdf:resource="https://w3id.org/dpv/sector/law/owl#"/>
    <dct:created rdf:datatype="http://www.w3.org/2001/XMLSchema#date">2024-12-01</dct:created>
    <rdf:type rdf:resource="http://www.w3.org/2000/01/rdf-schema#Class"/>
    <rdf:type rdf:resource="https://w3id.org/dpv/owl#Purpose"/>
    <rdf:type rdf:resource="http://www.w3.org/2002/07/owl#Class"/>
    <skos:definition xml:lang="en">Purposes associated with management of transit permits or transit visas, including collecting and processing of applications, determining elibility, making and communicating decisions, and enforcing the limits as related to immigration within the legal system</skos:definition>
    <sw:term_status xml:lang="en">accepted</sw:term_status>
    <skos:prefLabel xml:lang="en">Immigration Transit Permit Management</skos:prefLabel>
    <rdfs:subClassOf rdf:resource="https://w3id.org/dpv/sector/law/owl#ImmigrationManagement"/>
  </rdf:Description>
  <rdf:Description rdf:about="https://w3id.org/dpv/sector/law/owl#LegalSuspectedOffenceInvestigation">
    <rdf:type rdf:resource="http://www.w3.org/2000/01/rdf-schema#Class"/>
    <rdf:type rdf:resource="https://w3id.org/dpv/owl#Purpose"/>
    <rdf:type rdf:resource="http://www.w3.org/2002/07/owl#Class"/>
    <sw:term_status xml:lang="en">accepted</sw:term_status>
    <skos:definition xml:lang="en">Purposes associated with investigation of suspected offences, violations, crime, or other activities of interest within the legal system</skos:definition>
    <skos:prefLabel xml:lang="en">Legal Suspected Offence Investigation</skos:prefLabel>
    <rdfs:isDefinedBy rdf:resource="https://w3id.org/dpv/sector/law/owl#"/>
    <dct:created rdf:datatype="http://www.w3.org/2001/XMLSchema#date">2024-12-01</dct:created>
    <rdfs:subClassOf rdf:resource="https://w3id.org/dpv/sector/law/owl#LegalInvestigation"/>
  </rdf:Description>
  <rdf:Description rdf:about="https://w3id.org/dpv/sector/law/owl#ProbationManagement">
    <sw:term_status xml:lang="en">accepted</sw:term_status>
    <rdf:type rdf:resource="https://w3id.org/dpv/owl#Purpose"/>
    <rdf:type rdf:resource="http://www.w3.org/2000/01/rdf-schema#Class"/>
    <rdf:type rdf:resource="http://www.w3.org/2002/07/owl#Class"/>
    <skos:definition xml:lang="en">Purposes associated with management of probation institutions part of the legal system</skos:definition>
    <rdfs:isDefinedBy rdf:resource="https://w3id.org/dpv/sector/law/owl#"/>
    <skos:prefLabel xml:lang="en">Probation Management</skos:prefLabel>
    <dct:created rdf:datatype="http://www.w3.org/2001/XMLSchema#date">2024-12-01</dct:created>
    <rdfs:subClassOf rdf:resource="https://w3id.org/dpv/sector/law/owl#LegalInstitutionalManagement"/>
  </rdf:Description>
  <rdf:Description rdf:about="https://w3id.org/dpv/sector/law/owl#CriminalLawEnforcement">
    <skos:prefLabel xml:lang="en">Criminal Law Enforcement</skos:prefLabel>
    <rdf:type rdf:resource="https://w3id.org/dpv/owl#Purpose"/>
    <rdf:type rdf:resource="http://www.w3.org/2000/01/rdf-schema#Class"/>
    <rdf:type rdf:resource="http://www.w3.org/2002/07/owl#Class"/>
    <rdfs:isDefinedBy rdf:resource="https://w3id.org/dpv/sector/law/owl#"/>
    <dct:created rdf:datatype="http://www.w3.org/2001/XMLSchema#date">2024-12-01</dct:created>
    <skos:definition xml:lang="en">Purposes associated with criminal law enforcement within the legal system</skos:definition>
    <sw:term_status xml:lang="en">accepted</sw:term_status>
    <rdfs:subClassOf rdf:resource="https://w3id.org/dpv/sector/law/owl#LawEnforcement"/>
  </rdf:Description>
  <rdf:Description rdf:about="https://w3id.org/dpv/sector/law/owl#LegalAidProvision">
    <skos:definition xml:lang="en">Purposes associated with provision of legal aid within the judicial system</skos:definition>
    <rdfs:isDefinedBy rdf:resource="https://w3id.org/dpv/sector/law/owl#"/>
    <rdf:type rdf:resource="http://www.w3.org/2000/01/rdf-schema#Class"/>
    <rdf:type rdf:resource="https://w3id.org/dpv/owl#Purpose"/>
    <rdf:type rdf:resource="http://www.w3.org/2002/07/owl#Class"/>
    <sw:term_status xml:lang="en">accepted</sw:term_status>
    <skos:prefLabel xml:lang="en">Legal Aid Provision</skos:prefLabel>
    <dct:created rdf:datatype="http://www.w3.org/2001/XMLSchema#date">2024-12-01</dct:created>
    <rdfs:subClassOf rdf:resource="https://w3id.org/dpv/sector/law/owl#JudicialSystemManagement"/>
  </rdf:Description>
  <rdf:Description rdf:about="https://w3id.org/dpv/sector/law/owl#LegalOffenceSurveillance">
    <skos:prefLabel xml:lang="en">Legal Offence Surveillance</skos:prefLabel>
    <rdf:type rdf:resource="https://w3id.org/dpv/owl#Purpose"/>
    <rdf:type rdf:resource="http://www.w3.org/2000/01/rdf-schema#Class"/>
    <rdf:type rdf:resource="http://www.w3.org/2002/07/owl#Class"/>
    <rdfs:isDefinedBy rdf:resource="https://w3id.org/dpv/sector/law/owl#"/>
    <dct:created rdf:datatype="http://www.w3.org/2001/XMLSchema#date">2024-12-01</dct:created>
    <sw:term_status xml:lang="en">accepted</sw:term_status>
    <skos:definition xml:lang="en">Purposes associated with monitoring or observing to detect or deter potential or ongoing illegal activities or violations or offences within the legal system</skos:definition>
    <rdfs:subClassOf rdf:resource="https://w3id.org/dpv/sector/law/owl#LawEnforcement"/>
  </rdf:Description>
  <rdf:Description rdf:about="https://w3id.org/dpv/sector/law/owl#LegalEvidenceEligibilityAssessment">
    <skos:prefLabel xml:lang="en">Legal Evidence Eligibility Assessment</skos:prefLabel>
    <rdf:type rdf:resource="https://w3id.org/dpv/owl#Purpose"/>
    <rdf:type rdf:resource="http://www.w3.org/2000/01/rdf-schema#Class"/>
    <rdf:type rdf:resource="http://www.w3.org/2002/07/owl#Class"/>
    <dct:created rdf:datatype="http://www.w3.org/2001/XMLSchema#date">2024-12-01</dct:created>
    <skos:definition xml:lang="en">Purposes associated with the assessment of eligibility of evidence for investigation within the legal system</skos:definition>
    <rdfs:isDefinedBy rdf:resource="https://w3id.org/dpv/sector/law/owl#"/>
    <sw:term_status xml:lang="en">accepted</sw:term_status>
    <rdfs:subClassOf rdf:resource="https://w3id.org/dpv/sector/law/owl#LegalInvestigation"/>
  </rdf:Description>
  <rdf:Description rdf:about="https://w3id.org/dpv/sector/law/owl#ImmigrationApplicationManagement">
    <rdf:type rdf:resource="http://www.w3.org/2000/01/rdf-schema#Class"/>
    <rdf:type rdf:resource="https://w3id.org/dpv/owl#Purpose"/>
    <rdf:type rdf:resource="http://www.w3.org/2002/07/owl#Class"/>
    <skos:prefLabel xml:lang="en">Immigration Application Management</skos:prefLabel>
    <sw:term_status xml:lang="en">accepted</sw:term_status>
    <rdfs:isDefinedBy rdf:resource="https://w3id.org/dpv/sector/law/owl#"/>
    <skos:definition xml:lang="en">Purposes associated with management of applications related to immigration within the legal system</skos:definition>
    <dct:created rdf:datatype="http://www.w3.org/2001/XMLSchema#date">2024-12-01</dct:created>
    <rdfs:subClassOf rdf:resource="https://w3id.org/dpv/sector/law/owl#ImmigrationRequestManagement"/>
  </rdf:Description>
  <rdf:Description rdf:about="https://w3id.org/dpv/sector/law/owl#RoadVehicleCertificationEnforcement">
    <rdf:type rdf:resource="https://w3id.org/dpv/owl#Purpose"/>
    <rdf:type rdf:resource="http://www.w3.org/2000/01/rdf-schema#Class"/>
    <rdf:type rdf:resource="http://www.w3.org/2002/07/owl#Class"/>
    <dct:created rdf:datatype="http://www.w3.org/2001/XMLSchema#date">2024-12-01</dct:created>
    <skos:prefLabel xml:lang="en">Road Vehicle Certification Enforcement</skos:prefLabel>
    <skos:definition xml:lang="en">Purposes associated with detection and enforcement of road vehicle certifications</skos:definition>
    <rdfs:isDefinedBy rdf:resource="https://w3id.org/dpv/sector/law/owl#"/>
    <sw:term_status xml:lang="en">accepted</sw:term_status>
    <rdfs:subClassOf rdf:resource="https://w3id.org/dpv/sector/law/owl#RoadTrafficLawEnforcement"/>
  </rdf:Description>
  <rdf:Description rdf:about="https://w3id.org/dpv/sector/law/owl#ImmigrationBorderIdentityVerification">
    <rdfs:isDefinedBy rdf:resource="https://w3id.org/dpv/sector/law/owl#"/>
    <dct:created rdf:datatype="http://www.w3.org/2001/XMLSchema#date">2024-12-01</dct:created>
    <rdf:type rdf:resource="http://www.w3.org/2000/01/rdf-schema#Class"/>
    <rdf:type rdf:resource="https://w3id.org/dpv/owl#Purpose"/>
    <rdf:type rdf:resource="http://www.w3.org/2002/07/owl#Class"/>
    <sw:term_status xml:lang="en">accepted</sw:term_status>
    <skos:definition xml:lang="en">Purposes associated with verification of identity at the border as defined in the legal system</skos:definition>
    <skos:prefLabel xml:lang="en">Immigration Border Identity Verification</skos:prefLabel>
    <rdfs:subClassOf rdf:resource="https://w3id.org/dpv/sector/law/owl#ImmigrationBorderControlManagement"/>
  </rdf:Description>
  <rdf:Description rdf:about="https://w3id.org/dpv/sector/law/owl#RehabilitationManagement">
    <rdf:type rdf:resource="https://w3id.org/dpv/owl#Purpose"/>
    <rdf:type rdf:resource="http://www.w3.org/2000/01/rdf-schema#Class"/>
    <rdf:type rdf:resource="http://www.w3.org/2002/07/owl#Class"/>
    <skos:prefLabel xml:lang="en">Rehabilitation Management</skos:prefLabel>
    <skos:definition xml:lang="en">Purposes associated with management of rehabilitation institutions part of the legal system</skos:definition>
    <rdfs:isDefinedBy rdf:resource="https://w3id.org/dpv/sector/law/owl#"/>
    <dct:created rdf:datatype="http://www.w3.org/2001/XMLSchema#date">2024-12-01</dct:created>
    <sw:term_status xml:lang="en">accepted</sw:term_status>
    <rdfs:subClassOf rdf:resource="https://w3id.org/dpv/sector/law/owl#LegalInstitutionalManagement"/>
  </rdf:Description>
  <rdf:Description rdf:about="https://w3id.org/dpv/sector/law/owl#LegalFirstOffencePrediction">
    <rdf:type rdf:resource="https://w3id.org/dpv/owl#Purpose"/>
    <rdf:type rdf:resource="http://www.w3.org/2000/01/rdf-schema#Class"/>
    <rdf:type rdf:resource="http://www.w3.org/2002/07/owl#Class"/>
    <dct:created rdf:datatype="http://www.w3.org/2001/XMLSchema#date">2024-12-01</dct:created>
    <skos:definition xml:lang="en">Purposes associated with predicting the first occurence related to offences, violations, crime, or other activities of interest within the legal system</skos:definition>
    <rdfs:isDefinedBy rdf:resource="https://w3id.org/dpv/sector/law/owl#"/>
    <skos:prefLabel xml:lang="en">Legal First Offence Prediction</skos:prefLabel>
    <sw:term_status xml:lang="en">accepted</sw:term_status>
    <rdfs:subClassOf rdf:resource="https://w3id.org/dpv/sector/law/owl#LegalOffencePrediction"/>
  </rdf:Description>
  <rdf:Description rdf:about="https://w3id.org/dpv/sector/law/owl#ImmigrationAsylumManagement">
    <rdfs:isDefinedBy rdf:resource="https://w3id.org/dpv/sector/law/owl#"/>
    <rdf:type rdf:resource="http://www.w3.org/2000/01/rdf-schema#Class"/>
    <rdf:type rdf:resource="https://w3id.org/dpv/owl#Purpose"/>
    <rdf:type rdf:resource="http://www.w3.org/2002/07/owl#Class"/>
    <skos:prefLabel xml:lang="en">Immigration Asylum Management</skos:prefLabel>
    <sw:term_status xml:lang="en">accepted</sw:term_status>
    <skos:definition xml:lang="en">Purposes associated with management of requests or petitions for asylum including collecting and processing of applications, determining elibility, making and communicating decisions, and enforcing the limits as related to immigration within the legal system</skos:definition>
    <dct:created rdf:datatype="http://www.w3.org/2001/XMLSchema#date">2024-12-01</dct:created>
    <rdfs:subClassOf rdf:resource="https://w3id.org/dpv/sector/law/owl#ImmigrationManagement"/>
  </rdf:Description>
  <rdf:Description rdf:about="https://w3id.org/dpv/sector/law/owl#RoadTrafficLawViolationCommunication">
    <sw:term_status xml:lang="en">accepted</sw:term_status>
    <rdf:type rdf:resource="https://w3id.org/dpv/owl#Purpose"/>
    <rdf:type rdf:resource="http://www.w3.org/2000/01/rdf-schema#Class"/>
    <rdf:type rdf:resource="http://www.w3.org/2002/07/owl#Class"/>
    <dct:created rdf:datatype="http://www.w3.org/2001/XMLSchema#date">2024-12-01</dct:created>
    <skos:prefLabel xml:lang="en">Road Traffic Law Violation Communication</skos:prefLabel>
    <rdfs:isDefinedBy rdf:resource="https://w3id.org/dpv/sector/law/owl#"/>
    <skos:definition xml:lang="en">Purposes associated with managing communications related to violations of road traffic law violations</skos:definition>
    <rdfs:subClassOf rdf:resource="https://w3id.org/dpv/sector/law/owl#RoadTrafficLawEnforcement"/>
  </rdf:Description>
  <rdf:Description rdf:about="https://w3id.org/dpv/sector/law/owl#SuspectedCriminalBehaviourDetection">
    <rdfs:isDefinedBy rdf:resource="https://w3id.org/dpv/sector/law/owl#"/>
    <rdf:type rdf:resource="http://www.w3.org/2000/01/rdf-schema#Class"/>
    <rdf:type rdf:resource="https://w3id.org/dpv/owl#Purpose"/>
    <rdf:type rdf:resource="http://www.w3.org/2002/07/owl#Class"/>
    <skos:prefLabel xml:lang="en">Suspected Criminal Behaviour Detection</skos:prefLabel>
    <sw:term_status xml:lang="en">accepted</sw:term_status>
    <dct:created rdf:datatype="http://www.w3.org/2001/XMLSchema#date">2024-12-01</dct:created>
    <skos:definition xml:lang="en">Purposes associated with detection of suspected criminal behaviour within the legal system</skos:definition>
    <rdfs:subClassOf rdf:resource="https://w3id.org/dpv/sector/law/owl#LegalSuspectedOffenceInvestigation"/>
    <rdfs:subClassOf rdf:resource="https://w3id.org/dpv/sector/law/owl#CrimeDetection"/>
  </rdf:Description>
  <rdf:Description rdf:about="https://w3id.org/dpv/sector/law/owl#serialisation-jsonld">
    <profile:hasRole rdf:resource="http://www.w3.org/ns/dx/prof/role/vocabulary"/>
    <dct:title>Law Enforcement &amp; Justice Sector Concepts - JSON-LD serialiation</dct:title>
    <dct:conformsTo rdf:resource="https://www.w3.org/TR/json-ld11/"/>
    <dct:format rdf:resource="https://www.iana.org/assignments/media-types/application/ld+json"/>
    <profile:hasArtifact rdf:resource="https://w3id.org/dpv/sector/law/sector-law-owl.jsonld"/>
    <rdf:type rdf:resource="http://www.w3.org/ns/dx/prof/ResourceDescriptor"/>
  </rdf:Description>
  <rdf:Description rdf:nodeID="N2fe5586a82794e5a99ff2b47c1f2175e">
    <foaf:homepage>https://harshp.com/</foaf:homepage>
    <rdf:type rdf:resource="http://purl.org/dc/terms/Agent"/>
    <rdf:type rdf:resource="http://xmlns.com/foaf/0.1/Person"/>
    <foaf:name>Harshvardhan J. Pandit</foaf:name>
    <scoro:hasORCID>0000-0002-5068-3714</scoro:hasORCID>
    <org:memberOf rdf:nodeID="Nfbd61e1f087d467e81291e0c311268a5"/>
  </rdf:Description>
  <rdf:Description rdf:about="https://w3id.org/dpv/sector/law/owl#RoadTollViolationDetection">
    <rdf:type rdf:resource="http://www.w3.org/2000/01/rdf-schema#Class"/>
    <rdf:type rdf:resource="https://w3id.org/dpv/owl#Purpose"/>
    <rdf:type rdf:resource="http://www.w3.org/2002/07/owl#Class"/>
    <rdfs:isDefinedBy rdf:resource="https://w3id.org/dpv/sector/law/owl#"/>
    <skos:definition xml:lang="en">Purposes associated with detection of violations related to road toll collection and payment</skos:definition>
    <dct:created rdf:datatype="http://www.w3.org/2001/XMLSchema#date">2024-12-01</dct:created>
    <skos:prefLabel xml:lang="en">Road Toll Violation Detection</skos:prefLabel>
    <sw:term_status xml:lang="en">accepted</sw:term_status>
    <rdfs:subClassOf rdf:resource="https://w3id.org/dpv/sector/infra/owl#RoadTollManagement"/>
    <rdfs:subClassOf rdf:resource="https://w3id.org/dpv/sector/law/owl#RoadTrafficLawEnforcement"/>
  </rdf:Description>
  <rdf:Description rdf:about="https://w3id.org/dpv/sector/law/owl#serialisation-html">
    <profile:hasArtifact rdf:resource="https://w3id.org/dpv/sector/law/sector-law-owl.html"/>
    <rdf:type rdf:resource="http://www.w3.org/ns/dx/prof/ResourceDescriptor"/>
    <profile:hasRole rdf:resource="http://www.w3.org/ns/dx/prof/role/specification"/>
    <dct:format rdf:resource="https://www.iana.org/assignments/media-types/text/html"/>
    <dct:conformsTo rdf:resource="https://www.w3.org/TR/html/"/>
    <dct:title>Law Enforcement &amp; Justice Sector Concepts - HTML serialiation</dct:title>
  </rdf:Description>
  <rdf:Description rdf:about="https://w3id.org/dpv/sector/law/owl#CrimeVictimCounsellingManagement">
    <rdf:type rdf:resource="https://w3id.org/dpv/owl#Purpose"/>
    <rdf:type rdf:resource="http://www.w3.org/2000/01/rdf-schema#Class"/>
    <rdf:type rdf:resource="http://www.w3.org/2002/07/owl#Class"/>
    <skos:definition xml:lang="en">Purposes associated with management of counselling for victims of criminal activities within the legal system</skos:definition>
    <sw:term_status xml:lang="en">accepted</sw:term_status>
    <rdfs:isDefinedBy rdf:resource="https://w3id.org/dpv/sector/law/owl#"/>
    <dct:created rdf:datatype="http://www.w3.org/2001/XMLSchema#date">2024-12-01</dct:created>
    <skos:prefLabel xml:lang="en">Crime Victim Counselling Management</skos:prefLabel>
    <rdfs:subClassOf rdf:resource="https://w3id.org/dpv/sector/law/owl#CrimeVictimSafetyManagement"/>
  </rdf:Description>
  <rdf:Description rdf:about="https://w3id.org/dpv/sector/law/owl#LegalRepeatOffencePrediction">
    <skos:prefLabel xml:lang="en">Legal Repeat Offence Prediction</skos:prefLabel>
    <rdf:type rdf:resource="https://w3id.org/dpv/owl#Purpose"/>
    <rdf:type rdf:resource="http://www.w3.org/2000/01/rdf-schema#Class"/>
    <rdf:type rdf:resource="http://www.w3.org/2002/07/owl#Class"/>
    <skos:definition xml:lang="en">Purposes associated with predicting the subsequent or repeated occurences related to offences, violations, crime, or other activities of interest within the legal system</skos:definition>
    <rdfs:isDefinedBy rdf:resource="https://w3id.org/dpv/sector/law/owl#"/>
    <dct:created rdf:datatype="http://www.w3.org/2001/XMLSchema#date">2024-12-01</dct:created>
    <sw:term_status xml:lang="en">accepted</sw:term_status>
    <rdfs:subClassOf rdf:resource="https://w3id.org/dpv/sector/law/owl#LegalOffencePrediction"/>
  </rdf:Description>
  <rdf:Description rdf:about="https://w3id.org/dpv/sector/law/owl#LegalInvestigation">
    <skos:definition xml:lang="en">Purposes associated with investigations within the legal system</skos:definition>
    <rdfs:isDefinedBy rdf:resource="https://w3id.org/dpv/sector/law/owl#"/>
    <rdf:type rdf:resource="https://w3id.org/dpv/owl#Purpose"/>
    <rdf:type rdf:resource="http://www.w3.org/2000/01/rdf-schema#Class"/>
    <rdf:type rdf:resource="http://www.w3.org/2002/07/owl#Class"/>
    <dct:created rdf:datatype="http://www.w3.org/2001/XMLSchema#date">2024-12-01</dct:created>
    <skos:prefLabel xml:lang="en">Legal Investigation</skos:prefLabel>
    <sw:term_status xml:lang="en">accepted</sw:term_status>
    <rdfs:subClassOf rdf:resource="https://w3id.org/dpv/sector/law/owl#LawEnforcement"/>
  </rdf:Description>
  <rdf:Description rdf:about="https://w3id.org/dpv/examples">
    <dct:title>Examples for Data Privacy Vocabulary</dct:title>
    <dct:conformsTo rdf:resource="https://www.w3.org/TR/html/"/>
    <dct:format rdf:resource="https://www.iana.org/assignments/media-types/text/html"/>
    <profile:hasArtifact rdf:resource="https://w3id.org/dpv/examples"/>
    <profile:hasRole rdf:resource="http://www.w3.org/ns/dx/prof/role/guidance"/>
    <rdf:type rdf:resource="http://www.w3.org/ns/dx/prof/ResourceDescriptor"/>
  </rdf:Description>
  <rdf:Description rdf:about="https://w3id.org/dpv/sector/law/owl#LegalOffenceDetection">
    <sw:term_status xml:lang="en">accepted</sw:term_status>
    <rdf:type rdf:resource="https://w3id.org/dpv/owl#Purpose"/>
    <rdf:type rdf:resource="http://www.w3.org/2000/01/rdf-schema#Class"/>
    <rdf:type rdf:resource="http://www.w3.org/2002/07/owl#Class"/>
    <skos:prefLabel xml:lang="en">Legal Offence Detection</skos:prefLabel>
    <skos:definition xml:lang="en">Purposes associated with identifying or discovering illegal activities or violations or offences within the legal system</skos:definition>
    <rdfs:isDefinedBy rdf:resource="https://w3id.org/dpv/sector/law/owl#"/>
    <dct:created rdf:datatype="http://www.w3.org/2001/XMLSchema#date">2024-12-01</dct:created>
    <rdfs:subClassOf rdf:resource="https://w3id.org/dpv/sector/law/owl#LawEnforcement"/>
  </rdf:Description>
  <rdf:Description rdf:about="https://w3id.org/dpv/primer">
    <profile:hasRole rdf:resource="http://www.w3.org/ns/dx/prof/role/guidance"/>
    <rdf:type rdf:resource="http://www.w3.org/ns/dx/prof/ResourceDescriptor"/>
    <dct:format rdf:resource="https://www.iana.org/assignments/media-types/text/html"/>
    <dct:title>Primer for Data Privacy Vocabulary</dct:title>
    <dct:conformsTo rdf:resource="https://www.w3.org/TR/html/"/>
    <profile:hasArtifact rdf:resource="https://w3id.org/dpv/primer"/>
  </rdf:Description>
  <rdf:Description rdf:about="https://w3id.org/dpv/sector/law/owl#JudicialDecisionMaking">
    <skos:definition xml:lang="en">Purposes associated with making decisions related to legal determinations within the judicial system such as in courts cases or in authority rulings</skos:definition>
    <skos:prefLabel xml:lang="en">Judicial Decision Making</skos:prefLabel>
    <rdf:type rdf:resource="https://w3id.org/dpv/owl#Purpose"/>
    <rdf:type rdf:resource="http://www.w3.org/2000/01/rdf-schema#Class"/>
    <rdf:type rdf:resource="http://www.w3.org/2002/07/owl#Class"/>
    <dct:created rdf:datatype="http://www.w3.org/2001/XMLSchema#date">2024-12-01</dct:created>
    <sw:term_status xml:lang="en">accepted</sw:term_status>
    <rdfs:isDefinedBy rdf:resource="https://w3id.org/dpv/sector/law/owl#"/>
    <rdfs:subClassOf rdf:resource="https://w3id.org/dpv/sector/law/owl#JudicialSystemManagement"/>
  </rdf:Description>
  <rdf:Description rdf:about="https://w3id.org/dpv/sector/law/owl#ImmigrationRequestManagement">
    <dct:created rdf:datatype="http://www.w3.org/2001/XMLSchema#date">2024-12-01</dct:created>
    <rdf:type rdf:resource="http://www.w3.org/2000/01/rdf-schema#Class"/>
    <rdf:type rdf:resource="https://w3id.org/dpv/owl#Purpose"/>
    <rdf:type rdf:resource="http://www.w3.org/2002/07/owl#Class"/>
    <skos:definition xml:lang="en">Purposes associated with management of requests related to immigration within the legal system</skos:definition>
    <skos:prefLabel xml:lang="en">Immigration Request Management</skos:prefLabel>
    <rdfs:isDefinedBy rdf:resource="https://w3id.org/dpv/sector/law/owl#"/>
    <sw:term_status xml:lang="en">accepted</sw:term_status>
    <rdfs:subClassOf rdf:resource="https://w3id.org/dpv/sector/law/owl#ImmigrationManagement"/>
  </rdf:Description>
</rdf:RDF>
