<?xml version="1.0" encoding="utf-8"?>
<rdf:RDF
   xmlns:bibo="http://purl.org/ontology/bibo/"
   xmlns:dct="http://purl.org/dc/terms/"
   xmlns:foaf="http://xmlns.com/foaf/0.1/"
   xmlns:org="http://www.w3.org/ns/org#"
   xmlns:owl="http://www.w3.org/2002/07/owl#"
   xmlns:profile="http://www.w3.org/ns/dx/prof/"
   xmlns:rdf="http://www.w3.org/1999/02/22-rdf-syntax-ns#"
   xmlns:rdfs="http://www.w3.org/2000/01/rdf-schema#"
   xmlns:schema="https://schema.org/"
   xmlns:scoro="http://purl.org/spar/scoro/"
   xmlns:skos="http://www.w3.org/2004/02/skos/core#"
   xmlns:sw="http://www.w3.org/2003/06/sw-vocab-status/ns#"
   xmlns:vann="http://purl.org/vocab/vann/"
>
  <rdf:Description rdf:about="https://w3id.org/dpv/owl#ContractTerminated">
    <dct:contributor rdf:nodeID="Nb0b5fba741814592ba04e1a368a761fa"/>
    <dct:contributor rdf:nodeID="N2fe5586a82794e5a99ff2b47c1f2175e"/>
    <dct:contributor rdf:nodeID="N2acb95e70d08440bb095f34b511771ce"/>
    <skos:definition xml:lang="en">Status representing contract being terminated by one or more parties</skos:definition>
    <rdf:type rdf:resource="https://w3id.org/dpv/owl#ContractTerminationStatus"/>
    <rdf:type rdf:resource="http://www.w3.org/2000/01/rdf-schema#Class"/>
    <rdf:type rdf:resource="http://www.w3.org/2002/07/owl#Class"/>
    <dct:created rdf:datatype="http://www.w3.org/2001/XMLSchema#date">2025-01-09</dct:created>
    <sw:term_status xml:lang="en">accepted</sw:term_status>
    <rdfs:isDefinedBy rdf:resource="https://w3id.org/dpv/owl#"/>
    <skos:prefLabel xml:lang="en">Contract Terminated</skos:prefLabel>
    <rdfs:subClassOf rdf:resource="https://w3id.org/dpv/owl#ContractTerminationStatus"/>
  </rdf:Description>
  <rdf:Description rdf:about="https://w3id.org/dpv/owl#ContractStatus">
    <rdfs:subClassOf rdf:resource="https://w3id.org/dpv/owl#Status"/>
    <skos:prefLabel xml:lang="en">Contract Status</skos:prefLabel>
    <rdf:type rdf:resource="http://www.w3.org/2000/01/rdf-schema#Class"/>
    <rdf:type rdf:resource="http://www.w3.org/2002/07/owl#Class"/>
    <vann:example rdf:resource="https://w3id.org/dpv/examples/owl#E0077"/>
    <dct:contributor rdf:nodeID="N2fe5586a82794e5a99ff2b47c1f2175e"/>
    <sw:term_status xml:lang="en">accepted</sw:term_status>
    <skos:definition xml:lang="en">Status associated with a contract</skos:definition>
    <rdfs:isDefinedBy rdf:resource="https://w3id.org/dpv/owl#"/>
    <dct:created rdf:datatype="http://www.w3.org/2001/XMLSchema#date">2024-08-27</dct:created>
  </rdf:Description>
  <rdf:Description rdf:about="https://w3id.org/dpv/owl#ContractViolated">
    <rdf:type rdf:resource="https://w3id.org/dpv/owl#ContractFulfilmentStatus"/>
    <rdf:type rdf:resource="http://www.w3.org/2000/01/rdf-schema#Class"/>
    <rdf:type rdf:resource="http://www.w3.org/2002/07/owl#Class"/>
    <dct:created rdf:datatype="http://www.w3.org/2001/XMLSchema#date">2025-01-09</dct:created>
    <skos:prefLabel xml:lang="en">Contract Violated</skos:prefLabel>
    <dct:contributor rdf:nodeID="N2acb95e70d08440bb095f34b511771ce"/>
    <dct:contributor rdf:nodeID="N2fe5586a82794e5a99ff2b47c1f2175e"/>
    <dct:contributor rdf:nodeID="Nb0b5fba741814592ba04e1a368a761fa"/>
    <rdfs:isDefinedBy rdf:resource="https://w3id.org/dpv/owl#"/>
    <skos:definition xml:lang="en">Status representing contract where one or more terms have not been fulfiled or have been fulfiled, where either is considered a violation of the terms</skos:definition>
    <sw:term_status xml:lang="en">accepted</sw:term_status>
    <rdfs:subClassOf rdf:resource="https://w3id.org/dpv/owl#ContractFulfilmentStatus"/>
  </rdf:Description>
  <rdf:Description rdf:about="https://w3id.org/dpv/owl#ContractPartiallySigned">
    <sw:term_status xml:lang="en">accepted</sw:term_status>
    <rdf:type rdf:resource="https://w3id.org/dpv/owl#ContractExecutionStatus"/>
    <rdf:type rdf:resource="http://www.w3.org/2000/01/rdf-schema#Class"/>
    <rdf:type rdf:resource="http://www.w3.org/2002/07/owl#Class"/>
    <dct:contributor rdf:nodeID="Nb0b5fba741814592ba04e1a368a761fa"/>
    <dct:contributor rdf:nodeID="N2acb95e70d08440bb095f34b511771ce"/>
    <dct:contributor rdf:nodeID="N2fe5586a82794e5a99ff2b47c1f2175e"/>
    <skos:prefLabel xml:lang="en">Contract Partially Signed</skos:prefLabel>
    <dct:created rdf:datatype="http://www.w3.org/2001/XMLSchema#date">2025-01-09</dct:created>
    <rdfs:isDefinedBy rdf:resource="https://w3id.org/dpv/owl#"/>
    <skos:definition xml:lang="en">Status representing contract has been partially signed by parties i.e. some parties have signed the contract and others are yet to make a decision to sign it</skos:definition>
    <rdfs:subClassOf rdf:resource="https://w3id.org/dpv/owl#ContractExecutionStatus"/>
  </rdf:Description>
  <rdf:Description rdf:about="https://w3id.org/dpv/owl#serialisation-rdf">
    <rdf:type rdf:resource="http://www.w3.org/ns/dx/prof/ResourceDescriptor"/>
    <profile:hasArtifact rdf:resource="https://w3id.org/dpv/dpv/dpv-owl.rdf"/>
    <dct:format rdf:resource="https://www.iana.org/assignments/media-types/application/rdf+xml"/>
    <profile:hasRole rdf:resource="http://www.w3.org/ns/dx/prof/role/vocabulary"/>
    <dct:conformsTo rdf:resource="http://www.w3.org/1999/02/22-rdf-syntax-ns#"/>
    <dct:title>Data Privacy Vocabulary (DPV) - RDF/XML serialiation</dct:title>
  </rdf:Description>
  <rdf:Description rdf:about="https://w3id.org/dpv/owl#ContractBeingPerformed">
    <rdf:type rdf:resource="http://www.w3.org/2000/01/rdf-schema#Class"/>
    <rdf:type rdf:resource="https://w3id.org/dpv/owl#ContractPerformanceStatus"/>
    <rdf:type rdf:resource="http://www.w3.org/2002/07/owl#Class"/>
    <dct:contributor rdf:nodeID="N2acb95e70d08440bb095f34b511771ce"/>
    <dct:contributor rdf:nodeID="N2fe5586a82794e5a99ff2b47c1f2175e"/>
    <dct:contributor rdf:nodeID="Nb0b5fba741814592ba04e1a368a761fa"/>
    <rdfs:isDefinedBy rdf:resource="https://w3id.org/dpv/owl#"/>
    <sw:term_status xml:lang="en">accepted</sw:term_status>
    <skos:prefLabel xml:lang="en">Contract Being Performed</skos:prefLabel>
    <skos:definition xml:lang="en">Status representing contract that has been fully executed and whose terms are being carried out i.e. the contract is being performed</skos:definition>
    <dct:created rdf:datatype="http://www.w3.org/2001/XMLSchema#date">2025-01-09</dct:created>
    <rdfs:subClassOf rdf:resource="https://w3id.org/dpv/owl#ContractPerformanceStatus"/>
  </rdf:Description>
  <rdf:Description rdf:about="https://w3id.org/dpv/owl#ContractApproved">
    <dct:contributor rdf:nodeID="Nb0b5fba741814592ba04e1a368a761fa"/>
    <dct:contributor rdf:nodeID="N2acb95e70d08440bb095f34b511771ce"/>
    <dct:contributor rdf:nodeID="N2fe5586a82794e5a99ff2b47c1f2175e"/>
    <skos:definition xml:lang="en">Status representing contract has been approved and can be used for signing</skos:definition>
    <skos:prefLabel xml:lang="en">Contract Approved</skos:prefLabel>
    <dct:created rdf:datatype="http://www.w3.org/2001/XMLSchema#date">2025-01-09</dct:created>
    <rdf:type rdf:resource="http://www.w3.org/2000/01/rdf-schema#Class"/>
    <rdf:type rdf:resource="https://w3id.org/dpv/owl#ContractPreparationStatus"/>
    <rdf:type rdf:resource="http://www.w3.org/2002/07/owl#Class"/>
    <rdfs:isDefinedBy rdf:resource="https://w3id.org/dpv/owl#"/>
    <sw:term_status xml:lang="en">accepted</sw:term_status>
    <rdfs:subClassOf rdf:resource="https://w3id.org/dpv/owl#ContractPreparationStatus"/>
  </rdf:Description>
  <rdf:Description rdf:about="https://w3id.org/dpv/owl#ContractPerformanceStatus">
    <skos:prefLabel xml:lang="en">Contract Performance Status</skos:prefLabel>
    <rdf:type rdf:resource="http://www.w3.org/2000/01/rdf-schema#Class"/>
    <rdf:type rdf:resource="http://www.w3.org/2002/07/owl#Class"/>
    <dct:contributor rdf:nodeID="N2acb95e70d08440bb095f34b511771ce"/>
    <dct:contributor rdf:nodeID="N2fe5586a82794e5a99ff2b47c1f2175e"/>
    <dct:contributor rdf:nodeID="Nb0b5fba741814592ba04e1a368a761fa"/>
    <rdfs:isDefinedBy rdf:resource="https://w3id.org/dpv/owl#"/>
    <sw:term_status xml:lang="en">accepted</sw:term_status>
    <rdfs:subClassOf rdf:resource="https://w3id.org/dpv/owl#ContractStatus"/>
    <skos:definition xml:lang="en">Status associated with performance of a contract</skos:definition>
    <dct:created rdf:datatype="http://www.w3.org/2001/XMLSchema#date">2025-01-09</dct:created>
  </rdf:Description>
  <rdf:Description rdf:about="https://w3id.org/dpv/owl#ContractRenewed">
    <rdf:type rdf:resource="https://w3id.org/dpv/owl#ContractPerformanceStatus"/>
    <rdf:type rdf:resource="http://www.w3.org/2000/01/rdf-schema#Class"/>
    <rdf:type rdf:resource="http://www.w3.org/2002/07/owl#Class"/>
    <dct:contributor rdf:nodeID="Nb0b5fba741814592ba04e1a368a761fa"/>
    <dct:contributor rdf:nodeID="N2acb95e70d08440bb095f34b511771ce"/>
    <dct:contributor rdf:nodeID="N2fe5586a82794e5a99ff2b47c1f2175e"/>
    <dct:created rdf:datatype="http://www.w3.org/2001/XMLSchema#date">2025-01-09</dct:created>
    <skos:definition xml:lang="en">Status representing contract being renewed with new duration and/or applicability where the contract has been fully executed in the past</skos:definition>
    <rdfs:isDefinedBy rdf:resource="https://w3id.org/dpv/owl#"/>
    <skos:prefLabel xml:lang="en">Contract Renewed</skos:prefLabel>
    <sw:term_status xml:lang="en">accepted</sw:term_status>
    <rdfs:subClassOf rdf:resource="https://w3id.org/dpv/owl#ContractPerformanceStatus"/>
  </rdf:Description>
  <rdf:Description rdf:about="https://w3id.org/dpv/owl#ContractFullyExecuted">
    <rdf:type rdf:resource="http://www.w3.org/2000/01/rdf-schema#Class"/>
    <rdf:type rdf:resource="https://w3id.org/dpv/owl#ContractExecutionStatus"/>
    <rdf:type rdf:resource="http://www.w3.org/2002/07/owl#Class"/>
    <dct:contributor rdf:nodeID="N2acb95e70d08440bb095f34b511771ce"/>
    <dct:contributor rdf:nodeID="N2fe5586a82794e5a99ff2b47c1f2175e"/>
    <dct:contributor rdf:nodeID="Nb0b5fba741814592ba04e1a368a761fa"/>
    <rdfs:isDefinedBy rdf:resource="https://w3id.org/dpv/owl#"/>
    <sw:term_status xml:lang="en">accepted</sw:term_status>
    <skos:prefLabel xml:lang="en">Contract Fully Executed</skos:prefLabel>
    <skos:definition xml:lang="en">Status representing contract has been fully executed i.e. it has been signed by all parties and all other procedural aspects such as exchange of signed contract copies have been completed</skos:definition>
    <dct:created rdf:datatype="http://www.w3.org/2001/XMLSchema#date">2025-01-09</dct:created>
    <rdfs:subClassOf rdf:resource="https://w3id.org/dpv/owl#ContractExecutionStatus"/>
  </rdf:Description>
  <rdf:Description rdf:about="https://w3id.org/dpv/owl#ContractBreached">
    <rdf:type rdf:resource="https://w3id.org/dpv/owl#ContractTerminationStatus"/>
    <rdf:type rdf:resource="http://www.w3.org/2000/01/rdf-schema#Class"/>
    <rdf:type rdf:resource="http://www.w3.org/2002/07/owl#Class"/>
    <rdfs:isDefinedBy rdf:resource="https://w3id.org/dpv/owl#"/>
    <dct:contributor rdf:nodeID="N2fe5586a82794e5a99ff2b47c1f2175e"/>
    <dct:contributor rdf:nodeID="Nb0b5fba741814592ba04e1a368a761fa"/>
    <dct:contributor rdf:nodeID="N2acb95e70d08440bb095f34b511771ce"/>
    <sw:term_status xml:lang="en">accepted</sw:term_status>
    <dct:created rdf:datatype="http://www.w3.org/2001/XMLSchema#date">2025-01-09</dct:created>
    <skos:prefLabel xml:lang="en">Contract Breached</skos:prefLabel>
    <skos:definition xml:lang="en">Status representing contract being breached where its terms are not fulfiled or are violated with legal consequences</skos:definition>
    <rdfs:subClassOf rdf:resource="https://w3id.org/dpv/owl#ContractTerminationStatus"/>
  </rdf:Description>
  <rdf:Description rdf:about="https://w3id.org/dpv/owl#ContractOffered">
    <rdf:type rdf:resource="http://www.w3.org/2000/01/rdf-schema#Class"/>
    <rdf:type rdf:resource="https://w3id.org/dpv/owl#ContractPreparationStatus"/>
    <rdf:type rdf:resource="http://www.w3.org/2002/07/owl#Class"/>
    <dct:contributor rdf:nodeID="N2acb95e70d08440bb095f34b511771ce"/>
    <dct:contributor rdf:nodeID="N2fe5586a82794e5a99ff2b47c1f2175e"/>
    <dct:contributor rdf:nodeID="Nb0b5fba741814592ba04e1a368a761fa"/>
    <rdfs:isDefinedBy rdf:resource="https://w3id.org/dpv/owl#"/>
    <sw:term_status xml:lang="en">accepted</sw:term_status>
    <skos:prefLabel xml:lang="en">Contract Offered</skos:prefLabel>
    <skos:definition xml:lang="en">Status representing contract has been offered to a party or to parties for reviewing and signing</skos:definition>
    <dct:created rdf:datatype="http://www.w3.org/2001/XMLSchema#date">2025-01-09</dct:created>
    <rdfs:subClassOf rdf:resource="https://w3id.org/dpv/owl#ContractPreparationStatus"/>
  </rdf:Description>
  <rdf:Description rdf:about="https://w3id.org/dpv/owl#ContractPreparationStatus">
    <skos:definition xml:lang="en">Status associated with preparation of contracts before they are signed or accepted or executed</skos:definition>
    <rdf:type rdf:resource="http://www.w3.org/2000/01/rdf-schema#Class"/>
    <rdf:type rdf:resource="http://www.w3.org/2002/07/owl#Class"/>
    <dct:contributor rdf:nodeID="N2fe5586a82794e5a99ff2b47c1f2175e"/>
    <dct:contributor rdf:nodeID="N2acb95e70d08440bb095f34b511771ce"/>
    <dct:contributor rdf:nodeID="Nb0b5fba741814592ba04e1a368a761fa"/>
    <sw:term_status xml:lang="en">accepted</sw:term_status>
    <dct:created rdf:datatype="http://www.w3.org/2001/XMLSchema#date">2025-01-09</dct:created>
    <rdfs:isDefinedBy rdf:resource="https://w3id.org/dpv/owl#"/>
    <rdfs:subClassOf rdf:resource="https://w3id.org/dpv/owl#ContractStatus"/>
    <skos:prefLabel xml:lang="en">Contract Preparation Status</skos:prefLabel>
  </rdf:Description>
  <rdf:Description rdf:nodeID="Nfbd61e1f087d467e81291e0c311268a5">
    <foaf:name>ADAPT Centre, Dublin City University</foaf:name>
    <rdf:type rdf:resource="http://xmlns.com/foaf/0.1/Organization"/>
  </rdf:Description>
  <rdf:Description rdf:about="https://w3id.org/dpv/owl#ContractDrafted">
    <dct:created rdf:datatype="http://www.w3.org/2001/XMLSchema#date">2025-01-09</dct:created>
    <rdf:type rdf:resource="http://www.w3.org/2000/01/rdf-schema#Class"/>
    <rdf:type rdf:resource="https://w3id.org/dpv/owl#ContractPreparationStatus"/>
    <rdf:type rdf:resource="http://www.w3.org/2002/07/owl#Class"/>
    <skos:definition xml:lang="en">Status representing the drafting of contract text has been completed and it can now be offered for signing</skos:definition>
    <skos:prefLabel xml:lang="en">Contract Drafted</skos:prefLabel>
    <rdfs:isDefinedBy rdf:resource="https://w3id.org/dpv/owl#"/>
    <dct:contributor rdf:nodeID="N2fe5586a82794e5a99ff2b47c1f2175e"/>
    <dct:contributor rdf:nodeID="N2acb95e70d08440bb095f34b511771ce"/>
    <dct:contributor rdf:nodeID="Nb0b5fba741814592ba04e1a368a761fa"/>
    <sw:term_status xml:lang="en">accepted</sw:term_status>
    <rdfs:subClassOf rdf:resource="https://w3id.org/dpv/owl#ContractPreparationStatus"/>
  </rdf:Description>
  <rdf:Description rdf:about="https://w3id.org/dpv/owl#ContractUnderNegotiation">
    <skos:definition xml:lang="en">Status representing contract is under negotiation between parties</skos:definition>
    <dct:created rdf:datatype="http://www.w3.org/2001/XMLSchema#date">2025-01-09</dct:created>
    <rdf:type rdf:resource="http://www.w3.org/2000/01/rdf-schema#Class"/>
    <rdf:type rdf:resource="https://w3id.org/dpv/owl#ContractPreparationStatus"/>
    <rdf:type rdf:resource="http://www.w3.org/2002/07/owl#Class"/>
    <rdfs:isDefinedBy rdf:resource="https://w3id.org/dpv/owl#"/>
    <dct:contributor rdf:nodeID="N2fe5586a82794e5a99ff2b47c1f2175e"/>
    <dct:contributor rdf:nodeID="N2acb95e70d08440bb095f34b511771ce"/>
    <dct:contributor rdf:nodeID="Nb0b5fba741814592ba04e1a368a761fa"/>
    <sw:term_status xml:lang="en">accepted</sw:term_status>
    <skos:prefLabel xml:lang="en">Contract Under Negotiation</skos:prefLabel>
    <rdfs:subClassOf rdf:resource="https://w3id.org/dpv/owl#ContractPreparationStatus"/>
  </rdf:Description>
  <rdf:Description rdf:nodeID="N3f795f08d5094633824a00c38b4e8326">
    <org:memberOf rdf:nodeID="N7c4fc8003c00448b9c4536bd699ada5a"/>
    <rdf:type rdf:resource="http://xmlns.com/foaf/0.1/Person"/>
    <rdf:type rdf:resource="http://purl.org/dc/terms/Agent"/>
    <scoro:hasORCID>0000-0003-0770-2737</scoro:hasORCID>
    <foaf:name>Paul Ryan</foaf:name>
  </rdf:Description>
  <rdf:Description rdf:about="https://w3id.org/dpv/owl#ContractSignedByParty">
    <dct:created rdf:datatype="http://www.w3.org/2001/XMLSchema#date">2025-01-09</dct:created>
    <rdf:type rdf:resource="http://www.w3.org/2000/01/rdf-schema#Class"/>
    <rdf:type rdf:resource="https://w3id.org/dpv/owl#ContractExecutionStatus"/>
    <rdf:type rdf:resource="http://www.w3.org/2002/07/owl#Class"/>
    <rdfs:isDefinedBy rdf:resource="https://w3id.org/dpv/owl#"/>
    <dct:contributor rdf:nodeID="N2fe5586a82794e5a99ff2b47c1f2175e"/>
    <dct:contributor rdf:nodeID="N2acb95e70d08440bb095f34b511771ce"/>
    <dct:contributor rdf:nodeID="Nb0b5fba741814592ba04e1a368a761fa"/>
    <sw:term_status xml:lang="en">accepted</sw:term_status>
    <skos:scopeNote xml:lang="en">The signing party can be expressed using dpv:hasParty with the status along with metadata such as a timestamp, or the status can be used to list whether each party in the contract has signed or not e.g. it is reviewing the contract</skos:scopeNote>
    <skos:prefLabel xml:lang="en">Contract Signed By Party</skos:prefLabel>
    <skos:definition xml:lang="en">Status representing contract has been signed by the indicated signing party</skos:definition>
    <rdfs:subClassOf rdf:resource="https://w3id.org/dpv/owl#ContractExecutionStatus"/>
  </rdf:Description>
  <rdf:Description rdf:about="https://w3id.org/dpv/owl#ContractFulfilmentStatus">
    <skos:prefLabel xml:lang="en">Contract Fulfilment Status</skos:prefLabel>
    <vann:example rdf:resource="https://w3id.org/dpv/examples/owl#E0078"/>
    <vann:example rdf:resource="https://w3id.org/dpv/examples/owl#E0077"/>
    <dct:contributor rdf:nodeID="Nb0b5fba741814592ba04e1a368a761fa"/>
    <dct:contributor rdf:nodeID="N2acb95e70d08440bb095f34b511771ce"/>
    <dct:contributor rdf:nodeID="N2fe5586a82794e5a99ff2b47c1f2175e"/>
    <rdfs:subClassOf rdf:resource="https://w3id.org/dpv/owl#ContractStatus"/>
    <dct:created rdf:datatype="http://www.w3.org/2001/XMLSchema#date">2025-01-09</dct:created>
    <skos:definition xml:lang="en">Status associated with fulfilment of a contract</skos:definition>
    <rdf:type rdf:resource="http://www.w3.org/2000/01/rdf-schema#Class"/>
    <rdf:type rdf:resource="http://www.w3.org/2002/07/owl#Class"/>
    <rdfs:isDefinedBy rdf:resource="https://w3id.org/dpv/owl#"/>
    <sw:term_status xml:lang="en">accepted</sw:term_status>
  </rdf:Description>
  <rdf:Description rdf:about="https://w3id.org/dpv/owl#">
    <owl:versionIRI rdf:resource="https://w3id.org/dpv/2.1/owl#"/>
    <dct:conformsTo rdf:resource="http://www.w3.org/2002/07/owl"/>
    <dct:conformsTo>http://www.w3.org/2000/01/rdf-schema</dct:conformsTo>
    <dct:conformsTo>http://www.w3.org/2004/02/skos/core</dct:conformsTo>
    <dct:modified xml:lang="en">2025-02-01</dct:modified>
    <bibo:doi>10.5281/zenodo.12505841</bibo:doi>
    <dct:publisher rdf:resource="https://www.w3.org/"/>
    <dct:contributor rdf:nodeID="Nb0b5fba741814592ba04e1a368a761fa"/>
    <dct:contributor rdf:nodeID="N2acb95e70d08440bb095f34b511771ce"/>
    <dct:contributor rdf:nodeID="N2fe5586a82794e5a99ff2b47c1f2175e"/>
    <dct:issued xml:lang="en">2022-08-18</dct:issued>
    <dct:hasVersion rdf:resource="https://w3id.org/dpv/owl#"/>
    <profile:hasResource rdf:resource="https://w3id.org/dpv/examples"/>
    <profile:hasResource rdf:resource="https://w3id.org/dpv/guides"/>
    <profile:hasResource rdf:resource="https://w3id.org/dpv/owl#serialisation-ttl"/>
    <profile:hasResource rdf:resource="https://w3id.org/dpv/owl#serialisation-jsonld"/>
    <profile:hasResource rdf:resource="https://w3id.org/dpv/owl#serialisation-rdf"/>
    <profile:hasResource rdf:resource="https://w3id.org/dpv/primer"/>
    <profile:hasResource rdf:resource="https://w3id.org/dpv/owl#serialisation-n3"/>
    <profile:hasResource rdf:resource="https://w3id.org/dpv/owl#serialisation-html"/>
    <rdfs:Label xml:lang="en">DPV</rdfs:Label>
    <dct:identifier>https://w3id.org/dpv</dct:identifier>
    <bibo:status>http://purl.org/ontology/bibo/status/published</bibo:status>
    <dct:description xml:lang="en">The Data Privacy Vocabulary (DPV) provides terms (classes and properties) to represent information about processing of personal data, for example - purposes, processing operations, personal data, technical and organisational measures.</dct:description>
    <dct:creator rdf:nodeID="N3f795f08d5094633824a00c38b4e8326"/>
    <dct:creator rdf:nodeID="N18c0395db3e14fc6b2c509914ad20ef9"/>
    <dct:creator rdf:nodeID="N2fe5586a82794e5a99ff2b47c1f2175e"/>
    <dct:creator rdf:nodeID="Nf2624642076a4610a51afb2a4c6e9cdd"/>
    <dct:creator rdf:nodeID="Nb0b5fba741814592ba04e1a368a761fa"/>
    <dct:creator rdf:nodeID="N2acb95e70d08440bb095f34b511771ce"/>
    <owl:versionInfo>2.1</owl:versionInfo>
    <schema:version>2.1</schema:version>
    <vann:preferredNamespaceUri>https://w3id.org/dpv#</vann:preferredNamespaceUri>
    <profile:isProfileOf rdf:resource="http://www.w3.org/2002/07/owl"/>
    <profile:isProfileOf rdf:resource="https://w3id.org/dpv/owl#"/>
    <dct:title xml:lang="en">Data Privacy Vocabulary (DPV)</dct:title>
    <dct:source rdf:resource="https://www.w3.org/groups/cg/dpvcg/"/>
    <dct:bibliographicCitation>Data Privacy Vocabulary (DPV) -- Version 2. Harshvardhan J. Pandit, Beatriz Esteves, Georg P. Krog, Paul Ryan, Delaram Golpayegani, Julian Flake https://doi.org/10.48550/arXiv.2404.13426</dct:bibliographicCitation>
    <vann:preferredNamespacePrefix>dpv</vann:preferredNamespacePrefix>
    <dct:license rdf:resource="https://www.w3.org/copyright/document-license-2023/"/>
    <rdf:type rdf:resource="http://www.w3.org/2002/07/owl#Ontology"/>
    <rdf:type rdf:resource="http://www.w3.org/ns/dx/prof/Profile"/>
    <foaf:logo rdf:resource="https://w3id.org/dpv/media/logo.png"/>
    <dct:created xml:lang="en">2022-08-18</dct:created>
  </rdf:Description>
  <rdf:Description rdf:about="https://w3id.org/dpv/owl#ContractExecutionStatus">
    <skos:prefLabel xml:lang="en">Contract Execution Status</skos:prefLabel>
    <sw:term_status xml:lang="en">accepted</sw:term_status>
    <dct:created rdf:datatype="http://www.w3.org/2001/XMLSchema#date">2025-01-09</dct:created>
    <rdf:type rdf:resource="http://www.w3.org/2000/01/rdf-schema#Class"/>
    <rdf:type rdf:resource="http://www.w3.org/2002/07/owl#Class"/>
    <dct:contributor rdf:nodeID="N2acb95e70d08440bb095f34b511771ce"/>
    <dct:contributor rdf:nodeID="N2fe5586a82794e5a99ff2b47c1f2175e"/>
    <dct:contributor rdf:nodeID="Nb0b5fba741814592ba04e1a368a761fa"/>
    <rdfs:isDefinedBy rdf:resource="https://w3id.org/dpv/owl#"/>
    <skos:definition xml:lang="en">Status associated with execution of a contract (i.e. signing and procedural aspects before the contract terms come in to effect)</skos:definition>
    <rdfs:subClassOf rdf:resource="https://w3id.org/dpv/owl#ContractStatus"/>
  </rdf:Description>
  <rdf:Description rdf:about="https://w3id.org/dpv/owl#ContractExpired">
    <rdf:type rdf:resource="https://w3id.org/dpv/owl#ContractTerminationStatus"/>
    <rdf:type rdf:resource="http://www.w3.org/2000/01/rdf-schema#Class"/>
    <rdf:type rdf:resource="http://www.w3.org/2002/07/owl#Class"/>
    <dct:created rdf:datatype="http://www.w3.org/2001/XMLSchema#date">2025-01-09</dct:created>
    <skos:prefLabel xml:lang="en">Contract Expired</skos:prefLabel>
    <dct:contributor rdf:nodeID="N2acb95e70d08440bb095f34b511771ce"/>
    <dct:contributor rdf:nodeID="N2fe5586a82794e5a99ff2b47c1f2175e"/>
    <dct:contributor rdf:nodeID="Nb0b5fba741814592ba04e1a368a761fa"/>
    <skos:definition xml:lang="en">Status representing reaching the expiry defined in the contract, such as when the stated duration or the stated obligations have been completed</skos:definition>
    <rdfs:isDefinedBy rdf:resource="https://w3id.org/dpv/owl#"/>
    <sw:term_status xml:lang="en">accepted</sw:term_status>
    <rdfs:subClassOf rdf:resource="https://w3id.org/dpv/owl#ContractTerminationStatus"/>
  </rdf:Description>
  <rdf:Description rdf:about="https://w3id.org/dpv/owl#ContractFullySigned">
    <dct:contributor rdf:nodeID="N2fe5586a82794e5a99ff2b47c1f2175e"/>
    <dct:contributor rdf:nodeID="N2acb95e70d08440bb095f34b511771ce"/>
    <dct:contributor rdf:nodeID="Nb0b5fba741814592ba04e1a368a761fa"/>
    <dct:created rdf:datatype="http://www.w3.org/2001/XMLSchema#date">2025-01-09</dct:created>
    <sw:term_status xml:lang="en">accepted</sw:term_status>
    <rdf:type rdf:resource="https://w3id.org/dpv/owl#ContractExecutionStatus"/>
    <rdf:type rdf:resource="http://www.w3.org/2000/01/rdf-schema#Class"/>
    <rdf:type rdf:resource="http://www.w3.org/2002/07/owl#Class"/>
    <rdfs:isDefinedBy rdf:resource="https://w3id.org/dpv/owl#"/>
    <skos:definition xml:lang="en">Status representing contract has been signed by all concerned parties</skos:definition>
    <skos:prefLabel xml:lang="en">Contract Fully Signed</skos:prefLabel>
    <rdfs:subClassOf rdf:resource="https://w3id.org/dpv/owl#ContractExecutionStatus"/>
  </rdf:Description>
  <rdf:Description rdf:nodeID="Nf2624642076a4610a51afb2a4c6e9cdd">
    <rdf:type rdf:resource="http://purl.org/dc/terms/Agent"/>
    <rdf:type rdf:resource="http://xmlns.com/foaf/0.1/Person"/>
    <scoro:hasORCID>0000-0002-1208-186X</scoro:hasORCID>
    <org:memberOf rdf:nodeID="Nae82bf4b085a4b0cb8e01f78de3376c5"/>
    <foaf:name>Delaram Golpayegani</foaf:name>
  </rdf:Description>
  <rdf:Description rdf:about="https://w3id.org/dpv/owl#ContractDisputed">
    <dct:created rdf:datatype="http://www.w3.org/2001/XMLSchema#date">2025-01-09</dct:created>
    <rdf:type rdf:resource="http://www.w3.org/2000/01/rdf-schema#Class"/>
    <rdf:type rdf:resource="https://w3id.org/dpv/owl#ContractTerminationStatus"/>
    <rdf:type rdf:resource="http://www.w3.org/2002/07/owl#Class"/>
    <dct:contributor rdf:nodeID="N2acb95e70d08440bb095f34b511771ce"/>
    <dct:contributor rdf:nodeID="N2fe5586a82794e5a99ff2b47c1f2175e"/>
    <dct:contributor rdf:nodeID="Nb0b5fba741814592ba04e1a368a761fa"/>
    <rdfs:isDefinedBy rdf:resource="https://w3id.org/dpv/owl#"/>
    <skos:definition xml:lang="en">Status representing contract being disputed where one or more parties have an issue regarding the interpretation and performance of the contract</skos:definition>
    <sw:term_status xml:lang="en">accepted</sw:term_status>
    <skos:prefLabel xml:lang="en">Contract Disputed</skos:prefLabel>
    <rdfs:subClassOf rdf:resource="https://w3id.org/dpv/owl#ContractTerminationStatus"/>
  </rdf:Description>
  <rdf:Description rdf:about="https://w3id.org/dpv/owl#ContractRejected">
    <dct:created rdf:datatype="http://www.w3.org/2001/XMLSchema#date">2025-01-09</dct:created>
    <rdf:type rdf:resource="http://www.w3.org/2000/01/rdf-schema#Class"/>
    <rdf:type rdf:resource="https://w3id.org/dpv/owl#ContractPreparationStatus"/>
    <rdf:type rdf:resource="http://www.w3.org/2002/07/owl#Class"/>
    <rdfs:isDefinedBy rdf:resource="https://w3id.org/dpv/owl#"/>
    <dct:contributor rdf:nodeID="N2fe5586a82794e5a99ff2b47c1f2175e"/>
    <dct:contributor rdf:nodeID="N2acb95e70d08440bb095f34b511771ce"/>
    <dct:contributor rdf:nodeID="Nb0b5fba741814592ba04e1a368a761fa"/>
    <sw:term_status xml:lang="en">accepted</sw:term_status>
    <skos:prefLabel xml:lang="en">Contract Rejected</skos:prefLabel>
    <skos:definition xml:lang="en">Status representing contract has been rejected and cannot be used for signing</skos:definition>
    <rdfs:subClassOf rdf:resource="https://w3id.org/dpv/owl#ContractPreparationStatus"/>
  </rdf:Description>
  <rdf:Description rdf:about="https://w3id.org/dpv/owl#ContractUnderReview">
    <dct:created rdf:datatype="http://www.w3.org/2001/XMLSchema#date">2025-01-09</dct:created>
    <rdf:type rdf:resource="http://www.w3.org/2000/01/rdf-schema#Class"/>
    <rdf:type rdf:resource="https://w3id.org/dpv/owl#ContractPreparationStatus"/>
    <rdf:type rdf:resource="http://www.w3.org/2002/07/owl#Class"/>
    <skos:definition xml:lang="en">Status representing contract is under review and is being considered for signing</skos:definition>
    <dct:contributor rdf:nodeID="N2fe5586a82794e5a99ff2b47c1f2175e"/>
    <dct:contributor rdf:nodeID="N2acb95e70d08440bb095f34b511771ce"/>
    <dct:contributor rdf:nodeID="Nb0b5fba741814592ba04e1a368a761fa"/>
    <skos:prefLabel xml:lang="en">Contract Under Review</skos:prefLabel>
    <sw:term_status xml:lang="en">accepted</sw:term_status>
    <rdfs:isDefinedBy rdf:resource="https://w3id.org/dpv/owl#"/>
    <rdfs:subClassOf rdf:resource="https://w3id.org/dpv/owl#ContractPreparationStatus"/>
  </rdf:Description>
  <rdf:Description rdf:about="https://w3id.org/dpv/owl#serialisation-ttl">
    <dct:format rdf:resource="https://www.iana.org/assignments/media-types/text/turtle"/>
    <profile:hasRole rdf:resource="http://www.w3.org/ns/dx/prof/role/vocabulary"/>
    <dct:title>Data Privacy Vocabulary (DPV) - Turtle serialiation</dct:title>
    <dct:conformsTo rdf:resource="https://www.w3.org/TR/turtle/"/>
    <profile:hasArtifact rdf:resource="https://w3id.org/dpv/dpv/dpv-owl.ttl"/>
    <rdf:type rdf:resource="http://www.w3.org/ns/dx/prof/ResourceDescriptor"/>
  </rdf:Description>
  <rdf:Description rdf:about="https://w3id.org/dpv/owl#ContractTemporarilySuspended">
    <dct:contributor rdf:nodeID="N2fe5586a82794e5a99ff2b47c1f2175e"/>
    <dct:contributor rdf:nodeID="N2acb95e70d08440bb095f34b511771ce"/>
    <dct:contributor rdf:nodeID="Nb0b5fba741814592ba04e1a368a761fa"/>
    <sw:term_status xml:lang="en">accepted</sw:term_status>
    <rdfs:isDefinedBy rdf:resource="https://w3id.org/dpv/owl#"/>
    <rdf:type rdf:resource="https://w3id.org/dpv/owl#ContractPerformanceStatus"/>
    <rdf:type rdf:resource="http://www.w3.org/2000/01/rdf-schema#Class"/>
    <rdf:type rdf:resource="http://www.w3.org/2002/07/owl#Class"/>
    <skos:definition xml:lang="en">Status representing contract that has been temporarily suspended through mutual agreement or by some parties</skos:definition>
    <dct:created rdf:datatype="http://www.w3.org/2001/XMLSchema#date">2025-01-09</dct:created>
    <skos:prefLabel xml:lang="en">Contract Temporarily Suspended</skos:prefLabel>
    <rdfs:subClassOf rdf:resource="https://w3id.org/dpv/owl#ContractPerformanceStatus"/>
  </rdf:Description>
  <rdf:Description rdf:about="https://w3id.org/dpv/guides">
    <rdf:type rdf:resource="http://www.w3.org/ns/dx/prof/ResourceDescriptor"/>
    <profile:hasArtifact rdf:resource="https://w3id.org/dpv/guides"/>
    <profile:hasRole rdf:resource="http://www.w3.org/ns/dx/prof/role/guidance"/>
    <dct:title>Guides for Data Privacy Vocabulary</dct:title>
    <dct:format rdf:resource="https://www.iana.org/assignments/media-types/text/html"/>
    <dct:conformsTo rdf:resource="https://www.w3.org/TR/html/"/>
  </rdf:Description>
  <rdf:Description rdf:about="https://w3id.org/dpv/owl#ContractInactive">
    <rdf:type rdf:resource="http://www.w3.org/2000/01/rdf-schema#Class"/>
    <rdf:type rdf:resource="https://w3id.org/dpv/owl#ContractActivationStatus"/>
    <rdf:type rdf:resource="http://www.w3.org/2002/07/owl#Class"/>
    <dct:contributor rdf:nodeID="N2acb95e70d08440bb095f34b511771ce"/>
    <dct:contributor rdf:nodeID="N2fe5586a82794e5a99ff2b47c1f2175e"/>
    <dct:contributor rdf:nodeID="Nb0b5fba741814592ba04e1a368a761fa"/>
    <rdfs:isDefinedBy rdf:resource="https://w3id.org/dpv/owl#"/>
    <skos:prefLabel xml:lang="en">Contract Inactive</skos:prefLabel>
    <skos:scopeNote xml:lang="en">An example of an inactive contract is where its terms need to be fulfiled at a later date, at which point the contract will become active</skos:scopeNote>
    <skos:definition xml:lang="en">Status representing contract that has been fully executed and whose terms are not yet active i.e. they need to be performed at a later time</skos:definition>
    <dct:created rdf:datatype="http://www.w3.org/2001/XMLSchema#date">2025-01-09</dct:created>
    <sw:term_status xml:lang="en">accepted</sw:term_status>
    <rdfs:subClassOf rdf:resource="https://w3id.org/dpv/owl#ContractActivationStatus"/>
  </rdf:Description>
  <rdf:Description rdf:nodeID="Nb0b5fba741814592ba04e1a368a761fa">
    <org:memberOf rdf:nodeID="N1c229bec7c674c58a5bced416591f4f8"/>
    <rdf:type rdf:resource="http://purl.org/dc/terms/Agent"/>
    <rdf:type rdf:resource="http://xmlns.com/foaf/0.1/Person"/>
    <foaf:name>Georg P. Krog</foaf:name>
    <foaf:homepage>https://www.linkedin.com/in/georg-philip-krog-a2a278104/</foaf:homepage>
  </rdf:Description>
  <rdf:Description rdf:about="https://w3id.org/dpv/owl#ContractTerminationStatus">
    <skos:definition xml:lang="en">Status associated with termination of a contract</skos:definition>
    <dct:contributor rdf:nodeID="N2fe5586a82794e5a99ff2b47c1f2175e"/>
    <dct:contributor rdf:nodeID="N2acb95e70d08440bb095f34b511771ce"/>
    <dct:contributor rdf:nodeID="Nb0b5fba741814592ba04e1a368a761fa"/>
    <sw:term_status xml:lang="en">accepted</sw:term_status>
    <skos:prefLabel xml:lang="en">Contract Termination Status</skos:prefLabel>
    <rdfs:subClassOf rdf:resource="https://w3id.org/dpv/owl#ContractStatus"/>
    <dct:created rdf:datatype="http://www.w3.org/2001/XMLSchema#date">2025-01-09</dct:created>
    <rdf:type rdf:resource="http://www.w3.org/2000/01/rdf-schema#Class"/>
    <rdf:type rdf:resource="http://www.w3.org/2002/07/owl#Class"/>
    <rdfs:isDefinedBy rdf:resource="https://w3id.org/dpv/owl#"/>
  </rdf:Description>
  <rdf:Description rdf:nodeID="N4b871a5999ce4c73b92d6a31fb56b287">
    <rdf:type rdf:resource="http://xmlns.com/foaf/0.1/Organization"/>
    <foaf:name>University of Koblenz</foaf:name>
  </rdf:Description>
  <rdf:Description rdf:about="https://w3id.org/dpv/owl#ContractNegotiated">
    <skos:definition xml:lang="en">Status representing contract has been successfully negotiated by involved parties</skos:definition>
    <rdf:type rdf:resource="https://w3id.org/dpv/owl#ContractPreparationStatus"/>
    <rdf:type rdf:resource="http://www.w3.org/2000/01/rdf-schema#Class"/>
    <rdf:type rdf:resource="http://www.w3.org/2002/07/owl#Class"/>
    <dct:created rdf:datatype="http://www.w3.org/2001/XMLSchema#date">2025-01-09</dct:created>
    <sw:term_status xml:lang="en">accepted</sw:term_status>
    <rdfs:isDefinedBy rdf:resource="https://w3id.org/dpv/owl#"/>
    <dct:contributor rdf:nodeID="N2acb95e70d08440bb095f34b511771ce"/>
    <dct:contributor rdf:nodeID="N2fe5586a82794e5a99ff2b47c1f2175e"/>
    <dct:contributor rdf:nodeID="Nb0b5fba741814592ba04e1a368a761fa"/>
    <skos:prefLabel xml:lang="en">Contract Negotiated</skos:prefLabel>
    <rdfs:subClassOf rdf:resource="https://w3id.org/dpv/owl#ContractPreparationStatus"/>
  </rdf:Description>
  <rdf:Description rdf:about="https://w3id.org/dpv/owl#ContractExtended">
    <dct:created rdf:datatype="http://www.w3.org/2001/XMLSchema#date">2025-01-09</dct:created>
    <rdf:type rdf:resource="http://www.w3.org/2000/01/rdf-schema#Class"/>
    <rdf:type rdf:resource="https://w3id.org/dpv/owl#ContractTerminationStatus"/>
    <rdf:type rdf:resource="http://www.w3.org/2002/07/owl#Class"/>
    <dct:contributor rdf:nodeID="N2acb95e70d08440bb095f34b511771ce"/>
    <dct:contributor rdf:nodeID="N2fe5586a82794e5a99ff2b47c1f2175e"/>
    <dct:contributor rdf:nodeID="Nb0b5fba741814592ba04e1a368a761fa"/>
    <rdfs:isDefinedBy rdf:resource="https://w3id.org/dpv/owl#"/>
    <sw:term_status xml:lang="en">accepted</sw:term_status>
    <skos:prefLabel xml:lang="en">Contract Extended</skos:prefLabel>
    <skos:definition xml:lang="en">Status representing the duration associated with a contract being extended through mutual agreement or by a party</skos:definition>
    <rdfs:subClassOf rdf:resource="https://w3id.org/dpv/owl#ContractTerminationStatus"/>
  </rdf:Description>
  <rdf:Description rdf:about="https://w3id.org/dpv/owl#ContractAmended">
    <sw:term_status xml:lang="en">accepted</sw:term_status>
    <rdfs:isDefinedBy rdf:resource="https://w3id.org/dpv/owl#"/>
    <dct:contributor rdf:nodeID="N2acb95e70d08440bb095f34b511771ce"/>
    <dct:contributor rdf:nodeID="N2fe5586a82794e5a99ff2b47c1f2175e"/>
    <dct:contributor rdf:nodeID="Nb0b5fba741814592ba04e1a368a761fa"/>
    <skos:definition xml:lang="en">Status representing contract that has been fully executed and whose terms have been amended through mutual agreement or other means such that the contract is still required to be performed</skos:definition>
    <rdf:type rdf:resource="https://w3id.org/dpv/owl#ContractPerformanceStatus"/>
    <rdf:type rdf:resource="http://www.w3.org/2000/01/rdf-schema#Class"/>
    <rdf:type rdf:resource="http://www.w3.org/2002/07/owl#Class"/>
    <skos:prefLabel xml:lang="en">Contract Amended</skos:prefLabel>
    <dct:created rdf:datatype="http://www.w3.org/2001/XMLSchema#date">2025-01-09</dct:created>
    <rdfs:subClassOf rdf:resource="https://w3id.org/dpv/owl#ContractPerformanceStatus"/>
  </rdf:Description>
  <rdf:Description rdf:about="https://w3id.org/dpv/owl#ContractPartiallyFulfiled">
    <dct:contributor rdf:nodeID="Nb0b5fba741814592ba04e1a368a761fa"/>
    <dct:contributor rdf:nodeID="N2fe5586a82794e5a99ff2b47c1f2175e"/>
    <dct:contributor rdf:nodeID="N2acb95e70d08440bb095f34b511771ce"/>
    <skos:definition xml:lang="en">Status representing contract where some of its terms have been fulfiled, and others are yet to be fulfiled in a manner that does not constitute a violation or breach of the contract i.e. there is still time and opportunity to complete the terms</skos:definition>
    <dct:created rdf:datatype="http://www.w3.org/2001/XMLSchema#date">2025-01-09</dct:created>
    <rdf:type rdf:resource="http://www.w3.org/2000/01/rdf-schema#Class"/>
    <rdf:type rdf:resource="https://w3id.org/dpv/owl#ContractFulfilmentStatus"/>
    <rdf:type rdf:resource="http://www.w3.org/2002/07/owl#Class"/>
    <sw:term_status xml:lang="en">accepted</sw:term_status>
    <rdfs:isDefinedBy rdf:resource="https://w3id.org/dpv/owl#"/>
    <skos:prefLabel xml:lang="en">Contract Partially Fulfiled</skos:prefLabel>
    <rdfs:subClassOf rdf:resource="https://w3id.org/dpv/owl#ContractFulfilmentStatus"/>
  </rdf:Description>
  <rdf:Description rdf:nodeID="N7c4fc8003c00448b9c4536bd699ada5a">
    <rdf:type rdf:resource="http://xmlns.com/foaf/0.1/Organization"/>
    <foaf:name>Uniphar PLC</foaf:name>
  </rdf:Description>
  <rdf:Description rdf:nodeID="Nae82bf4b085a4b0cb8e01f78de3376c5">
    <foaf:name>ADAPT Centre, Trinity College Dublin</foaf:name>
    <rdf:type rdf:resource="http://xmlns.com/foaf/0.1/Organization"/>
  </rdf:Description>
  <rdf:Description rdf:about="https://w3id.org/dpv/owl#ContractNotFulfiled">
    <skos:prefLabel xml:lang="en">Contract Not Fulfiled</skos:prefLabel>
    <rdf:type rdf:resource="https://w3id.org/dpv/owl#ContractFulfilmentStatus"/>
    <rdf:type rdf:resource="http://www.w3.org/2000/01/rdf-schema#Class"/>
    <rdf:type rdf:resource="http://www.w3.org/2002/07/owl#Class"/>
    <dct:created rdf:datatype="http://www.w3.org/2001/XMLSchema#date">2025-01-09</dct:created>
    <skos:definition xml:lang="en">Status representing contract where none of its terms have been fulfiled in a manner that does not constitutea violation or breach of the contract i.e. there is still time and opportunity to complete the terms</skos:definition>
    <rdfs:isDefinedBy rdf:resource="https://w3id.org/dpv/owl#"/>
    <dct:contributor rdf:nodeID="N2acb95e70d08440bb095f34b511771ce"/>
    <dct:contributor rdf:nodeID="N2fe5586a82794e5a99ff2b47c1f2175e"/>
    <dct:contributor rdf:nodeID="Nb0b5fba741814592ba04e1a368a761fa"/>
    <sw:term_status xml:lang="en">accepted</sw:term_status>
    <rdfs:subClassOf rdf:resource="https://w3id.org/dpv/owl#ContractFulfilmentStatus"/>
  </rdf:Description>
  <rdf:Description rdf:about="https://w3id.org/dpv/owl#serialisation-html">
    <dct:conformsTo rdf:resource="https://www.w3.org/TR/html/"/>
    <dct:title>Data Privacy Vocabulary (DPV) - HTML serialiation</dct:title>
    <rdf:type rdf:resource="http://www.w3.org/ns/dx/prof/ResourceDescriptor"/>
    <profile:hasRole rdf:resource="http://www.w3.org/ns/dx/prof/role/specification"/>
    <dct:format rdf:resource="https://www.iana.org/assignments/media-types/text/html"/>
    <profile:hasArtifact rdf:resource="https://w3id.org/dpv/dpv-owl.html"/>
  </rdf:Description>
  <rdf:Description rdf:about="https://w3id.org/dpv/owl#ContractFulfiled">
    <rdf:type rdf:resource="http://www.w3.org/2000/01/rdf-schema#Class"/>
    <rdf:type rdf:resource="https://w3id.org/dpv/owl#ContractFulfilmentStatus"/>
    <rdf:type rdf:resource="http://www.w3.org/2002/07/owl#Class"/>
    <dct:contributor rdf:nodeID="N2acb95e70d08440bb095f34b511771ce"/>
    <dct:contributor rdf:nodeID="N2fe5586a82794e5a99ff2b47c1f2175e"/>
    <dct:contributor rdf:nodeID="Nb0b5fba741814592ba04e1a368a761fa"/>
    <rdfs:isDefinedBy rdf:resource="https://w3id.org/dpv/owl#"/>
    <sw:term_status xml:lang="en">accepted</sw:term_status>
    <skos:definition xml:lang="en">Status representing contract where all its terms have been fulfiled in a manner that does not constitute a violation or breach of the contract</skos:definition>
    <skos:prefLabel xml:lang="en">Contract Fulfiled</skos:prefLabel>
    <dct:created rdf:datatype="http://www.w3.org/2001/XMLSchema#date">2025-01-09</dct:created>
    <rdfs:subClassOf rdf:resource="https://w3id.org/dpv/owl#ContractFulfilmentStatus"/>
  </rdf:Description>
  <rdf:Description rdf:nodeID="Ned4fceae20ce40ff92e5a6d6d2cde0cb">
    <rdf:type rdf:resource="http://xmlns.com/foaf/0.1/Organization"/>
    <foaf:name>IDLab, IMEC, Ghent University</foaf:name>
  </rdf:Description>
  <rdf:Description rdf:nodeID="N2acb95e70d08440bb095f34b511771ce">
    <foaf:name>Julian Flake</foaf:name>
    <org:memberOf rdf:nodeID="N4b871a5999ce4c73b92d6a31fb56b287"/>
    <rdf:type rdf:resource="http://xmlns.com/foaf/0.1/Person"/>
    <rdf:type rdf:resource="http://purl.org/dc/terms/Agent"/>
    <scoro:hasORCID>0009-0006-4623-1463</scoro:hasORCID>
  </rdf:Description>
  <rdf:Description rdf:nodeID="N2fe5586a82794e5a99ff2b47c1f2175e">
    <rdf:type rdf:resource="http://xmlns.com/foaf/0.1/Person"/>
    <rdf:type rdf:resource="http://purl.org/dc/terms/Agent"/>
    <scoro:hasORCID>0000-0002-5068-3714</scoro:hasORCID>
    <foaf:homepage>https://harshp.com/</foaf:homepage>
    <foaf:name>Harshvardhan J. Pandit</foaf:name>
    <org:memberOf rdf:nodeID="Nfbd61e1f087d467e81291e0c311268a5"/>
  </rdf:Description>
  <rdf:Description rdf:nodeID="N18c0395db3e14fc6b2c509914ad20ef9">
    <rdf:type rdf:resource="http://xmlns.com/foaf/0.1/Person"/>
    <rdf:type rdf:resource="http://purl.org/dc/terms/Agent"/>
    <org:memberOf rdf:nodeID="Ned4fceae20ce40ff92e5a6d6d2cde0cb"/>
    <scoro:hasORCID>0000-0003-0259-7560</scoro:hasORCID>
    <foaf:name>Beatriz Esteves</foaf:name>
  </rdf:Description>
  <rdf:Description rdf:about="https://w3id.org/dpv/owl#ContractActive">
    <sw:term_status xml:lang="en">accepted</sw:term_status>
    <skos:prefLabel xml:lang="en">Contract Active</skos:prefLabel>
    <dct:contributor rdf:nodeID="N2acb95e70d08440bb095f34b511771ce"/>
    <dct:contributor rdf:nodeID="Nb0b5fba741814592ba04e1a368a761fa"/>
    <dct:contributor rdf:nodeID="N2fe5586a82794e5a99ff2b47c1f2175e"/>
    <rdfs:isDefinedBy rdf:resource="https://w3id.org/dpv/owl#"/>
    <skos:scopeNote xml:lang="en">A contract being active only refers to its terms now being required to be fulfiled, while dpv:ContractBeingPerformed states that they are being performed</skos:scopeNote>
    <dct:created rdf:datatype="http://www.w3.org/2001/XMLSchema#date">2025-01-09</dct:created>
    <skos:definition xml:lang="en">Status representing contract that has been fully executed and whose terms are considered active i.e. they are applicable and are required to be performed</skos:definition>
    <rdf:type rdf:resource="https://w3id.org/dpv/owl#ContractActivationStatus"/>
    <rdf:type rdf:resource="http://www.w3.org/2000/01/rdf-schema#Class"/>
    <rdf:type rdf:resource="http://www.w3.org/2002/07/owl#Class"/>
    <rdfs:subClassOf rdf:resource="https://w3id.org/dpv/owl#ContractActivationStatus"/>
  </rdf:Description>
  <rdf:Description rdf:about="https://w3id.org/dpv/owl#serialisation-n3">
    <rdf:type rdf:resource="http://www.w3.org/ns/dx/prof/ResourceDescriptor"/>
    <profile:hasArtifact rdf:resource="https://w3id.org/dpv/dpv/dpv-owl.n3"/>
    <dct:conformsTo rdf:resource="https://www.w3.org/TeamSubmission/n3/"/>
    <profile:hasRole rdf:resource="http://www.w3.org/ns/dx/prof/role/vocabulary"/>
    <dct:format rdf:resource="https://www.iana.org/assignments/media-types/text/n3"/>
    <dct:title>Data Privacy Vocabulary (DPV) - N3 serialiation</dct:title>
  </rdf:Description>
  <rdf:Description rdf:about="https://w3id.org/dpv/owl#ContractActivationStatus">
    <dct:created rdf:datatype="http://www.w3.org/2001/XMLSchema#date">2025-01-09</dct:created>
    <rdf:type rdf:resource="http://www.w3.org/2000/01/rdf-schema#Class"/>
    <rdf:type rdf:resource="http://www.w3.org/2002/07/owl#Class"/>
    <dct:contributor rdf:nodeID="N2acb95e70d08440bb095f34b511771ce"/>
    <dct:contributor rdf:nodeID="N2fe5586a82794e5a99ff2b47c1f2175e"/>
    <dct:contributor rdf:nodeID="Nb0b5fba741814592ba04e1a368a761fa"/>
    <rdfs:isDefinedBy rdf:resource="https://w3id.org/dpv/owl#"/>
    <skos:prefLabel xml:lang="en">Contract Activation Status</skos:prefLabel>
    <skos:definition xml:lang="en">Status associated with activation of a contract i.e. whether its terms are active and are required to be performed</skos:definition>
    <sw:term_status xml:lang="en">accepted</sw:term_status>
    <rdfs:subClassOf rdf:resource="https://w3id.org/dpv/owl#ContractStatus"/>
  </rdf:Description>
  <rdf:Description rdf:about="https://w3id.org/dpv/owl#serialisation-jsonld">
    <dct:conformsTo rdf:resource="https://www.w3.org/TR/json-ld11/"/>
    <profile:hasRole rdf:resource="http://www.w3.org/ns/dx/prof/role/vocabulary"/>
    <dct:format rdf:resource="https://www.iana.org/assignments/media-types/application/ld+json"/>
    <rdf:type rdf:resource="http://www.w3.org/ns/dx/prof/ResourceDescriptor"/>
    <profile:hasArtifact rdf:resource="https://w3id.org/dpv/dpv/dpv-owl.jsonld"/>
    <dct:title>Data Privacy Vocabulary (DPV) - JSON-LD serialiation</dct:title>
  </rdf:Description>
  <rdf:Description rdf:about="https://w3id.org/dpv/examples">
    <dct:title>Examples for Data Privacy Vocabulary</dct:title>
    <dct:format rdf:resource="https://www.iana.org/assignments/media-types/text/html"/>
    <profile:hasArtifact rdf:resource="https://w3id.org/dpv/examples"/>
    <profile:hasRole rdf:resource="http://www.w3.org/ns/dx/prof/role/guidance"/>
    <dct:conformsTo rdf:resource="https://www.w3.org/TR/html/"/>
    <rdf:type rdf:resource="http://www.w3.org/ns/dx/prof/ResourceDescriptor"/>
  </rdf:Description>
  <rdf:Description rdf:nodeID="N1c229bec7c674c58a5bced416591f4f8">
    <foaf:name>Signatu AS</foaf:name>
    <rdf:type rdf:resource="http://xmlns.com/foaf/0.1/Organization"/>
  </rdf:Description>
  <rdf:Description rdf:about="https://w3id.org/dpv/primer">
    <dct:format rdf:resource="https://www.iana.org/assignments/media-types/text/html"/>
    <dct:title>Primer for Data Privacy Vocabulary</dct:title>
    <profile:hasRole rdf:resource="http://www.w3.org/ns/dx/prof/role/guidance"/>
    <dct:conformsTo rdf:resource="https://www.w3.org/TR/html/"/>
    <rdf:type rdf:resource="http://www.w3.org/ns/dx/prof/ResourceDescriptor"/>
    <profile:hasArtifact rdf:resource="https://w3id.org/dpv/primer"/>
  </rdf:Description>
</rdf:RDF>
